@prefix : <https://purl.org/fisa#> .
@prefix owl: <http://www.w3.org/2002/07/owl#> .
@prefix rdf: <http://www.w3.org/1999/02/22-rdf-syntax-ns#> .
@prefix xml: <http://www.w3.org/XML/1998/namespace> .
@prefix xsd: <http://www.w3.org/2001/XMLSchema#> .
@prefix rdfs: <http://www.w3.org/2000/01/rdf-schema#> .
@base <https://purl.org/fisa#> .

<https://purl.org/fisa> rdf:type owl:Ontology ;
                         owl:versionIRI <https://purl.org/fisa/0.0.1> ;
                         <http://purl.org/dc/terms/created> "2023"@en ;
                         <http://purl.org/dc/terms/creator> "Isabelle Fitkau" ,
                                                            "Timo Hartmann" ;
                         <http://purl.org/dc/terms/description> "Die Fire Safety (Brandschutz)-Ontologie (FiSa) ermöglicht die Klassifizierung von Gebäuden und ihren Komponenten auf der Grundlage von Brandschutzerwägungen. FiSa legt eine Brandschutzperspektive für Gebäude fest, indem es eine Kombination aus Bauvorschriften, technischen Vorschriften, Richtlinien und halbstrukturierten Interviews mit Brandschutzplanern verwendet. Anschließend wurden die Erkenntnisse von Brandschutzexperten mit dem Wissen über die Gebäudeplanung aus anderen Bereichen, wie z. B. der Architektur, abgeglichen. Durch diese Zusammenarbeit und die Instanziierung von Gebäudedaten innerhalb der Ontologie wurden die Anforderungen an den baulichen Brandschutz aus den Vorschriften automatisch abgeleitet, indem mit gängigen Inferenzmaschinen eine automatische Prüfung der Einhaltung der Vorschriften simuliert wurde."@de ,
                                                                "The Fire Safety Ontology (FiSa) enables the classification of buildings and its components based on fire safety considerations. FiSa establish a fire safety perspective for buildings utilizing a combination of building codes, technical regulations, guidelines, and semi-structured interviews with fire safety planners. Subsequently, fire safety domain insights from experts were aligned to knowledge about building design from other domains, such as architecture. Through this collaborative effort and the instantiation of building data within the ontology, structural fire safety requirements from regulations were automatically inferred by reasoning with common inference engines, simulating an automatic compliance checking."@en ;
                         <http://purl.org/dc/terms/license> "https://creativecommons.org/licenses/by/4.0/" ;
                         <http://purl.org/dc/terms/title> "Fire Safety Ontology (FiSa)" ;
                         <http://purl.org/vocab/vann/preferredNamespacePrefix> "fisa" ;
                         <http://purl.org/vocab/vann/preferredNamespaceUri> : ;
                         owl:versionInfo "0.0.1"@en .

#################################################################
#    Annotation properties
#################################################################

###  http://purl.org/dc/terms/contributor
<http://purl.org/dc/terms/contributor> rdf:type owl:AnnotationProperty .


###  http://purl.org/dc/terms/created
<http://purl.org/dc/terms/created> rdf:type owl:AnnotationProperty .


###  http://purl.org/dc/terms/creator
<http://purl.org/dc/terms/creator> rdf:type owl:AnnotationProperty .


###  http://purl.org/dc/terms/description
<http://purl.org/dc/terms/description> rdf:type owl:AnnotationProperty .


###  http://purl.org/dc/terms/license
<http://purl.org/dc/terms/license> rdf:type owl:AnnotationProperty .


###  http://purl.org/dc/terms/title
<http://purl.org/dc/terms/title> rdf:type owl:AnnotationProperty .


###  http://purl.org/vocab/vann/preferredNamespacePrefix
<http://purl.org/vocab/vann/preferredNamespacePrefix> rdf:type owl:AnnotationProperty .


###  http://purl.org/vocab/vann/preferredNamespaceUri
<http://purl.org/vocab/vann/preferredNamespaceUri> rdf:type owl:AnnotationProperty .


###  http://swrl.stanford.edu/ontologies/3.3/swrla.owl#isRuleEnabled
<http://swrl.stanford.edu/ontologies/3.3/swrla.owl#isRuleEnabled> rdf:type owl:AnnotationProperty .


###  http://www.w3.org/2000/01/rdf-schema#isDefinedBy
rdfs:isDefinedBy rdfs:range <http://www.systemsEngineering.org/isabellefitkau/fisa.owl#Anwendungsregel> .


###  http://www.w3.org/2004/02/skos/core#altLabel
<http://www.w3.org/2004/02/skos/core#altLabel> rdf:type owl:AnnotationProperty .


###  https://purl.org/fisa#anwendungsbereich
:anwendungsbereich rdf:type owl:AnnotationProperty ;
                   rdfs:comment "To explain the application area of regulations, guidelines, prescriptions, etc. Mostly it refers to the first section of a paragaph of the respective legal basis."@en ,
                                "Um den Anwendungsbereich von Vorschriften, Verordnungen, Richtlinien etc. zu erläutern. Meist bezieht es sich auf den ersten Absatz eines Paragaphens der jeweiligen rechtlichen Grundlage."@de ;
                   rdfs:label "anwendungsbereich"@de ,
                              "applicationArea"@en .


###  https://purl.org/fisa#gemäß
:gemäß rdf:type owl:AnnotationProperty ;
       <http://purl.org/dc/terms/description> """Wenn ein Konzept sinngemäß einem bestimmten Paragraphen einer rechtlichen Grundlage entnommen wurde, kann man damit auf ihn verweisen.

Beispiel:
Das sub-Konzept [fisa:Verkaufsstaette] des Konzepts [fisa:Sonderbautatbestand] wurde zur Definition/Beschreibung/Klassifizierung des §2 (4) 4. MBO nötig und verweist daher auf ihn durch diese Annotation."""@de ;
       rdfs:label "accordingTo"@en ,
                  "gemäß"@de ;
       rdfs:range <http://www.systemsEngineering.org/isabellefitkau/fisa.owl#Anwendungsregel> .


###  https://purl.org/fisa#thematik
:thematik rdf:type owl:AnnotationProperty ;
          rdfs:comment """Is used or can be used to unite concepts and attributes under one subject matter. Like e.g. everything that influences each other rescue concept-wise can be marked this way.

Queries can be also supported.

___
Remark:
This is mainly due to the conception of the ontology that knowledge is mostly inferred by reasoners and less class restrictions are used. -> Disjoint classes play a major role using complex rule sets; reasoners can be supported a bit this way. A fine mix of both makes fisa a usable scheme for compliance checks."""@en ,
                       """Wird genutzt oder kann genutzt werden, um Konzepte und Attribute unter eine Thematik zu vereinen. Wie z.B. alles, was Rettungskonzept-mäßig einander beeinflusst kann so gekennzeichnet werden.

Auch ist dies hilfreich bei Abfragen an die Ontologie.

___
Anmerkung:
Dies liegt vor Allem an der Konzeption der Ontologie, dass Wissen größtenteils durch Reasoner geschlussfolgert wird und weniger Klassenrestriktionen verwendet werden. -> Disjointe Klassen spielen unter Nutzung von komplexen Regelsätzen eine große Bedeutung; Reasoner können so ein wenig unterstützt werden. Eine feine Mischung aus beidem macht die fisa zu einem nutzbaren Schema für Compliance Checks."""@de ;
          rdfs:label "subject"@en ,
                     "thematik"@de .


###  https://purl.org/fisa#unter400_meta
:unter400_meta rdf:type owl:AnnotationProperty .


###  https://purl.org/fisa#zurDefinitionVon
:zurDefinitionVon rdf:type owl:AnnotationProperty ;
                  <http://purl.org/dc/terms/description> """Wird zur Definition von Konzepten benötigt.

Beispiel:
Das Datentypattribut [fisa:hatBGFVerkaufsRaeume] dient der Definition des Sonderbautatbestandes Verkaufsstätte, gemäß §2 (4) 4. MBO."""@de ;
                  rdfs:label "toDefine"@en ,
                             "zurDefinitionVon"@de .


#################################################################
#    Object Properties
#################################################################

###  http://www.w3.org/2002/07/owl#differentFrom
owl:differentFrom rdf:type owl:ObjectProperty .


###  http://www.w3.org/2002/07/owl#sameAs
owl:sameAs rdf:type owl:ObjectProperty .


###  https://purl.org/fisa#asARuleOfApplicationFollowedBy
:asARuleOfApplicationFollowedBy rdf:type owl:ObjectProperty ;
                                rdfs:subPropertyOf :isAssessmentBasisOf ;
                                owl:inverseOf :followsRulesOfApplication ;
                                rdfs:comment "Bezug zu Gebäuden und deren Komponenten, die anhand von Verordnungen, Richtlinien und anderen Vorschriften klassifiziert werden müssen. Der typische Bereich von fisa:alsAnwendungsregelBefolgtVon sind Instanzen von fisa:BaulicheAnlage."@de ,
                                             "Relation to buildings and its components needing classification using regulations, guidelines and other directives. The typical range of fisa:asARuleOfApplicationFollowedBy are instances of fisa:StructuralFacility."@en ;
                                rdfs:label "alsAnwendungsregelBefolgtVon"@de ,
                                           "asARuleOfApplicationFollowedBy"@en .


###  https://purl.org/fisa#followsRulesOfApplication
:followsRulesOfApplication rdf:type owl:ObjectProperty ;
                           rdfs:subPropertyOf :hasAssessmentBasis ;
                           rdfs:comment "Bezug zu Verordnungen, Richtlinien und anderen Vorschriften, die für die Klassifizierung von Gebäuden und deren Komponenten benötigt werden. Die typischen Domänen von fisa:folgtAnwendungsregel sind Instanzen von fisa:BaulicheAnlage."@de ,
                                        "Relation to regulations, guidelines and other directives needed for classifiying buildings and its components. The typical domains of fisa:followsRuleOfApplication are instances of fisa:StructuralFacility."@en ;
                           rdfs:label "folgtAnwendungsregel"@de ,
                                      "followsRulesOfApplication"@en .


###  https://purl.org/fisa#hasAccessiblePositionForFireServices
:hasAccessiblePositionForFireServices rdf:type owl:ObjectProperty ;
                                      rdfs:subPropertyOf owl:topObjectProperty ;
                                      owl:inverseOf :isAnAccessiblePositionForFireServicesOf ;
                                      rdfs:comment "Beziehung zu zugänglichen Positionen zum Anleitern für die Feuerwehr in Bezug auf eine Komponente. Die typischen Domänen von fisa:hatAnleiterbareStelle sind Instanzen von fisa:Komponente."@de ,
                                                   "Relation to accessible positions for fire services related to a component. The typical domains of fisa:hasAccessiblePossitionForFireServices are instances of fisa:Component."@en ;
                                      rdfs:label "hasAccessiblePositionForFireServices"@en ,
                                                 "hatAnleitbareStelle"@de .


###  https://purl.org/fisa#hasAssessmentBasis
:hasAssessmentBasis rdf:type owl:ObjectProperty ;
                    rdfs:subPropertyOf owl:topObjectProperty ;
                    owl:inverseOf :isAssessmentBasisOf ;
                    rdfs:range :AssessmentBasis ;
                    rdfs:comment "Beziehung zu den Unterbegriffen einer Beurteilungsgrundlage. Eine Bemessungsgrundlage ist eine Art Dokument, das dem Ingenieur bei der Erstellung des Brandschutznachweises für Baugenehmigungen hilft."@de ,
                                 "Relationship to the subconcepts of an assessment basis. An assessment basis is a a type of document that helps the engineer to develop the fire safety certificate for building permits."@en ;
                    rdfs:label "hasAssessmentBasis"@en ,
                               "hatBeurteilungsgrundlage"@de .


###  https://purl.org/fisa#hasAtticSpace
:hasAtticSpace rdf:type owl:ObjectProperty ;
               rdfs:subPropertyOf <https://w3id.org/bot#containsZone> ;
               rdfs:comment "Beziehung von Dachräumen, die sich in einer Zone befinden. Oft ist die rdfs:domain eine Instanz von bot:Storey oder fisa:StructuralFacility."@de ,
                            "Relation to attic spaces contained in a zone. The typical domains of fisa:hasAtticSpace are instances of bot:Storey or fisa:StructuralFacility."@en ;
               rdfs:label "hasAtticSpace"@en ,
                          "hatDachraum"@de .


###  https://purl.org/fisa#hasBuildingClass
:hasBuildingClass rdf:type owl:ObjectProperty ;
                  rdfs:subPropertyOf :hasClassification ;
                  owl:inverseOf :isBuildingClassOf ;
                  rdfs:domain <https://w3id.org/bot#Zone> ;
                  rdfs:range :BuildingClass ;
                  rdfs:comment "Beziehung zu Klassifizierungen von Gebäuden. Die typischen Domänen von fisa:hatGebäudeklasse sind Instanzen von bot:Gebäude."@de ,
                               "Relationship to classifications of buildings. The typical domains of fisa:hasBuildingClass are instances of bot:Building."@en ;
                  rdfs:label "hasBuildingClass"@en ,
                             "hatGebäudeklasse"@de .


###  https://purl.org/fisa#hasBuildingFacility
:hasBuildingFacility rdf:type owl:ObjectProperty ;
                     rdfs:subPropertyOf <https://w3id.org/bot#containsZone> ;
                     rdfs:comment "Beziehung von baulichen Anlagen, die sich in einer Zone befinden. Oft ist die rdfs:domain eine Instanz von bot:Grundstück."@de ,
                                  "Relation to structural facilities contained in a zone. The typical domains of fisa:hasBuildingFacility are instances of bot:Site."@en ;
                     rdfs:label "hasBuildingFacility"@en ,
                                "hatBaulicheAnlage"@de .


###  https://purl.org/fisa#hasBuildingMaterialClass
:hasBuildingMaterialClass rdf:type owl:ObjectProperty ;
                          rdfs:subPropertyOf :hasClassification ;
                          owl:inverseOf :isBuildingMaterialClassOf ;
                          rdfs:range :BuildingMaterialClass ;
                          rdfs:comment "Beziehung zu Baustoffklassen von Baumaterialn und Komponenten. Die typischen Domänen von fisa:hatBaustoffklasse sind Instanzen von fisa:Komponente."@de ,
                                       "Relationship to building material classes of building materials and components. The typical domains of fisa:hasBuildingMaterialClass are instances of fisa:Component."@en ;
                          rdfs:label "hasBuildingMaterialClass"@en ,
                                     "hatBaustoffklasse"@de .


###  https://purl.org/fisa#hasCavity
:hasCavity rdf:type owl:ObjectProperty ;
           rdfs:subPropertyOf <https://w3id.org/bot#containsZone> ;
           rdfs:domain <https://w3id.org/bot#Zone> ;
           rdfs:range :CavitySpace ;
           rdfs:comment "Beziehung von Hohlräumen, die sich in einer Zone befinden. Oft ist die rdfs:domain eine Instanz von bot:Raum, bot:Geschoss oder bot:Gebäude."@de ,
                        "Relation to cavities contained in a zone. The typical domains of fisa:hasCavity are instances of bot:Space, bot:Storey or fisa:StructuralFacility."@en ;
           rdfs:label "hasCavity"@en ,
                      "hatHohlraum"@de .


###  https://purl.org/fisa#hasClassification
:hasClassification rdf:type owl:ObjectProperty ;
                   rdfs:subPropertyOf owl:topObjectProperty ;
                   owl:inverseOf :isClassificationOf ;
                   rdf:type owl:TransitiveProperty ;
                   rdfs:comment "Beziehung zu Klassifizierungen von Gebäuden und deren Komponenten. Die typischen Domänen von fisa:hatKlassifizierung sind Instanzen von bot:Gebäude oder fisa:Komponente."@de ,
                                "Relationship to classifications of buildings and their components. The typical domains of fisa:hasClassification are instances of bot:Building or fisa:Component."@en ;
                   rdfs:label "hasClassification"@en ,
                              "hatKlassifizierung"@de .


###  https://purl.org/fisa#hasClientSpecification
:hasClientSpecification rdf:type owl:ObjectProperty ;
                        rdfs:subPropertyOf :hasAssessmentBasis ;
                        owl:inverseOf :isClientSpecificationOf ;
                        rdfs:comment "Beziehung zu Spezifikationen von Bauherren, die für die Klassifizierung von Gebäuden und deren Komponenten benötigt werden. Die typischen Domänen von fisa:hatBauherrenVorgabe sind Instanzen von fisa:BaulicheAnlage."@de ,
                                     "Relation to specifications made by clients needed for classifiying buildings and its components. The typical domains of fisa:hasClientSpecification are instances of fisa:StructuralFacility."@en ;
                        rdfs:label "hasClientSpecification"@en ,
                                   "hatBauherrenVorgabe"@de .


###  https://purl.org/fisa#hasComponentType
:hasComponentType rdf:type owl:ObjectProperty ;
                  owl:inverseOf :isComponentTypeOf ;
                  rdfs:domain <https://w3id.org/bot#Element> ;
                  rdfs:range :ComponentType ;
                  rdfs:comment """Links a Component to an Component Type.
The intended use of this relationship is not to be stated explicitly, but to be inferred from its sub-properties. It will, for example, allow one to query for all the possible accessible positions for fire fighting services like an instructable position."""@en ,
                               """Verknüpft eine Komponente mit einem Komponententyp.
Der Verwendungszweck dieser Beziehung muss nicht explizit angegeben werden, sondern ist aus den Untereigenschaften abzuleiten, wenn detaillierte Beschreibung vorhanden sind. Sie ermöglicht beispielsweise die Abfrage aller möglichen zugänglichen Positionen für die Brandbekämpfung wie eine anleiterbare Position."""@de ;
                  rdfs:label "hasComponentType"@en ,
                             "hatKomponententyp"@de .


###  https://purl.org/fisa#hasEscapeRoute
:hasEscapeRoute rdf:type owl:ObjectProperty ;
                owl:inverseOf :isEscapeRouteOf ;
                rdfs:comment """Links a zone with an escape route.
It allows, for example, to query all rooms involved in the escape route and, deriving from this, the adjacent components of these rooms, which in turn receive special requirements."""@en ,
                             """Verknüpft eine Zone mit einem Rettungsweg.
Sie ermöglicht beispielsweise die Abfrage aller am Rettungsweg beteiligten Räume und daraus ableitend die angrenzenden Komponenten dieser Räume, die wiederum spezielle Anforderungen erhalten."""@de ;
                rdfs:label "hasEscapeRoute"@en ,
                           "hatRettungsweg"@de .


###  https://purl.org/fisa#hasFireBehaviour
:hasFireBehaviour rdf:type owl:ObjectProperty ;
                  rdfs:subPropertyOf :hasStructuralFireSafetyMeasure ;
                  rdfs:range :FireBehaviour ;
                  rdfs:comment "Associates a component with the fire behaviour assigned to it (as-is state)."@en ,
                               "Verknüpft eine Komponente mit dem ihr zugewiesenen Brandverhalten (Ist-Zustand)."@de ;
                  rdfs:label "hasFireBehaviour"@en ,
                             "hatBrandverhalten"@de .


###  https://purl.org/fisa#hasFireCompartment
:hasFireCompartment rdf:type owl:ObjectProperty ;
                    rdfs:subPropertyOf <https://w3id.org/bot#containsZone> ;
                    rdfs:domain <https://w3id.org/bot#Zone> ;
                    rdfs:range :FireCompartment ;
                    rdfs:comment "Beziehung von Brandabschnitten, die sich in einer Zone befinden. Oft ist die rdfs:domain eine Instanz von bot:Geschoss oder fisa:BaulicheAnlage."@de ,
                                 "Relation to fire compartments contained in a zone. The typical domains of fisa:hasFireCompartment are instances of bot:Storey or fisa:StructuralFacility."@en ;
                    rdfs:label "hasFireCompartment"@en ,
                               "hatBrandabschnitt"@de .


###  https://purl.org/fisa#hasFireResistance
:hasFireResistance rdf:type owl:ObjectProperty ;
                   rdfs:subPropertyOf :hasStructuralFireSafetyMeasure ;
                   rdfs:range :FireResistance ;
                   rdfs:comment "Associates a component with the fire resistant assigned to it (as-is state)."@en ,
                                "Verknüpft eine Komponente mit der ihr zugewiesenen Feuerwiderstandsfähigkeit (Ist-Zustand)."@de ;
                   rdfs:label "hasFireResistance"@en ,
                              "hatFeuerwiderstandsfähigkeit"@de .


###  https://purl.org/fisa#hasGarage
:hasGarage rdf:type owl:ObjectProperty ;
           rdfs:subPropertyOf :hasBuildingFacility ;
           rdfs:comment "Beziehung von Garagen, die sich in einer Zone befinden. Oft ist die rdfs:domain eine Instanz von bot:Grundstück."@de ,
                        "Relation to garages contained in a zone. The typical domains of fisa:hasGarage are instances of bot:Site."@en ;
           rdfs:label "hasGarage"@en ,
                      "hatGarage"@de .


###  https://purl.org/fisa#hasGeneralInformation
:hasGeneralInformation rdf:type owl:ObjectProperty ;
                       rdfs:subPropertyOf :hasAssessmentBasis ;
                       owl:inverseOf :isGeneralInformationOf ;
                       rdf:type owl:TransitiveProperty ;
                       rdfs:comment "Beziehung zu allgemeinen Informationen, die für die Klassifizierung von Gebäuden und deren Komponenten benötigt werden. Die typischen Domänen von fisa:hatAllgemeineInformation sind Instanzen von fisa:BaulicheAnlage."@de ,
                                    "Relation to general information needed for classifiying buildings and its components. The typical domains of fisa:hasGeneralInformation are instances of fisa:StructuralFacility."@en ;
                       rdfs:label "hasGeneralInformation"@en ,
                                  "hatAllgemeineInformation"@de .


###  https://purl.org/fisa#hasPart
:hasPart rdf:type owl:ObjectProperty ;
         owl:inverseOf :isPartOf ;
         rdfs:comment "Links a Concept to another concept that is in close relationship with it. It will, for example, allow one to query for all the necessary parts of a rescue concepts."@en ,
                      "Verknüpft ein Konzept mit einem anderen Konzept, das in enger Beziehung zu ihm steht. So kann man zum Beispiel alle notwendigen Teile eines Rettungskonzepts abfragen."@de ;
         rdfs:label "hasPart"@en ,
                    "hatTeil"@de .


###  https://purl.org/fisa#hasPlanningDocument
:hasPlanningDocument rdf:type owl:ObjectProperty ;
                     rdfs:subPropertyOf :hasAssessmentBasis ;
                     owl:inverseOf :isPlanningDocumentOf ;
                     rdfs:comment "Beziehung zu Grundrissen und anderen Planungsunterlagen zur Klassifizierung von Gebäuden und deren Komponenten. Die typischen Domänen von fisa:hatPlanungsunterlage sind Instanzen von fisa:BaulicheAnlage oder/und bot:Grundstück."@de ,
                                  "Relation to floor plans and other planning documents for classifiying buildings and its components. The typical domains of fisa:hasPlanningDocument are instances of fisa:StructuralFacility."@en ;
                     rdfs:label "hasPlanningDocument"@en ,
                                "hatPlanungsunterlage"@de .


###  https://purl.org/fisa#hasProtectiveGoal
:hasProtectiveGoal rdf:type owl:ObjectProperty ;
                   rdfs:subPropertyOf owl:topObjectProperty ;
                   rdfs:comment "Links a structural facility to the protective goals it needs to comply with/fulfill."@en ,
                                "Verbindet eine bauliche Anlage mit den Schutzzielen, die sie erfüllen muss."@de ;
                   rdfs:label "hasProtectiveGoal"@en ,
                              "hatSchutzziel"@de .


###  https://purl.org/fisa#hasRequirement
:hasRequirement rdf:type owl:ObjectProperty ;
                rdfs:subPropertyOf owl:topObjectProperty ;
                rdfs:comment "Connects a component to the minimum requirements it must meet."@en ,
                             "Verbindet eine Komponente mit den Mindestanforderungen, die es erfüllen muss."@de ;
                rdfs:label "hasRequirement"@en ,
                           "hatAnforderung"@de .


###  https://purl.org/fisa#hasRequirementOfFireBehaviour
:hasRequirementOfFireBehaviour rdf:type owl:ObjectProperty ;
                               rdfs:subPropertyOf :hasRequirement ;
                               rdfs:comment "Connects a component to the minimum requirements of fire behaviour it must meet."@en ,
                                            "Verbindet eine Komponente und Komponententeile mit den Mindestanforderungen an das Brandverhalten, die es erfüllen muss."@de ;
                               rdfs:label "hasRequirementOfFireBehaviour"@en ,
                                          "hatAnforderungAnBrandverhalten"@de .


###  https://purl.org/fisa#hasRequirementOfFireResistance
:hasRequirementOfFireResistance rdf:type owl:ObjectProperty ;
                                rdfs:subPropertyOf :hasRequirement ;
                                rdfs:range :FireResistance ;
                                rdfs:comment "Connects a component to the minimum requirements of fire resistance it must meet."@en ,
                                             "Verbindet eine Komponente und Komponententeile mit den Mindestanforderungen an den Feuerwiderstand, die es erfüllen muss."@de ;
                                rdfs:label "hasRequirementOfFireResistance"@en ,
                                           "hatAnforderungAnFeuerwiderstandsfähigkeit"@de .


###  https://purl.org/fisa#hasRequirementOfSpaceClosure
:hasRequirementOfSpaceClosure rdf:type owl:ObjectProperty ;
                              rdfs:subPropertyOf :hasRequirement ;
                              rdfs:comment "Connects a component to the minimum requirements of space closure it must meet."@en ,
                                           "Verbindet eine Komponente und Komponententeile mit den Mindestanforderungen an den Raumabschluss, die sie erfüllen muss."@de ;
                              rdfs:label "hasRequirementOfSpaceClosure"@en ,
                                         "hatAnforderungAnRaumabschluss"@de .


###  https://purl.org/fisa#hasRescueConcept
:hasRescueConcept rdf:type owl:ObjectProperty ;
                  owl:inverseOf :isRescueConceptOf ;
                  rdfs:comment "Beziehung von einem Rettungskonzept in Bezug auf eine bauliche Anlage. Die typischen Domänen von fisa:hatRettungskonzept sind Instanzen von fisa:BaulicheAnlage."@de ,
                               "Relationship of a rescue concept with respect to a structural facility. The typical domains of fisa:hasRescueConcept are instances of fisa:StructuralFacility."@en ;
                  rdfs:label "hasRescueConcept"@en ,
                             "hatRettungskonzept"@de .


###  https://purl.org/fisa#hasSmokeCompartment
:hasSmokeCompartment rdf:type owl:ObjectProperty ;
                     rdfs:subPropertyOf <https://w3id.org/bot#containsZone> ;
                     rdfs:comment "Beziehung von Rauchabschnitten, die sich in einer Zone befinden. Oft ist die rdfs:domain eine Instanz von bot:Geschoss oder fisa:BaulicheAnlage."@de ,
                                  "Relation to smoke compartments contained in a zone. The typical domains of fisa:hasSmokeCompartment are instances of bot:Storey or fisa:StructuralFacility."@en ;
                     rdfs:label "hasSmokeCompartment"@en ,
                                "hatRauchabschnitt"@de .


###  https://purl.org/fisa#hasSpaceClosure
:hasSpaceClosure rdf:type owl:ObjectProperty ;
                 rdfs:subPropertyOf :hasStructuralFireSafetyMeasure ;
                 rdfs:domain [ rdf:type owl:Class ;
                               owl:unionOf ( :Closing
                                             :Opening
                                             :Slab
                                             :Wall
                                           )
                             ] ;
                 rdfs:range [ rdf:type owl:Class ;
                              owl:oneOf ( :BauartBrandwand
                                          :feuerbeständig
                                          :feuerhemmend
                                          :hochfeuerbeständig
                                          :hochfeuerhemmend
                                          :ohneAnforderung
                                        )
                            ] ;
                 rdfs:comment "Associates a component with the space closure assigned to it (as-is state)."@en ,
                              "Verknüpft eine Komponente mit dem ihr zugewiesenen Raumabschluss (Ist-Zustand)."@de ;
                 rdfs:label "hasSpaceClosure"@en ,
                            "hatRaumabschluss"@de .


###  https://purl.org/fisa#hasSpaceUsage
:hasSpaceUsage rdf:type owl:ObjectProperty ;
               rdfs:subPropertyOf :hasUsage ;
               owl:inverseOf :isSpaceUsageOf ;
               rdf:type owl:TransitiveProperty ;
               rdfs:range :SpaceUsage ;
               rdfs:comment "Beziehung zu Raumnutzungen, die mit einer Zone verbunden sind. Die typischen Domänen von fisa:hatRaumNutzung sind Instanzen von bot:Raum."@de ,
                            "Relation to space uses associated with a zone. The typical domains of fisa:hasSpaceUsage are instances of bot:Space."@en ;
               rdfs:label "hasSpaceUsage"@en ,
                          "hatRaumNutzung"@de .


###  https://purl.org/fisa#hasSpecialPurposeCondition
:hasSpecialPurposeCondition rdf:type owl:ObjectProperty ;
                            rdfs:subPropertyOf :hasUsage ;
                            owl:inverseOf :isSpecialPurposeConditionOf ;
                            rdfs:range :SpecialPurposeCondition ;
                            rdfs:comment "Beziehung zu Sinderbautatbeständen, die mit einer Zone verbunden sind. Die typischen Domänen von fisa:hatSonderbautatbestand sind Instanzen von fisa:BaulicheAnlage."@de ,
                                         "Relation to special purpose conditions associated with a zone. The typical domains of fisa:hasSpecialPurposeCondition are instances of fisa:StructuralFacility."@en ;
                            rdfs:label "hasSpecialPurposeCondition"@en ,
                                       "hatSonderbautatbestand"@de .


###  https://purl.org/fisa#hasStairSpaceExit
:hasStairSpaceExit rdf:type owl:ObjectProperty ;
                   rdfs:subPropertyOf <https://w3id.org/bot#hasSpace> ;
                   rdfs:domain [ rdf:type owl:Class ;
                                 owl:unionOf ( :NecessaryStairSpace
                                               :SafetyStairSpace
                                             )
                               ] ;
                   rdfs:range [ rdf:type owl:Class ;
                                owl:unionOf ( :StairSpaceExtension
                                              <https://w3id.org/bot#Site>
                                            )
                              ] ;
                   rdfs:comment "Beziehung zu den Arten von Ausgängen, die ein Treppenraum haben kann, da er in einer Zone enthalten ist. Die typischen Domänen und Bereiche von bot:hatTreppenraumAusgang sind auf Instanzen von fisa:NotwendigerTreppenraum oder fisa:Sicherheitstreppenraum als Domänen und fisa:Treppenraumerweiterung oder bot:Grundstück als Bereich beschränkt."@de ,
                                "Relation to the kinds of exits a stair space can have, being contained in a zone. The typical domains and ranges of bot:hasStairSpaceExit are limited to instances of fisa:NecessaryStairSpace or fisa:SafetyStairSpace as domains and fisa:StairSpaceExtension or bot:Site as range."@en ;
                   rdfs:label "hasStairSpaceExit"@en ,
                              "hatTreppenraumAusgang"@de ;
                   :thematik <http://www.systemsEngineering.org/isabellefitkau/fisa.owl#Rettungskonzept> .


###  https://purl.org/fisa#hasStandardConstructionType
:hasStandardConstructionType rdf:type owl:ObjectProperty ;
                             rdfs:subPropertyOf :hasUsage ;
                             owl:inverseOf :isStandardConstructionTypeOf ;
                             rdfs:range :StandardConstructionType ;
                             rdfs:comment "Beziehung zu Standardbautypen, die mit einer Zone verbunden sind. Die typischen Domänen von fisa:hatStandardbauArt sind Instanzen von fisa:BaulicheAnlage."@de ,
                                          "Relation to standard construction types associated with a zone. The typical domains of fisa:hasStandardConstructionType are instances of fisa:StructuralFacility."@en ;
                             rdfs:label "hasStandardConstructionType"@en ,
                                        "hatStandardbauArt"@de .


###  https://purl.org/fisa#hasStructuralFireSafetyMeasure
:hasStructuralFireSafetyMeasure rdf:type owl:ObjectProperty ;
                                rdfs:subPropertyOf owl:topObjectProperty ;
                                rdfs:comment "Associates a component with the measures assigned to it (actual state)."@en ,
                                             "Verbindet eine Komponente mit den Anforderungeneigenschaften, die ihr zugewiesen wurden (Ist-Zustand)."@de ;
                                rdfs:label "hasStructuralFireSafetyMeasure"@en ,
                                           "hatBaulicheBrandschutzmaßnahme"@de .


###  https://purl.org/fisa#hasUsage
:hasUsage rdf:type owl:ObjectProperty ;
          rdfs:subPropertyOf owl:topObjectProperty ;
          owl:inverseOf :isUsageOf ;
          rdfs:range :Usage ;
          rdfs:comment "Beziehung von Nutzungen, die mit einer Zone verbunden sind. Die typischen Domänen von bot:hatNutzung sind Instanzen von bot:Zone."@de ,
                       "Relation to usages related to a zone. The typical domains of fisa:hasUsage are instances of bot:Zone."@en ;
          rdfs:label "hasUsage"@en ,
                     "hatNutzung"@de .


###  https://purl.org/fisa#hasUtilizationPurpose
:hasUtilizationPurpose rdf:type owl:ObjectProperty ;
                       rdfs:subPropertyOf :hasUsage ;
                       owl:inverseOf :isUtilizationPurposeOf ;
                       rdfs:range :UtilizationPurpose ;
                       rdfs:comment "Beziehung zu Nutzungszwecken, die mit einer Zone verbunden sind. Die typischen Domänen von fisa:hatNutzungszweck sind Instanzen von bot:Zone."@de ,
                                    "Relation to usage purposes associated with a zone. The typical domains of fisa:hasUsagePurpose are instances of bot:Zone."@en ;
                       rdfs:label "hasUtilizationPurpose"@en ,
                                  "hatNutzungszweck"@de .


###  https://purl.org/fisa#hasUtilizationSpace
:hasUtilizationSpace rdf:type owl:ObjectProperty ;
                     rdfs:subPropertyOf <https://w3id.org/bot#containsZone> ;
                     owl:inverseOf :isUtilizationSpaceOf ;
                     rdfs:domain <https://w3id.org/bot#Zone> ;
                     rdfs:range :UtilizationUnit ;
                     rdfs:comment "Beziehung von Nutzungseinheiten, die sich in einer Zone befinden. Oft ist die rdfs:domain eine Instanz von bot:Geschoss oder fisa:BaulicheAnlage."@de ,
                                  "Relation to utilization spaces contained in a zone. The typical domains of fisa:hasUtilizationSpace are instances of bot:Storey or fisa:StructuralFacility."@en ;
                     rdfs:label "hasUtilizationSpace"@en ,
                                "hatNutzungseinheit"@de .


###  https://purl.org/fisa#isAnAccessiblePositionForFireServicesOf
:isAnAccessiblePositionForFireServicesOf rdf:type owl:ObjectProperty ;
                                         rdfs:subPropertyOf owl:topObjectProperty ;
                                         rdfs:comment "Beziehung einer Komponente zu zugänglichen Positionen, anleiterbaren Stellen, für Feuerwehrdienste. Der typische Bereich von fisa:istAnleiterbareStelleVon sind Instanzen von fisa:Komponente."@de ,
                                                      "Relation of a component to accessible positions for fire services related . The typical range of fisa:ifAccessiblePossitionForFireServicesOf are instances of fisa:Component."@en ;
                                         rdfs:label "isAnAccessiblePositionForFireServicesOf"@en ,
                                                    "istAnleitbareStelleVon"@de .


###  https://purl.org/fisa#isAssessmentBasisOf
:isAssessmentBasisOf rdf:type owl:ObjectProperty ;
                     rdfs:subPropertyOf owl:topObjectProperty ;
                     rdfs:comment "Beziehung zu dem Bereich, auf den sich die Unterkonzepte einer Bemessungsgrundlage beziehen. Eine Bemessungsgrundlage ist eine Art Dokument, das dem Ingenieur hilft, den Brandschutznachweis für die Baugenehmigung zu erstellen. fisa:istBemessungsgrundlageFür ist ein typischer Bereich von Instanzen von fisa:BaulicheAnlage."@de ,
                                  "Relationship to the range that subconcepts of an assessment basis relate to. An assessment basis is a a type of document that helps the engineer to develop the fire safety certificate for building permits.The typical range of fisa:isAssessmentBasisOf are instances of fisa:StructuralFacility."@en ;
                     rdfs:label "isAssessmentBasisOf"@en ,
                                "istBeurteilungsgrundlageVon"@de .


###  https://purl.org/fisa#isBasedOn
:isBasedOn rdf:type owl:ObjectProperty ;
           rdfs:subPropertyOf owl:topObjectProperty ;
           owl:inverseOf :isBasisOf ;
           rdf:type owl:TransitiveProperty ;
           rdfs:comment "Beziehung zwischen zwei Konzepten, bei dem das eine Konzept nur beschrieben werden kann, wenn das andere Konzept vorhanden und beschrieben ist."@de ,
                        "Relation between two concepts where one concept can only be described if the other concept is present and described."@en ;
           rdfs:label "basiertAuf"@de ,
                      "isBasedOn"@en .


###  https://purl.org/fisa#isBasisOf
:isBasisOf rdf:type owl:ObjectProperty ;
           rdfs:subPropertyOf owl:topObjectProperty ;
           rdf:type owl:TransitiveProperty ;
           rdfs:comment "Beziehung zwischen zwei Begriffen, wobei der andere Begriff nur dann beschrieben werden kann, wenn dieser Begriff vorhanden und beschrieben ist."@de ,
                        "Relation between two concepts where the other concept can only be described if this concept is present and described."@en ;
           rdfs:label "isBasisOf"@en ,
                      "istGrundlageVon"@de .


###  https://purl.org/fisa#isBuildingClassOf
:isBuildingClassOf rdf:type owl:ObjectProperty ;
                   rdfs:subPropertyOf :isClassificationOf ;
                   rdfs:comment "Beziehung zu Gebäuden und deren Gebäudeklassen. Der typische Bereich von fisa:istGebäudeklasseVon sind Instanzen von bot:Gebäude."@de ,
                                "Relationship to buildings and their building classifications. The typical range of fisa:isBuildingClassOf are instances of bot:Building."@en ;
                   rdfs:label "isBuildingClassOf"@en ,
                              "istGebäudeklasseVon"@de .


###  https://purl.org/fisa#isBuildingMaterialClassOf
:isBuildingMaterialClassOf rdf:type owl:ObjectProperty ;
                           rdfs:subPropertyOf :isClassificationOf ;
                           rdfs:comment "Beziehung zu Komponenten und deren Baustoffklassen. Der typische Bereich von fisa:istBaustoffklasseVon sind Instanzen von fisa:Komponente."@de ,
                                        "Relationship to components and their classifications. The typical range of fisa:isBuildingMaterialClassOf are instances of fisa:Component."@en ;
                           rdfs:label "isBuildingMaterialClassOf"@en ,
                                      "istBaustoffklasseVon"@de .


###  https://purl.org/fisa#isClassificationOf
:isClassificationOf rdf:type owl:ObjectProperty ;
                    rdfs:subPropertyOf owl:topObjectProperty ;
                    rdfs:domain :Classification ;
                    rdfs:comment "Beziehung zu Gebäuden und deren Komponenten und deren Klassifizierungen. Der typische Bereich von fisa:istKlassifizierungVon sind Instanzen von bot:Gebäude oder fisa:Komponente."@de ,
                                 "Relationship to buildings and their components and their classifications. The typical range of fisa:isClassificationOf are instances of bot:Building or fisa:Component."@en ;
                    rdfs:label "isClassificationOf"@en ,
                               "istKlassifizierungVon"@de .


###  https://purl.org/fisa#isClientSpecificationOf
:isClientSpecificationOf rdf:type owl:ObjectProperty ;
                         rdfs:subPropertyOf :isAssessmentBasisOf ;
                         rdfs:comment "Bezug zu Gebäuden und deren Komponenten, die von Spezifierungen von Bauherren beeinflusst werden. Der typische Bereich von fisa:istBauherrenVorgabeVon sind Instanzen von fisa:BaulicheAnlage."@de ,
                                      "Relation to buildings and its components influenced by specifications of clients. The typical range of fisa:isClientSpecificationOf are instances of fisa:StructuralFacility."@en ;
                         rdfs:label "isClientSpecificationOf"@en ,
                                    "istBauherrenVorgabeVon"@de .


###  https://purl.org/fisa#isComponentTypeOf
:isComponentTypeOf rdf:type owl:ObjectProperty ;
                   rdfs:subPropertyOf owl:topObjectProperty ;
                   rdfs:comment "Links a Component Type to an Component."@en ,
                                "Verknüpft einen Komponententyp mit einer Komponente."@de ;
                   rdfs:label "isComponentTypeOf"@en ,
                              "istKomponentenTypVon"@de .


###  https://purl.org/fisa#isEscapeRouteOf
:isEscapeRouteOf rdf:type owl:ObjectProperty ;
                 rdfs:comment "Links an escape route to a zone."@en ,
                              "Verknüpft einen Rettungsweg mit einer Zone."@de ;
                 rdfs:label "isEscapeRouteOf"@en ,
                            "istRettungswegVon"@de .


###  https://purl.org/fisa#isGeneralInformationOf
:isGeneralInformationOf rdf:type owl:ObjectProperty ;
                        rdfs:subPropertyOf :isAssessmentBasisOf ;
                        rdfs:comment "Bezug zu Gebäuden und deren Komponenten, die anhand von allgemeinen Informationen klassifiziert werden müssen. Der typische Bereich von fisa:istAllgemeineInformationVon sind Instanzen von fisa:BaulicheAnlage."@de ,
                                     "Relation to buildings and its components needing classification using general information. The typical range of fisa:isGeneralInformationof are instances of fisa:StructuralFacility."@en ;
                        rdfs:label "isGeneralInformationOf"@en ,
                                   "istAllgemeineInformationVon"@de .


###  https://purl.org/fisa#isLessFireResistantThan
:isLessFireResistantThan rdf:type owl:ObjectProperty ;
                         owl:inverseOf :isMoreFireResistantThan ;
                         rdfs:comment """Relation of descending fire resistance of components.
Used to create a kind of list from instances of fire resistance."""@en ,
                                      """Relation von absteigendem Feuerwiderstandsfähigkeit von Komponenten.
Wird genutzt, um aus Instanzen der Feuerwiderstandsfähigkeiten eine Art Liste zu erstellen."""@de ;
                         rdfs:label "isLessFireResistantThan"@en ,
                                    "istWenigerFeuerbeständigerAls"@de .


###  https://purl.org/fisa#isLessFlammableThan
:isLessFlammableThan rdf:type owl:ObjectProperty ;
                     owl:inverseOf :isMoreFlammableThan ;
                     rdfs:comment """Relation of descending fire behavior of components.
Used to create a kind of list from instances of fire behavior."""@en ,
                                  """Relation von absteigendem Brandverhalten von Komponenten.
Wird genutzt, um aus Instanzen des Brandverhaltens eine Art Liste zu erstellen."""@de ;
                     rdfs:label "isLessFlammableThan"@en ,
                                "istWenigerBrennbarerAls"@de ;
                     <http://www.w3.org/2004/02/skos/core#altLabel> "isLessCombustibleThan"@en .


###  https://purl.org/fisa#isMoreFireResistantThan
:isMoreFireResistantThan rdf:type owl:ObjectProperty ,
                                  owl:TransitiveProperty ;
                         rdfs:domain :FireResistance ;
                         rdfs:range :FireResistance ;
                         rdfs:comment """Relation of ascending fire resistance of components.
Used to create a kind of list from instances of fire resistance."""@en ,
                                      """Relation von aufsteigendem Feuerwiderstandsfähigkeit von Komponenten.
Wird genutzt, um aus Instanzen der Feuerwiderstandsfähigkeiten eine Art Liste zu erstellen."""@de ;
                         rdfs:label "isMoreFireResistantThan"@en ,
                                    "istFeuerbeständigerAls"@de .


###  https://purl.org/fisa#isMoreFlammableThan
:isMoreFlammableThan rdf:type owl:ObjectProperty ,
                              owl:TransitiveProperty ;
                     rdfs:domain :FireBehaviour ;
                     rdfs:range :FireBehaviour ;
                     rdfs:comment """Relation of ascending fire behavior of components.
Used to create a kind of list from instances of fire behavior."""@en ,
                                  """Relation von aufsteigendem Brandverhalten von Komponenten.
Wird genutzt, um aus Instanzen des Brandverhaltens eine Art Liste zu erstellen."""@de ;
                     rdfs:label "isMoreFlammableThan"@en ,
                                "istBrennbarerAls"@de ;
                     <http://www.w3.org/2004/02/skos/core#altLabel> "isMoreCombustibleThan"@en .


###  https://purl.org/fisa#isNeededBy
:isNeededBy rdf:type owl:ObjectProperty ;
            rdfs:subPropertyOf owl:topObjectProperty ;
            owl:inverseOf :needs ;
            rdf:type owl:TransitiveProperty ;
            rdfs:comment "Relation of required concepts to describe other concepts."@en ,
                         "Relation von benötigten Konzepten, um andere Konzepte zu beschreiben."@de ;
            rdfs:label "isNeededBy"@en ,
                       "wirdBenötigtVon"@de .


###  https://purl.org/fisa#isPartOf
:isPartOf rdf:type owl:ObjectProperty ;
          rdfs:comment "Links a Concept to another concept that is in close relationship with it."@en ,
                       "Verknüpft ein Konzept mit einem anderen Konzept, das in enger Beziehung zu ihm steht."@de ;
          rdfs:label "isPartOf"@en ,
                     "istTeilVon"@de .


###  https://purl.org/fisa#isPermittedWith
:isPermittedWith rdf:type owl:ObjectProperty ;
                 rdfs:subPropertyOf owl:topObjectProperty ;
                 rdfs:comment "Connects a component to the requirements it is permitted to have under certain circumstances/actual states."@en ,
                              "Verbindet eine Komponente mit den Anforderungen, die sie unter bestimmten Umständen/Ist-Zuständen haben darf."@de ;
                 rdfs:label "isPermittedWith"@en ,
                            "istZulässigMit"@de .


###  https://purl.org/fisa#isPermittedWithFireBehaviour
:isPermittedWithFireBehaviour rdf:type owl:ObjectProperty ;
                              rdfs:subPropertyOf :isPermittedWith ;
                              rdfs:range :FireBehaviour ;
                              rdfs:comment "Connects a component to the requirements of fire behaviour it is permitted to have under certain circumstances/actual states."@en ,
                                           "Verbindet eine Komponente mit den Anforderungen an das Brandverhalten, die sie unter bestimmten Umständen/Ist-Zuständen haben darf."@de ;
                              rdfs:label "isPermittedWithFireBehaviour"@en ,
                                         "istZulässigMitBrandverhalten"@de .


###  https://purl.org/fisa#isPermittedWithFireResistance
:isPermittedWithFireResistance rdf:type owl:ObjectProperty ;
                               rdfs:subPropertyOf :isPermittedWith ;
                               rdfs:range :FireResistance ;
                               rdfs:comment "Connects a component to the requirements of fire resistance it is permitted to have under certain circumstances/actual states."@en ,
                                            "Verbindet eine Komponente mit den Anforderungen an die Feuerwiderstandsfähigkeit, die sie unter bestimmten Umständen/Ist-Zuständen haben darf."@de ;
                               rdfs:label "isPermittedWithFireResistance"@en ,
                                          "istZulässigMitFeuerwiderstandsfähigkeit"@de .


###  https://purl.org/fisa#isPermittedWithSpaceClosure
:isPermittedWithSpaceClosure rdf:type owl:ObjectProperty ;
                             rdfs:subPropertyOf :isPermittedWith ;
                             rdfs:comment "Connects a component to the requirements of space closure it is permitted to have under certain circumstances/actual states."@en ,
                                          "Verbindet eine Komponente mit den Anforderungen an den Raumabschluss, die sie unter bestimmten Umständen/Ist-Zuständen haben darf."@de ;
                             rdfs:label "isPermittedWithSpaceClosure"@en ,
                                        "istZulässigMitRaumabschluss"@de .


###  https://purl.org/fisa#isPlanningDocumentOf
:isPlanningDocumentOf rdf:type owl:ObjectProperty ;
                      rdfs:subPropertyOf :isAssessmentBasisOf ;
                      rdfs:comment "Bezug zu Gebäuden und deren Komponenten und den verbundenen Planungsunterlagen. Der typische Bereich von fisa:istPlanungsunterlageVon sind Instanzen von fisa:BaulicheAnlage."@de ,
                                   "Relation to buildings and its components and its related planning documents. The typical range of fisa:isPlanningDocumentOf are instances of fisa:StructuralFacility."@en ;
                      rdfs:label "isPlanningDocumentOf"@en ,
                                 "istPlanungsunterlageVon"@de .


###  https://purl.org/fisa#isRescueConceptOf
:isRescueConceptOf rdf:type owl:ObjectProperty ;
                   rdfs:comment "Beziehung einer baulichen Anlage zu einem Rettungskonzept. Der typische Bereich von fisa:istRettungskonzeptVon sind Instanzen von fisa:BaulicheAnlage."@de ,
                                "Relation of a structural facility with respect to the rescue concept . The typical range of fisa:isRescueConceptOf are instances of fisa:StructuralFacility."@en ;
                   rdfs:label "isRescueConceptOf"@en ,
                              "istRettungskonzeptVon"@de .


###  https://purl.org/fisa#isSpaceUsageOf
:isSpaceUsageOf rdf:type owl:ObjectProperty ;
                rdfs:subPropertyOf :isUsageOf ;
                rdfs:comment "Beziehung zu Zonen, die mit einer Raumnutzungen verbunden sind. Die typischen Bereiche von fisa:istRaumNutzungVon sind Instanzen von bot:Raum."@de ,
                             "Relation of a zone associated with space uses. The typical range of fisa:isSpaceUsageOf are instances of bot:Space."@en ;
                rdfs:label "isSpaceUsageOf"@en ,
                           "istRaumNutzungVon"@de .


###  https://purl.org/fisa#isSpecialPurposeConditionOf
:isSpecialPurposeConditionOf rdf:type owl:ObjectProperty ;
                             rdfs:subPropertyOf :isUsageOf ;
                             rdfs:comment "Beziehung zu Zonen, die mit Sinderbautatbeständen verbunden sind. Die typischen Bereiche von fisa:istSonderbautatbestandVon sind Instanzen von fisa:BaulicheAnlage."@de ,
                                          "Relation of a zone associated with special purpose conditions. The typical range of fisa:isSpecialPurposeConditionOf are instances of fisa:StructuralFacility."@en ;
                             rdfs:label "isSpecialPurposeConditionOf"@en ,
                                        "istSonderbautatbestandVon"@de .


###  https://purl.org/fisa#isStandardConstructionTypeOf
:isStandardConstructionTypeOf rdf:type owl:ObjectProperty ;
                              rdfs:subPropertyOf :isUsageOf ;
                              rdfs:comment "Beziehung von Zonen, die mit Standardbautypen verbunden sind. Die typischen Bereiche von fisa:istStandardbauArt sind Instanzen von fisa:BaulicheAnlage."@de ,
                                           "Relation of a zone associated with standard construction types. The typical range of fisa:isStandardConstructionTypeOf are instances of fisa:StructuralFacility."@en ;
                              rdfs:label "isStandardConstructionTypeOf"@en ,
                                         "istStandardbauArtVon"@de .


###  https://purl.org/fisa#isSubElementOf
:isSubElementOf rdf:type owl:ObjectProperty ;
                owl:inverseOf <https://w3id.org/bot#hasSubElement> ;
                rdfs:domain :Component ;
                rdfs:range :Component ;
                rdfs:comment "Relation between several building elements, either one element hosting another (e.g. window being hosted by a wall) or a subcomposition of a building element into bigger parts (e.g. a fan has a sub part that is an air handling unit)."@en ;
                rdfs:label "isSub-ElementOf"@en ,
                           "istUnterbauteilVon"@de .


###  https://purl.org/fisa#isUsageOf
:isUsageOf rdf:type owl:ObjectProperty ;
           rdfs:subPropertyOf owl:topObjectProperty ;
           rdfs:comment "Beziehung zwischen einer Zone und einer Nutzung. Der typische Bereich von fisa:istNutzungVon sind Instanzen von bot:Zone."@de ,
                        "Relation of a zone  to a usage. The typical range of fisa:isUsageOf are instances of bot:Zone."@en ;
           rdfs:label "isUsageOf"@en ,
                      "istNutzungVon"@de .


###  https://purl.org/fisa#isUtilizationPurposeOf
:isUtilizationPurposeOf rdf:type owl:ObjectProperty ;
                        rdfs:subPropertyOf :isUsageOf ;
                        rdfs:domain :UtilizationPurpose ;
                        rdfs:comment "Beziehung von Zonen, die mit einem Nutzungszwecken verbunden sind. Die typischen Bereiche von fisa:istNutzungszweckVon sind Instanzen von bot:Zone."@de ,
                                     "Relation of a zone associated with usage purposese. The typical range of fisa:ifUsagePurposeOf are instances of bot:Zone."@en ;
                        rdfs:label "isUtilizationPurposeOf"@en ,
                                   "istNutzungszweckVon"@de .


###  https://purl.org/fisa#isUtilizationSpaceOf
:isUtilizationSpaceOf rdf:type owl:ObjectProperty ;
                      rdfs:subPropertyOf owl:topObjectProperty ;
                      rdfs:comment "Beziehung von Zonen, in der sich Nutzungseinheiten befinden. Oft ist der Bereich von fisa:istNutzungseinheitVon eine Instanz von bot:Geschoss oder fisa:BaulicheAnlage."@de ,
                                   "Relation to a zone, which contains utilization spaces. The typical range of fisa:isUtilizationSpaceOf are instances of bot:Storey or fisa:StructuralFacility."@en ;
                      rdfs:label "isUtilizationSpaceOf"@en ,
                                 "istNutzungseinheitVon"@de .


###  https://purl.org/fisa#needs
:needs rdf:type owl:ObjectProperty ;
       rdfs:subPropertyOf owl:topObjectProperty ;
       rdf:type owl:TransitiveProperty ;
       rdfs:comment "Relation of required concepts to describe other concepts."@en ,
                    "Relation von benötigten Konzepten, um andere Konzepte zu beschreiben."@de ;
       rdfs:label "benötigt"@de ,
                  "needs"@en .


###  https://purl.org/fisa#remoteZone
:remoteZone rdf:type owl:ObjectProperty ;
            rdfs:domain <https://w3id.org/bot#Zone> ;
            rdfs:range <https://w3id.org/bot#Zone> ;
            rdfs:comment "Beziehung zwischen zwei Zonen, die keine gemeinsame Schnittstelle haben und voneinander entfernt sind, sich aber gegenseitig beeinflussen."@de ,
                         "Relationship between two zones that share no common interface and are remote to one another, but influence each other."@en ;
            rdfs:label "entfernteZone"@de ,
                       "remoteZone"@en .


###  https://w3id.org/bot#adjacentElement
<https://w3id.org/bot#adjacentElement> rdf:type owl:ObjectProperty ;
                                       rdfs:subPropertyOf <https://w3id.org/bot#hasElement> ;
                                       owl:propertyDisjointWith <https://w3id.org/bot#intersectingElement> ;
                                       rdfs:comment <https://w3id.org/bot#> ,
                                                    "Beziehung zwischen einer Zone und dessen angrenzenden Komponenten. Die Komponenten begrenzen die Zone."@de ,
                                                    "Relation between a zone and its adjacent building components, bounding the zone."@en ;
                                       rdfs:label "adjacentElement"@en ,
                                                  "benachbartesBauteil"@de .


###  https://w3id.org/bot#adjacentZone
<https://w3id.org/bot#adjacentZone> rdf:type owl:ObjectProperty ,
                                             owl:SymmetricProperty ;
                                    rdfs:domain <https://w3id.org/bot#Zone> ;
                                    rdfs:range <https://w3id.org/bot#Zone> ;
                                    owl:propertyDisjointWith <https://w3id.org/bot#intersectsZone> ;
                                    rdfs:comment "Beziehung zwischen zwei Zonen die eine gemeinsame Grenzfläche haben, aber sich nicht schneiden."@de ,
                                                 "Relationship between two zones that share a common interface, but do not intersect."@en ;
                                    rdfs:isDefinedBy <https://w3id.org/bot#> ;
                                    rdfs:label "adjacentZone"@en ,
                                               "angrenzendeZone"@de .


###  https://w3id.org/bot#containsElement
<https://w3id.org/bot#containsElement> rdf:type owl:ObjectProperty ;
                                       rdfs:subPropertyOf <https://w3id.org/bot#hasElement> ;
                                       owl:propertyChainAxiom ( <https://w3id.org/bot#containsZone>
                                                                <https://w3id.org/bot#containsElement>
                                                              ) ;
                                       rdfs:comment <https://w3id.org/bot#> ,
                                                    "Beziehung einer Zone zu einer Komponente, dass es enthält."@de ,
                                                    "Relation to a building component contained in a zone."@en ;
                                       rdfs:label "containsElement"@en ,
                                                  "enthältBauteil"@de .


###  https://w3id.org/bot#containsZone
<https://w3id.org/bot#containsZone> rdf:type owl:ObjectProperty ,
                                             owl:TransitiveProperty ;
                                    rdfs:domain <https://w3id.org/bot#Zone> ;
                                    rdfs:range <https://w3id.org/bot#Zone> ;
                                    rdfs:comment "Beziehung zwischen Zonen, wobei eine die andere enthält. Zum Beispiel kann eine Raumzone in einer Geschossszone enthalten sein, die wiederrum in einer Gebäudezone enthalten ist. bot:containsZone is eine transitive Beziehung, dass heisst zwischen der Raumzone im vorherigen Beispiel und der Gebäudezone besteht auch die Beziehung bot:containsZone."@de ,
                                                 "Relationship to the subzones of a major zone. A space zone could for instance be contained in a storey zone which is further contained in a building zone. bot:containsZone is a transitive property. This implies that in the previous example a bot:containsZone relationship holds between the space zone and the building zone."@en ;
                                    rdfs:isDefinedBy <https://w3id.org/bot#> ;
                                    rdfs:label "containsZone"@en ,
                                               "enthältZone"@de .


###  https://w3id.org/bot#hasBuilding
<https://w3id.org/bot#hasBuilding> rdf:type owl:ObjectProperty ;
                                   rdfs:subPropertyOf :hasBuildingFacility ;
                                   rdfs:domain <https://w3id.org/bot#Zone> ;
                                   rdfs:range <https://w3id.org/bot#Building> ;
                                   rdfs:comment <https://w3id.org/bot#> ,
                                                "Beziehung zwischen Gebäuden, die in einer Zone enthalten sind. Oft ist hier die rdfs:domain eine Instanz von bot:Site."@de ,
                                                "Relation to buildings contained in a zone. The typical domains of bot:hasBuilding are instances of bot:Site."@en ;
                                   rdfs:label "hasBuilding"@en ,
                                              "hatGebäude"@de .


###  https://w3id.org/bot#hasElement
<https://w3id.org/bot#hasElement> rdf:type owl:ObjectProperty ;
                                  rdfs:domain <https://w3id.org/bot#Zone> ;
                                  rdfs:range :Component ;
                                  owl:propertyChainAxiom ( <https://w3id.org/bot#containsZone>
                                                           <https://w3id.org/bot#hasElement>
                                                         ) ;
                                  rdfs:comment <https://w3id.org/bot#> ,
                                               """Beziehung zwischen einer Zone und einer Komponente, dass entweder in der Zone enthalten ist, angrenzend ist, oder sich mit ihr schneidet. Diese Beziehung sollte nicht explizit benutzt werden, sondern ergibt sich implizit aus den Unterbeziehungen. Es ermöglicht, zum Beispiel, dass mit einer Abfrage alle Türen eines Gebäudes, die sich mit einer Zone schneiden ermittelt werden können.

__
In FiSa und seinem Schichtensystem lautet der Bereich fisa:Komponente anstelle von bot:Bauteil."""@de ,
                                               """Links a Zone to an Component that is either contained in, adjacent to or intersecting with the Zone. The intended use of this relationship is not to be stated explicitly, but to be inferred from its sub-properties. It will, for example, allow one to query for all the doors of a building given that they have an adjacency to spaces of the building.


__
In FiSa and its layering system, the range is fisa:Component instead of bot:BuildingElement."""@en ;
                                  rdfs:label "hasElement"@en ,
                                             "hatBauteil"@de .


###  https://w3id.org/bot#hasSpace
<https://w3id.org/bot#hasSpace> rdf:type owl:ObjectProperty ;
                                rdfs:subPropertyOf <https://w3id.org/bot#containsZone> ;
                                rdfs:domain <https://w3id.org/bot#Zone> ;
                                rdfs:range <https://w3id.org/bot#Space> ;
                                rdfs:comment <https://w3id.org/bot#> ,
                                             "Beziehung von Räumen, die sich in einer Zone befinden. Oft ist die rdfs:domain eine Instanz von bot:Storey oder bot:Building."@de ,
                                             "Relation to spaces contained in a zone. The typical domains of bot:hasSpace are instances of bot:Storey or bot:Building."@en ;
                                rdfs:label "hasSpace"@en ,
                                           "hatRaum"@de .


###  https://w3id.org/bot#hasStorey
<https://w3id.org/bot#hasStorey> rdf:type owl:ObjectProperty ;
                                 rdfs:subPropertyOf <https://w3id.org/bot#containsZone> ;
                                 rdfs:domain <https://w3id.org/bot#Zone> ;
                                 rdfs:range <https://w3id.org/bot#Storey> ;
                                 rdfs:comment <https://w3id.org/bot#> ,
                                              "Beziehung zwischen Geschossen, die in einer Zone enthalten sind. Oft ist die rdfs:domain eine Instanz von bot:Building."@de ,
                                              "Relation to storeys contained in a zone. The typical domains of bot:hasStorey are instances of bot:Building."@en ;
                                 rdfs:label "hasStorey"@en ,
                                            "hatGeschoss"@de .


###  https://w3id.org/bot#hasSubElement
<https://w3id.org/bot#hasSubElement> rdf:type owl:ObjectProperty ;
                                     rdfs:domain :Component ;
                                     rdfs:range :Component ;
                                     rdfs:comment <https://w3id.org/bot#> ,
                                                  "Beziehung zwischen mehreren Komponenten, wobei entweder eines das andere enthält (z.B. eine Wand enthält ein Fenster) oder ein ganzes, das aus anderen Teilen zusammen gesetzt ist (z.B. eine Lüftungsanlage hat eine Komponente Lüfter)."@de ,
                                                  "Relation between several building components, either one element hosting another (e.g. a wall hosts a window) or a subcomposition of a building element into smaller parts (e.g. an air handling unit has as a part a fan)."@en ;
                                     rdfs:label "hasSub-Element"@en ,
                                                "hatUnterbauteil"@de ;
                                     <http://www.w3.org/2004/02/skos/core#altLabel> "hatUnterkomponente"@de .


###  https://w3id.org/bot#interfaceOf
<https://w3id.org/bot#interfaceOf> rdf:type owl:ObjectProperty ;
                                   rdfs:domain <https://w3id.org/bot#Interface> ;
                                   rdfs:comment <https://w3id.org/bot#> ,
                                                "Beziehung zwischen einer Schnittstelle und einem anderen Ding (Zone, Komponente oder owl:Thing)."@de ,
                                                "Relationship between an interface and another thing (building zone, component or owl:Thing)"@en ;
                                   rdfs:label "SchnittstelleVon"@de ,
                                              "interfaceOf"@en .


###  https://w3id.org/bot#intersectingElement
<https://w3id.org/bot#intersectingElement> rdf:type owl:ObjectProperty ;
                                           rdfs:subPropertyOf <https://w3id.org/bot#hasElement> ;
                                           rdfs:comment <https://w3id.org/bot#> ,
                                                        "Beziehung zwischen einer Zone und einer Komponente, das die Zone schneidet."@de ,
                                                        "Relation between a Zone and a building component that intersects it."@en ;
                                           rdfs:label "intersectingElement"@en ,
                                                      "schneidendesBauteil"@de .


###  https://w3id.org/bot#intersectsZone
<https://w3id.org/bot#intersectsZone> rdf:type owl:ObjectProperty ,
                                               owl:SymmetricProperty ;
                                      rdfs:domain <https://w3id.org/bot#Zone> ;
                                      rdfs:range <https://w3id.org/bot#Zone> ;
                                      rdfs:comment <https://w3id.org/bot#> ,
                                                   "Beziehung zwischen zwei Zonen, die sich schneiden. Zum Beispiel schneidet eine Treppe verschiedene Geschosse."@de ,
                                                   "Relationship between two zones whose 3D extent intersect. For example, a stairwell intersects different storeys."@en ;
                                      rdfs:label "intersectsZone"@en ,
                                                 "sichSchneidendeZone"@de .


#################################################################
#    Data properties
#################################################################

###  https://purl.org/fisa#accessibleForFireServices
:accessibleForFireServices rdf:type owl:DatatypeProperty ;
                           rdfs:subPropertyOf owl:topDataProperty ;
                           rdfs:domain [ rdf:type owl:Class ;
                                         owl:unionOf ( :Door
                                                       :Opening
                                                       :Parapet
                                                       :Window
                                                     )
                                       ] ;
                           rdfs:range xsd:boolean ;
                           rdfs:comment "Beschreibt ob eine Komponente anleiterbar ist."@de ,
                                        "Describes whether a component is instructable and therefore accessible for fire services."@en ;
                           rdfs:label "accessibleForFireServices"@en ,
                                      "istAnleiterbar"@de ;
                           :thematik <http://www.systemsEngineering.org/isabellefitkau/fisa.owl#Rettungskonzept> .


###  https://purl.org/fisa#hasAge
:hasAge rdf:type owl:DatatypeProperty ;
        rdfs:subPropertyOf owl:topDataProperty ;
        rdfs:range xsd:integer ;
        rdfs:comment """Beschreibt, ob es sich um Einrichtungen handelt, die mit alten Menschen zu tun hat.

(kann durch andere, bestehende Ontologiekonzepte ersetzt werden)"""@de ,
                     """Describes whether a facility deals with elderly persons.

(can be replaced by other existing ontology concepts)."""@en ;
        rdfs:label "hasAge"@en ,
                   "hatAlter"@de .


###  https://purl.org/fisa#hasAverageHeight
:hasAverageHeight rdf:type owl:DatatypeProperty ;
                  rdfs:subPropertyOf owl:topDataProperty ;
                  rdfs:range xsd:double ;
                  rdfs:comment "Height in the sense of sentence 1 is the dimension of the upper floor edge of the highest floor in which a residential space is possible, above the ground surface on average."@en ,
                               "Höhe im Sinne des Satzes 1 ist das Maß der Fußbodenoberkante des höchstgelegenen Geschosses, in dem ein Aufenthaltsraum möglich ist, über der Geländeoberfläche im Mittel."@de ;
                  rdfs:isDefinedBy :MBO ;
                  rdfs:label "hasAverageHeight"@en ,
                             "hatMittlereHöhe"@de ;
                  <http://www.w3.org/2004/02/skos/core#altLabel> "hasHeightAccordingTo§2"@en ,
                                                                 "hatHöheNach§2"@de ;
                  :gemäß "§2 (3) S2 MBO"@de .


###  https://purl.org/fisa#hasCombinedGrossFloorArea
:hasCombinedGrossFloorArea rdf:type owl:DatatypeProperty ;
                           rdfs:subPropertyOf owl:topDataProperty ;
                           rdfs:range xsd:double ;
                           rdfs:comment "Die Grundflächen der Nutzungseinheiten im Sinne dieses Gesetzes sind die Brutto-Grundflächen; bei der Berechnung der Brutto-Grundflächen nach Satz 1 bleiben Flächen in Kellergeschossen außer Betracht."@de ,
                                        "Dient dem Speichern des Additionswertes von einzelnen [fisa:nutztBruttogrundfläche]-Werten der Nutzungseinheiten."@de ,
                                        "The floor areas of the utilization spaces within the meaning of this Act shall be the gross floor areas; areas in basements shall not be taken into account when calculating the gross floor areas pursuant to sentence 1."@en ,
                                        "Used to store the addition value of individual [fisa:usesGrossFloorArea] values of the utilization spaces."@en ;
                           rdfs:isDefinedBy :MBO ;
                           rdfs:label "hasCombinedGrossFloorArea"@en ,
                                      "hatGemeinsameBruttogrundfläche"@de ;
                           :gemäß "§2 (3) S3 MBO"@de .


###  https://purl.org/fisa#hasDescription
:hasDescription rdf:type owl:DatatypeProperty ;
                rdfs:subPropertyOf owl:topDataProperty ;
                rdfs:range xsd:string ;
                rdfs:comment "Used to further describe concepts."@en ,
                             "Wird genutzt, um Konzepte weitergehend zu beschreiben."@de ;
                rdfs:label "hasDescription"@en ,
                           "hatBeschreibung"@de .


###  https://purl.org/fisa#hasDisability
:hasDisability rdf:type owl:DatatypeProperty ;
               rdfs:subPropertyOf owl:topDataProperty ;
               rdfs:range xsd:boolean ;
               rdfs:comment "Beschreibt, ob eine Person einer Behinderung ausgesetzt ist."@de ,
                            "Describes whether a person is exposed to a disability."@en ;
               rdfs:label "hasDisability"@en ,
                          "hatBehinderung"@de .


###  https://purl.org/fisa#hasEscapeRouteWidth
:hasEscapeRouteWidth rdf:type owl:DatatypeProperty ;
                     rdfs:domain [ rdf:type owl:Class ;
                                   owl:unionOf ( :Door
                                                 :Opening
                                                 :Stairs
                                                 <https://w3id.org/bot#Space>
                                               )
                                 ] ;
                     rdfs:range xsd:double ;
                     rdfs:comment "Beschreibt die Breite die Rettungswege."@de ,
                                  "Describes the width of the escape routes."@en ;
                     rdfs:label "hasEscapeRouteWidth"@en ,
                                "hatRettungswegBreite"@de ;
                     :thematik <http://www.systemsEngineering.org/isabellefitkau/fisa.owl#Rettungskonzept> .


###  https://purl.org/fisa#hasGFASalesSpaces
:hasGFASalesSpaces rdf:type owl:DatatypeProperty ;
                   rdfs:subPropertyOf owl:topDataProperty ;
                   rdfs:range xsd:double ;
                   rdfs:comment "Used to define the combined griss floor area of sales premises and store street for the special purpose construction as sales premises, §2 (4) 4. MBO."@en ,
                                "Wird genutzt, um die gemeinsame Grundfläche von Verkaufsräumen und Ladenstraße für den Sonderbautatbestand Verkaufsstätte, §2 (4) 4. MBO, zu definieren."@de ;
                   rdfs:label "hasGFASalesSpaces"@en ,
                              "hatBGFVerkaufsRaeume"@de ;
                   <http://www.w3.org/2004/02/skos/core#altLabel> "hasCombinedGrossFloorAreaOfSalesSpaces"@en ;
                   :zurDefinitionVon "§2 (4) 4. MBO"@de .


###  https://purl.org/fisa#hasHeight
:hasHeight rdf:type owl:DatatypeProperty ;
           rdfs:range xsd:double ;
           rdfs:comment "Beschreibt die Gesamthöhe einer baulichen Anlage."@de ,
                        "Describes the overall height of a building structure."@en ;
           rdfs:label "hasHeight"@en ,
                      "hatHöhe"@de .


###  https://purl.org/fisa#hasIntensiveCareNeed
:hasIntensiveCareNeed rdf:type owl:DatatypeProperty ;
                      rdfs:range xsd:boolean ;
                      rdfs:comment "Beschreibt, ob ein Intensivpflegebedarf besteht."@de ,
                                   "Describes whether there is a need for intensive care."@en ;
                      rdfs:label "hasIntensiveCareNeed"@en ,
                                 "hatIntensivpflegebedarf"@de .


###  https://purl.org/fisa#hasNeedForCare
:hasNeedForCare rdf:type owl:DatatypeProperty ;
                rdfs:subPropertyOf owl:topDataProperty ;
                rdfs:range xsd:boolean ;
                rdfs:comment "Beschreibt, ob eine allgemeine Pflegebedürftigkeit vorliegt."@de ,
                             "Describes whether there is a need for general care."@en ;
                rdfs:label "hasNeedForCare"@en ,
                           "hatPflegebedürftigkeit"@de .


###  https://purl.org/fisa#hasNumberOfBeds
:hasNumberOfBeds rdf:type owl:DatatypeProperty ;
                 rdfs:subPropertyOf owl:topDataProperty ;
                 rdfs:range xsd:integer ;
                 rdfs:comment "Beschreibt die Anzahl an Betten, in Verbindung mit den Sonderbautatbeständen von Berherbungsstätten."@de ,
                              "Describes the number of beds, associated with accommodations."@en ;
                 rdfs:label "hasNumberOfBeds"@en ,
                            "hatAnzahlBetten"@de .


###  https://purl.org/fisa#hasNumberOfHostPlaces
:hasNumberOfHostPlaces rdf:type owl:DatatypeProperty ;
                       rdfs:subPropertyOf owl:topDataProperty ;
                       rdfs:range xsd:integer ;
                       rdfs:comment "Beschreibt die Anzahl an Gastplätzen, in Verbindung mit den Sonderbautatbeständen der Gastwirtschaft."@de ,
                                    "Describes the number of host places, associated with accommodations."@en ;
                       rdfs:label "hasNumberOfHostPlaces"@en ,
                                  "hatAnzahlGastplatz"@de .


###  https://purl.org/fisa#hasNumberOfPeople
:hasNumberOfPeople rdf:type owl:DatatypeProperty ;
                   rdfs:subPropertyOf owl:topDataProperty ;
                   rdfs:range xsd:integer ;
                   rdfs:comment "Beschreibt die Anzahl an Personen, in Verbindung mit den Sonderbautatbeständen von Versammlungsstätten."@de ,
                                "Describes the number of people, associated with gatherings/meetings."@en ;
                   rdfs:label "hasNumberOfPeople"@en ,
                              "hatAnzahlPersonen"@de .


###  https://purl.org/fisa#hasNumberOfVisitors
:hasNumberOfVisitors rdf:type owl:DatatypeProperty ;
                     rdfs:subPropertyOf owl:topDataProperty ;
                     rdfs:range xsd:integer ;
                     rdfs:comment "Beschreibt die Anzahl an Besuchern, in Verbindung mit den Sonderbautatbeständen der Versammlungsstätten."@de ,
                                  "Describes the number of visitors, associated with gatherings/meetings."@en ;
                     rdfs:label "hasNumberOfVisitors"@en ,
                                "hatAnzahlBesucher"@de .


###  https://purl.org/fisa#hasOutdoorHostPlaces
:hasOutdoorHostPlaces rdf:type owl:DatatypeProperty ;
                      rdfs:subPropertyOf owl:topDataProperty ;
                      rdfs:range xsd:boolean ;
                      rdfs:comment "Beschreibt die Anzahl an Gastplätzen im Freien, in Verbindung mit den Sonderbautatbeständen der Gastwirtschaft."@de ,
                                   "Describes the number of outdoor host places, associated with hospitalities/restaurants."@en ;
                      rdfs:label "hasOutdoorHostPlaces"@en ,
                                 "hatGastplatzImFreien"@de .


###  https://purl.org/fisa#hasSharedEscapeRoute
:hasSharedEscapeRoute rdf:type owl:DatatypeProperty ;
                      rdfs:subPropertyOf owl:topDataProperty ;
                      rdfs:range xsd:boolean ;
                      rdfs:comment "Beschreibt, ob zwei Konzepte einen gemeinsamen Rettungsweg haben/sich teilen."@de ,
                                   "Describes whether concepts share the same escape route."@en ;
                      rdfs:label "hasSharedEscapeRoute"@en ,
                                 "hatGemeinsamenRettungsweg"@de .


###  https://purl.org/fisa#hasStairSpaceLocation
:hasStairSpaceLocation rdf:type owl:DatatypeProperty ;
                       rdfs:domain [ rdf:type owl:Class ;
                                     owl:unionOf ( :NecessaryStairSpace
                                                   :SafetyStairSpace
                                                   :StairSpaceExtension
                                                 )
                                   ] ;
                       rdfs:range [ rdf:type rdfs:Datatype ;
                                    owl:oneOf [ rdf:type rdf:List ;
                                                rdf:first "außenliegend" ;
                                                rdf:rest [ rdf:type rdf:List ;
                                                           rdf:first "innenliegend" ;
                                                           rdf:rest rdf:nil
                                                         ]
                                              ]
                                  ] ;
                       rdfs:comment "Beschreibt die Lage eines Treppenraums, innerhalb einer baulichen Anlage."@de ,
                                    "Describes the location of stair spaces, located within a structural facility."@en ;
                       rdfs:label "hasStairSpaceLocation"@en ,
                                  "hatTreppenraumLage"@de ;
                       :thematik <http://www.systemsEngineering.org/isabellefitkau/fisa.owl#Rettungskonzept> .


###  https://purl.org/fisa#hasStiffening
:hasStiffening rdf:type owl:DatatypeProperty ;
               rdfs:subPropertyOf owl:topDataProperty ;
               rdfs:range xsd:boolean ;
               rdfs:comment "Beschreibt, ob eine Komponente ausgesteift ist."@de ,
                            "Describes whether a component has stiffening."@en ;
               rdfs:label "hasStiffening"@en ,
                          "hatAussteiffung"@de .


###  https://purl.org/fisa#hasStorageItemHeight
:hasStorageItemHeight rdf:type owl:DatatypeProperty ;
                      rdfs:range xsd:double ;
                      rdfs:comment "Describes the storage item height according to §2 (4) 18. MBO"@en ,
                                   "Oberkante Lagerguthoehe nach §2 (4) 18. MBO" ;
                      rdfs:label "hasStorageItemHeight"@en ,
                                 "hatLagerguthöhe"@de .


###  https://purl.org/fisa#hasTotalAmountOfUtilizationUnits
:hasTotalAmountOfUtilizationUnits rdf:type owl:DatatypeProperty ;
                                  rdfs:subPropertyOf owl:topDataProperty ;
                                  rdfs:range xsd:int ;
                                  rdfs:comment "Beschreibt die Gesamtanzahl an Nutzungseinheiten."@de ,
                                               "Describes the total amount of utilization spaces."@en ;
                                  rdfs:label "hasTotalAmountOfUtilizationUnits"@en ,
                                             "hatGesamtanzahlAnNutzungseinheiten"@de ;
                                  <http://www.w3.org/2004/02/skos/core#altLabel> "hasNumberOfUtilizationSpaces"@en ,
                                                                                 "hasTotalAmountOfUU"@en ,
                                                                                 "hatGesamtanzahlAnNE"@de .


###  https://purl.org/fisa#hasTotalNumberOfStoreys
:hasTotalNumberOfStoreys rdf:type owl:DatatypeProperty ;
                         rdfs:subPropertyOf owl:topDataProperty ;
                         rdfs:range xsd:int ;
                         rdfs:comment "Beschreibt die Gesamtanzahl von Geschossen."@de ,
                                      "Describes the total amount of storeys."@en ;
                         rdfs:label "hasTotalNumberOfStoreys"@en ,
                                    "hatGesamtanzahlAnGeschossen"@de .


###  https://purl.org/fisa#hasUnit
:hasUnit rdf:type owl:DatatypeProperty ;
         rdfs:range xsd:string ;
         rdfs:comment """Beschreibt, welche Einheit Werte haben.
_
Notiz: In FiSa 1.0.0, sind diese vorausgesetzt."""@de ,
                      """Describes what unit values have.
_
Note: In FiSa 1.0.0, these are implied."""@en ;
         rdfs:label "hasUnit"@en ,
                    "hatEinheit"@de .


###  https://purl.org/fisa#hasUpperEndingAt
:hasUpperEndingAt rdf:type owl:DatatypeProperty ;
                  rdfs:subPropertyOf owl:topDataProperty ;
                  rdfs:range xsd:string ;
                  rdfs:comment """has upper ending at = is led up to
e.g. raw ceiling"""@en ,
                               """hat Oberkante an = wird geführt bis
z.B. Rohdecke"""@de ;
                  rdfs:label "hasUpperEndingAt"@en ,
                             "hatOberkanteAn"@de .


###  https://purl.org/fisa#hasUsefulWidth
:hasUsefulWidth rdf:type owl:DatatypeProperty ;
                rdfs:subPropertyOf owl:topDataProperty ;
                rdfs:domain [ rdf:type owl:Class ;
                              owl:unionOf ( :Door
                                            :Opening
                                            :Stairs
                                            <https://w3id.org/bot#Space>
                                          )
                            ] ;
                rdfs:range xsd:boolean ;
                rdfs:comment "Beschreibt, ob die Breite von Zonen und/oder Komponenten nutzbar ist."@de ,
                             "Describes wheter the width of zones and/or components are useful (in terms of escaping)."@en ;
                rdfs:label "hasUsefulWidth"@en ,
                           "hatNutzbareBreite"@de .


###  https://purl.org/fisa#hasUser
:hasUser rdf:type owl:DatatypeProperty ;
         rdfs:subPropertyOf owl:topDataProperty ;
         rdfs:domain :UtilizationUnit ;
         rdfs:range xsd:string ;
         rdfs:comment "Beschreibt die Namen der Nutzer einer Nutzungseinheit."@de ,
                      "Describes the names of utilization space users."@en ;
         rdfs:label "hasUser"@en ,
                    "hatNutzer"@de .


###  https://purl.org/fisa#isBarrierFree
:isBarrierFree rdf:type owl:DatatypeProperty ;
               rdfs:range xsd:boolean ;
               <http://purl.org/dc/terms/description> "Barrierefrei sind bauliche Anlagen, soweit sie für Menschen mit Behinderung in der allgemein üblichen Weise, ohne besondere Erschwernis und grundsätzlich ohne fremde Hilfe zugänglich und nutzbar sind."@de ;
               rdfs:comment "Structural facilities are barrier-free if they are accessible and usable for people with disabilities in the generally usual manner, without particular difficulty and generally without outside assistance."@en ;
               rdfs:label "isBarrierFree"@en ,
                          "istBarrierefrei"@de ;
               :gemäß "§2 (9) MBO"@de .


###  https://purl.org/fisa#isClosedProfile
:isClosedProfile rdf:type owl:DatatypeProperty ;
                 rdfs:subPropertyOf :isProfile ;
                 rdfs:range xsd:boolean ;
                 rdfs:comment """Beschreibt, ob das Bauteil ein geschlossenes Profil ist.
Es kann z.B. zur Definition von Teilen nichttragender Außenwände nach §28 MBO verwendet werden."""@de ,
                              """Describes whether the component is a closed profile.
It can be used, for instance, to define parts of non-load-bearing external walls according to §28 MBO."""@en ;
                 rdfs:label "isClosedProfile"@en ,
                            "istGeschlossenesProfil"@de .


###  https://purl.org/fisa#isExternal
:isExternal rdf:type owl:DatatypeProperty ;
            rdfs:range xsd:boolean ;
            rdfs:comment "Beschreibt, ob eine Komponente außenliegend ist."@de ,
                         "Describes wheter a component is external."@en ;
            rdfs:label "isExternal"@en ,
                       "istAußenliegend"@de .


###  https://purl.org/fisa#isFreestanding
:isFreestanding rdf:type owl:DatatypeProperty ;
                rdfs:subPropertyOf owl:topDataProperty ;
                rdfs:range xsd:boolean ;
                rdfs:comment "Beschreibt, ob eine bauliche Anlage freistehend ist."@de ,
                             "Describes whether a structural facility is freestanding /detached."@en ;
                rdfs:label "isFreestanding"@en ,
                           "istFreistehend"@de .


###  https://purl.org/fisa#isFullStorey
:isFullStorey rdf:type owl:DatatypeProperty ;
              rdfs:subPropertyOf owl:topDataProperty ;
              rdfs:range xsd:boolean ;
              rdfs:comment "Beschreibt, ob es sich um ein Vollgeschoss handelt."@de ,
                           "Describes whether this is a full storey."@en ;
              rdfs:label "isFullStorey"@en ,
                         "istVollgeschoss"@de .


###  https://purl.org/fisa#isHighestStoreyWithPossibleResidenceSpace
:isHighestStoreyWithPossibleResidenceSpace rdf:type owl:DatatypeProperty ;
                                           rdfs:subPropertyOf owl:topDataProperty ;
                                           rdfs:range xsd:boolean ;
                                           rdfs:comment "Beschreibt, ob es das höchste Geschoss mit einem möglichen Aufenthaltsraum in der baulichen Anlage ist."@de ,
                                                        "Describes wheter it is the highest storey with a possible residence space."@en ;
                                           rdfs:label "isHighestStoreyWithPossibleResidenceSpace"@en ,
                                                      "istHöchsteGeschossMitMöglichenAufenthaltsraum"@de .


###  https://purl.org/fisa#isLoadBearing
:isLoadBearing rdf:type owl:DatatypeProperty ;
               rdfs:subPropertyOf owl:topDataProperty ;
               rdfs:range xsd:boolean ;
               rdfs:comment "Beschreibt, ob die Komponente tragend ist."@de ,
                            "Describes whether a component is load-bearing."@en ;
               rdfs:label "isLoadBearing"@en ,
                          "istTragend"@de .


###  https://purl.org/fisa#isNecessary
:isNecessary rdf:type owl:DatatypeProperty ;
             rdfs:subPropertyOf owl:topDataProperty ;
             rdfs:range xsd:boolean ;
             rdfs:comment "Beschreibt, ob die Komponente oder Zone notwendig ist."@de ,
                          "Describes whether a component or zone is necessary."@en ;
             rdfs:label "isNecessary"@en ,
                        "istNotwendig"@de .


###  https://purl.org/fisa#isOpenedProfile
:isOpenedProfile rdf:type owl:DatatypeProperty ;
                 rdfs:subPropertyOf :isProfile ;
                 rdfs:range xsd:boolean ;
                 rdfs:comment """Beschreibt, ob das Bauteil ein offenes Profil ist.
Es kann z.B. zur Definition von Teilen nichttragender Außenwände nach §28 MBO verwendet werden."""@de ,
                              """Describes whether the component is an open profile.
It can be used, for instance, to define parts of non-load-bearing external walls according to §28 MBO."""@en ;
                 rdfs:label "isOpenedProfile"@en ,
                            "istOffenesProfil"@de .


###  https://purl.org/fisa#isPossibleForResidence
:isPossibleForResidence rdf:type owl:DatatypeProperty ;
                        rdfs:domain <https://w3id.org/bot#Space> ;
                        rdfs:range xsd:boolean ;
                        rdfs:comment "Beschreibt, ob in der Zone ein Aufenthalt möglich ist."@de ,
                                     "Describes whether a zone is capable of residence."@en ;
                        rdfs:label "isPossibleForResidence"@en ,
                                   "istAufenthaltMöglich"@de .


###  https://purl.org/fisa#isProfile
:isProfile rdf:type owl:DatatypeProperty ;
           rdfs:subPropertyOf owl:topDataProperty ;
           rdfs:range xsd:boolean ;
           rdfs:comment """Beschreibt, ob das Bauteil ein Profil ist.
Es kann z.B. zur Definition von Teilen nichttragender Außenwände nach §28 MBO verwendet werden."""@de ,
                        """Describes whether the component is a profile.
It can be used, for instance, to define parts of non-load-bearing external walls according to §28 MBO."""@en ;
           rdfs:label "isProfile"@en ,
                      "istProfil"@de .


###  https://purl.org/fisa#isSelfClosing
:isSelfClosing rdf:type owl:DatatypeProperty ;
               rdfs:subPropertyOf owl:topDataProperty ;
               rdfs:range xsd:boolean ;
               rdfs:comment "Beschreibt, ob eine Komponente selbstschließend ist."@de ,
                            "Describes whether a component is self closing."@en ;
               rdfs:label "isSelfClosing"@en ,
                          "istSelbstschließend"@de .


###  https://purl.org/fisa#isSmokeResistant
:isSmokeResistant rdf:type owl:DatatypeProperty ;
                  rdfs:range xsd:boolean ;
                  rdfs:comment "Beschreibt, ob eine Komponente oder Zone rauchdicht ist."@de ,
                               "Describes wheter a component or zone is smoke resistant."@en ;
                  rdfs:label "isSmokeResistant"@en ,
                             "istRauchdicht"@de .


###  https://purl.org/fisa#isSpaceEnclosing
:isSpaceEnclosing rdf:type owl:DatatypeProperty ;
                  rdfs:subPropertyOf owl:topDataProperty ;
                  rdfs:range xsd:boolean ;
                  rdfs:comment "Beschreibt, ob eine Komponente oder Zone raumabschließend ist bzw. Anforderungen an den Raumabschluss hat."@de ,
                               "Describes wheter a component or zome is space closed or has a requirement for a room closure."@en ,
                               "istRaumabschließend"@de ;
                  rdfs:label "isSpaceEnclosing"@en .


###  https://purl.org/fisa#isStoreySlab
:isStoreySlab rdf:type owl:DatatypeProperty ;
              rdfs:domain :Slab ;
              rdfs:range xsd:boolean ;
              rdfs:comment "Beschreibt, ob eine Decke als Geschossdecke dient."@de ,
                           "Describes wheter a slab serves as a storey slab."@en ;
              rdfs:label "isStoreySlab"@en ,
                         "istGeschossdecke"@de .


###  https://purl.org/fisa#isTightClosing
:isTightClosing rdf:type owl:DatatypeProperty ;
                rdfs:subPropertyOf owl:topDataProperty ;
                rdfs:range xsd:boolean ;
                rdfs:comment "Beschreibt, ob eine Komponente dichschließend ist."@de ,
                             "Describes wheter a component is tight closing."@en ;
                rdfs:label "isTightClosing"@en ,
                           "istDichtschließend"@de .


###  https://purl.org/fisa#isType
:isType rdf:type owl:DatatypeProperty ;
        rdfs:range xsd:string ;
        rdfs:comment "Can be used to represent other concepts/components not yet assigned."@en ,
                     "Kann genutzt werden, um weitere, noch nicht zugewiesene Konzepte/Komponenten darzustellen."@de ;
        rdfs:label "isType"@en ,
                   "istTyp"@de .


###  https://purl.org/fisa#isUndergroundBuilding
:isUndergroundBuilding rdf:type owl:DatatypeProperty ;
                       rdfs:range xsd:boolean ;
                       rdfs:comment "Beschreibt, ob es sich um ein unterirdisches Gebäude handelt."@de ,
                                    "Describes whether a building is defined an underground building."@en ;
                       rdfs:label "isUndergroundBuilding"@en ,
                                  "istUnterirdischesGebäude"@de .


###  https://purl.org/fisa#isUsable
:isUsable rdf:type owl:DatatypeProperty ;
          rdfs:domain :AtticSpace ;
          rdfs:range xsd:boolean ;
          rdfs:comment """Beschreibt, ob eine Zone oder ein Bauteil nach MBO nutzbar ist.
Zur Definition z.B. der Dachfläche und verwandter Konzepte nach MBO."""@de ,
                       """Describes wheter a zone or component is usable according to MBO.
To define, for instance, the roof space and related concepts according to MBO."""@en ;
          rdfs:label "isUsable"@en ,
                     "istBenutzbar"@de ;
          <http://www.w3.org/2004/02/skos/core#altLabel> "istNutzbar"@de .


###  https://purl.org/fisa#largestUtilizationSpace
:largestUtilizationSpace rdf:type owl:DatatypeProperty ;
                         rdfs:range xsd:double ;
                         rdfs:comment "Beschreibt, wie viel Quadratmeter Bruttogrundfläche die größte Nutzungseinheit hat."@de ,
                                      "Describes the amount of square meters of gross floor area of the largest utilizaton space."@en ;
                         rdfs:label "größteNutzungseinheit"@de ,
                                    "largestUtilizationSpace"@en .


###  https://purl.org/fisa#outdoors
:outdoors rdf:type owl:DatatypeProperty ;
          rdfs:range xsd:boolean ;
          rdfs:comment "Beschreibt, ob sich etwas im Freien befindet."@de ,
                       "Describes whether something is in the outdoors."@en ;
          rdfs:label "imFreien"@de ,
                     "outdoors"@en .


###  https://purl.org/fisa#under400_meta
:under400_meta rdf:type owl:DatatypeProperty ;
               rdfs:range xsd:boolean ;
               rdfs:comment """Used as an example to temporarily store values calculated from queries. So they can be used for the next query or for inference.
-> therefore meta data.


Example:
In [under400_meta] can be stored if all utilization units of a building occupy <= 400m2 gross floor area. 
From this meta attribute, e.g. building classes can then be directly inferred.

----

Tip:
By using the data type attribute [largestUtilizationSpace] you can achieve similar results."""@en ,
                            """Wird als Beispiel genutzt, um Wert, die aus Abfragen ausgerechnet wurden, zwischenzuspeichern. So können Sie für die nächste Abfrage oder zum Schlussfolgern genutzt werden.
-> daher Meta-Daten.


Beispiel:
In [unter400_meta] kann gespeichert werden, ob alle Nutzungseinheiten eines Gebäudes <= 400m2 Bruttogrundfläche vereinnahmen. 
Aus diesem Meta-Attribut können dann z.B. Gebäudeklassen direkt geschlussfolgert werden.

----

Tip:
Durch Nutzung des Datentypattributs [größteNutzungseinheit] kann man ähnliches erreichen."""@de ;
               rdfs:label "under400_meta"@en ,
                          "unter400_meta"@de .


###  https://purl.org/fisa#usesGrossFloorArea
:usesGrossFloorArea rdf:type owl:DatatypeProperty ;
                    rdfs:range xsd:double ;
                    rdfs:comment """Describes the gross floor area of individual utilization spaces or rooms.

For an addition of the gross floor area for the determination of building classes, a combined sum value is stored in [fisa:hasCombinedGrossFloorArea]."""@en ,
                                 "Die Grundflächen der Nutzungseinheiten im Sinne dieses Gesetzes sind die Brutto-Grundflächen; bei der Berechnung der Brutto-Grundflächen nach Satz 1 bleiben Flächen in Kellergeschossen außer Betracht."@de ,
                                 """Dient der Beschreibung der Flächennutzung einzelner Nutzungseinheiten oder auch Räumen.

Für eine Addition der Flächennutzung zur Bestimmung von Gebäudeklassen, wird der Wert am Ende in [fisa:hatGemeinsameBruttogrundfläche] gespeichert."""@de ,
                                 "The floor areas of the units of use within the meaning of this Act shall be the gross floor areas; areas in basements shall not be taken into account when calculating the gross floor areas pursuant to sentence 1."@en ;
                    rdfs:label "nutztBruttogrundfläche"@de ,
                               "usesGrossFloorArea"@en .


#################################################################
#    Classes
#################################################################

###  https://purl.org/fisa#AboveGroundStorey
:AboveGroundStorey rdf:type owl:Class ;
                   rdfs:subClassOf <https://w3id.org/bot#Storey> ;
                   owl:disjointWith :Basement ;
                   <http://purl.org/dc/terms/description> "Geschosse sind oberirdische Geschosse, wenn ihre Deckenoberkanten im Mittel mehr als 1,40 m über die Geländeoberfläche hinausragen;[...]"@de ,
                                                          "Storeys are above-ground storeys if their upper ceiling edges protrude on average more than 1.40 m above the ground surface;[...]"@en ;
                   rdfs:isDefinedBy :MBO ;
                   rdfs:label "AboveGroundStorey"@en ,
                              "OberirdischesGeschoss"@de ;
                   :gemäß "§2 (6) S1 MBO"@de .


###  https://purl.org/fisa#AccessibilityOfFireFighters
:AccessibilityOfFireFighters rdf:type owl:Class ;
                             rdfs:subClassOf :SiteDevelopmentMeasure ;
                             rdfs:label "AccessibilityOfFireFighters"@en ,
                                        "ZugänglichkeitDerFeuerwehr"@de .


###  https://purl.org/fisa#Accommodation
:Accommodation rdf:type owl:Class ;
               rdfs:subClassOf :SpecialPurposeCondition ;
               rdfs:comment """§2 (4) 8. MBO (Teil)

[...]'Beherbergungsstätten mit mehr als 12 Betten'[...]"""@de ,
                            """§2 (4) 8. MBO (parts)

'accommodations with more than 12 beds,'"""@en ;
               rdfs:isDefinedBy :MBeVO ;
               rdfs:label "Accommodation"@en ,
                          "Beherbergungsstätte"@de ;
               :gemäß "§2 (4) 8. MBO" .


###  https://purl.org/fisa#AccommodationFacility
:AccommodationFacility rdf:type owl:Class ;
                       rdfs:subClassOf :SpecialPurposeCondition ;
                       rdfs:comment """§2 (4) 11. MBO

'sonstige Einrichtungen zur Unterbringung von Personen sowie Wohnheime,'"""@de ,
                                    """§2 (4) 11. MBO

Other facilities for lodging individuals, including dormitories."""@en ;
                       rdfs:label "AccommodationFacility"@en ,
                                  "EinrichtungZurUnterbringung"@de ;
                       :gemäß "§2 (4) 11. MBO" .


###  https://purl.org/fisa#Administrative
:Administrative rdf:type owl:Class ;
                rdfs:subClassOf :SpaceUsage .


###  https://purl.org/fisa#Agriculture
:Agriculture rdf:type owl:Class ;
             rdfs:subClassOf :UtilizationPurpose .


###  https://purl.org/fisa#AmusementPark
:AmusementPark rdf:type owl:Class ;
               rdfs:subClassOf :SpecialPurposeCondition ;
               rdfs:comment "Ort, der der Unterhaltung und der Freizeitgestaltung dient."@de ,
                            "Venue designed for entertainment and leisure."@en ;
               rdfs:label "AmusementPark"@en ,
                          "Vergnügungspark"@de ;
               :gemäß "§2 (4) 16. MBO" .


###  https://purl.org/fisa#AnimalHusbandry
:AnimalHusbandry rdf:type owl:Class ;
                 rdfs:subClassOf :UtilizationPurpose .


###  https://purl.org/fisa#Anteroom
:Anteroom rdf:type owl:Class ;
          rdfs:subClassOf <https://w3id.org/bot#Space> ;
          rdfs:comment "An anteroom refers to an area within a building that is used to act as a buffer zone between different rooms or areas. For example, an anteroom can be used to delay or prevent the entry of smoke, fire, or contaminants from one area into another."@en ,
                       "Der Vorraum bezeichnet einen Bereich innerhalb eines Gebäudes, der dazu dient, als Pufferzone zwischen verschiedenen Räumen oder Bereichen zu fungieren. Ein Vorraum kann beispielsweise genutzt werden, um den Eintritt von Rauch, Feuer oder Schadstoffen von einem Bereich in einen anderen zu verzögern oder zu verhindern."@de ;
          rdfs:label "Anteroom"@en ,
                     "Vestibule"@en-gb ,
                     "Vorraum"@de .


###  https://purl.org/fisa#Apron
:Apron rdf:type owl:Class ;
       rdfs:subClassOf :WallParts ;
       rdfs:comment "A structural or building device used to cover or protect a specific area or opening."@en ,
                    "Eine strukturelle oder bauliche Vorrichtung, die dazu dient, eine bestimmte Fläche oder Öffnung abzudecken oder zu schützen."@de ;
       rdfs:label "Apron"@en ,
                  "Schürze"@de .


###  https://purl.org/fisa#ArcadeSpace
:ArcadeSpace rdf:type owl:Class ;
             rdfs:subClassOf :SpecialPurposeCondition ;
             rdfs:comment """§2 (4) 8. MBO (Teile)

[...]'und Spielhallen mit mehr als 150 m2 Grundfläche,'"""@de ,
                          """§2 (4) 8. MBO (parts)

'gambling halls larger than 150 square meters.'"""@en ;
             rdfs:label "ArcadeSpace"@en ,
                        "Spielhalle"@de ;
             :gemäß "§2 (4) 8. MBO" .


###  https://purl.org/fisa#AreaForFireFighters
:AreaForFireFighters rdf:type owl:Class ;
                     rdfs:subClassOf :SiteDevelopmentMeasure ;
                     rdfs:label "AreaForFireFighters"@en ,
                                "FlächenFürDieFeuerwehr"@de .


###  https://purl.org/fisa#AssemblyBuilding
:AssemblyBuilding rdf:type owl:Class ;
                  rdfs:subClassOf :SpecialPurposeCondition ;
                  rdfs:comment """§2 (4) 7. MBO

'Versammlungsstätten
a) mit Versammlungsräumen, die insgesamt mehr als 200 Besucher fassen, wenn diese Versammlungsräume gemeinsame Rettungswege haben,
b) im Freien mit Szenenflächen sowie Freisportanlagen jeweils mit Tribünen, die keine Fliegenden Bauten sind und insgesamt mehr als 1000 Besucher fassen,'"""@de ,
                               """§2 (4) 7. MBO

'a) With assembly rooms collectively accommodating more than 200 visitors and sharing common escape routes
b) Outdoors, with stage areas or open sports facilities including stands, totaling more than 1,000 visitors, excluding temporary structures'"""@en ;
                  rdfs:isDefinedBy :MVStättVO ;
                  rdfs:label "AssemblyBuilding"@en ,
                             "Versammlungsstätte"@de ;
                  :gemäß "§2 (4) 7. MBO" .


###  https://purl.org/fisa#AssemblyProduct
:AssemblyProduct rdf:type owl:Class ;
                 rdfs:subClassOf <https://w3id.org/bot#Element> ;
                 rdfs:comment "Bauprodukt zum Zusammenführen bzw. Zusammensetzen"@de ,
                              "Construction product for merging or assembling."@en ;
                 rdfs:label "AssemblyProduct"@en ,
                            "Verbindungsprodukt"@de .


###  https://purl.org/fisa#AssessmentBasis
:AssessmentBasis rdf:type owl:Class ;
                 rdfs:comment "Beschreibt die Unterlagen, die ein Brandschützer zum Erstellen eines Brandschutznachweises zu Rate zieht."@de ,
                              "Describes the documents that a fire safety professional consults to prepare a fire safety certificate."@en ;
                 rdfs:label "AssessmentBasis"@en ,
                            "Beurteilungsgrundlage"@de .


###  https://purl.org/fisa#AtticSpace
:AtticSpace rdf:type owl:Class ;
            rdfs:subClassOf <https://w3id.org/bot#Zone> ;
            rdfs:comment "By definition, the upper edge of the roof space, is the lower edge of the roof."@en ,
                         "Per Definition ist die Oberkannte des Dachraums, die Unterkante des Daches."@de ;
            rdfs:label "AtticSpace"@en ,
                       "Dachraum"@de .


###  https://purl.org/fisa#Basement
:Basement rdf:type owl:Class ;
          rdfs:subClassOf <https://w3id.org/bot#Storey> ;
          <http://purl.org/dc/terms/description> """= NOT Above ground floor

From §2(6)MBO:
Storeys are above-ground storeys if their upper edges of the ceilings project on average more than 1.40 m above the ground surface; otherwise they are basement storeys.

we conclude:
If their upper ceiling edges protrude on average less than or equal to 1.40 m above the ground surface, they are basement floors."""@en ,
                                                 """= NOT Oberirdisches Geschoss

Aus §2(6)MBO:
Geschosse sind oberirdische Geschosse, wenn ihre Deckenoberkanten im Mittel mehr als 1,40 m über die Geländeoberfläche hinausragen; im Übrigen sind sie Kellergeschosse.

schlussfolgern wir:
Wenn ihre Deckenoberkanten im Mittel geringer oder gleich 1,40 m über die Geländeoberfläche hinausragen, sind sie Kellergeschosse."""@de ;
          rdfs:isDefinedBy :MBO ;
          rdfs:label "Basement"@en ,
                     "Kellergeschoss"@de ;
          :gemäß "§2 (6) S1 MBO"@de .


###  https://purl.org/fisa#Bathroom
:Bathroom rdf:type owl:Class ;
          rdfs:subClassOf :SpaceUsage .


###  https://purl.org/fisa#BuildingClass
:BuildingClass rdf:type owl:Class ;
               rdfs:subClassOf :Classification ;
               owl:disjointWith :BuildingMaterialClass ;
               rdfs:comment "Categorization of buildings based on certain characteristics such as use, size, height, and functional requirements."@en ,
                            "Kategorisierung von Gebäuden basierend auf bestimmten Merkmalen wie Nutzung, Größe, Höhe und funktionale Anforderungen."@de ;
               rdfs:isDefinedBy :MBO ;
               rdfs:label "BuildingClass"@en ,
                          "Gebäudeklasse"@de ;
               :gemäß "§2 (3) MBO"@de .


###  https://purl.org/fisa#BuildingClass1
:BuildingClass1 rdf:type owl:Class ;
                rdfs:subClassOf :BuildingClass ,
                                [ rdf:type owl:Restriction ;
                                  owl:onProperty :isFreestanding ;
                                  owl:hasValue "true"^^xsd:boolean
                                ] ;
                <http://purl.org/dc/terms/description> """Gebäude werden in folgende Gebäudeklassen eingeteilt:
1. Gebäudeklasse 1:
a) freistehende Gebäude mit einer Höhe bis zu 7 m und nicht mehr als zwei Nutzungseinheiten von insgesamt nicht mehr als 400 m2 und
b) freistehende land- oder forstwirtschaftlich genutzte Gebäude,
[...]"""@de ;
                rdfs:comment """Buildings are divided into the following building classes:
1. building class 1:
(a) freestanding/detached buildings not exceeding 7 m in height and not more than two units of use not exceeding 400 m2 in total; and
(b) freestanding/detached agricultural or forestry buildings,
[...]"""@en ;
                rdfs:isDefinedBy :MBO ;
                rdfs:label "BuildingClass1"@en ,
                           "Gebäudeklasse1"@de ;
                :gemäß "§2 (3) 1. MBO"@de .


###  https://purl.org/fisa#BuildingClass1a
:BuildingClass1a rdf:type owl:Class ;
                 rdfs:subClassOf :BuildingClass1 ,
                                 [ rdf:type owl:Restriction ;
                                   owl:onProperty :hasAverageHeight ;
                                   owl:allValuesFrom [ rdf:type rdfs:Datatype ;
                                                       owl:onDatatype xsd:double ;
                                                       owl:withRestrictions ( [ xsd:maxInclusive "7.0"^^xsd:double
                                                                              ]
                                                                            )
                                                     ]
                                 ] ,
                                 [ rdf:type owl:Restriction ;
                                   owl:onProperty :hasCombinedGrossFloorArea ;
                                   owl:allValuesFrom [ rdf:type rdfs:Datatype ;
                                                       owl:onDatatype xsd:double ;
                                                       owl:withRestrictions ( [ xsd:maxInclusive "400.0"^^xsd:double
                                                                              ]
                                                                            )
                                                     ]
                                 ] ,
                                 [ rdf:type owl:Restriction ;
                                   owl:onProperty :hasTotalAmountOfUtilizationUnits ;
                                   owl:maxQualifiedCardinality "2"^^xsd:nonNegativeInteger ;
                                   owl:onDataRange xsd:integer
                                 ] ;
                 owl:disjointWith :BuildingClass1b .


###  https://purl.org/fisa#BuildingClass1b
:BuildingClass1b rdf:type owl:Class ;
                 rdfs:subClassOf :BuildingClass1 .


###  https://purl.org/fisa#BuildingClass2
:BuildingClass2 rdf:type owl:Class ;
                rdfs:subClassOf :BuildingClass ,
                                [ owl:intersectionOf ( [ rdf:type owl:Restriction ;
                                                         owl:onProperty :hasAverageHeight ;
                                                         owl:allValuesFrom [ rdf:type rdfs:Datatype ;
                                                                             owl:onDatatype xsd:double ;
                                                                             owl:withRestrictions ( [ xsd:maxInclusive "7.0"^^xsd:double
                                                                                                    ]
                                                                                                  )
                                                                           ]
                                                       ]
                                                       [ rdf:type owl:Restriction ;
                                                         owl:onProperty :hasCombinedGrossFloorArea ;
                                                         owl:allValuesFrom [ rdf:type rdfs:Datatype ;
                                                                             owl:onDatatype xsd:double ;
                                                                             owl:withRestrictions ( [ xsd:maxInclusive "400.0"^^xsd:double
                                                                                                    ]
                                                                                                  )
                                                                           ]
                                                       ]
                                                       [ rdf:type owl:Restriction ;
                                                         owl:onProperty :isFreestanding ;
                                                         owl:hasValue "true"^^xsd:boolean
                                                       ]
                                                       [ rdf:type owl:Restriction ;
                                                         owl:onProperty :hasTotalAmountOfUtilizationUnits ;
                                                         owl:maxCardinality "2"^^xsd:nonNegativeInteger
                                                       ]
                                                     ) ;
                                  rdf:type owl:Class
                                ] .


###  https://purl.org/fisa#BuildingClass3
:BuildingClass3 rdf:type owl:Class ;
                rdfs:subClassOf :BuildingClass ,
                                [ owl:intersectionOf ( [ rdf:type owl:Class ;
                                                         owl:unionOf ( [ rdf:type owl:Class ;
                                                                         owl:complementOf :BuildingClass1
                                                                       ]
                                                                       [ rdf:type owl:Class ;
                                                                         owl:complementOf :BuildingClass2
                                                                       ]
                                                                     )
                                                       ]
                                                       [ rdf:type owl:Restriction ;
                                                         owl:onProperty :hasAverageHeight ;
                                                         owl:allValuesFrom [ rdf:type rdfs:Datatype ;
                                                                             owl:onDatatype xsd:double ;
                                                                             owl:withRestrictions ( [ xsd:maxInclusive "7.0"^^xsd:double
                                                                                                    ]
                                                                                                  )
                                                                           ]
                                                       ]
                                                     ) ;
                                  rdf:type owl:Class
                                ] .


###  https://purl.org/fisa#BuildingClass4
:BuildingClass4 rdf:type owl:Class ;
                rdfs:subClassOf :BuildingClass ,
                                [ owl:intersectionOf ( [ rdf:type owl:Restriction ;
                                                         owl:onProperty :hasUtilizationSpace ;
                                                         owl:someValuesFrom :UtilizationUnit
                                                       ]
                                                       [ rdf:type owl:Restriction ;
                                                         owl:onProperty :usesGrossFloorArea ;
                                                         owl:allValuesFrom [ rdf:type rdfs:Datatype ;
                                                                             owl:onDatatype xsd:double ;
                                                                             owl:withRestrictions ( [ xsd:maxInclusive "400.0"^^xsd:double
                                                                                                    ]
                                                                                                  )
                                                                           ]
                                                       ]
                                                     ) ;
                                  rdf:type owl:Class
                                ] ,
                                [ rdf:type owl:Restriction ;
                                  owl:onProperty :hasAverageHeight ;
                                  owl:allValuesFrom [ rdf:type rdfs:Datatype ;
                                                      owl:intersectionOf ( [ rdf:type rdfs:Datatype ;
                                                                             owl:onDatatype xsd:double ;
                                                                             owl:withRestrictions ( [ xsd:minExclusive "7.0"^^xsd:double
                                                                                                    ]
                                                                                                  )
                                                                           ]
                                                                           [ rdf:type rdfs:Datatype ;
                                                                             owl:onDatatype xsd:double ;
                                                                             owl:withRestrictions ( [ xsd:maxInclusive "13.0"^^xsd:double
                                                                                                    ]
                                                                                                  )
                                                                           ]
                                                                         )
                                                    ]
                                ] .


###  https://purl.org/fisa#BuildingClass5
:BuildingClass5 rdf:type owl:Class ;
                rdfs:subClassOf :BuildingClass ,
                                [ owl:intersectionOf ( [ owl:intersectionOf ( [ rdf:type owl:Restriction ;
                                                                                owl:onProperty :hasUtilizationSpace ;
                                                                                owl:someValuesFrom :UtilizationUnit
                                                                              ]
                                                                              [ rdf:type owl:Restriction ;
                                                                                owl:onProperty :usesGrossFloorArea ;
                                                                                owl:allValuesFrom [ rdf:type rdfs:Datatype ;
                                                                                                    owl:onDatatype xsd:double ;
                                                                                                    owl:withRestrictions ( [ xsd:maxInclusive "400.0"^^xsd:double
                                                                                                                           ]
                                                                                                                         )
                                                                                                  ]
                                                                              ]
                                                                            ) ;
                                                         rdf:type owl:Class
                                                       ]
                                                       [ rdf:type owl:Restriction ;
                                                         owl:onProperty :hasAverageHeight ;
                                                         owl:allValuesFrom [ rdf:type rdfs:Datatype ;
                                                                             owl:onDatatype xsd:double ;
                                                                             owl:withRestrictions ( [ xsd:minExclusive "7.0"^^xsd:double
                                                                                                    ]
                                                                                                  )
                                                                           ]
                                                       ]
                                                     ) ;
                                  rdf:type owl:Class
                                ] ,
                                [ rdf:type owl:Restriction ;
                                  owl:onProperty :hasAverageHeight ;
                                  owl:someValuesFrom [ rdf:type rdfs:Datatype ;
                                                       owl:onDatatype xsd:double ;
                                                       owl:withRestrictions ( [ xsd:minExclusive "13.0"^^xsd:double
                                                                              ]
                                                                            )
                                                     ]
                                ] .


###  https://purl.org/fisa#BuildingMaterialClass
:BuildingMaterialClass rdf:type owl:Class ;
                       rdfs:subClassOf :Classification ;
                       rdfs:comment """Is used to ensure the extension for the fire safety properties.
Thus, in addition to the properties of the building regulatory specifications already specified in fisa:StructuralFireSafetyRequirements\", the building material classes according to DIN 4102-1 and also the harmonized technical specifications with their additional performance parameters according to e.g. DIN EN 13501-2 can be incorporated.
More detailed information can also be found in the MVVTB."""@en ,
                                    """Wird genutzt, um die Erweiterung für die Brandschutzeigenschaften sicherzustellen.
So können zusätzlich zu den schon in \"Bauliche Brandschutzmaßnahme\" vorgegebenen Eigenschaften der bauaufsichtlichen Benennung auch die Baustoffklassen nach DIN 4102-1 und auch die harmonisiert technischen Spezifikationen mit ihren zusätzlichen Leistungsparametern nach z.B. DIN EN 13501-2 eingearbeitet werden.
Nähere Informationen lassen sich auch der MVVTB entnehmen."""@de ;
                       rdfs:isDefinedBy <https://purl.org/fisa#DIN4102-1:1998-05> ;
                       rdfs:label "Baustoffklasse"@de ,
                                  "BuildingMaterialClass"@en .


###  https://purl.org/fisa#Campsite
:Campsite rdf:type owl:Class ;
          rdfs:subClassOf :SpecialPurposeCondition ;
          rdfs:comment "Freiflächen, die zur Freizeitgestaltung für Campingaktivitäten ausgestattet sind."@de ,
                       "Outdoor areas equipped for recreational use for camping activities."@en ;
          rdfs:label "Campingplatz"@de ,
                     "Campsite"@en ;
          :gemäß "§2 (4) 15. MBO" .


###  https://purl.org/fisa#Canteen
:Canteen rdf:type owl:Class ;
         rdfs:subClassOf :SpaceUsage .


###  https://purl.org/fisa#Care
:Care rdf:type owl:Class ;
      rdfs:subClassOf :UtilizationPurpose .


###  https://purl.org/fisa#CareForPeople
:CareForPeople rdf:type owl:Class ;
               rdfs:subClassOf :UtilizationPurpose .


###  https://purl.org/fisa#CavitySpace
:CavitySpace rdf:type owl:Class ;
             rdfs:subClassOf <https://w3id.org/bot#Zone> ;
             <http://purl.org/dc/terms/description> "Cavities between the uppermost ceiling and the roofing, in which residence rooms are not possible, are not storeys."@en ,
                                                    "Hohlräume zwischen der obersten Decke und der Bedachung, in denen Aufenthaltsräume nicht möglich sind, sind keine Geschosse."@de ;
             rdfs:isDefinedBy :MBO ;
             rdfs:label "CavitySpace"@en ,
                        "Hohlraum"@de ;
             :gemäß "§2 (6) S2 MBO"@de .


###  https://purl.org/fisa#ChildCare
:ChildCare rdf:type owl:Class ;
           rdfs:subClassOf :UtilizationPurpose .


###  https://purl.org/fisa#Cladding
:Cladding rdf:type owl:Class ;
          rdfs:subClassOf <https://w3id.org/bot#Element> ;
          rdfs:comment "Anbringung von feuerbeständigen Materialien oder Schichten auf Bauelemente wie Träger, Stützen, Wände oder Decken. Diese Bekleidung dient dazu, die Feuerbeständigkeit und Brandschutzeigenschaften dieser Bauteile zu verbessern und somit die Ausbreitung von Feuer und Rauch zu verlangsamen."@de ,
                       "Application of fire-resistant materials or coatings to structural elements such as beams, columns, walls or ceilings. This cladding serves to improve the fire resistance and fire protection properties of these structural elements, thus slowing down the spread of fire and smoke."@en ;
          rdfs:label "Bekleidung"@de ,
                     "Cladding"@en .


###  https://purl.org/fisa#Classification
:Classification rdf:type owl:Class ;
                rdfs:subClassOf [ rdf:type owl:Restriction ;
                                  owl:onProperty :isBasedOn ;
                                  owl:someValuesFrom :AssessmentBasis
                                ] ;
                rdfs:comment "Die Einteilung von Bauelementen, Materialien, Gebäuden oder Systemen in verschiedene Klassen oder Kategorien basierend auf bestimmten festgelegten Kriterien. Diese Klassifizierungen dienen dazu, Standards zu etablieren, Informationen zu strukturieren und einheitliche Regeln oder Anforderungen für verschiedene Aspekte des Bauwesens festzulegen."@de ,
                             "The classification of building elements, materials, buildings or systems into different classes or categories based on certain established criteria. These classifications are used to establish standards, structure information, and establish uniform rules or requirements for various aspects of construction."@en ;
                rdfs:label "Classification"@en ,
                           "Klassifizierung"@de .


###  https://purl.org/fisa#ClientSpecification
:ClientSpecification rdf:type owl:Class ;
                     rdfs:subClassOf :AssessmentBasis ;
                     rdfs:comment "Specifications from the building owner can have a significant influence on fire safety, e.g. by providing information on the utilization concept."@en ,
                                  "Vorgaben des Bauherren können z.B. durch Angaben zum Nutzungskonzept den Brandschutz maßgeblich beeinflussen."@de ;
                     rdfs:label "BauherrenVorgabe"@de ,
                                "ClientSpecification"@en .


###  https://purl.org/fisa#ClosedProfile
:ClosedProfile rdf:type owl:Class ;
               owl:equivalentClass [ owl:intersectionOf ( :Profile
                                                          [ rdf:type owl:Restriction ;
                                                            owl:onProperty :isClosedProfile ;
                                                            owl:hasValue "true"^^xsd:boolean
                                                          ]
                                                        ) ;
                                     rdf:type owl:Class
                                   ] ;
               rdfs:subClassOf :Profile ;
               owl:disjointWith :OpenProfile ;
               rdfs:comment "Wall profile with a closed shape."@en ,
                            "Wandprofil mit geschlossener Querschnittsform."@de ;
               rdfs:label "ClosedProfile"@en ,
                          "GeschlossenesProfil"@de .


###  https://purl.org/fisa#Closing
:Closing rdf:type owl:Class ;
         rdfs:subClassOf <https://w3id.org/bot#Element> ;
         rdfs:comment "Die ordnungsgemäße Beendigung oder Abdeckung von Öffnungen oder Durchführungen in Gebäuden, um die Ausbreitung von Feuer, Rauch und giftigen Gasen zwischen verschiedenen Räumen oder Abschnitten zu verhindern."@de ,
                      "The proper termination or covering of openings or penetrations in buildings to prevent the spread of fire, smoke, and toxic gases between different rooms or sections."@en ;
         rdfs:label "Abschluss"@de ,
                    "Closing"@en .


###  https://purl.org/fisa#CombustionAppliance
:CombustionAppliance rdf:type owl:Class ;
                     rdfs:subClassOf :Component ;
                     <http://purl.org/dc/terms/description> "Feuerstätten sind in oder an Gebäuden ortsfest benutzte Anlagen oder Einrichtungen, die dazu bestimmt sind, durch Verbrennung Wärme zu erzeugen."@de ;
                     rdfs:isDefinedBy :MBO ;
                     rdfs:label "Combustion appliances are fixed installations or equipment used in or on buildings and intended to generate heat by combustion."@en ,
                                "CombustionAppliance"@en ,
                                "Feuerstätte"@de ;
                     :gemäß "§2 (8) MBO"@de .


###  https://purl.org/fisa#CompartmentWall
:CompartmentWall rdf:type owl:Class ;
                 rdfs:subClassOf :Wall ;
                 rdfs:comment "A space-enclosing structural member of a space or utilization units of use within storeys."@en ,
                              "Ein raumabschließendes Bauteile von Räumen oder Nutzungseinheiten innerhalb von Geschossen."@de ;
                 rdfs:label "CompartmentWall"@en ,
                            "Trennwand"@de .


###  https://purl.org/fisa#Component
:Component rdf:type owl:Class ;
           rdfs:label "Component"@en ,
                      "Komponente"@de .


###  https://purl.org/fisa#ComponentType
:ComponentType rdf:type owl:Class ;
               rdfs:comment "Component types are used for extended categorization of components."@en ,
                            "Komponententypen dienen zur erweiterten Kategorisierung von Komponenten."@de ;
               rdfs:label "ComponentType"@en ,
                          "Komponententyp"@de .


###  https://purl.org/fisa#ConstructionalMovingArea
:ConstructionalMovingArea rdf:type owl:Class ;
                          rdfs:subClassOf :SiteDevelopmentMeasure ;
                          rdfs:label "Bewegungsfläche"@de ,
                                     "ConstructionalMovingArea"@en .


###  https://purl.org/fisa#Corridor
:Corridor rdf:type owl:Class ;
          rdfs:subClassOf :SpaceUsage .


###  https://purl.org/fisa#DIN4102
:DIN4102 rdf:type owl:Class ;
         rdfs:subClassOf :Norm ;
         rdfs:label "DIN4102"@de ,
                    "DIN4102"@en .


###  https://purl.org/fisa#DIN_EN13501
:DIN_EN13501 rdf:type owl:Class ;
             rdfs:subClassOf :Eurocode ;
             rdfs:comment "Classification of construction products and types of construction for their fire behavior."@en ,
                          "Klassifizierung von Bauprodukten und Bauarten zu ihrem Brandverhalten"@de ;
             rdfs:label "DIN_EN_13501"@de ,
                        "DIN_EN_13501"@en .


###  https://purl.org/fisa#DayCareCenter
:DayCareCenter rdf:type owl:Class ;
               rdfs:subClassOf :SpecialPurposeCondition ;
               rdfs:comment """§2 (4) 12. MBO

'Tageseinrichtungen für Kinder, Menschen mit Behinderung und alte Menschen, ausgenommen Tageseinrichtungen1 einschließlich Tagespflege für nicht mehr als zehn Kinder,'"""@de ,
                            """§2 (4) 12. MBO

Daycare facilities for children, people with disabilities, and the elderly, excluding those accommodating no more than ten children, including day care."""@en ;
               rdfs:label "DayCareCenter"@en ,
                          "Tageseinrichtung"@de ;
               :gemäß "§2 (4) 12. MBO" .


###  https://purl.org/fisa#DefensiveFireSafety
:DefensiveFireSafety rdf:type owl:Class ;
                     rdfs:subClassOf :FireSafety ;
                     rdfs:comment "Defensive fire safety includes all passive and active measures taken by the fire department and other emergency services before and during a fire incident."@en ,
                                  "Der abwehrende Brandschutz beinhaltet alle passiven und aktiven Maßnahmen, die durch Feuerwehren und andere Hilfe leistenden Stellen vor und während des Brandereignisses ergriffen werden"@de ;
                     rdfs:label "AbwehrenderBrandschutz"@de ,
                                "DefensiveFireSafety"@en .


###  https://purl.org/fisa#Door
:Door rdf:type owl:Class ;
      rdfs:subClassOf :Closing ;
      rdfs:comment "A movable device or closure of an opening in a building wall or structure used to provide or restrict access for persons, goods, or vehicles."@en ,
                   "Eine bewegliche Vorrichtung oder Abschluss einer Öffnung in einer Gebäudewand oder -struktur, die dazu dient, den Zugang für Personen, Güter oder Fahrzeuge zu ermöglichen oder zu beschränken."@de ;
      rdfs:label "Door"@en ,
                 "Tür"@de .


###  https://purl.org/fisa#Dormitory
:Dormitory rdf:type owl:Class ;
           rdfs:subClassOf :SpecialPurposeCondition ;
           rdfs:comment """§2 (4) 11. MBO

'Other facilities for lodging individuals, including dormitories'"""@en ,
                        """§2 (4) 11. MBO

'sonstige Einrichtungen zur Unterbringung von Personen sowie Wohnheime,'"""@de ;
           rdfs:label "Dormitory"@en ,
                      "Wohnheim"@de ;
           :gemäß "§2 (4) 11. MBO" .


###  https://purl.org/fisa#DriveShaftWall
:DriveShaftWall rdf:type owl:Class ;
                rdfs:subClassOf :Wall ;
                <http://swrl.stanford.edu/ontologies/3.3/swrla.owl#isRuleEnabled> "LiftShaftWall"@en ;
                rdfs:comment "Aufzüge im Innern von Gebäuden müssen eigene Fahrschächte haben, um eine Brandausbreitung in andere Geschosse ausreichend lang zu verhindern."@de ,
                             "Elevators inside buildings must have their own drive shafts to prevent fire spread to other floors for a sufficient length of time."@en ;
                rdfs:label "DriveShaftWall"@en ,
                           "Fahrschachtwand"@de .


###  https://purl.org/fisa#Education
:Education rdf:type owl:Class ;
           rdfs:subClassOf :UtilizationPurpose .


###  https://purl.org/fisa#EducationalInstitution
:EducationalInstitution rdf:type owl:Class ;
                        rdfs:subClassOf :SpecialPurposeCondition ;
                        rdfs:comment "Einrichtungen, die sich dem Lernen widmen."@de ,
                                     "Establishments dedicated to learning."@en ;
                        rdfs:label "Bildungsstätte"@de ,
                                   "EducationalInstitution"@en ;
                        :gemäß "§2 (4) 13. MBO" .


###  https://purl.org/fisa#Elevator
:Elevator rdf:type owl:Class ;
          rdfs:subClassOf <https://w3id.org/bot#Space> ;
          rdfs:comment "An elevator refers to a space for a device for the vertical or inclined transportation of persons or goods between different levels of a building."@en ,
                       "Ein Aufzug bezeichnet einen Raum zur Einrichtung zur vertikalen oder schrägen Beförderung von Personen oder Gütern zwischen verschiedenen Ebenen eines Gebäudes."@de ;
          rdfs:label "Aufzug"@de ,
                     "Elevator"@en .


###  https://purl.org/fisa#EmergencyMedicalService
:EmergencyMedicalService rdf:type owl:Class ;
                         rdfs:subClassOf :UtilizationPurpose .


###  https://purl.org/fisa#EscapeRoute
:EscapeRoute rdf:type owl:Class ;
             rdfs:subClassOf :FireSafety ,
                             [ owl:intersectionOf ( [ rdf:type owl:Restriction ;
                                                      owl:onProperty :hasEscapeRouteWidth ;
                                                      owl:someValuesFrom xsd:double
                                                    ]
                                                    [ rdf:type owl:Restriction ;
                                                      owl:onProperty :hasUsefulWidth ;
                                                      owl:someValuesFrom xsd:boolean
                                                    ]
                                                  ) ;
                               rdf:type owl:Class
                             ] ;
             rdfs:comment """Escape routes (as in rescue) in the strict sense are accesses and routes for emergency services such as the fire department, via which the rescue (= external rescue) of e.g. injured persons and animals as well as fire fighting (extinguishing work) are possible. (see also §14 MBO)

Escape routes are routes, e.g. corridors, staircases and exits to the outside, via which people and animals can leave structural facilities in the event of danger (in the event of fire) and bring themselves to safety (= self-rescue).

In general, the two terms are combined in the building regulations under the escape route."""@en ,
                          """Rettungswege im strengen Sinn sind Zugänge und Wege für Einsatzkräfte wie der Feuerwehr, über die die Bergung (= Fremdrettung) von z.B. verletzten Personen und Tieren sowie die Brandbekämpfung (Löscharbeiten) möglich sind. (siehe auch §14 MBO)

Fluchtwege sind Wege, z.B. Flure, Treppen und Ausgänge ins Freie, über die Menschen und Tiere im Gefahrenfall (bei Brand) bauliche Anlagen verlassen und sich in Sicherheit bringen können (= Selbstrettung).

Allgemein werden in den Bauordnungen die beiden Begriffe unter dem Rettungsweg zusammengefasst."""@de ;
             rdfs:label "EscapeRoute"@en ,
                        "Rettungsweg"@de ;
             :thematik <http://www.systemsEngineering.org/isabellefitkau/fisa.owl#Rettungskonzept> .


###  https://purl.org/fisa#Eurocode
:Eurocode rdf:type owl:Class ;
          rdfs:subClassOf :RuleOfApplication ;
          rdfs:comment "Eurocodes are fundamental European standards to be applied as unified design rules in civil engineering and structural design."@en ,
                       "Eurocodes sind grundlegende europäische Normen als vereinheitlichte Bemessungsregeln im Bauwesen und in der Tragwerksplanung anzuwenden."@de ;
          rdfs:label "Eurocode"@de ,
                     "Eurocode"@en .


###  https://purl.org/fisa#ExternalDevelopment
:ExternalDevelopment rdf:type owl:Class ;
                     rdfs:subClassOf :UtilizationPurpose ,
                                     <https://w3id.org/bot#Site> .


###  https://purl.org/fisa#ExternalWall
:ExternalWall rdf:type owl:Class ;
              owl:equivalentClass [ rdf:type owl:Restriction ;
                                    owl:onProperty :isExternal ;
                                    owl:hasValue "true"^^xsd:boolean
                                  ] ;
              rdfs:subClassOf :Wall ;
              <http://swrl.stanford.edu/ontologies/3.3/swrla.owl#isRuleEnabled> "ExternalWall"@en ;
              rdfs:comment "A wall that forms the outer boundary and protects the building from environmental factors such as weather, wind, moisture and temperature fluctuations."@en ,
                           "Eine Wand, die die äußere Begrenzung bildet und das Gebäude vor Umwelteinflüssen wie Wetter, Wind, Feuchtigkeit und Temperaturschwankungen schützt."@de ;
              rdfs:label "Außenwand"@de ,
                         "ExternalWall"@en .


###  https://purl.org/fisa#ExtinguishingWaterAccess
:ExtinguishingWaterAccess rdf:type owl:Class ;
                          rdfs:subClassOf :SiteDevelopmentMeasure ;
                          rdfs:label "ExtinguishingWaterAccess"@en ,
                                     "Löschwasserzugang"@de .


###  https://purl.org/fisa#ExtinguishingWaterRetention
:ExtinguishingWaterRetention rdf:type owl:Class ;
                             rdfs:subClassOf :ExtinguishingWaterAccess ;
                             owl:disjointWith :ExtinguishingWaterSupply ;
                             rdfs:label "ExtinguishingWaterRetention"@en ,
                                        "Löschwasserrückhaltung"@de .


###  https://purl.org/fisa#ExtinguishingWaterSupply
:ExtinguishingWaterSupply rdf:type owl:Class ;
                          rdfs:subClassOf :ExtinguishingWaterAccess ;
                          rdfs:label "ExtinguishingWaterSupply"@en ,
                                     "Löschwasserversorgung"@de .


###  https://purl.org/fisa#Fastening
:Fastening rdf:type owl:Class ;
           rdfs:subClassOf :AssemblyProduct ;
           rdfs:comment "Bauelemente oder Konstruktionen, die dazu dienen, verschiedene Komponenten eines Gebäudes oder einer Struktur sicher miteinander zu verbinden oder zu verankern."@de ,
                        "Building elements used to securely connect or anchor together various components of a building or structure."@en ;
           rdfs:label "Befestigung"@de ,
                      "Fastening"@en .


###  https://purl.org/fisa#FireBehaviour
:FireBehaviour rdf:type owl:Class ;
               owl:equivalentClass [ rdf:type owl:Class ;
                                     owl:oneOf ( :brennbar
                                                 :leichtentflammbar
                                                 :nichtbrennbar
                                                 :normalentflammbar
                                                 :schwerentflammbar
                                               )
                                   ] ;
               rdfs:subClassOf :StructuralFireSafetyMeasures ;
               owl:disjointWith :FireResistance ,
                                :SpaceClosure ;
               rdfs:comment "Baustoffe werden nach den Anforderungen an ihr Brandverhalten, ihrer Brenn- und Entflammbarkeit, unterschieden."@de ,
                            "Building materials are differentiated according to the requirements for their fire behavior, such as their combustibility and flammability."@en ;
               rdfs:label "Brandverhalten"@de ,
                          "FireBehaviour"@en .


###  https://purl.org/fisa#FireBrigadeLifts
:FireBrigadeLifts rdf:type owl:Class ;
                  rdfs:subClassOf :TechnicalComponent ;
                  rdfs:comment "Feuerwehraufzüge sind besonders abgesicherte Aufzüge, die der Feuerwehr im Brandfall ein Erreichen der Brandetage ermöglichen."@de ,
                               "Firefighters' elevators are specially secured elevators that allow firefighters to reach the fire storeys in case of fire."@en ;
                  rdfs:label "Feuerwehraufzüge"@de ,
                             "FireBrigadeLifts"@en .


###  https://purl.org/fisa#FireCompartment
:FireCompartment rdf:type owl:Class ;
                 rdfs:subClassOf <https://w3id.org/bot#Zone> ;
                 rdfs:comment "A fire compartment is a structurally demarcated area that burns out as intended in the event of damage and thus must not allow fire to spread to other fire compartments."@en ,
                              "Ein Brandabschnitt ist ein baulich abgegrenzter Bereich, der im Schadensfall bestimmungsgemäß ausbrennt und somit keinen Brandüberschlag auf andere Brandabschnitte zulassen darf."@de ;
                 rdfs:label "Brandabschnitt"@de ,
                            "FireCompartment"@en .


###  https://purl.org/fisa#FireControlOfLifts
:FireControlOfLifts rdf:type owl:Class ;
                    rdfs:subClassOf :TechnicalComponent ;
                    rdfs:comment "Mit der Brandfallsteuerung eines Aufzuges soll verhindert werden, dass bei einem festgestellten Brand (Gefahr) in einem Gebäude der Aufzug weiterhin als Bewegungsmittel genutzt werden kann."@de ,
                                 "The fire control of lifts is intended to prevent the elevator from continuing to be used as a means of movement in the event of a detected fire (hazard) in a building."@en ;
                    rdfs:label "Brandfallsteuerung_von_Aufzügen"@de ,
                               "FireControl_of_Lifts"@en .


###  https://purl.org/fisa#FireDamper
:FireDamper rdf:type owl:Class ;
            rdfs:subClassOf :Closing ;
            rdfs:comment "Dienen dazu, im Brandfall Öffnungen in brandschutztechnisch relevanten Durchführungen wie Lüftungs- oder Kabelschächten zu verschließen und so die Ausbreitung von Feuer und Rauch zu verhindern."@de ,
                         "In the event of a fire, they are used to close off openings in penetrations relevant to fire safety, such as ventilation or cable shafts, thus preventing the spread of fire and smoke."@en ;
            rdfs:label "Brandschutzklappe"@de ,
                       "FireDamper"@en .


###  https://purl.org/fisa#FireFighterAccessEntrance
:FireFighterAccessEntrance rdf:type owl:Class ;
                           rdfs:subClassOf :SiteDevelopmentMeasure ;
                           rdfs:label "Feuerwehrzufahrt"@de ,
                                      "FireFighterAccess_Entrance"@en .


###  https://purl.org/fisa#FireFighterAccessPoint
:FireFighterAccessPoint rdf:type owl:Class ;
                        rdfs:subClassOf :SiteDevelopmentMeasure ;
                        rdfs:label "Feuerwehranlaufpunkt"@de ,
                                   "FireFighterAccessPoint"@en ;
                        <http://www.w3.org/2004/02/skos/core#altLabel> "FAP"@de .


###  https://purl.org/fisa#FireFighterLift
:FireFighterLift rdf:type owl:Class ;
                 rdfs:subClassOf <https://w3id.org/bot#Space> ,
                                 [ rdf:type owl:Restriction ;
                                   owl:onProperty :isPartOf ;
                                   owl:someValuesFrom :RescueConcept
                                 ] ;
                 rdfs:comment "Als Feuerwehraufzüge werden besonders gesicherte Aufzüge bezeichnet, die auch im Brandfall genutzt werden können – vorrangig von der Feuerwehr."@de ,
                              "Firefighters' elevators are specially secured elevators that can also be used in the event of a fire - primarily by the fire department."@en ;
                 rdfs:label "Feuerwehraufzug"@de ,
                            "FireFighterLift"@en .


###  https://purl.org/fisa#FireResistance
:FireResistance rdf:type owl:Class ;
                owl:equivalentClass [ rdf:type owl:Class ;
                                      owl:oneOf ( :feuerbeständig
                                                  :feuerhemmend
                                                  :hochfeuerbeständig
                                                  :hochfeuerhemmend
                                                  :höchstfeuerbeständig
                                                )
                                    ] ;
                rdfs:subClassOf :StructuralFireSafetyMeasures ;
                rdfs:comment "Bauteile werden nach den Anforderungen an ihre Feuerwiderstandsfähigkeit, d.h.  die Dauer, während der ein Bauteil seine Funktion bei einem Normbrand beibehält, unterschieden."@de ,
                             "Building components are differentiated according to their fire resistance requirements, i.e. the duration during which a component retains its function in the event of a standard fire/fire according to norm bzw. testing standards."@en ;
                rdfs:label "Feuerwiderstandsfähigkeit"@de ,
                           "FireResistance"@en .


###  https://purl.org/fisa#FireResistantEnclosure
:FireResistantEnclosure rdf:type owl:Class ;
                        owl:equivalentClass [ rdf:type owl:Class ;
                                              owl:unionOf ( [ owl:intersectionOf ( [ owl:intersectionOf ( [ rdf:type owl:Restriction ;
                                                                                                            owl:onProperty :hasFireResistance ;
                                                                                                            owl:someValuesFrom :FireResistance
                                                                                                          ]
                                                                                                          [ rdf:type owl:Restriction ;
                                                                                                            owl:onProperty :isSelfClosing ;
                                                                                                            owl:hasValue "true"^^xsd:boolean
                                                                                                          ]
                                                                                                          [ rdf:type owl:Restriction ;
                                                                                                            owl:onProperty :isSmokeResistant ;
                                                                                                            owl:hasValue "true"^^xsd:boolean
                                                                                                          ]
                                                                                                        ) ;
                                                                                     rdf:type owl:Class
                                                                                   ]
                                                                                   [ rdf:type owl:Class ;
                                                                                     owl:unionOf ( :Door
                                                                                                   :FireDamper
                                                                                                   :Gate
                                                                                                 )
                                                                                   ]
                                                                                 ) ;
                                                              rdf:type owl:Class
                                                            ]
                                                            [ owl:intersectionOf ( [ owl:intersectionOf ( [ rdf:type owl:Restriction ;
                                                                                                            owl:onProperty :hasFireResistance ;
                                                                                                            owl:someValuesFrom :FireResistance
                                                                                                          ]
                                                                                                          [ rdf:type owl:Restriction ;
                                                                                                            owl:onProperty :isSelfClosing ;
                                                                                                            owl:hasValue "true"^^xsd:boolean
                                                                                                          ]
                                                                                                          [ rdf:type owl:Restriction ;
                                                                                                            owl:onProperty :isTightClosing ;
                                                                                                            owl:hasValue "true"^^xsd:boolean
                                                                                                          ]
                                                                                                        ) ;
                                                                                     rdf:type owl:Class
                                                                                   ]
                                                                                   [ rdf:type owl:Class ;
                                                                                     owl:unionOf ( :Door
                                                                                                   :FireDamper
                                                                                                   :Gate
                                                                                                 )
                                                                                   ]
                                                                                 ) ;
                                                              rdf:type owl:Class
                                                            ]
                                                          )
                                            ] ;
                        rdfs:subClassOf :ComponentType ,
                                        [ rdf:type owl:Restriction ;
                                          owl:onProperty :hasRequirement ;
                                          owl:someValuesFrom :StructuralFireSafety
                                        ] ;
                        rdfs:comment "Feuerschutzabschlüsse werden entweder manuell geöffnet und schließen immer selbsttätig oder werden normalerweise offengehalten und schließen im Fall von Feuer oder Rauch selbst."@de ,
                                     "Fire resistant enclosures are either opened manually and always close automatically or are normally held open and close themselves in case of fire or smoke.en"@en ;
                        rdfs:label "Feuerschutzabschluss"@de ,
                                   "FireResistantEnclosure"@en .


###  https://purl.org/fisa#FireSafety
:FireSafety rdf:type owl:Class ;
            rdfs:comment "Fire safety refers to all measures that prevent the development and spread of a fire and enable the rescue of people and animals as well as effective extinguishing work in the event of a fire."@en ,
                         "Unter Brandschutz versteht man alle Maßnahmen, die der Entstehung und Ausbreitung eines Brandes vorbeugen und die Rettung von Menschen und Tieren sowie wirksame Löscharbeiten bei einem Brand ermöglichen."@de ,
                         """§14 MBO
Bauliche Anlagen sind so anzuordnen, zu errichten, zu ändern und instand zu halten, dass der Entstehung eines Brandes und der Ausbreitung von Feuer und Rauch (Brandausbreitung) vorgebeugt wird und bei einem Brand die Rettung von Menschen und Tieren sowie wirksame Löscharbeiten möglich sind."""@de ,
                         """§14 MBO (Protective Goal)
Structural facilites are to be arranged, erected, modified and maintained in such a way that the development of fire and the spread of fire and smoke (fire spread) is prevented and, in the event of fire, the rescue of people and animals and effective extinguishing work are possible."""@en ;
            rdfs:label "Brandschutz"@de ,
                       "FireSafety"@en .


###  https://purl.org/fisa#FireSafetyCertificate
:FireSafetyCertificate rdf:type owl:Class ;
                       rdfs:subClassOf :TechnicalStructuralCertificate ,
                                       [ rdf:type owl:Restriction ;
                                         owl:onProperty :isBasedOn ;
                                         owl:someValuesFrom :ProtectiveGoal
                                       ] ;
                       owl:disjointWith :OtherCertificate ;
                       rdfs:comment "A document prepared by professionals such as fire safety professionals, to confirm compliance with fire safety requirements and standards/regulations for a building project."@en ,
                                    "Ein Dokument, das von Fachleuten wie Brandschutzplanern, erstellt wird, um die Einhaltung der brandschutztechnischen Anforderungen und Normen für ein Bauvorhaben zu bestätigen."@de ;
                       rdfs:label "BrandschutzNachweis"@de ,
                                  "FireSafetyCertificate"@en .


###  https://purl.org/fisa#FireWall
:FireWall rdf:type owl:Class ;
          rdfs:subClassOf :Wall ;
          rdfs:comment "Brandwände müssen als raumabschließende Bauteile zum Abschluss von Gebäuden (Gebäudeabschlusswand) oder zur Unterteilung von Gebäuden in Brand abschnitte (innere Brandwand) ausreichend lang die Brandausbreitung auf andere Gebäude oder Brandabschnitte verhindern."@de ,
                       "Firewalls must be used as room-enclosing components to close off buildings (fire wall as external wall) or to divide buildings into fire compartments (internal fire wall) and must be long enough to prevent the spread of fire to other buildings or fire compartments."@en ;
          rdfs:isDefinedBy :MBO ;
          rdfs:label "Brandwand"@de ,
                     "FireWall"@en ;
          :gemäß "§30 (1) MBO"@de .


###  https://purl.org/fisa#FireWallAsExternalWall
:FireWallAsExternalWall rdf:type owl:Class ;
                        rdfs:subClassOf :FireWall ;
                        <http://swrl.stanford.edu/ontologies/3.3/swrla.owl#isRuleEnabled> "FireWall_as_ExternalWall"@en ;
                        rdfs:comment """to: §30 (2) 1. and 4.

Fire walls are required
1.
As an external wall, except for buildings without living quarters and without fireplaces with no more than 50 m3 gross volume, if these external walls are erected at or with a distance of less than 2.50 m from the property boundary, unless a distance of at least 5 m from existing buildings or future buildings permitted under the building regulations is ensured,
[...]
4.
as an external wall between residential buildings and attached agricultural buildings, as well as an internal fire wall between the residential part and the agricultural part of a building."""@en ,
                                     """zu: §30 (2) 1. und 4.

Brandwände sind erforderlich
1.
als Gebäudeabschlusswand, ausgenommen von Gebäuden ohne Aufenthaltsräume und ohne Feuerstätten mit nicht mehr als 50 m3 Brutto- Rauminhalt, wenn diese Abschlusswände an oder mit einem Abstand von weniger als 2,50 m gegenüber der Grundstücksgrenze errichtet werden, es sei denn, dass ein Abstand von mindestens 5 m zu bestehenden oder nach den baurechtlichen Vorschriften zulässigen künftigen Gebäuden gesichert ist,
[...]
4.
als Gebäudeabschlusswand zwischen W ohngebäuden und angebauten landwirtschaftlich genutzten Gebäuden sowie als innere Brandwand zwischen dem Wohnteil und dem landwirtschaftlich genutzten Teil eines Gebäudes."""@de ;
                        rdfs:isDefinedBy "§30 (2) 1. MBO"@de ,
                                         "§30 (2) 4. MBO"@de ;
                        rdfs:label "FireWallAsExternalWall"@en ,
                                   "Gebäudeabschlusswand"@de .


###  https://purl.org/fisa#FirstEscapeRoute
:FirstEscapeRoute rdf:type owl:Class ;
                  rdfs:subClassOf :EscapeRoute ;
                  owl:disjointWith :SecondEscapeRoute ;
                  rdfs:comment "Der erste Rettungsweg muss immer baulich sein (eine ständig vorhandene feste bauliche Einrichtung) und der Selbstrettung dienen."@de ,
                               "The first escape route must always be structural (a permanently existing fixed structural facility) and serve self-rescue."@en ;
                  rdfs:label "ErsterRettungsweg"@de ,
                             "FirstEscapeRoute"@en .


###  https://purl.org/fisa#Foyer
:Foyer rdf:type owl:Class ;
       rdfs:subClassOf :SpaceUsage .


###  https://purl.org/fisa#Garage
:Garage rdf:type owl:Class ;
        rdfs:subClassOf :StructuralFacility ;
        owl:disjointWith <https://w3id.org/bot#Building> ;
        <http://purl.org/dc/terms/description> "Garagen sind Gebäude oder Gebäudeteile zum Abstellen von Kraftfahrzeugen."@de ;
        rdfs:comment """Ausnahme aus §2 (7) S3 MBO:
Ausstellungs-, Verkaufs-, Werk- und Lagerräume für Kraftfahrzeuge sind keine Stellplätze oder Garagen."""@de ,
                     """Exception from §2 (7) S3 MBO:
Showrooms, salesrooms, workshops and storage rooms for motor vehicles are not parking spaces or garages."""@en ,
                     "Garages are buildings or parts of buildings for parking (motor) vehicles."@en ;
        rdfs:isDefinedBy :MBO ;
        rdfs:label "Garage"@de ,
                   "Garage"@en ;
        :gemäß "§2 (7) S2 MBO"@de .


###  https://purl.org/fisa#Gate
:Gate rdf:type owl:Class ;
      rdfs:subClassOf :Closing ;
      rdfs:comment "A large, movable device or closure of an opening in a building wall or structure used to provide or restrict access for persons, vehicles, or goods."@en ,
                   "Eine große, bewegliche Vorrichtung oder Abschluss einer Öffnung in einer Gebäudewand oder -struktur, die dazu dient, den Zugang für Personen, Fahrzeuge oder Güter zu ermöglichen oder zu beschränken."@de ;
      rdfs:label "Gate"@en ,
                 "Tor"@de .


###  https://purl.org/fisa#GeneralInformation
:GeneralInformation rdf:type owl:Class ;
                    rdfs:subClassOf :AssessmentBasis ,
                                    [ rdf:type owl:Restriction ;
                                      owl:onProperty :isBasedOn ;
                                      owl:someValuesFrom :ClientSpecification
                                    ] ,
                                    [ rdf:type owl:Restriction ;
                                      owl:onProperty :isBasedOn ;
                                      owl:someValuesFrom :PlanningDocument
                                    ] ;
                    rdfs:comment "Beinhaltet im Brandschutznachweis Informationen zu Abmessungen, Bauart, Lage und Nutzung vom Gebäude."@de ,
                                 "Contains information on dimensions, construction type, location and use of the building in the fire safety certificate."@en ;
                    rdfs:label "AllgemeineInformation"@de ,
                               "GeneralInformation"@en .


###  https://purl.org/fisa#GeneralSlab
:GeneralSlab rdf:type owl:Class ;
             owl:equivalentClass [ rdf:type owl:Restriction ;
                                   owl:onProperty :isStoreySlab ;
                                   owl:hasValue "false"^^xsd:boolean
                                 ] ;
             rdfs:subClassOf :Slab ;
             owl:disjointWith :StoreySlab ;
             rdfs:comment "A slab that is not a storey slab."@en ,
                          "Eine Decke, die keine Geschossdecke ist."@de ;
             rdfs:label "AllgemeineDecke"@de ,
                        "GeneralSlab"@en .


###  https://purl.org/fisa#Glazing
:Glazing rdf:type owl:Class ;
         rdfs:subClassOf :Closing ;
         rdfs:comment "Die Verwendung von Glas als Baumaterial zur Erstellung von transparenten Elementen wie Fenstern, Türen oder anderen Glasflächen in Gebäuden."@de ,
                      "The use of glass as a construction material to create transparent elements such as windows, doors or other glass surfaces in buildings."@en ;
         rdfs:label "Glazing"@en ,
                    "Verglasung"@de .


###  https://purl.org/fisa#GroundStorey
:GroundStorey rdf:type owl:Class ;
              rdfs:subClassOf :AboveGroundStorey ;
              owl:disjointWith :UpperStorey ;
              rdfs:label "Erdgeschoss"@de ,
                         "GroundStorey"@en .


###  https://purl.org/fisa#Gym
:Gym rdf:type owl:Class ;
     rdfs:subClassOf :SpaceUsage .


###  https://purl.org/fisa#HazardousEnvironment
:HazardousEnvironment rdf:type owl:Class ;
                      rdfs:subClassOf :UtilizationPurpose .


###  https://purl.org/fisa#HeatExtractionDevice
:HeatExtractionDevice rdf:type owl:Class ;
                      rdfs:subClassOf :TechnicalComponent ;
                      rdfs:comment "Diese Komponenten leiten im Brandfall Wärme/heiße Rauchgase ab, um einen rauchfreien Bereich in Bodennähe und auf Fluchtwegen sicherzustellen."@de ,
                                   "These components dissipate heat/hot smoke gases in the event of a fire to ensure a smoke-free area near the floor and on escape routes."@en ;
                      rdfs:label "HeatExtractionDevice"@en ,
                                 "Wärmeabzugsgerät"@de .


###  https://purl.org/fisa#HighRiseBuilding
:HighRiseBuilding rdf:type owl:Class ;
                  owl:equivalentClass [ rdf:type owl:Restriction ;
                                        owl:onProperty :hasAverageHeight ;
                                        owl:someValuesFrom [ rdf:type rdfs:Datatype ;
                                                             owl:onDatatype xsd:double ;
                                                             owl:withRestrictions ( [ xsd:minExclusive "22.0"^^xsd:double
                                                                                    ]
                                                                                  )
                                                           ]
                                      ] ;
                  rdfs:subClassOf :SpecialPurposeCondition ;
                  rdfs:comment """§2 (4) 1. MBO

'Buildings with a height surpassing 22 meters as specified in Section 3, Clause 2.'


_
Note:
The height being the average height."""@en ,
                               """§2 (4) 1. MBO

'Hochhäuser (Gebäude mit einer Höhe nach Absatz 3 Satz 2 von mehr als 22 m),'"""@de ;
                  rdfs:isDefinedBy :MHHR ;
                  rdfs:label "HighRiseBuilding"@en ,
                             "Hochhaus"@de ;
                  :gemäß "§2 (4) 1. MBO" .


###  https://purl.org/fisa#Hospital
:Hospital rdf:type owl:Class ;
          rdfs:subClassOf :SpecialPurposeCondition ;
          rdfs:comment "Medical facilities designed for diagnosing and treating patients, often equipped with medical technology and specialized personnel."@en ,
                       "Medizinische Einrichtungen, die zur Diagnose und Behandlung von Patienten dienen und oft mit medizinischer Technologie und spezialisiertem Personal ausgestattet sind."@de ;
          rdfs:label "Hospital"@en ,
                     "Krankenhaus"@de ;
          :gemäß "§2 (4) 10. MBO" .


###  https://purl.org/fisa#Hospitality
:Hospitality rdf:type owl:Class ;
             rdfs:subClassOf :UtilizationPurpose .


###  https://purl.org/fisa#Installation
:Installation rdf:type owl:Class ;
              rdfs:subClassOf <https://w3id.org/bot#Element> ;
              rdfs:comment "Einrichtungen oder Strukturen, die für die Verlegung von technischen Versorgungsleitungen, wie elektrische Kabel, Datenleitungen, Rohrleitungen für Wasser, Gas oder Heizung, vorgesehen sind."@de ,
                           "Facilities or structures intended for the installation of technical supply lines, such as electrical cables, data lines, pipelines for water, gas or heating."@en ;
              rdfs:label "Installation"@de ,
                         "Installation"@en .


###  https://purl.org/fisa#InstallationArea
:InstallationArea rdf:type owl:Class ;
                  rdfs:subClassOf :SiteDevelopmentMeasure ;
                  rdfs:label "Aufstellfläche"@de ,
                             "InstallationArea"@en ;
                  <http://www.w3.org/2004/02/skos/core#altLabel> "Footprint"@en .


###  https://purl.org/fisa#InstallationDuct
:InstallationDuct rdf:type owl:Class ;
                  rdfs:subClassOf :Installation ;
                  owl:disjointWith :InstallationShaft ;
                  rdfs:comment "Installation ducts are used to protect technical supply lines from damage and external influences."@en ,
                               "Installationskanäle dienen dazu, technische Versorgungsleitungen vor Beschädigungen und äußeren Einflüssen zu schützen."@de ;
                  rdfs:label "InstallationDuct"@en ,
                             "Installationskanal"@de .


###  https://purl.org/fisa#InstallationShaft
:InstallationShaft rdf:type owl:Class ;
                   rdfs:subClassOf :Installation ;
                   rdfs:comment "By using installation shafts, lines can be routed together from storey to storey through a building over several floors."@en ,
                                "Durch den Einsatz von Installationsschächten können Leitungen über mehrere Geschosse gemeinsam von Etage zu Etage durch ein Gebäude geführt werden."@de ;
                   rdfs:label "InstallationShaft"@en ,
                              "Installationsschacht"@de .


###  https://purl.org/fisa#Institution
:Institution rdf:type owl:Class ;
             rdfs:subClassOf :UtilizationPurpose .


###  https://purl.org/fisa#Insulation
:Insulation rdf:type owl:Class ;
            rdfs:subClassOf <https://w3id.org/bot#Element> ;
            rdfs:comment "A material used to reduce heat transfer between building components and thus improve the energy efficiency of a building."@en ,
                         "Ein Material, das verwendet wird, um die Wärmeübertragung zwischen Bauelementen zu reduzieren und somit die Energieeffizienz eines Gebäudes zu verbessern."@de ;
            rdfs:label "Dämmstoff"@de ,
                       "Insulation"@en .


###  https://purl.org/fisa#InternalFireWall
:InternalFireWall rdf:type owl:Class ;
                  rdfs:subClassOf :FireWall ;
                  <http://swrl.stanford.edu/ontologies/3.3/swrla.owl#isRuleEnabled> "InternalFireWall"@en ;
                  rdfs:comment """To: §30 (2) 2. and 3.

Fire walls are required
[...]
2.
As an internal fire wall for the subdivision of extensive buildings at intervals of no more than 40 m,
3. as an internal fire wall to divide agricultural buildings into fire compartments of not more than 10 000 m3 gross volume,
[...]"""@en ,
                               """zu: §30 (2) 2. und 3.

Brandwände sind erforderlich
[...]
2.
als innere Brandwand zur Unterteilung ausgedehnter Gebäude in Abständen von nicht mehr als 40 m,
3. als innere Brandwand zur Unterteilung landwirtschaftlich genutzter Gebäude in Brandabschnitte von nicht mehr als 10 000 m3 Brutto-Rauminhalt,
[...]"""@de ;
                  rdfs:label "InnereBrandwand"@de ,
                             "InternalFireWall"@en .


###  https://purl.org/fisa#JointSealing
:JointSealing rdf:type owl:Class ;
              rdfs:subClassOf :AssemblyProduct ;
              rdfs:comment "Process or technique of sealing joints or gaps between different building elements, materials or surfaces."@en ,
                           "Prozess oder die Technik des Abdichtens von Fugen oder Spalten zwischen verschiedenen Bauelementen, Materialien oder Oberflächen."@de ;
              rdfs:label "Fugendichtung"@de ,
                         "JointSealing"@en .


###  https://purl.org/fisa#Kindergarden
:Kindergarden rdf:type owl:Class ;
              rdfs:subClassOf :UtilizationPurpose .


###  https://purl.org/fisa#Kitchen
:Kitchen rdf:type owl:Class ;
         rdfs:subClassOf :SpaceUsage .


###  https://purl.org/fisa#Lab
:Lab rdf:type owl:Class ;
     rdfs:subClassOf :UtilizationPurpose .


###  https://purl.org/fisa#LawEnforcement
:LawEnforcement rdf:type owl:Class ;
                rdfs:subClassOf :UtilizationPurpose .


###  https://purl.org/fisa#Leisure
:Leisure rdf:type owl:Class ;
         rdfs:subClassOf :UtilizationPurpose .


###  https://purl.org/fisa#LightningSafetySystem
:LightningSafetySystem rdf:type owl:Class ;
                       rdfs:subClassOf :TechnicalComponent ;
                       rdfs:comment "Precautions against the harmful effects of lightning strikes on building structures."@en ,
                                    "Vorkehrungen gegen schädliche Auswirkungen von Blitzeinschlägen auf bauliche Anlagen."@de ;
                       rdfs:label "Blitzschutzanlage"@de ,
                                  "LightningSafetySystem"@en .


###  https://purl.org/fisa#LivingRoom
:LivingRoom rdf:type owl:Class ;
            rdfs:subClassOf :SpaceUsage .


###  https://purl.org/fisa#LoadbearingEnclosingComponent
:LoadbearingEnclosingComponent rdf:type owl:Class ;
                               rdfs:subClassOf :ComponentType ;
                               rdfs:comment "Load-bearing, space-enclosing components meet both load-bearing and space-enclosing requirements."@en ,
                                            "Tragende, raumabschließende Komponenten erfüllen sowohl Anforderungen an die Tragfähigkeit, als auch an den Raumabschluss."@de ;
                               rdfs:label "LoadbearingEnclosingComponent"@en ,
                                          "TragendeRaumabschließendeKomponente"@de .


###  https://purl.org/fisa#LoadbearingNonEnclosingComponent
:LoadbearingNonEnclosingComponent rdf:type owl:Class ;
                                  rdfs:subClassOf :ComponentType ;
                                  rdfs:comment "Load-bearing, non space-enclosing components meet only load-bearing and no space-enclosing requirements."@en ,
                                               "Tragende,nicht-raumabschließende Komponenten erfüllen Anforderungen an die Tragfähigkeit, aber nicht an den Raumabschluss."@de ;
                                  rdfs:label "LoadbearingNonEnclosingComponent"@en ,
                                             "TragendeNichtraumabschließendeKomponented"@de .


###  https://purl.org/fisa#MBO
:MBO rdf:type owl:Class ;
     rdfs:subClassOf :Mustervorschrift ;
     rdfs:comment """-Stand August 2023-
Nutzung von:
Musterbauordnung - Fassung November 2022, zuletzt geändert 25.09.2020"""@de ,
                  """-as of August 2023-
Use of:
Musterbauordnung- version November 2022, last amended 25.09.2020"""@en ,
                  """A = Absatz
P = Punkt
S = Satz"""@de ,
                  """S = Section
P = Point
Se = Sentence"""@en ,
                  """§1 MBO

(1) [S1]This Act applies to structural facilities and construction products. [S2]It also applies to land and other facilities and installations for which requirements are set out in this Act or in regulations based on this Act.
(2) This Act shall not apply to
1. public transportation facilities, including appurtenances, ancillary facilities, and ancillary operations, except buildings,
2. facilities subject to mining supervision, except buildings,
3. pipelines serving the public supply of water, gas, electricity, heat, public sewage disposal or telecommunications,
4. pipelines serving the long-distance transport of materials,
5. cranes and crane systems,
6. exhibition stands in trade fair and exhibition buildings."""@en ;
     rdfs:label "MBO"@de ,
                "MBO"@en ;
     <http://www.w3.org/2004/02/skos/core#altLabel> "Federal Building Code"@en ,
                                                    "General Building Code"@en ,
                                                    "Musterbauordnung"@de ;
     :anwendungsbereich """§1 MBO

(1) [S1]Dieses Gesetz gilt für bauliche Anlagen und Bauprodukte. [S2]Es gilt auch für Grundstücke sowie für andere Anlagen und Einrichtungen, an die in diesem Gesetz oder in Vorschriften aufgrund dieses Gesetzes Anforderungen gestellt werden.
(2) Dieses Gesetz gilt nicht für
1. Anlagen des öffentlichen Verkehrs einschließlich Zubehör, Nebenanlagen und Nebenbetrieben, ausgenommen Gebäude,
2. Anlagen, die der Bergaufsicht unterliegen, ausgenommen Gebäude,
3. Leitungen, die der öffentlichen Versorgung mit Wasser, Gas, Elektrizität, Wärme, der öffentlichen Abwasserentsorgung oder der Telekommunikation dienen,
4. Rohrleitungen, die dem Ferntransport von Stoffen dienen,
5. Kräne und Krananlagen,
6. Messestände in Messe- und Ausstellungsgebäuden."""@de .


###  https://purl.org/fisa#MBeVO
:MBeVO rdf:type owl:Class ;
       rdfs:subClassOf :Sonderbauverordnung ;
       rdfs:comment "Die Sonderbauverordnung über Berherbungsstätten."@de ,
                    "The special purpose construction regulation on accommodations."@en ;
       rdfs:label "MBeVO"@de ,
                  "MBeVO"@en ;
       <http://www.w3.org/2004/02/skos/core#altLabel> "Accommodation-Regulation"@en ,
                                                      "Beherbergungsstättenverordnung"@de .


###  https://purl.org/fisa#MEltBauVO
:MEltBauVO rdf:type owl:Class ;
           rdfs:subClassOf :Sonderbauverordnung ;
           rdfs:comment "Die Sonderbauverordnung über den Bau von Betriebsräumen für elektrische Anlagen."@de ,
                        "The special purpose construction regulation on the construction and operation for electrical equipment."@en ;
           rdfs:label "MEltBauVO"@de ,
                      "MEltBauVO"@en ;
           <http://www.w3.org/2004/02/skos/core#altLabel> "Regulation on the construction of operating spaces for electrical equipment"@en ,
                                                          "Verordnung über den Bau von Betriebsräumen für elektrische Anlagen"@de .


###  https://purl.org/fisa#MHHR
:MHHR rdf:type owl:Class ;
      rdfs:subClassOf :Sonderbaurichtlinie ;
      rdfs:comment "Die Sonderbaurichtlinie über Hochhäuser."@de ,
                   "The special purpose construction guideline on high-rise buildings."@en ;
      rdfs:label "MHHR"@de ,
                 "MHHR"@en ;
      <http://www.w3.org/2004/02/skos/core#altLabel> "Guideline on the construction and operation of Highrise-Buildings"@en ,
                                                     "Richtlinie über den Bau und Betrieb von Hochhäusern"@de .


###  https://purl.org/fisa#MSchulbauR
:MSchulbauR rdf:type owl:Class ;
            rdfs:subClassOf :Sonderbaurichtlinie ;
            rdfs:comment "Die Sonderbaurichtlinie über Schulgebäude."@de ,
                         "The special purpose construction guideline on school buildings."@en ;
            rdfs:label "MSchulbauR"@de ,
                       "MSchulbauR"@en ;
            <http://www.w3.org/2004/02/skos/core#altLabel> "General-School-Guideline"@en ,
                                                           "Muster-Schulbau-Richtlinie"@de .


###  https://purl.org/fisa#MVKVO
:MVKVO rdf:type owl:Class ;
       rdfs:subClassOf :Sonderbauverordnung ;
       rdfs:comment "Die Sonderbauverordnung über Verkaufsstätten."@de ,
                    "The special purpose construction regulation on sales premises."@en ;
       rdfs:label "MVKVO"@de ,
                  "MVKVO"@en ;
       <http://www.w3.org/2004/02/skos/core#altLabel> "Sales Premises-Regulation"@en ,
                                                      "Verkaufsstättenverordnung"@de .


###  https://purl.org/fisa#MVStättVO
:MVStättVO rdf:type owl:Class ;
           rdfs:subClassOf :Sonderbauverordnung ;
           rdfs:comment "Die Sonderbauverordnung über Versammlungsstätten."@de ,
                        "The special purpose construction regulation on places of assembly."@en ;
           rdfs:label "MVStättVO"@de ,
                      "MVStättVO"@en ;
           <http://www.w3.org/2004/02/skos/core#altLabel> "General-Regulation on Places of Assembly"@en ,
                                                          "Muster-Versammlungsstättenverordnung"@de .


###  https://purl.org/fisa#MVV_TB
:MVV_TB rdf:type owl:Class ;
        rdfs:subClassOf :MusterVerwaltungsvorschrift ;
        owl:disjointWith :M_FIBauVwV ;
        rdfs:comment """- Stand August 2013 -
Ausgabe 2023/1 (angehört als MVV TB 2022/1)"""@de ,
                     """- as of August 2023 -
Edition 2023/1 (heard as MVV TB 2022/1)en"""@en ,
                     """Administrative regulations are abstract-general rules issued by the administration for the administration, i.e. rules that the administration issues itself.

Technical building regulations are the generally recognized rules of technology introduced by public notice."""@en ,
                     """Bei Verwaltungsvorschriften handelt es sich um abstrakt-generelle Regeln der Verwaltung für die Verwaltung, also Regeln die sich die Verwaltung selbst gibt.

Technische Baubestimmungen sind die durch öffentliche Bekanntmachung eingeführten, allgemein anerkannten Regeln der Technik."""@de ;
        rdfs:label "MVV_TB"@de ,
                   "MVV_TB"@en ;
        <http://www.w3.org/2004/02/skos/core#altLabel> "General-Administrative Technical Building-Prescription"@en ,
                                                       "Muster-Verwaltungsvorschrift Technische Baubestimmungen"@de .


###  https://purl.org/fisa#MWR
:MWR rdf:type owl:Class ;
     rdfs:subClassOf :Sonderbaurichtlinie ;
     rdfs:comment "Die Sonderbaurichtlinie über Wohnformen."@de ,
                  "The special purpose construction guideline on Residential Facilities."@en ;
     rdfs:label "MWR"@de ,
                "MWR"@en ;
     <http://www.w3.org/2004/02/skos/core#altLabel> "General-Residential-Guideline"@en ,
                                                    "Muster-Richtlinie über bauaufsichtliche Anforderungen an Wohnformen für Menschen mit Pflegebedürftigkeit oder mit Behinderung"@de ,
                                                    "Muster-Wohnformen-Richtlinie"@de .


###  https://purl.org/fisa#M_FIBauR
:M_FIBauR rdf:type owl:Class ;
          rdfs:subClassOf :Sonderbaurichtlinie ;
          rdfs:comment "Die Sonderbaurichtlinie über Fliegende Bauten."@de ,
                       "The special purpose construction guideline on portable construction."@en ;
          rdfs:label "M_FIBauR"@de ,
                     "M_FIBauR"@en ;
          <http://www.w3.org/2004/02/skos/core#altLabel> "General-Guideline on the construction and operation of Flying Structures"@en ,
                                                         "Muster-Richtlinie über den Bau und Betrieb Fliegender Bauten"@de .


###  https://purl.org/fisa#M_FIBauVwV
:M_FIBauVwV rdf:type owl:Class ;
            rdfs:subClassOf :MusterVerwaltungsvorschrift ;
            rdfs:comment "Administrative regulations are abstract-general rules issued by the administration for the administration, i.e. rules that the administration issues itself."@en ,
                         "Bei Verwaltungsvorschriften handelt es sich um abstrakt-generelle Regeln der Verwaltung für die Verwaltung, also Regeln die sich die Verwaltung selbst gibt."@de ;
            rdfs:label "M_FIBauVwV"@de ,
                       "M_FIBauVwV"@en ;
            <http://www.w3.org/2004/02/skos/core#altLabel> "General Administrative Prescription on execution permits for Flying Structures and their acceptance for use"@en ,
                                                           "Muster-Verwaltungsvorschrift über Ausführungsgenehmigungen für Fliegende Bauten und deren Gebrauchsabnahmen"@de .


###  https://purl.org/fisa#MeetingRoom
:MeetingRoom rdf:type owl:Class ;
             rdfs:subClassOf :SpaceUsage .


###  https://purl.org/fisa#MusterVerwaltungsvorschrift
:MusterVerwaltungsvorschrift rdf:type owl:Class ;
                             rdfs:subClassOf :Mustervorschrift ;
                             rdfs:comment "Administrative regulations are abstract-general rules issued by the administration for the administration, i.e. rules that the administration issues itself."@en ,
                                          "Bei Verwaltungsvorschriften handelt es sich um abstrakt-generelle Regeln der Verwaltung für die Verwaltung, also Regeln die sich die Verwaltung selbst gibt."@de ;
                             rdfs:label "GeneralAdministrativeRegulation"@en ,
                                        "MusterVerwaltungsvorschrift"@de ;
                             <http://www.w3.org/2004/02/skos/core#altLabel> "SampleAdministrativeRegulation"@en .


###  https://purl.org/fisa#Musterrichtlinie
:Musterrichtlinie rdf:type owl:Class ;
                  rdfs:subClassOf :Mustervorschrift ;
                  rdfs:comment "A guideline is a legal act in which a goal to be achieved by all countries/counties is specified. However, it is up to the individual countries/counties to enact their own legislation to achieve this goal."@en ,
                               "Eine Richtlinie ist ein Rechtsakt, in dem ein von allen EU-Ländern zu erreichendes Ziel festgelegt wird. Es ist jedoch Sache der einzelnen Länder, eigene Rechtsvorschriften zur Verwirklichung dieses Ziels zu erlassen."@de ;
                  rdfs:label "GeneralGuideline"@en ,
                             "Musterrichtlinie"@de ;
                  <http://www.w3.org/2004/02/skos/core#altLabel> "SampleGuideline"@en .


###  https://purl.org/fisa#Mustervorschrift
:Mustervorschrift rdf:type owl:Class ;
                  rdfs:subClassOf :RuleOfApplication ;
                  rdfs:label "GeneralPrescription"@en ,
                             "Mustervorschrift"@de ;
                  <http://www.w3.org/2004/02/skos/core#altLabel> "SamplePrescription"@en .


###  https://purl.org/fisa#NecessaryCorridor
:NecessaryCorridor rdf:type owl:Class ;
                   owl:equivalentClass [ owl:intersectionOf ( [ rdf:type owl:Restriction ;
                                                                owl:onProperty :hasSpaceUsage ;
                                                                owl:hasValue :Corridor
                                                              ]
                                                              [ rdf:type owl:Restriction ;
                                                                owl:onProperty :isNecessary ;
                                                                owl:hasValue "true"^^xsd:boolean
                                                              ]
                                                            ) ;
                                         rdf:type owl:Class
                                       ] ;
                   rdfs:subClassOf <https://w3id.org/bot#Space> ,
                                   [ rdf:type owl:Restriction ;
                                     owl:onProperty :isPartOf ;
                                     owl:someValuesFrom :RescueConcept
                                   ] ;
                   rdfs:comment "Der horizontale Flucht- und Rettungsweg zwischen Nutzungseinheiten und dem Treppenraum oder ins Freie wird als notwendiger Flur bezeichnet."@de ,
                                "The horizontal escape and rescue route between utilization units and the stairwell or to the outside is called a necessary corridor."@en ;
                   rdfs:label "NecessaryCorridor"@en ,
                              "NotwendigerFlur"@de .


###  https://purl.org/fisa#NecessaryStairSpace
:NecessaryStairSpace rdf:type owl:Class ;
                     owl:equivalentClass [ owl:intersectionOf ( [ rdf:type owl:Restriction ;
                                                                  owl:onProperty :hasSpaceUsage ;
                                                                  owl:hasValue :StairSpace
                                                                ]
                                                                [ rdf:type owl:Restriction ;
                                                                  owl:onProperty :isNecessary ;
                                                                  owl:hasValue "true"^^xsd:boolean
                                                                ]
                                                              ) ;
                                           rdf:type owl:Class
                                         ] ;
                     rdfs:subClassOf <https://w3id.org/bot#Space> ,
                                     [ rdf:type owl:Restriction ;
                                       owl:onProperty :isPartOf ;
                                       owl:someValuesFrom :RescueConcept
                                     ] ;
                     rdfs:comment "Necessary stairwells are vertically continuous spaces in which one or more stairways may be located that serve to protect a necessary stairway."@en ,
                                  "Notwendige Treppenräume sind vertikal durchgehende Räume, in denen sich eine oder mehrere Treppen befinden können, die dem Schutz einer notwendigen Treppe dienen."@de ;
                     rdfs:label "NecessaryStairSpace"@en ,
                                "NotwendigerTreppenraum"@de .


###  https://purl.org/fisa#NonLoadbearingEnclosingComponent
:NonLoadbearingEnclosingComponent rdf:type owl:Class ;
                                  rdfs:subClassOf :ComponentType ;
                                  rdfs:comment "Nicht-tragende, raumabschließende Komponenten erfüllen keine Anforderungen an die Tragfähigkeit, aber an den Raumabschluss."@de ,
                                               "Non-load-bearing, space-enclosing components meet no load-bearing, but space-enclosing requirements."@en ;
                                  rdfs:label "NichttragendeRaumabschließendeKomponente"@de ,
                                             "NonLoadbearingEnclosingComponent"@en .


###  https://purl.org/fisa#NonLoadbearingNonEnclosingComponent
:NonLoadbearingNonEnclosingComponent rdf:type owl:Class ;
                                     rdfs:subClassOf :ComponentType ;
                                     rdfs:comment "Nicht-tragende, nicht-raumabschließende Komponenten erfüllen weder Anforderungen an die Tragfähigkeit, noch an den Raumabschluss."@de ,
                                                  "Non-load-bearing, non-space-enclosing components meet neither load-bearing nor space-enclosing requirements."@en ;
                                     rdfs:label "NichttragendeNichtraumabschließendeKomponente"@de ,
                                                "NonLoadbearingNonEnclosingComponent"@en .


###  https://purl.org/fisa#Norm
:Norm rdf:type owl:Class ;
      rdfs:subClassOf :RuleOfApplication ;
      rdfs:label "Norm"@de ,
                 "Norm"@en .


###  https://purl.org/fisa#NursingHome
:NursingHome rdf:type owl:Class ;
             rdfs:subClassOf :SpecialPurposeCondition ;
             rdfs:comment """§2 (4) 9. MBO

'Buildings with units for care or assistance of individuals with limited self-evacuation capability due to disabilities, if the units:
a) Serve more than 6 individuals individually
b) Serve individuals requiring intensive care
c) Share a common escape route and serve more than 12 individuals collectively'"""@en ,
                          """§2 (4) 9. MBO

'Gebäude mit Nutzungseinheiten zum Zwecke der Pflege oder Betreuung von Personen mit Pflegebedürftigkeit oder Behinderung, deren Selbstrettungsfähigkeit eingeschränkt ist, wenn die Nutzungseinheiten
a) einzeln für mehr als 6 Personen oder
b) für Personen mit Intensivpflegebedarf bestimmt sind, oder
c) einen gemeinsamen Rettungsweg haben und für insgesamt mehr als 12 Personen bestimmt sind,'"""@de ;
             rdfs:isDefinedBy :MWR ;
             rdfs:label "NursingHome"@en ,
                        "Pflegestätte"@de ;
             :gemäß "§2 (4) 9. MBO" .


###  https://purl.org/fisa#ObjectRadioSystemForFireBrigade
:ObjectRadioSystemForFireBrigade rdf:type owl:Class ;
                                 rdfs:subClassOf :TechnicalComponent ;
                                 rdfs:comment "An object radio system is a stationary radio-technical device for the operational support of the fire department."@en ,
                                              "Eine Objektfunkanlage ist eine stationäre funktechnische Einrichtung zur Einsatzunterstützung der Feuerwehr."@de ;
                                 rdfs:label "ObjectRadioSystem_for_FireBrigade"@en ,
                                            "Objektfunkanlage_für_die_Feuerwehr"@de .


###  https://purl.org/fisa#OfficeRoom
:OfficeRoom rdf:type owl:Class ;
            rdfs:subClassOf :SpaceUsage .


###  https://purl.org/fisa#OpenProfile
:OpenProfile rdf:type owl:Class ;
             owl:equivalentClass [ owl:intersectionOf ( :Profile
                                                        [ rdf:type owl:Restriction ;
                                                          owl:onProperty :isClosedProfile ;
                                                          owl:hasValue "false"^^xsd:boolean
                                                        ]
                                                      ) ;
                                   rdf:type owl:Class
                                 ] ;
             rdfs:subClassOf :Profile ;
             rdfs:comment "Wall profile with an open shape."@en ,
                          "Wandprofil mit offener Querschnittsform."@de ;
             rdfs:label "OffenesProfil"@de ,
                        "OpenProfile"@en .


###  https://purl.org/fisa#Opening
:Opening rdf:type owl:Class ;
         rdfs:subClassOf :Component ;
         rdfs:comment "Die Komponente 'Öffnung' steht für eine Öffnung, eine Aussparung oder einen Schlitz, die alle die Leere widerspiegeln. Es steht für eine Leerstelle innerhalb eines Elements, das eine physische Manifestation hat. [IfcOpeningElement]"@de ,
                      "The opening element stands for opening, recess or chase, all reflecting voids. It represents a void within any element that has physical manifestation. [IfcOpeningElement]"@en ;
         rdfs:isDefinedBy :MBO ;
         rdfs:label "Opening"@en ,
                    "Öffnung"@de ;
         :gemäß "§37 MBO"@de .


###  https://purl.org/fisa#OrganizationalFireSafety
:OrganizationalFireSafety rdf:type owl:Class ;
                          rdfs:subClassOf :FireSafety ;
                          rdfs:comment """Der Organisatorische Brandschutz ist Teil des vorbeugenden Brandschutzes. Aufgabengebiete sind:
- Instandhaltung, Wartung, Nutzung von und richtiger Umgang mit baulichen und technischen Brandschutzeinrichtungen
- Kennzeichnung und Freihaltung von Flucht- und Rettungswegen
- Aushang von Brandschutzordnungen zur Brandvermeidung und
- für Maßnahmen im Notfall (Notruf Feuerwehr)"""@de ,
                                       """Organizational fire safety is part of preventive fire safety. Tasks contain:
- Maintenance, servicing, use of and correct handling of structural and technical fire protection equipment
Marking and keeping clear escape and rescue routes
- Posting of fire protection regulations for fire prevention and
- for measures to be taken in an emergency (emergency call to the fire department)"""@en ;
                          rdfs:label "OrganisatorischeBrandschutz"@de ,
                                     "OrganizationalFireSafety"@en .


###  https://purl.org/fisa#OtherCertificate
:OtherCertificate rdf:type owl:Class ;
                  rdfs:subClassOf :TechnicalStructuralCertificate ;
                  rdfs:comment "Andere Bautechnischen Nachweise, die keine Brandschutznachweise sind."@de ,
                               "Other technical structural certificates that are not fire safety certificates."@en ;
                  rdfs:label "AndererNachweis"@de ,
                             "OtherCertificate"@en .


###  https://purl.org/fisa#OtherRoomUsage
:OtherRoomUsage rdf:type owl:Class ;
                rdfs:subClassOf :SpaceUsage .


###  https://purl.org/fisa#OvernightAccommodation
:OvernightAccommodation rdf:type owl:Class ;
                        rdfs:subClassOf :UtilizationPurpose .


###  https://purl.org/fisa#PanelInstitutionForLegalExecutiveRegulations
:PanelInstitutionForLegalExecutiveRegulations rdf:type owl:Class ;
                                              rdfs:subClassOf :SpecialPurposeCondition ;
                                              <http://purl.org/dc/terms/description> """§2 (4) 14. MBO

'Justizvollzugsanstalten und bauliche Anlagen für den Maßregelvollzug,'"""@de ;
                                              rdfs:comment "Buildings and structures used for detention or rehabilitation as part of the judicial system."@en ,
                                                           "Gebäude und Strukturen, die für Inhaftierung oder Rehabilitation im Rahmen des Justizsystems genutzt werden."@de ;
                                              rdfs:label "BaulicheAnlageFürDenMaßregelvollzug"@de ,
                                                         "PanelInstitutionForLegalExecutiveRegulations"@en ;
                                              :gemäß "§2 (4) 14. MBO" .


###  https://purl.org/fisa#Parapet
:Parapet rdf:type owl:Class ;
         rdfs:subClassOf :WallParts ;
         rdfs:comment "A raised area that borders or covers a lower area or opening."@en ,
                      "Einen erhöhten Bereich, der eine niedrigere Fläche oder eine Öffnung begrenzt oder abdeckt."@de ;
         rdfs:label "Brüstung"@de ,
                    "Parapet"@en .


###  https://purl.org/fisa#Parking
:Parking rdf:type owl:Class ;
         rdfs:subClassOf :UtilizationPurpose .


###  https://purl.org/fisa#ParkingSpace
:ParkingSpace rdf:type owl:Class ;
              rdfs:subClassOf <https://w3id.org/bot#Site> ;
              <http://purl.org/dc/terms/description> "Stellplätze sind Flächen, die dem Abstellen von Kraftfahrzeugen außerhalb der öffentlichen Verkehrsflächen dienen."@de ;
              rdfs:comment """Ausnahme aus §2 (7) S3 MBO:
Ausstellungs-, Verkaufs-, Werk- und Lagerräume für Kraftfahrzeuge sind keine Stellplätze oder Garagen."""@de ,
                           """Exception from §2 (7) S3 MBO:
Showrooms, salesrooms, workshops and storage rooms for motor vehicles are not parking spaces or garages."""@en ,
                           "Parking spaces are areas used for parking (motor) vehicles outside of public traffic areas."@en ;
              rdfs:isDefinedBy :MBO ;
              rdfs:label "ParkingSpace"@en ,
                         "Stellplatz"@de ;
              :gemäß "§2 (7) S1 MBO"@de .


###  https://purl.org/fisa#PenalInstitution
:PenalInstitution rdf:type owl:Class ;
                  rdfs:subClassOf :SpecialPurposeCondition ;
                  <http://purl.org/dc/terms/description> """§2 (4) 14. MBO

'Justizvollzugsanstalten und bauliche Anlagen für den Maßregelvollzug,'"""@de ;
                  rdfs:comment "Buildings and structures used for detention or rehabilitation as part of the judicial system."@en ,
                               "Gebäude und Strukturen, die für Inhaftierung oder Rehabilitation im Rahmen des Justizsystems genutzt werden."@de ;
                  rdfs:label "Justizvollzugsanstalt"@de ,
                             "PenalInstitution"@en ;
                  :gemäß "§2 (4) 14. MBO" .


###  https://purl.org/fisa#PlanningDocument
:PlanningDocument rdf:type owl:Class ;
                  rdfs:subClassOf :AssessmentBasis ;
                  rdfs:comment "Planning documents include 2D-documents and/or 3D-models."@en ,
                               "Planungsunterlagen können 2D-Plände oder 3D-Modelle sein."@de ;
                  rdfs:label "PlanningDocument"@en ,
                             "Planungsunterlage"@de .


###  https://purl.org/fisa#PortableConstruction
:PortableConstruction rdf:type owl:Class ;
                      rdfs:subClassOf :SpecialPurposeCondition ;
                      rdfs:comment "Non-permanent constructions needing authorization for erection, often used for events or specific purposes."@en ,
                                   "Soweit sie einer Ausnahmegenehmigung bedürfen." ;
                      rdfs:isDefinedBy :M_FIBauR ;
                      rdfs:label "FliegendeBauten"@de ,
                                 "PortableConstruction"@en ;
                      :gemäß "§2 (4) 17. MBO" .


###  https://purl.org/fisa#PositionAccessibleForFireService
:PositionAccessibleForFireService rdf:type owl:Class ;
                                  owl:equivalentClass [ owl:intersectionOf ( [ rdf:type owl:Class ;
                                                                               owl:unionOf ( :Opening
                                                                                             :Parapet
                                                                                             :Window
                                                                                           )
                                                                             ]
                                                                             [ rdf:type owl:Restriction ;
                                                                               owl:onProperty :accessibleForFireServices ;
                                                                               owl:hasValue "true"^^xsd:boolean
                                                                             ]
                                                                           ) ;
                                                        rdf:type owl:Class
                                                      ] ;
                                  rdfs:subClassOf :ComponentType ;
                                  rdfs:comment "Areas, locations, or positions in a building that can be reached by a ladder or similar access device in the event of a fire or emergency by rescue or evacuation teams."@en ,
                                               "Bereiche, Standorte oder Positionen in einem Gebäude, die durch eine Leiter oder eine ähnliche Aufstiegsvorrichtung im Falle eines Brands oder Notfalls von Rettungskräften oder Evakuierungsteams erreichbar sind."@de ;
                                  rdfs:label "AnleiterStelle"@de ,
                                             "PositionAccessibleForFireService"@en ;
                                  :thematik <http://www.systemsEngineering.org/isabellefitkau/fisa.owl#Rettungskonzept> .


###  https://purl.org/fisa#Posts
:Posts rdf:type owl:Class ;
       rdfs:subClassOf :AssemblyProduct ;
       rdfs:comment "Vertical structural element that usually has a supporting or load-bearing function."@en ,
                    "Vertikales Bauelement, das in der Regel eine stützende oder tragende Funktion hat."@de ;
       rdfs:label "Pfosten"@de ,
                  "Posts"@en .


###  https://purl.org/fisa#PrescriptiveCertificate
:PrescriptiveCertificate rdf:type owl:Class ;
                         rdfs:subClassOf :FireSafetyCertificate ;
                         owl:disjointWith :ProtectiveGoalOrientedCertificate ;
                         rdfs:comment "Dieser Ansatz basiert auf vorgegebenen Bauordnungen, Vorschriften, Normen und Regeln, die spezifische Brandschutzanforderungen für verschiedene Baukomponenten, Baustoffe und Situationen festlegen."@de ,
                                      "This approach is based on predetermined building regulations, standards and rules that establish specific fire safety requirements for various building components, materials and situations."@en ;
                         rdfs:label "PrescriptiveCertificate"@en ,
                                    "PräskriptiverNachweis"@de .


###  https://purl.org/fisa#Profile
:Profile rdf:type owl:Class ;
         rdfs:subClassOf :WallParts ;
         rdfs:comment "Wall profile with specific cross-sectional shape."@en ,
                      "Wandprofil mit bestimmter Querschnittsform."@de ;
         rdfs:label "Profil"@de ,
                    "Profile"@en .


###  https://purl.org/fisa#ProtectiveGoal
:ProtectiveGoal rdf:type owl:Class ;
                rdfs:comment """Protection goals based on the MBO:

§14 MBO
Structural facilites are to be arranged, erected, modified and maintained in such a way that the development of fire and the spread of fire and smoke (fire spread) is prevented and, in the event of fire, the rescue of people and animals and effective extinguishing work are possible."""@en ,
                             """Schutzziele basierend auf der MBO:

§14 MBO

Bauliche Anlagen sind so anzuordnen, zu errichten, zu ändern und instand zu halten, dass der Entstehung eines Brandes und der Ausbreitung von Feuer und Rauch (Brandausbreitung) vorgebeugt wird und bei einem Brand die Rettung von Menschen und Tieren sowie wirksame Löscharbeiten möglich sind."""@de ;
                rdfs:label "ProtectiveGoal"@en ,
                           "Schutzziel"@de .


###  https://purl.org/fisa#ProtectiveGoalOrientedCertificate
:ProtectiveGoalOrientedCertificate rdf:type owl:Class ;
                                   rdfs:subClassOf :FireSafetyCertificate ,
                                                   [ rdf:type owl:Restriction ;
                                                     owl:onProperty :isBasedOn ;
                                                     owl:allValuesFrom :ProtectiveGoal
                                                   ] ;
                                   rdfs:comment "Dieser Ansatz zielt darauf ab, übergeordnete Schutzziele zu erreichen und individuelle Lösungen (für Abweichungen) zu erarbeiten, die diese Schutzziele erreichen."@de ,
                                                "This approach aims to achieve overall protective goals and to develop individual solutions (for deviations) that achieve these protective goals."@en ;
                                   rdfs:label "ProtectiveGoalOrientedCertificate"@en ,
                                              "SchutzzielorienterterNachweis"@de .


###  https://purl.org/fisa#RegulatedSpecialPurposeConstruction
:RegulatedSpecialPurposeConstruction rdf:type owl:Class ;
                                     rdfs:subClassOf :SpecialPurposeConstruction ;
                                     owl:disjointWith :UnregulatedSpecialPurposeConstruction ;
                                     rdfs:comment "Geregelte Sonderbauten sind Sonderbauten, für die es eine Sonderbau-Vorschrift gibt. Im Gegensatz zu ungeregelten Sonderbauten gibt es für geregelte Sonderbauten einheitlichen Vorschriften."@de ,
                                                  "Regulated special purpose constructions are special purpose constructions for which there is a special purpose construction regulation. In contrast to unregulated special purpose construction, there are uniform regulations for regulated special puprose construction."@en ;
                                     rdfs:label "GeregelterSonderbau"@de ,
                                                "RegulatedSpecialPurposeConstruction"@en .


###  https://purl.org/fisa#RescueConcept
:RescueConcept rdf:type owl:Class ;
               rdfs:subClassOf :FireSafety ,
                               [ rdf:type owl:Restriction ;
                                 owl:onProperty :isNeededBy ;
                                 owl:someValuesFrom :StructuralFacility
                               ] ,
                               [ rdf:type owl:Restriction ;
                                 owl:onProperty :hasPart ;
                                 owl:minQualifiedCardinality "0"^^xsd:nonNegativeInteger ;
                                 owl:onClass [ owl:intersectionOf ( :EscapeRoute
                                                                    :PositionAccessibleForFireService
                                                                  ) ;
                                               rdf:type owl:Class
                                             ]
                               ] ;
               rdfs:comment "A rescue concept or deployment strategy describes the approach taken by emergency service personnel in taking their actions in an emergency."@en ,
                            "Ein Rettungskonzept oder eine Einsatzstrategie beschreibt das Vorgehen von Einsatzkräften des Rettungsdienstes beim Ergreifen ihrer Maßnahmen im Notfall."@de ;
               rdfs:label "RescueConcept"@en ,
                          "Rettungskonzept"@de .


###  https://purl.org/fisa#ResidenceSpace
:ResidenceSpace rdf:type owl:Class ;
                owl:equivalentClass [ rdf:type owl:Restriction ;
                                      owl:onProperty :isPossibleForResidence ;
                                      owl:hasValue "true"^^xsd:boolean
                                    ] ;
                rdfs:subClassOf <https://w3id.org/bot#Space> ;
                rdfs:comment "Aufenthaltsräume sind Räume, die zum nicht nur vorübergehenden Aufenthalt von Menschen bestimmt oder geeignet sind."@de ,
                             "Residence Rooms are rooms which are intended or suitable for the not only temporary stay of people."@en ;
                rdfs:label "Aufenthaltsraum"@de ,
                           "ResidenceSpace"@en ;
                :gemäß "§2 (5) MBO"@de .


###  https://purl.org/fisa#Residential
:Residential rdf:type owl:Class ;
             rdfs:subClassOf :UtilizationPurpose .


###  https://purl.org/fisa#Roof
:Roof rdf:type owl:Class ;
      rdfs:subClassOf <https://w3id.org/bot#Element> ;
      rdfs:comment "Die oberste strukturelle Abdeckung eines Gebäudes, die dazu dient, es vor Witterungseinflüssen wie Regen, Schnee, Sonneneinstrahlung und Wind zu schützen."@de ,
                   "The top structural covering of a building used to protect it from the elements such as rain, snow, sunlight, and wind."@en ;
      rdfs:label "Dach"@de ,
                 "Roof"@en .


###  https://purl.org/fisa#RoofStructure
:RoofStructure rdf:type owl:Class ;
               rdfs:subClassOf :Structure ;
               owl:disjointWith :Roofing ;
               rdfs:comment "Beschreibt die tragenden Komponenten, das Tragwerk, des Daches."@de ,
                            "Describes the load-bearing components, the supporting structure, of the roof."@en ;
               rdfs:label "Dachtragwerk"@de ,
                          "RoofStructure"@en .


###  https://purl.org/fisa#Roofing
:Roofing rdf:type owl:Class ;
         rdfs:subClassOf <https://w3id.org/bot#Element> ;
         rdfs:comment "Die Gesamtheit der strukturellen Elemente, Materialien und Vorrichtungen, die verwendet werden, um das Dach eines Gebäudes zu konstruieren und zu schützen."@de ,
                      "The set of structural elements, materials and devices used to construct and protect the roof of a building."@en ;
         rdfs:label "Bedachung"@de ,
                    "Roofing"@en .


###  https://purl.org/fisa#RuleOfApplication
:RuleOfApplication rdf:type owl:Class ;
                   rdfs:subClassOf :AssessmentBasis ;
                   rdfs:comment """Represents the application rule according to which the requirements are \"according to\".

Example:
The partition wall must be at least \"fire-retardant\", according to §19 (3) MusterBauO."""@en ,
                                """Stellt die Anwendungsregel da, nach der die Anforderungen \"gemäß\" sind.

Beispiel:
Die Trennwand muss mindestens \"feuerhemmend\" ausgeführt werden, gemäß §19 (3) MusterBauO."""@de ;
                   rdfs:label "Anwendungsregel"@de ,
                              "RuleOfApplication"@en ;
                   <http://www.w3.org/2004/02/skos/core#altLabel> "LegalBasis"@en ,
                                                                  "RechtlicheGrundlage"@de .


###  https://purl.org/fisa#SafetyStairSpace
:SafetyStairSpace rdf:type owl:Class ;
                  rdfs:subClassOf <https://w3id.org/bot#Space> ,
                                  [ rdf:type owl:Restriction ;
                                    owl:onProperty :isPartOf ;
                                    owl:someValuesFrom :RescueConcept
                                  ] ;
                  rdfs:comment "A safety stair space is a special type of necessary stair space: the necessary staircase running in it represents both the first and the second escape route in one."@en ,
                               "Ein Sicherheitstreppenraum ist eine spezielle Art des notwendigen Treppenraums: Die in ihm verlaufende notwendige Treppe stellt sowohl den ersten als auch den zweiten Rettungsweg in einem dar."@de ;
                  rdfs:label "SafetyStairSpace"@en ,
                             "Sicherheitstreppenraum"@de .


###  https://purl.org/fisa#Sales
:Sales rdf:type owl:Class ;
       rdfs:subClassOf :UtilizationPurpose .


###  https://purl.org/fisa#SalesPremises
:SalesPremises rdf:type owl:Class ;
               rdfs:subClassOf :SpecialPurposeCondition ;
               rdfs:comment """§2 (4) 4. MBO

'Retail establishments/sales premises, where the gross floor area of sales spaces and store streets exceeds 800 square meters'"""@en ,
                            """§2 (4) 4. MBO

'Verkaufsstätten, deren Verkaufsräume und Ladenstraßen eine Grundfläche von insgesamt mehr als 800 m2 haben,'"""@de ;
               rdfs:isDefinedBy :MVKVO ;
               rdfs:label "SalesPremises"@en ,
                          "Verkaufsstätte"@de ;
               :gemäß "§2 (4) 4. MBO" .


###  https://purl.org/fisa#SalesRoom
:SalesRoom rdf:type owl:Class ;
           rdfs:subClassOf :SpaceUsage .


###  https://purl.org/fisa#SceneArea
:SceneArea rdf:type owl:Class ;
           rdfs:subClassOf :UtilizationPurpose .


###  https://purl.org/fisa#School
:School rdf:type owl:Class ;
        rdfs:subClassOf :SpecialPurposeCondition ;
        rdfs:comment "Einrichtungen, die dem Lernen dienen - hier Schulen."@de ,
                     "Establishments dedicated to learning - here schools."@en ;
        rdfs:isDefinedBy :MSchulbauR ;
        rdfs:label "School"@en ,
                   "Schule"@de ;
        :gemäß "§2 (4) 13. MBO" .


###  https://purl.org/fisa#SecondEscapeRoute
:SecondEscapeRoute rdf:type owl:Class ;
                   rdfs:subClassOf :EscapeRoute ;
                   rdfs:comment "Der zweite Rettungsweg kann entweder baulich sein = Fluchtweg (eine weitere ständig vorhandene feste bauliche Einrichtung) und der Selbstrettung dienen oder er wird im Gefahrenfall durch Rettungsgeräte der Feuerwehr hergestellt."@de ,
                                "The second escape route can either be structural = escape route (another permanently existing fixed structural facility) and serve for self-rescue, or it can be created in case of danger by rescue equipment of the fire department."@en ;
                   rdfs:label "SecondEscapeRoute"@en ,
                              "ZweiterRettungsweg"@de .


###  https://purl.org/fisa#SecurityGate
:SecurityGate rdf:type owl:Class ;
              rdfs:subClassOf <https://w3id.org/bot#Space> ;
              rdfs:comment "Security gate are devices or equipment in buildings that are used to control access to certain sensitive areas and to ensure security-related aspects such as access authorizations, identification and security checks."@en ,
                           "Sicherheitsschleusen sind Vorrichtungen oder Einrichtungen in Gebäuden, die dazu dienen, den Zugang zu bestimmten sensiblen Bereichen zu kontrollieren und sicherheitsrelevante Aspekte wie Zugangsberechtigungen, Identifikation und Sicherheitsüberprüfungen zu gewährleisten."@de ;
              rdfs:label "SecurityGate"@en ,
                         "Sicherheitsschleuse"@de ;
              <http://www.w3.org/2004/02/skos/core#altLabel> "SafetyGate"@en .


###  https://purl.org/fisa#ShelfWarehouse
:ShelfWarehouse rdf:type owl:Class ;
                rdfs:subClassOf :SpecialPurposeCondition ;
                rdfs:comment """§2 (4) 18. MBO

'Regallager mit einer Oberkante Lagerguthöhe von mehr als 7,50 m,'"""@de ,
                             """§2 (4) 18. MBO

'Warehouses with shelf heights exceeding 7.50 meters'"""@en ;
                rdfs:label "Regallager"@de ,
                           "ShelfWarehouse"@en ;
                :gemäß "§2 (4) 18. MBO" .


###  https://purl.org/fisa#SiteDevelopmentMeasure
:SiteDevelopmentMeasure rdf:type owl:Class ;
                        rdfs:subClassOf :FireSafety ;
                        rdfs:comment "Der Begriff steht für sämtliche baulichen Maßnahmen und gesetzliche Regelungen für die ordnungsgemäße Nutzung des späteren Gebäudes."@de ,
                                     "The term stands for all structural measures and legal regulations for the proper use of the subsequent building."@en ;
                        rdfs:label "Erschließungsmaßnahme"@de ,
                                   "SiteDevelopmentMeasure"@en .


###  https://purl.org/fisa#Slab
:Slab rdf:type owl:Class ;
      rdfs:subClassOf <https://w3id.org/bot#Element> ;
      rdfs:comment "Die horizontale Oberfläche oder das Bauelement, das die oberste Begrenzung eines Raums bildet."@de ,
                   "The horizontal surface or structural element that forms the uppermost boundary of a space."@en ;
      rdfs:label "Decke"@de ,
                 "Slab"@en .


###  https://purl.org/fisa#SmokeCompartment
:SmokeCompartment rdf:type owl:Class ;
                  rdfs:subClassOf <https://w3id.org/bot#Zone> ;
                  rdfs:comment "A smoke compartment is a structurally delimited area that prevents the spread of smoke for a certain period of time. Escape and rescue routes should be kept free of smoke and accessible for a certain period of time so that the rescue of persons is possible for a sufficiently long time."@en ,
                               "Ein Rauchabschnitt ist ein baulich abgegrenzter Bereich, der die Ausbreitung von Rauch für einen bestimmten Zeitraum verhindert. Flucht- und Rettungswege sollen für eine gewisse Zeit rauchfrei und begehbar gehalten werden, damit die Rettung von Personen ausreichend lange möglich ist."@de ;
                  rdfs:label "Rauchabschnitt"@de ,
                             "SmokeCompartment"@en .


###  https://purl.org/fisa#Sonderbaurichtlinie
:Sonderbaurichtlinie rdf:type owl:Class ;
                     rdfs:subClassOf :Sonderbauvorschrift ;
                     owl:disjointWith :Sonderbauverordnung ;
                     rdfs:comment "Dieses Konzept vereinigt die Sonderbauten, für die es eine Richtlinie gibt."@de ,
                                  "This concept unites the special purpose constructions for which there is a guideline."@en ;
                     rdfs:label "Sonderbaurichtlinie"@de ,
                                "SpecialPurposeGuideline"@en .


###  https://purl.org/fisa#Sonderbauverordnung
:Sonderbauverordnung rdf:type owl:Class ;
                     rdfs:subClassOf :Sonderbauvorschrift ;
                     rdfs:comment "Dieses Konzept vereinigt die Sonderbauten, für die es eine Verordnung gibt."@de ,
                                  "This concept unites the special purpose constructions for which there is a regulation."@en ;
                     rdfs:label "Sonderbauverordnung"@de ,
                                "SpecialPurposeRegulation"@en .


###  https://purl.org/fisa#Sonderbauvorschrift
:Sonderbauvorschrift rdf:type owl:Class ;
                     rdfs:subClassOf :Mustervorschrift ;
                     rdfs:comment "An Sonderbauten können besondere Anforderungen gestellt oder Erleichterungen gestattet werden, wenn dadurch die allgemeinen Schutzziele gleichwertig erreicht werden. Für sogenannte geregelte Sonderbauten (Sonderbauten, für die Sonderbauverordnungen vorliegen) sind diese besonderen Anforderungen oder Erleichterungen in entsprechenden Verordnungen zusammengefasst."@de ,
                                  """Special purpose constructions may be subject to special requirements or relief may be permitted if the general safety goal objectives are achieved in an equivalent manner.
For so-called regulated special purpose constructions (special purpose constructions for which special purpose regulations exist), these special requirements or relief measures are summarized in corresponding regulations."""@en ;
                     rdfs:label "Sonderbauvorschrift"@de ,
                                "SpecialPurposePrescription"@en .


###  https://purl.org/fisa#SpaceClosure
:SpaceClosure rdf:type owl:Class ;
              rdfs:subClassOf :StructuralFireSafetyMeasures ;
              rdfs:comment "Ability of a space-enclosing component under fire exposure from one side to prevent the passage of flames and hot gases or the appearance of flames on the non-exposed side for a defined period of time and under standardized fire test conditions. (Construction lexicon)"@en ,
                           "Fähigkeit eines raumabschließenden Bauteils unter Feuerbeanspruchung von einer Seite, den Durchgang von Flammen und heißen Gasen oder die Erscheinung von Flammen auf der nicht beanspruchten Seite während eines definierten Zeitraums und unter normierten Brandversuchsbedingungen zu verhindern. [Baulexikon]"@de ;
              rdfs:label "Raumabschluss"@de ,
                         "SpaceClosure"@en .


###  https://purl.org/fisa#SpaceOfIncreasedFireRisk
:SpaceOfIncreasedFireRisk rdf:type owl:Class ;
                          rdfs:subClassOf <https://w3id.org/bot#Space> ;
                          rdfs:comment "An increased fire hazard exists in particular if oxidizing, highly flammable or extremely flammable substances are stored, processed or handled in not insignificant quantities according to the hazard characteristics as defined in the Ordinance on Hazardous Substances (GefStoffV)."@en ,
                                       "Eine erhöhte Brandgefahr liegt insbesondere vor, wenn brandfördernde, leichtentzündliche oder hochentzündliche Stoffe entsprechend den Gefährlichkeitsmerkmalen nach der Gefahrstoffverordnung (GefStoffV) in nicht geringen Mengen gelagert, be- oder verarbeitet werden."@de ;
                          rdfs:label "RaumErhöhterBrandgefahr"@de ,
                                     "SpaceOfIncreasedFireRisk"@en ;
                          <http://www.w3.org/2004/02/skos/core#altLabel> "High-Hazard Occupancies"@en .


###  https://purl.org/fisa#SpaceUsage
:SpaceUsage rdf:type owl:Class ;
            rdfs:subClassOf :Usage ;
            rdfs:comment "Beschreibt sowohl Raumnutzungen aus Regularien als auch weitergehende Nutzungsmöglichkeiten, in Form von alltäglichen Raumnutzungen, wie z.B. Küche."@de ,
                         "Describes both uses of space from regularities and more extensive uses, in the form of everyday uses of space, such as a kitchen."@en ;
            rdfs:label "RaumNutzung"@de ,
                       "SpaceUsage"@en .


###  https://purl.org/fisa#SpecialPurposeCondition
:SpecialPurposeCondition rdf:type owl:Class ;
                         rdfs:subClassOf :Usage ;
                         rdfs:comment "Special purpose conditions applicable to buildings classified as \"special purpose construction\" because of their use, size, special hazards, or other factors."@en ,
                                      "Spezielle bauliche Anforderungen, die für Gebäude gelten, die aufgrund ihrer Nutzung, Größe, besonderen Gefährdung oder anderen Faktoren als \"Sonderbauten\" eingestuft werden."@de ;
                         rdfs:isDefinedBy :MBO ;
                         rdfs:label "Sonderbautatbestand"@de ,
                                    "SpecialPurposeCondition"@en .


###  https://purl.org/fisa#SpecialPurposeConstruction
:SpecialPurposeConstruction rdf:type owl:Class ;
                            rdfs:subClassOf <https://w3id.org/bot#Building> ;
                            owl:disjointWith :StandardConstruction ;
                            <http://purl.org/dc/terms/description> "Sonderbauten sind Anlagen und Räume besonderer Art oder Nutzung,[...]"@de ;
                            rdfs:comment "Special buildings are facilities and spaces of a special type or use,[...]."@en ;
                            rdfs:isDefinedBy :MBO ;
                            rdfs:label "Sonderbau"@de ,
                                       "SpecialPurposeConstruction"@en ;
                            :gemäß "§2 (4) MBO"@de .


###  https://purl.org/fisa#SpectatorFacility
:SpectatorFacility rdf:type owl:Class ;
                   rdfs:subClassOf :UtilizationPurpose .


###  https://purl.org/fisa#Sport
:Sport rdf:type owl:Class ;
       rdfs:subClassOf :UtilizationPurpose .


###  https://purl.org/fisa#StairSpace
:StairSpace rdf:type owl:Class ;
            rdfs:subClassOf :SpaceUsage .


###  https://purl.org/fisa#StairSpaceExtension
:StairSpaceExtension rdf:type owl:Class ;
                     rdfs:subClassOf <https://w3id.org/bot#Space> ,
                                     [ rdf:type owl:Restriction ;
                                       owl:onProperty :isPartOf ;
                                       owl:someValuesFrom :RescueConcept
                                     ] ;
                     rdfs:comment "Stair space extensions are spaces that connect stairwells with exits to the outdoors."@en ,
                                  "Treppenraumerweiterungen sind Räume, die Treppenräume mit Ausgängen ins Freie verbinden."@de ;
                     rdfs:label "StairSpaceExtension"@en ,
                                "Treppenraumerweiterung"@de .


###  https://purl.org/fisa#Stairs
:Stairs rdf:type owl:Class ;
        rdfs:subClassOf <https://w3id.org/bot#Element> ;
        owl:disjointWith :StairsSupportingStructure ;
        rdfs:comment "An immovable structural member permanently attached to the structure for climbing in steps, which are vertical paths in structural systems."@en ,
                     "Ein fest mit dem Bauwerk verbundenes, unbewegbares Bauteil zum stufenweisen Steigen, welche vertikale Wege in baulichen Anlagen darstellen."@de ;
        rdfs:label "Stairs"@en ,
                   "Treppe"@de .


###  https://purl.org/fisa#StairsParts
:StairsParts rdf:type owl:Class ;
             rdfs:subClassOf <https://w3id.org/bot#Element> ;
             rdfs:comment "Beschreibt die Teile einer Treppe, an die Brandschutzanforderungen gestellt werden können, z.B. an den Treppenlauf."@de ,
                          "Describes the parts of a staircase to which fire safety requirements may be applied, e.g. the flight of stairs."@en ;
             rdfs:label "StairsParts"@en ,
                        "Treppenteile"@de .


###  https://purl.org/fisa#StairsSupportingStructure
:StairsSupportingStructure rdf:type owl:Class ;
                           rdfs:subClassOf :Structure ;
                           rdfs:comment "Beschreibt die tragenden Komponenten, das Tragwerk, der Treppe."@de ,
                                        "Describes the load-bearing components, the supporting structure, of stairs."@en ;
                           rdfs:label "StairsSupportingStructure"@en ,
                                      "Treppentragwerk"@de .


###  https://purl.org/fisa#StandardConstruction
:StandardConstruction rdf:type owl:Class ;
                      rdfs:subClassOf <https://w3id.org/bot#Building> ;
                      rdfs:comment "Buildings are designated as regular or standard construction when there is no feature or condition that leads to classification as special purpose construction."@en ,
                                   "Gebäude werden als Regel- oder Standardbau bezeichnet, wenn keine Eigenschaft vorhanden ist, die zur Einstufung als Sonderbau führt."@de ;
                      rdfs:label "StandardConstruction"@en ,
                                 "Standardbau"@de .


###  https://purl.org/fisa#StandardConstructionType
:StandardConstructionType rdf:type owl:Class ;
                          rdfs:subClassOf :Usage ;
                          rdfs:comment "Der Begriff \"Standardbau\" bezieht sich auf Gebäude oder Konstruktionen, die nach vorgegebenen Normen, Richtlinien und Bauvorschriften errichtet werden. Es sind Gebäude, die keinen Sonderbautatbestand erfüllen."@de ,
                                       "The term \"standard construction\" refers to buildings that are constructed according to specified standards, guidelines and building regulations. They are buildings that do not meet any special purpose condition of construction."@en ;
                          rdfs:label "StandardConstructionType"@en ,
                                     "StandardbauArt"@de .


###  https://purl.org/fisa#Storage
:Storage rdf:type owl:Class ;
         rdfs:subClassOf :UtilizationPurpose .


###  https://purl.org/fisa#StoreStreet
:StoreStreet rdf:type owl:Class ;
             rdfs:subClassOf :SpaceUsage .


###  https://purl.org/fisa#StoreySlab
:StoreySlab rdf:type owl:Class ;
            owl:equivalentClass [ rdf:type owl:Restriction ;
                                  owl:onProperty :isStoreySlab ;
                                  owl:hasValue "true"^^xsd:boolean
                                ] ;
            rdfs:subClassOf :Slab ;
            rdfs:comment "Die horizontale Fläche oder das Bauelement, das zwischen den einzelnen Stockwerken oder Geschossen eines Gebäudes liegt."@de ,
                         "The horizontal surface or structural element located between the floors or stories of a building."@en ;
            rdfs:label "Geschossdecke"@de ,
                       "StoreySlab"@en .


###  https://purl.org/fisa#StructuralFacility
:StructuralFacility rdf:type owl:Class ;
                    rdfs:subClassOf <https://w3id.org/bot#Zone> ,
                                    [ rdf:type owl:Restriction ;
                                      owl:onProperty :hasAssessmentBasis ;
                                      owl:someValuesFrom :AssessmentBasis
                                    ] ,
                                    [ rdf:type owl:Restriction ;
                                      owl:onProperty :hasProtectiveGoal ;
                                      owl:someValuesFrom :ProtectiveGoal
                                    ] ,
                                    [ rdf:type owl:Restriction ;
                                      owl:onProperty :needs ;
                                      owl:someValuesFrom :ExternalDevelopment
                                    ] ,
                                    [ rdf:type owl:Restriction ;
                                      owl:onProperty :needs ;
                                      owl:someValuesFrom :RescueConcept
                                    ] ,
                                    [ rdf:type owl:Restriction ;
                                      owl:onProperty :needs ;
                                      owl:someValuesFrom :TechnicalStructuralCertificate
                                    ] ;
                    <http://purl.org/dc/terms/description> """Bauliche Anlagen sind mit dem Erdboden verbundene, aus Bauprodukten hergestellte Anlagen; eine Verbindung mit dem Boden besteht auch dann, wenn die Anlage durch eigene Schwere auf dem Boden ruht oder auf ortsfesten Bahnen begrenzt beweglich ist oder wenn die Anlage nach ihrem Verwendungszweck dazu bestimmt ist, überwiegend ortsfest benutzt zu werden. 2Bauliche Anlagen sind auch
1. Aufschüttungen und Abgrabungen,
2. Lagerplätze, Abstellplätze und Ausstellungsplätze,
3. Sport- und Spielflächen,
4. Campingplätze, Wochenendplätze und Zeltplätze,
5. Freizeit- und Vergnügungsparks,
6. Stellplätze für Kraftfahrzeuge und Abstellplätze für Fahrräder,
7. Gerüste,
8. Hilfseinrichtungen zur statischen Sicherung von Bauzuständen.
Anlagen sind bauliche Anlagen und sonstige Anlagen und Einrichtungen im Sinne des § 1 Abs. 1 Satz 2."""@de ;
                    rdfs:comment """Structural facilities are connected to the ground and made of construction components; a connection to the ground also exists if the structural facility rests on the ground by its own weight or is movable to a limited extent on fixed tracks or if the structural facility is intended by its purpose to be used predominantly in a fixed location.
2Building structures are also
1. fillings and excavations,
2. storage areas, parking areas and exhibition areas,
3. sports and play areas,
4. camping sites, weekend sites and tent sites,
5. recreational and amusement parks,
6. parking places for motor vehicles and parking places for bicycles,
7. scaffolds,
8. auxiliary facilities for static securing of construction conditions.
Installations are structural installations and other installations and facilities within the meaning of § 1 Para. 1 Sentence 2."""@en ;
                    rdfs:isDefinedBy :MBO ;
                    rdfs:label "BaulicheAnlage"@de ,
                               "StructuralFacility"@en ;
                    :gemäß "§2 (1) MBO"@de .


###  https://purl.org/fisa#StructuralFireSafety
:StructuralFireSafety rdf:type owl:Class ;
                      rdfs:subClassOf :FireSafety ;
                      rdfs:comment """All fire safety measures taken in connection with the construction or alteration of building facilities, e.g.:
- the formation of fire compartments, e.g. by fire walls,
- the dimensioning or standard-compliant construction of load-bearing and room-enclosing structures, e.g. to protect areas with a high fire risk.

Essential criteria are
- the fire behavior of building materials
- the fire resistance of building components,
- the planning and creation of sufficient escape and rescue routes for people and animals."""@en ,
                                   """Alle Maßnahmen des Brandschutzes, die im Zusammenhang mit der Errichtung oder der Änderung von baulichen Anlagen getroffen werden, z.B.:
- die Bildung von Brandabschnitten z.B. durch Brandwände,
- die Bemessung oder normgerechte Erstellung von tragenden und raumabschließenden Konstruktionen, z.B. zum Schutz von Bereichen mit hoher Brandgefahr.

Wesentliche Kriterien sind dabei:
- das Brandverhalten von Baustoffen,
- der Feuerwiderstand der Bauteile,
- die Planung und Erstellung ausreichender Flucht- und Rettungswege für Menschen und Tiere."""@de ;
                      rdfs:label "BaulicherBrandschutz"@de ,
                                 "StructuralFireSafety"@en .


###  https://purl.org/fisa#StructuralFireSafetyMeasures
:StructuralFireSafetyMeasures rdf:type owl:Class ;
                              rdfs:subClassOf :StructuralFireSafety ;
                              rdfs:comment """Unites the essential structural fire safety criteria such as
- the fire behavior of building materials
- the fire resistance of building components,
- the space-enclosing option for components."""@en ,
                                           """Vereint die wesentlichen Kriterien des baulichen Brandschutzes wie z.B.
- das Brandverhalten von Baumaterialien
- den Feuerwiderstand von Bauteilen,
- Raumabschluss von Bauteilen."""@de ;
                              rdfs:label "BaulicheBrandschutzmaßnahmen"@de ,
                                         "StructuralFireSafetyMeasures"@en .


###  https://purl.org/fisa#Structure
:Structure rdf:type owl:Class ;
           rdfs:subClassOf :Component ;
           rdfs:comment """Dieses Konzept dient dazu, die Anforderungen die tragenden Teile jedes Bauteils separat noch einmal betrachten zu können. Das ist vor allem Hilfreich, wenn am Ende bei Ausführungen wie dem Layerprinzip der Außenwand in §28 (2) die Wand eingeteilt wird.

Da Komponenten ja mit Komponenten verbunden werden und das Objektattribut bot:hatBauteil und bot:hatUnterbauteil nicht eingegrenzt wurden durch die originale BOT-Ontologie, ist ein Verweis und die Aufteilung der Layer sogar innerhalb der gesamten fisa:Komponente möglich, und nicht nur im Konzept bot:Bauteil."""@de ,
                        """This concept serves to be able to consider the requirements the load-bearing parts of each component separately again. This is especially helpful if at the end the wall is divided in designs like the layer principle of the exterior wall in §28 (2).

Since components are connected to components and the object attribute bot:hasElement and bot:hasSubComponent are not delimited by the original BOT ontology, a reference and the division of the layers is even possible within the whole fisa:Component and not only in the concept bot:BuildingElement.""" ;
           rdfs:label "Structure"@en ,
                      "Tragwerk"@de ;
           <http://www.w3.org/2004/02/skos/core#altLabel> "LoadbearingSubstructure"@en ,
                                                          "TragendeUnterkonstruktion"@de .


###  https://purl.org/fisa#SurfaceType
:SurfaceType rdf:type owl:Class ;
             rdfs:subClassOf :Component ;
             rdfs:comment "Die äußere Schicht oder den sichtbaren Bereich von Komponenten."@de ,
                          "The outer layer or visible area of components.e"@en ;
             rdfs:label "Oberfläche"@de ,
                        "SurfaceType"@en .


###  https://purl.org/fisa#Surrounding
:Surrounding rdf:type owl:Class ;
             rdfs:subClassOf <https://w3id.org/bot#Zone> ;
             rdfs:comment "An environment describes a delimited zone that influences an adjacent or remote zone."@en ,
                          "Eine Umgebung beschreibt eine abgegrenzte Zone, die Einfluss auf eine andere angrenzende oder entfernte Zone nimmt."@de ;
             rdfs:label "Surrounding"@en ,
                        "Umgebung"@de .


###  https://purl.org/fisa#SystemFlooring
:SystemFlooring rdf:type owl:Class ;
                rdfs:subClassOf <https://w3id.org/bot#Element> ;
                rdfs:comment "A special design or structural floor assembly used to create levels in a building on which various activities can be performed."@en ,
                             "Eine spezielle Konstruktion oder ein struktureller Bodenaufbau, die/der verwendet wird, um Ebenen in einem Gebäude zu schaffen, auf denen verschiedene Aktivitäten durchgeführt werden können."@de ;
                rdfs:label "SystemFlooring"@en ,
                           "Systemboden"@de .


###  https://purl.org/fisa#TavernAndRestaurant
:TavernAndRestaurant rdf:type owl:Class ;
                     rdfs:subClassOf :SpecialPurposeCondition ;
                     rdfs:comment """§2 (4) 8. MBO

'Drinking and dining establishments with more than 40 indoor guest seats or more than 1,000 outdoor guest seats,'[...]"""@en ,
                                  """§2 (4) 8. MBO

'Schank- und Speisegaststätten mit mehr als 40 Gastplätzen in Gebäuden oder mehr als 1000 Gastplätzen im Freien,'[...]"""@de ;
                     rdfs:label "SchankUndSpeisegaststätte"@de ,
                                "TavernAndRestaurant"@en ;
                     :gemäß "§2 (4) 8. MBO" .


###  https://purl.org/fisa#TechnicalComponent
:TechnicalComponent rdf:type owl:Class ;
                    rdfs:subClassOf :Component ;
                    rdfs:comment "Combines all technical components relevant to fire safety."@en ,
                                 "Vereint alle technischen, brandschutzrelevanten Komponenten."@de ;
                    rdfs:label "TechnicalComponent"@en ,
                               "TechnischeKomponente"@de .


###  https://purl.org/fisa#TechnicalFireSafety
:TechnicalFireSafety rdf:type owl:Class ;
                     rdfs:subClassOf :FireSafety ;
                     rdfs:comment """Der anlagentechnische Brandschutz ist Teil des vorbeugenden Brandschutzes. Zu ihm zählen alle technischen Systeme, die u.a.
- der Brandverhinderung dienen,
- Brände erkennen,
- Löschfunktionen haben (Sprinkler, Feuerlöscher, ...)
- die Feuerwehr unterstützen, wie z.B. Feuerwehraufzüge."""@de ,
                                  """Technical fire safety is part of preventive fire safety. It includes all technical systems which, among other things:
- serve to prevent fires,
- detect fires,
- have extinguishing functions (sprinklers, fire extinguishers, ...)
- support the fire department, e.g. fire department elevators."""@en ;
                     rdfs:label "AnlagentechnischeBrandschutz"@de ,
                                "TechnicalFireSafety"@en .


###  https://purl.org/fisa#TechnicalStructuralCertificate
:TechnicalStructuralCertificate rdf:type owl:Class ;
                                rdfs:subClassOf [ rdf:type owl:Restriction ;
                                                  owl:onProperty :isBasedOn ;
                                                  owl:someValuesFrom :AssessmentBasis
                                                ] ;
                                rdfs:comment "Die schriftlichen oder rechnerischen Belege, die von Fachleuten wie Ingenieuren, Architekten oder anderen qualifizierten Personen erstellt werden, um die Einhaltung der relevanten bautechnischen Anforderungen und Normen für ein Bauprojekt zu bestätigen. Diese Nachweise dienen dazu, die Sicherheit, Stabilität, Tragfähigkeit, Brandschutz, Wärmedämmung und andere wichtige Aspekte eines Bauwerks zu gewährleisten."@de ,
                                             "The written or calculated evidence prepared by professionals such as engineers, architects, or other qualified persons to confirm compliance with relevant structural engineering requirements and standards for a construction project. These verifications are used to ensure the safety, stability, load-bearing capacity, fire safety, thermal insulation, and other important aspects of a structure."@en ;
                                rdfs:label "BautechnischerNachweis"@de ,
                                           "TechnicalStructuralCertificate"@en .


###  https://purl.org/fisa#Technology
:Technology rdf:type owl:Class ;
            rdfs:subClassOf :UtilizationPurpose .


###  https://purl.org/fisa#ThemePark
:ThemePark rdf:type owl:Class ;
           rdfs:subClassOf :SpecialPurposeCondition ;
           rdfs:comment "Ort, der der Unterhaltung und der Freizeitgestaltung dient."@de ,
                        "Venue designed for entertainment and leisure."@en ;
           rdfs:label "Freizeitpark"@de ,
                      "ThemePark"@en ;
           :gemäß "§2 (4) 16. MBO" .


###  https://purl.org/fisa#Transom
:Transom rdf:type owl:Class ;
         rdfs:subClassOf :AssemblyProduct ;
         rdfs:comment "Horizontal structural element or partition used to prevent the spread of fire, smoke and hot gases within a building or between different areas."@en ,
                      "Horizontales Bauelement oder eine Abschottung, die dazu dient, die Ausbreitung von Feuer, Rauch und heißen Gasen innerhalb eines Gebäudes oder zwischen verschiedenen Bereichen zu verhindern."@de ;
         rdfs:label "Riegel"@de ,
                    "Transom"@en .


###  https://purl.org/fisa#University
:University rdf:type owl:Class ;
            rdfs:subClassOf :SpecialPurposeCondition ;
            rdfs:comment "Einrichtungen, die dem Lernen dienen - hier Universitäten."@de ,
                         "Establishments dedicated to learning - here universities."@en ;
            rdfs:label "Hochschule"@de ,
                       "University"@en ;
            :gemäß "§2 (4) 13. MBO" .


###  https://purl.org/fisa#UnregulatedSpecialPurposeConstruction
:UnregulatedSpecialPurposeConstruction rdf:type owl:Class ;
                                       rdfs:subClassOf :SpecialPurposeConstruction ;
                                       rdfs:comment "Ungeregelte Sonderbauten sind Sonderbauten, für die es keine Sonderbau-Vorschriften gibt. Im Gegensatz zu geregelten Sonderbauten gibt es für ungeregelte Sonderbauten keine einheitlichen Vorschriften."@de ,
                                                    "Unregulated special purpose constructions are special purpose constructions for which there are no special purpose construction regulations. In contrast to regulated special purpose constructions, there are no uniform regulations for unregulated special purpose construction."@en ;
                                       rdfs:label "UngeregelterSonderbau"@de ,
                                                  "UnregulatedSpecialPurposeConstruction"@en .


###  https://purl.org/fisa#UpperStorey
:UpperStorey rdf:type owl:Class ;
             rdfs:subClassOf :AboveGroundStorey ;
             rdfs:label "Obergeschoss"@de ,
                        "UpperStorey"@en .


###  https://purl.org/fisa#Usage
:Usage rdf:type owl:Class ;
       rdfs:comment "Beschreibt die Nutzung einer baulichen Anlage oder Raumes, oder Teile von baulichen Anlagen und ihren Räumen sowie Nutzungen, die Nutzungseinheiten auferlegen."@de ,
                    "Describes the use of a structural facility or space, or parts of structural facilities and their spaces, as well as uses that impose utilization units."@en ;
       rdfs:label "Nutzung"@de ,
                  "Usage"@en .


###  https://purl.org/fisa#UtilizationPurpose
:UtilizationPurpose rdf:type owl:Class ;
                    rdfs:subClassOf :Usage ;
                    rdfs:label "Nutzungszweck"@de ,
                               "UtilizationPurpose"@en .


###  https://purl.org/fisa#UtilizationUnit
:UtilizationUnit rdf:type owl:Class ;
                 rdfs:subClassOf <https://w3id.org/bot#Zone> ;
                 rdfs:comment "A utilization unit is a self-contained series of (residential) spaces available for use by one person or a group of persons."@en ,
                              "Als Nutzungseinheit gilt eine in sich abgeschlossene Folge von (Aufenthalts-)Räumen, die einer Person oder einem gemeinschaftlichen Personenkreis zur Benutzung zur Verfügung stehen."@de ;
                 rdfs:label "Nutzungseinheit"@de ,
                            "UtilizationUnit"@en .


###  https://purl.org/fisa#Wall
:Wall rdf:type owl:Class ;
      rdfs:subClassOf <https://w3id.org/bot#Element> ;
      owl:disjointWith :WallStructure ;
      rdfs:comment "Is a vertical flat component that has a space-forming or space-enclosing function."@en ,
                   "Ist ein vertikales flächiges Bauteil, das eine raumbildende oder raumabschließende Funktion hat."@de ;
      rdfs:label "Wall"@en ,
                 "Wand"@de .


###  https://purl.org/fisa#WallOfANecessaryCorridor
:WallOfANecessaryCorridor rdf:type owl:Class ;
                          rdfs:subClassOf :Wall ;
                          rdfs:comment """Die notwendigen Flure bilden die Verbindung zum sicheren Ort im Brandfall und sind erforderlich, wenn ein bauaufsichtlicher Rettungsweg aus einem Raum oder einer Nutzungseinheit nicht direkt ins Freie oder in einen Treppenraum führt.
Die Wände dieser notwendigen Flure haben Anforderungen."""@de ,
                                       """The necessary corridors form the connection to the safe place in case of fire and are required if a building authority escape route from a room or a utilization unit does not lead directly to the outside or to a stairwell.
The walls of these necessary corridors have requirements."""@en ;
                          rdfs:label "WallOfANecessaryCorridor"@en ,
                                     "WandEinesNotwendigenFlures"@de .


###  https://purl.org/fisa#WallOfANecessaryStaircase
:WallOfANecessaryStaircase rdf:type owl:Class ;
                           rdfs:subClassOf :Wall ;
                           rdfs:comment """Necessary staircases are part of the system of vertical escape and rescue routes.
The walls of these necessary staircases have requirements."""@en ,
                                        """Notwendige Treppenräume gehören zum System der vertikalen Flucht- und Rettungswege.
Die Wänder dieser notwendigen Treppenräume haben Anforderungen."""@de ;
                           rdfs:label "WallOfANecessaryStaircase"@en ,
                                      "WandEinesNotwendigenTreppenraums"@de .


###  https://purl.org/fisa#WallParts
:WallParts rdf:type owl:Class ;
           rdfs:subClassOf <https://w3id.org/bot#Element> ;
           rdfs:comment "Beschreibt die Teile bzw. Variationen einer Wand, an die Brandschutzanforderungen gestellt werden können, z.B. Brüstung."@de ,
                        "Describes the parts or variations of a wall that may be subject to fire safety requirements, e.g. parapet."@en ;
           rdfs:label "WallParts"@en ,
                      "Wandteile"@de .


###  https://purl.org/fisa#WallStructure
:WallStructure rdf:type owl:Class ;
               rdfs:subClassOf :Structure ;
               rdfs:comment "Beschreibt die tragenden Komponenten, das Tragwerk, der Wand."@de ,
                            "Describes the load-bearing components, the supporting structure, of a wall."@en ;
               rdfs:label "WallStructure"@en ,
                          "Wandtragwerk"@de ;
               <http://www.w3.org/2004/02/skos/core#altLabel> "LoadbearingWallSubstructure"@en ,
                                                              "TragendeWandunterkonstruktion"@de .


###  https://purl.org/fisa#WallinsteadOfFireWall
:WallinsteadOfFireWall rdf:type owl:Class ;
                       rdfs:subClassOf :FireWall ;
                       rdfs:comment "Under certain conditions, other walls are permitted instead of fire walls, provided they meet the requirements resulting from the state building regulations."@en ,
                                    "Unter bestimmten Voraussetzungen sind anstelle von Brandwänden auch andere Wände zulässig, sofern sie die Anforderungen erfüllen, die sich aus den Landesbauordnungen ergeben."@de ;
                       rdfs:label "WallinsteadOfFireWall"@en ,
                                  "WandAnstelleBrandwand"@de .


###  https://purl.org/fisa#WeekendPlace
:WeekendPlace rdf:type owl:Class ;
              rdfs:subClassOf :SpecialPurposeCondition ;
              rdfs:comment "Freiluftflächen mit Einrichtungen für Freizeitaktivitäten und Camping, oft mit Annehmlichkeiten."@de ,
                           "Outdoor areas equipped for recreational use, often featuring amenities for camping and leisure activities."@en ;
              rdfs:label "WeekendPlace"@en ,
                         "Wochenendplatz"@de ;
              :gemäß "§2 (4) 15. MBO" .


###  https://purl.org/fisa#Window
:Window rdf:type owl:Class ;
        rdfs:subClassOf :Closing ;
        rdfs:comment "Auf einen Abschluss einer Öffnung in der Wand eines Gebäudes, die normalerweise verglast ist und Licht, Luft und Sicht ermöglicht."@de ,
                     "The closing of an opening in the wall of a building, usually glazed, allowing light, air, and view."@en ;
        rdfs:label "Fenster"@de ,
                   "Window"@en .


###  https://purl.org/fisa#Work
:Work rdf:type owl:Class ;
      rdfs:subClassOf :UtilizationPurpose .


###  https://purl.org/fisa#DIN4102-12:1998-11
<https://purl.org/fisa#DIN4102-12:1998-11> rdf:type owl:Class ;
                                           rdfs:subClassOf :DIN4102 ;
                                           rdfs:label "DIN4102-12:1998-11"@de ,
                                                      "DIN4102-12:1998-11"@en .


###  https://purl.org/fisa#DIN4102-15:1990-05
<https://purl.org/fisa#DIN4102-15:1990-05> rdf:type owl:Class ;
                                           rdfs:subClassOf :DIN4102 ;
                                           rdfs:label "DIN4102-15:1990-05"@de ,
                                                      "DIN4102-15:1990-05"@en .


###  https://purl.org/fisa#DIN4102-17:2017-12
<https://purl.org/fisa#DIN4102-17:2017-12> rdf:type owl:Class ;
                                           rdfs:subClassOf :DIN4102 ;
                                           rdfs:label "DIN4102-17:2017-12"@de ,
                                                      "DIN4102-17:2017-12"@en .


###  https://purl.org/fisa#DIN4102-1:1998-05
<https://purl.org/fisa#DIN4102-1:1998-05> rdf:type owl:Class ;
                                          rdfs:subClassOf :DIN4102 ;
                                          rdfs:label "DIN4102-1:1998-05"@de ,
                                                     "DIN4102-1:1998-05"@en .


###  https://purl.org/fisa#SpecialPurposeConditionAcc§2_S4_P19
<https://purl.org/fisa#SpecialPurposeConditionAcc§2_S4_P19> rdf:type owl:Class ;
                                                            rdfs:subClassOf :SpecialPurposeCondition ;
                                                            rdfs:comment """A = Absatz
P = Punkt
S = Satz"""@de ,
                                                                         """S = Section
P = Point
Se = Sentence"""@en ,
                                                                         """§2 (4) 19. MBO

'Structures with activities involving hazardous substances, explosives, or elevated fire risks'"""@en ,
                                                                         """§2 (4) 19. MBO

'bauliche Anlagen, deren Nutzung durch Umgang oder Lagerung von Stoffen mit Explosions- oder erhöhter Brandgefahr verbunden ist,'"""@de ;
                                                            rdfs:label "SpecialPurposeConditionAcc§2_S4_P19"@en ,
                                                                       "TatbestandNach§2_A4_P19"@de ;
                                                            :gemäß "§2 (4) 19. MBO" .


###  https://purl.org/fisa#SpecialPurposeConditionAcc§2_S4_P2
<https://purl.org/fisa#SpecialPurposeConditionAcc§2_S4_P2> rdf:type owl:Class ;
                                                           owl:equivalentClass [ rdf:type owl:Restriction ;
                                                                                 owl:onProperty :hasHeight ;
                                                                                 owl:someValuesFrom [ rdf:type rdfs:Datatype ;
                                                                                                      owl:onDatatype xsd:double ;
                                                                                                      owl:withRestrictions ( [ xsd:minExclusive "30.0"^^xsd:double
                                                                                                                             ]
                                                                                                                           )
                                                                                                    ]
                                                                               ] ;
                                                           rdfs:subClassOf :SpecialPurposeCondition ;
                                                           rdfs:comment """A = Absatz
P = Punkt
S = Satz"""@de ,
                                                                        """S = Section
P = Point
Se = Sentence"""@en ,
                                                                        """§2 (4) 2. MBO

'Structures with a height exceeding 30 meters'"""@en ,
                                                                        """§2 (4) 2. MBO

'bauliche Anlagen mit einer Höhe von mehr als 30 m,'"""@de ;
                                                           rdfs:label "SpecialPurposeConditionAcc§2_S4_P2"@en ,
                                                                      "TatbestandNach§2_A4_P2"@de ;
                                                           :gemäß "§2 (4) 2. MBO" .


###  https://purl.org/fisa#SpecialPurposeConditionAcc§2_S4_P20
<https://purl.org/fisa#SpecialPurposeConditionAcc§2_S4_P20> rdf:type owl:Class ;
                                                            rdfs:subClassOf :SpecialPurposeCondition ;
                                                            rdfs:comment """A = Absatz
P = Punkt
S = Satz"""@de ,
                                                                         """S = Section
P = Point
Se = Sentence"""@en ,
                                                                         """§2 (4) 20. MBO

'Facilities and rooms not listed in numbers 1 to 19 but associated with similar hazards due to their nature or use.'"""@en ,
                                                                         """§2 (4) 20. MBO

Anlagen und Räume, die in den Nummern 1 bis 19 nicht aufgeführt und deren Art oder Nutzung mit vergleichbaren Gefahren verbunden sind."""@de ;
                                                            rdfs:label "SpecialPurposeConditionAcc§2_S4_P20"@en ,
                                                                       "TatbestandNach§2_A4_P20"@de ;
                                                            :gemäß "§2 (4) 20. MBO" .


###  https://purl.org/fisa#SpecialPurposeConditionAcc§2_S4_P3
<https://purl.org/fisa#SpecialPurposeConditionAcc§2_S4_P3> rdf:type owl:Class ;
                                                           rdfs:subClassOf :SpecialPurposeCondition ;
                                                           rdfs:comment """A = Absatz
P = Punkt
S = Satz"""@de ,
                                                                        """S = Section
P = Point
Se = Sentence"""@en ,
                                                                        """§2 (4) 3. MBO

'Buildings with a gross floor area of more than 1,600 square meters for the largest floor dimension, excluding residential buildings, garages, and rooms/buildings for bicycle parking spaces'"""@en ,
                                                                        """§2 (4) 3. MBO

'Gebäude mit mehr als 1 600 m2 Grundfläche des Geschosses mit der größten Ausdehnung, ausgenommen Wohngebäude und Garagen sowie Räume und Gebäude für Abstellplätze für Fahrräder,'"""@de ;
                                                           rdfs:label "SpecialPurposeConditionAcc§2_S4_P3"@en ,
                                                                      "TatbestandNach§2_A4_P3"@de ;
                                                           :gemäß "§2 (4) 3. MBO" .


###  https://purl.org/fisa#SpecialPurposeConditionAcc§2_S4_P5
<https://purl.org/fisa#SpecialPurposeConditionAcc§2_S4_P5> rdf:type owl:Class ;
                                                           rdfs:subClassOf :SpecialPurposeCondition ;
                                                           rdfs:comment """A = Absatz
P = Punkt
S = Satz"""@de ,
                                                                        """S = Section
P = Point
Se = Sentence"""@en ,
                                                                        """§2 (4) 5. MBO

'Buildings with spaces designated for office or administrative use, each having an individual floor area exceeding 400 square meters'"""@en ,
                                                                        """§2 (4) 5. MBO

'Gebäude mit Räumen, die einer Büro- oder Verwaltungsnutzung dienen und einzeln eine Grundfläche von mehr als 400 m2 haben,'"""@de ;
                                                           rdfs:label "SpecialPurposeConditionAcc§2_S4_P5"@en ,
                                                                      "TatbestandNach§2_A4_P5"@de ;
                                                           :gemäß "§2 (4) 5. MBO" .


###  https://purl.org/fisa#SpecialPurposeConditionAcc§2_S4_P6
<https://purl.org/fisa#SpecialPurposeConditionAcc§2_S4_P6> rdf:type owl:Class ;
                                                           rdfs:subClassOf :SpecialPurposeCondition ;
                                                           rdfs:comment """A = Absatz
P = Punkt
S = Satz"""@de ,
                                                                        """S = Section
P = Point
Se = Sentence"""@en ,
                                                                        """§2 (4) 6. MBO

'Buildings with rooms designated for individual use by more than 100 persons'"""@en ,
                                                                        """§2 (4) 6. MBO

'Gebäude mit Räumen, die einzeln für die Nutzung durch mehr als 100 Personen bestimmt sind,'"""@de ;
                                                           rdfs:label "SpecialPurposeConditionAcc§2_S4_P6"@en ,
                                                                      "TatbestandNach§2_A4_P6"@de ;
                                                           :gemäß "§2 (4) 6. MBO" .


###  https://w3id.org/bot#Building
<https://w3id.org/bot#Building> rdf:type owl:Class ;
                                rdfs:subClassOf :StructuralFacility ,
                                                [ rdf:type owl:Restriction ;
                                                  owl:onProperty :hasBuildingClass ;
                                                  owl:someValuesFrom :BuildingClass
                                                ] ;
                                <http://purl.org/dc/terms/description> "Gebäude sind selbstständig benutzbare, überdeckte bauliche Anlagen, die von Menschen betreten werden können und geeignet oder bestimmt sind, dem Schutz von Menschen, Tieren oder Sachen zu dienen."@de ;
                                rdfs:comment "An independent unit of the built environment with a characteristic spatial structure, intended to serve at least one function or user activity [ISO 12006-2:2013]. A bot:Building is a part of the physical world or a virtual world that is inherently both located in this world and having a 3D spatial extent, is contained in a building site, and can contain one or more storeys that are vertically connected."@en ,
                                             "Eine eigenständige Einheit der bebauten Umgebung mit einer charakteristischen räumlichen Struktur. Es besteht die Absicht das es eine Funktion oder Nutzung erlaubt [ISO 12006-2:2013]. Ein bot:Building ist Teil der realen und virtuellen Welt und hat eine räumliche Ausdehnung. Es ist enthalten in einem Grundstück und kann ein oder mehrere Stockwerke enthalten, die vertical miteinander verbunden sind."@de ;
                                rdfs:isDefinedBy <http://www.systemsEngineering.org/isabellefitkau/fisa.owl#MBO> ;
                                rdfs:label "Building"@en ,
                                           "Gebäude"@de ;
                                :gemäß "§2 (2) MBOde"@de .


###  https://w3id.org/bot#Element
<https://w3id.org/bot#Element> rdf:type owl:Class ;
                               rdfs:subClassOf :Component ,
                                               [ rdf:type owl:Restriction ;
                                                 owl:onProperty :hasComponentType ;
                                                 owl:qualifiedCardinality "1"^^xsd:nonNegativeInteger ;
                                                 owl:onClass :ComponentType
                                               ] ;
                               rdfs:label "Bauteil"@de ,
                                          "BuildingElement"@en ;
                               rdfs:seeAlso "Bauteil (Bauwesen)" .


###  https://w3id.org/bot#Interface
<https://w3id.org/bot#Interface> rdf:type owl:Class ;
                                 rdfs:comment """A generic concept to qualify the relationship of two or more things in the world, where at least one is a building element or zone. Examples:
    - Qualification of heat transmission between zones through one or more building elements. This includes one-dimensional (surface) heat losses from one zone to another through a single building element, a two dimensional (line) loss from one zone to another through the connection in which the two elements meet or a three dimensional (point) loss from one zone to another through the connection where three elements (typically two walls and a slab) meet. 
    - Connection of an electric device to the electric system of a building. 
    - A door between one room and another."""@en ,
                                              """Ein allgemeines Konzept um eine qualifizierte Beziehung zwischen einem oder mehreren Dingen auf der Welt auszudrücken. Hierbei ist wenigstens eines der Dinge ein Bauteil oder eine Zone eines Gebäudes. Beispiele:
- Qualifizierung des Wärmeübergangs durch ein oder mehrere Bauteile. Dies umfasst eindimensionale Wärmeübertragung (Fläche) durch ein Bauteil von einer Zone zur nächsten; zweidimensionaler Wärmeübergang (Linie) von einer Zone zur nächsten an der Kontaktstelle, an der sich diese treffen oder dreidimensional (Punkt) von einer zone zur nächsten an der drei Bauteile sich treffen  (typischerweise ist dies der Fall, wenn zwei Wände und die Decke sich treffen);
- Verbindung eines elektrischen Geräts mit dem elektrischen Versorgungssystem eines Gebäudes;
- Eine Tür zwischen zwei Räumen."""@de ;
                                 rdfs:label "Interface"@en ,
                                            "Schnittstelle"@de .


###  https://w3id.org/bot#Site
<https://w3id.org/bot#Site> rdf:type owl:Class ;
                            rdfs:subClassOf <https://w3id.org/bot#Zone> ;
                            rdfs:comment "A part of the physical world or a virtual world that is inherently both located in this world and having a 3D spatial extent. It is intended to contain or contains one or more buildings."@en ,
                                         "Ein Teil der realen oder virtuellen Welt die beide Teil dieser Welt sind und eine räumliche Ausdehnung hat. Es besteht die Absicht, dass es Gebäude enthält, oder es enthält ein oder mehr Gebäude."@de ;
                            rdfs:label "Grundstück"@de ,
                                       "Site"@en .


###  https://w3id.org/bot#Space
<https://w3id.org/bot#Space> rdf:type owl:Class ;
                             rdfs:subClassOf <https://w3id.org/bot#Zone> ;
                             rdfs:comment """A part of the physical world or a virtual world whose 3D spatial extent is bounded actually or theoretically, and provides for certain functions within the zone it is contained in.

_

In FiSa, the concept is typically used to instantiate actual rooms."""@en ,
                                          """Ein Teil der realen oder virtuellen Welt, dessen räumliche Ausdehnung tatsächlich oder virtuell begrenzt ist. In der Zone in der es enthalten ist stellt es bestimmte Funktionen bereit.

_

In FiSa wird das Konzept typischerweise zur Instanziierung von tatsächlichen Räumen verwendet."""@de ;
                             rdfs:label "Raum"@de ,
                                        "Space"@en .


###  https://w3id.org/bot#Storey
<https://w3id.org/bot#Storey> rdf:type owl:Class ;
                              rdfs:subClassOf <https://w3id.org/bot#Zone> ;
                              rdfs:comment "A part of the physical world or a virtual world that is inherently both located in this world and having a 3D spatial extent. A bot:Storey is contained in one or more buildings, and is intended to contain one or more spaces that are horizontally connected. Storeys of a building are connected by means of vertical connections such as elevators and stairs. A bot:Storey encompasses both zones above and below ground, for example, a building with 21 floors above ground, one ground floor and 3 basements is equal to the sentence: A building has 25 instances of bot:Storey."@en ,
                                           "Ein Teil der realen oder virtuellen Welt die beide Teil dieser Welt sind und eine räumliche Ausdehnung hat. Ein bot:Storey ist in einem oder mehreren Gebäuden enthalten und es besteht die Absicht oder es ist der Fall, dass es ein oder mehrere Räume enthält, die horizontal miteinander verbunden sind. Geschosse eines Gebäudes sind vertikal miteinander verbunden, durch zum Beispiel Aufzüge oder Treppen. Ein bot:Storey umfassst zonen die über und unter der Erdoberfläche liegen. Zum Beispiel hat ein Gebäude mit 21 Geschossen über der Erde, ein Erdgeschoss und 3 Kellerstockwerken insgesamt 25 Instanzen von bot:Storey."@de ;
                              rdfs:label "Geschoss (Architektur)"@de ,
                                         "Storey"@en .


###  https://w3id.org/bot#Zone
<https://w3id.org/bot#Zone> rdf:type owl:Class ;
                            rdfs:label "Zone"@de ,
                                       "Zone"@en .


#################################################################
#    Individuals
#################################################################

###  https://purl.org/fisa#Administrative
:Administrative rdf:type owl:NamedIndividual ,
                         :Administrative .


###  https://purl.org/fisa#Agriculture
:Agriculture rdf:type owl:NamedIndividual ,
                      :Agriculture .


###  https://purl.org/fisa#AnimalHusbandry
:AnimalHusbandry rdf:type owl:NamedIndividual ,
                          :AnimalHusbandry .


###  https://purl.org/fisa#Bathroom
:Bathroom rdf:type owl:NamedIndividual ,
                   :Bathroom .


###  https://purl.org/fisa#BauartBrandwand
:BauartBrandwand rdf:type owl:NamedIndividual ,
                          :SpaceClosure ;
                 rdfs:label "BauartBrandwand"@de ,
                            "TypeFireWall"@en .


###  https://purl.org/fisa#BuildingClass1a
:BuildingClass1a rdf:type owl:NamedIndividual ,
                          :BuildingClass1a .


###  https://purl.org/fisa#BuildingClass1b
:BuildingClass1b rdf:type owl:NamedIndividual ,
                          :BuildingClass1b .


###  https://purl.org/fisa#BuildingClass2
:BuildingClass2 rdf:type owl:NamedIndividual ,
                         :BuildingClass2 .


###  https://purl.org/fisa#BuildingClass3
:BuildingClass3 rdf:type owl:NamedIndividual ,
                         :BuildingClass3 .


###  https://purl.org/fisa#BuildingClass4
:BuildingClass4 rdf:type owl:NamedIndividual ,
                         :BuildingClass4 .


###  https://purl.org/fisa#BuildingClass5
:BuildingClass5 rdf:type owl:NamedIndividual ,
                         :BuildingClass5 ;
                :hasDescription "Dies ist die Beschreibung für Klasse 5." .


###  https://purl.org/fisa#Canteen
:Canteen rdf:type owl:NamedIndividual ,
                  :Canteen .


###  https://purl.org/fisa#Care
:Care rdf:type owl:NamedIndividual ,
               :Care .


###  https://purl.org/fisa#CareForPeople
:CareForPeople rdf:type owl:NamedIndividual ,
                        :CareForPeople .


###  https://purl.org/fisa#ChildCare
:ChildCare rdf:type owl:NamedIndividual ,
                    :ChildCare .


###  https://purl.org/fisa#Corridor
:Corridor rdf:type owl:NamedIndividual ,
                   :Corridor .


###  https://purl.org/fisa#Education
:Education rdf:type owl:NamedIndividual ,
                    :Education .


###  https://purl.org/fisa#EmergencyMedicalService
:EmergencyMedicalService rdf:type owl:NamedIndividual ,
                                  :EmergencyMedicalService .


###  https://purl.org/fisa#ErsterRettungswegGeb06
:ErsterRettungswegGeb06 rdf:type owl:NamedIndividual ,
                                 :FirstEscapeRoute ;
                        rdfs:label "B06_FirstEscapeRoute"@en ,
                                   "Geb06_ErsterRettungsweg"@de .


###  https://purl.org/fisa#ExternalDevelopment
:ExternalDevelopment rdf:type owl:NamedIndividual ,
                              :ExternalDevelopment .


###  https://purl.org/fisa#Foyer
:Foyer rdf:type owl:NamedIndividual ,
                :Foyer .


###  https://purl.org/fisa#Geb01_NE01
:Geb01_NE01 rdf:type owl:NamedIndividual ,
                     :UtilizationUnit ;
            :usesGrossFloorArea "350.0"^^xsd:double ;
            rdfs:label "B1a_UtilizationUnit01"@en ,
                       "Geb01_NE01"@de .


###  https://purl.org/fisa#Geb02_NE01
:Geb02_NE01 rdf:type owl:NamedIndividual ,
                     :UtilizationUnit ;
            :usesGrossFloorArea "150.0"^^xsd:double ;
            rdfs:label "B02_UtilizationUnit01"@en ,
                       "Geb02_NE01"@de .


###  https://purl.org/fisa#Geb02_NE02
:Geb02_NE02 rdf:type owl:NamedIndividual ,
                     :UtilizationUnit ;
            :usesGrossFloorArea "100.0"^^xsd:double ;
            rdfs:label "B02_UtilizationUnit02"@en ,
                       "Geb02_NE02"@de .


###  https://purl.org/fisa#Geb03_Dachraum
:Geb03_Dachraum rdf:type owl:NamedIndividual ,
                         :AtticSpace .


###  https://purl.org/fisa#Geb03_NE01
:Geb03_NE01 rdf:type owl:NamedIndividual ,
                     :UtilizationUnit ;
            :usesGrossFloorArea "200.0"^^xsd:double ;
            rdfs:label "B03_UtilizationUnit01"@en ,
                       "Geb03_NE01"@de .


###  https://purl.org/fisa#Geb03_NE02
:Geb03_NE02 rdf:type owl:NamedIndividual ,
                     :UtilizationUnit ;
            :usesGrossFloorArea "100.0"^^xsd:double ;
            rdfs:label "B03_UtilizationUnit02"@en ,
                       "Geb03_NE02"@de .


###  https://purl.org/fisa#Geb03_NE03
:Geb03_NE03 rdf:type owl:NamedIndividual ,
                     :UtilizationUnit ;
            :usesGrossFloorArea "100.0"^^xsd:double ;
            rdfs:label "B03_UtilizationUnit03"@en ,
                       "Geb03_NE03"@de .


###  https://purl.org/fisa#Geb04_NE01
:Geb04_NE01 rdf:type owl:NamedIndividual ,
                     :UtilizationUnit ;
            :usesGrossFloorArea "380.0"^^xsd:double ;
            rdfs:label "B04_UtilizationUnit01"@en ,
                       "Geb04_NE01"@de .


###  https://purl.org/fisa#Geb04_NE02
:Geb04_NE02 rdf:type owl:NamedIndividual ,
                     :UtilizationUnit ;
            :usesGrossFloorArea "200.0"^^xsd:double ;
            rdfs:label "B04_UtilizationUnit02"@en ,
                       "Geb04_NE02"@de .


###  https://purl.org/fisa#Geb05_NE01
:Geb05_NE01 rdf:type owl:NamedIndividual ,
                     :UtilizationUnit ;
            :usesGrossFloorArea "500.0"^^xsd:double ;
            rdfs:label "B05_UtilizationUnit01"@en ,
                       "Geb04_NE01"@de .


###  https://purl.org/fisa#Geb06_Raum01
:Geb06_Raum01 rdf:type owl:NamedIndividual ,
                       <https://w3id.org/bot#Space> ;
              :hasUsage :OfficeRoom ;
              :usesGrossFloorArea "450.0"^^xsd:double ;
              rdfs:label "B06_Space01"@en ,
                         "Geb06_Raum01"@de .


###  https://purl.org/fisa#Geb06_Raum02
:Geb06_Raum02 rdf:type owl:NamedIndividual ,
                       <https://w3id.org/bot#Space> ;
              :hasUsage :MeetingRoom ;
              :hasNumberOfVisitors 100 ;
              rdfs:label "B06_Space02"@en ,
                         "Geb06_Raum02"@en .


###  https://purl.org/fisa#Geb06_Raum03
:Geb06_Raum03 rdf:type owl:NamedIndividual ,
                       <https://w3id.org/bot#Space> ;
              :hasEscapeRoute :ErsterRettungswegGeb06 ;
              :hasUsage :MeetingRoom ;
              :hasNumberOfVisitors 50 ;
              rdfs:label "B06_Space03"@en ,
                         "Geb06_Raum03"@de .


###  https://purl.org/fisa#Geb06_Raum04
:Geb06_Raum04 rdf:type owl:NamedIndividual ,
                       <https://w3id.org/bot#Space> ;
              :hasEscapeRoute :ErsterRettungswegGeb06 ;
              :hasUsage :MeetingRoom ;
              :hasNumberOfVisitors 125 ;
              rdfs:label "B06_Space04"@en ,
                         "Geb06_Raum04"@de .


###  https://purl.org/fisa#Geb08_GeschlossenesProfil02
:Geb08_GeschlossenesProfil02 rdf:type owl:NamedIndividual ,
                                      :ClosedProfile ;
                             :hasFireBehaviour :nichtbrennbar ;
                             :hasFireResistance :feuerhemmend ;
                             <https://w3id.org/bot#containsElement> <https://purl.org/fisa#11_Dämmstoff02> ;
                             rdfs:label "B08_ClosedProfile02"@en ,
                                        "Geb08_GeschlossenesProfil02"@de .


###  https://purl.org/fisa#Gebäude02
:Gebäude02 rdf:type owl:NamedIndividual ,
                    <https://w3id.org/bot#Building> ;
           :hasUtilizationSpace :Geb02_NE01 ,
                                :Geb02_NE02 ;
           :hasAverageHeight "6.0"^^xsd:double ;
           :hasCombinedGrossFloorArea "250.0"^^xsd:double ;
           :hasTotalAmountOfUtilizationUnits 2 ;
           :isFreestanding "false"^^xsd:boolean ;
           :under400_meta "true"^^xsd:boolean ;
           rdfs:label "Building02"@en ,
                      "Gebäude02"@de ;
           :unter400_meta "true"^^xsd:boolean .


###  https://purl.org/fisa#Gebäude03
:Gebäude03 rdf:type owl:NamedIndividual ,
                    <https://w3id.org/bot#Building> ;
           :hasUtilizationSpace :Geb03_NE01 ,
                                :Geb03_NE02 ,
                                :Geb03_NE03 ;
           <https://w3id.org/bot#hasSpace> :Raum01 ;
           :hasAverageHeight "7.0"^^xsd:double ;
           :hasCombinedGrossFloorArea "400.0"^^xsd:double ;
           :hasTotalAmountOfUtilizationUnits 3 ;
           :under400_meta "true"^^xsd:boolean ;
           rdfs:label "Building03"@en ,
                      "Gebäude03"@de ;
           :unter400_meta "true"^^xsd:boolean .


###  https://purl.org/fisa#Gebäude04
:Gebäude04 rdf:type owl:NamedIndividual ,
                    <https://w3id.org/bot#Building> ;
           :hasUsage :Residential ;
           :hasUtilizationSpace :Geb04_NE01 ,
                                :Geb04_NE02 ;
           :hasAverageHeight "10.0"^^xsd:double ;
           :hasCombinedGrossFloorArea "580.0"^^xsd:double ;
           :hasTotalAmountOfUtilizationUnits 2 ;
           :under400_meta "true"^^xsd:boolean ;
           rdfs:label "Building04"@en ,
                      "Gebäude04"@de ;
           :unter400_meta "true"^^xsd:boolean .


###  https://purl.org/fisa#Gebäude05
:Gebäude05 rdf:type owl:NamedIndividual ,
                    <https://w3id.org/bot#Building> ;
           :hasUtilizationSpace :Geb05_NE01 ;
           :hasAverageHeight "25.0"^^xsd:double ;
           :hasCombinedGrossFloorArea "500.0"^^xsd:double ;
           :hasTotalAmountOfUtilizationUnits 1 ;
           :under400_meta "false"^^xsd:boolean ;
           rdfs:label "Building05"@en ,
                      "Gebäude05"@de ;
           :unter400_meta "false"^^xsd:boolean .


###  https://purl.org/fisa#Gebäude06
:Gebäude06 rdf:type owl:NamedIndividual ,
                    <https://w3id.org/bot#Building> ;
           :hasEscapeRoute :ErsterRettungswegGeb06 ;
           <https://w3id.org/bot#hasSpace> :Geb06_Raum01 ,
                                           :Geb06_Raum02 ,
                                           :Geb06_Raum03 ,
                                           :Geb06_Raum04 ;
           rdfs:label "Building06_(Assembly)"@en ,
                      "Gebäude06_(Versammlungsstätte)"@de .


###  https://purl.org/fisa#Gebäude10
:Gebäude10 rdf:type owl:NamedIndividual ,
                    :SalesPremises ,
                    <https://w3id.org/bot#Building> ;
           <https://w3id.org/bot#hasStorey> <https://purl.org/fisa#10_EG> ;
           :hasGFASalesSpaces "2200.0"^^xsd:double ;
           rdfs:label "Building07_(SalesPremises)"@en ,
                      "Gebäude07_(Verkaufsstätte)"@de ;
           <http://www.w3.org/2004/02/skos/core#altLabel> "Testgebäude10"@de .


###  https://purl.org/fisa#Gebäude11
:Gebäude11 rdf:type owl:NamedIndividual ,
                    <https://w3id.org/bot#Building> ;
           :hasBuildingClass :BuildingClass4 ;
           <https://w3id.org/bot#hasStorey> <https://purl.org/fisa#11_OG> ;
           rdfs:label "Building08_(LayerSystem)"@en ,
                      "Gebäude08_(LayerSystem)"@de .


###  https://purl.org/fisa#Gebäude1a
:Gebäude1a rdf:type owl:NamedIndividual ,
                    <https://w3id.org/bot#Building> ;
           :hasUtilizationSpace :Geb01_NE01 ;
           :hasAverageHeight "6.0"^^xsd:double ;
           :hasCombinedGrossFloorArea "350.0"^^xsd:double ;
           :hasTotalAmountOfUtilizationUnits 1 ;
           :isFreestanding "true"^^xsd:boolean ;
           :under400_meta "true"^^xsd:boolean ;
           rdfs:label "Building1a"@en ,
                      "Gebäude1a"@de ;
           :unter400_meta "true"^^xsd:boolean .


###  https://purl.org/fisa#Gebäude1b
:Gebäude1b rdf:type owl:NamedIndividual ,
                    <https://w3id.org/bot#Building> ;
           :hasUsage :Agriculture ;
           :isFreestanding "true"^^xsd:boolean ;
           rdfs:label "Building1b"@en ,
                      "Gebäude1b"@de .


###  https://purl.org/fisa#Gym
:Gym rdf:type owl:NamedIndividual ,
              :Gym .


###  https://purl.org/fisa#HazardousEnvironment
:HazardousEnvironment rdf:type owl:NamedIndividual ,
                               :HazardousEnvironment .


###  https://purl.org/fisa#Hospitality
:Hospitality rdf:type owl:NamedIndividual ,
                      :Hospitality .


###  https://purl.org/fisa#Institution
:Institution rdf:type owl:NamedIndividual ,
                      :Institution .


###  https://purl.org/fisa#Kindergarden
:Kindergarden rdf:type owl:NamedIndividual ,
                       :Kindergarden .


###  https://purl.org/fisa#Kitchen
:Kitchen rdf:type owl:NamedIndividual ,
                  :Kitchen .


###  https://purl.org/fisa#Lab
:Lab rdf:type owl:NamedIndividual ,
              :Lab .


###  https://purl.org/fisa#LawEnforcement
:LawEnforcement rdf:type owl:NamedIndividual ,
                         :LawEnforcement .


###  https://purl.org/fisa#Leisure
:Leisure rdf:type owl:NamedIndividual ,
                  :Leisure .


###  https://purl.org/fisa#LivingRoom
:LivingRoom rdf:type owl:NamedIndividual ,
                     :LivingRoom .


###  https://purl.org/fisa#MeetingRoom
:MeetingRoom rdf:type owl:NamedIndividual ,
                      :MeetingRoom .


###  https://purl.org/fisa#OfficeRoom
:OfficeRoom rdf:type owl:NamedIndividual ,
                     :OfficeRoom ;
            :usesGrossFloorArea "600.0"^^xsd:double .


###  https://purl.org/fisa#OtherRoomUsage
:OtherRoomUsage rdf:type owl:NamedIndividual ,
                         :OtherRoomUsage .


###  https://purl.org/fisa#OvernightAccommodation
:OvernightAccommodation rdf:type owl:NamedIndividual ,
                                 :OvernightAccommodation .


###  https://purl.org/fisa#Parking
:Parking rdf:type owl:NamedIndividual ,
                  :Parking .


###  https://purl.org/fisa#Raum01
:Raum01 rdf:type owl:NamedIndividual ,
                 <https://w3id.org/bot#Space> ;
        :hasSpaceUsage :OfficeRoom ;
        :hasNumberOfPeople 120 ;
        rdfs:label "B03_Space01"@en ,
                   "Geb03_Raum01"@de .


###  https://purl.org/fisa#Residential
:Residential rdf:type owl:NamedIndividual ,
                      :Residential .


###  https://purl.org/fisa#Sales
:Sales rdf:type owl:NamedIndividual ,
                :Sales .


###  https://purl.org/fisa#SalesRoom
:SalesRoom rdf:type owl:NamedIndividual ,
                    :SalesRoom .


###  https://purl.org/fisa#SceneArea
:SceneArea rdf:type owl:NamedIndividual ,
                    :SceneArea .


###  https://purl.org/fisa#SpectatorFacility
:SpectatorFacility rdf:type owl:NamedIndividual ,
                            :SpectatorFacility .


###  https://purl.org/fisa#Sport
:Sport rdf:type owl:NamedIndividual ,
                :Sport .


###  https://purl.org/fisa#StairSpace
:StairSpace rdf:type owl:NamedIndividual ,
                     :StairSpace .


###  https://purl.org/fisa#Storage
:Storage rdf:type owl:NamedIndividual ,
                  :Storage .


###  https://purl.org/fisa#StoreStreet
:StoreStreet rdf:type owl:NamedIndividual ,
                      :StoreStreet .


###  https://purl.org/fisa#Technology
:Technology rdf:type owl:NamedIndividual ,
                     :Technology .


###  https://purl.org/fisa#Tor01
:Tor01 rdf:type owl:NamedIndividual ,
                :Gate ;
       :isSelfClosing "true"^^xsd:boolean ;
       :isTightClosing "true"^^xsd:boolean .


###  https://purl.org/fisa#Tor02
:Tor02 rdf:type owl:NamedIndividual ,
                :Gate ;
       :hasFireResistance :feuerhemmend ;
       :isSelfClosing "true"^^xsd:boolean ;
       :isTightClosing "true"^^xsd:boolean .


###  https://purl.org/fisa#Work
:Work rdf:type owl:NamedIndividual ,
               :Work .


###  https://purl.org/fisa#brennbar
:brennbar rdf:type owl:NamedIndividual ,
                   :FireBehaviour ;
          :isMoreFlammableThan :leichtentflammbar ;
          rdfs:label "brennbar"@de ,
                     "flammable"@en .


###  https://purl.org/fisa#feuerbeständig
:feuerbeständig rdf:type owl:NamedIndividual ,
                         :FireResistance ;
                :isMoreFireResistantThan :hochfeuerhemmend ;
                rdfs:label "feuerbeständig"@de ,
                           "fire-resistant"@en .


###  https://purl.org/fisa#feuerhemmend
:feuerhemmend rdf:type owl:NamedIndividual ,
                       :FireResistance ;
              rdfs:label "feuerhemmend"@de ,
                         "fire-retardent"@en .


###  https://purl.org/fisa#hochfeuerbeständig
:hochfeuerbeständig rdf:type owl:NamedIndividual ,
                             :FireResistance ;
                    :isMoreFireResistantThan :feuerbeständig ;
                    rdfs:label "highly-fire-resistant"@en ,
                               "hochfeuerbeständig"@de .


###  https://purl.org/fisa#hochfeuerhemmend
:hochfeuerhemmend rdf:type owl:NamedIndividual ,
                           :FireResistance ;
                  :isMoreFireResistantThan :feuerhemmend ;
                  rdfs:label "highly-fire-retardent"@en ,
                             "hochfeuerhemmend"@de .


###  https://purl.org/fisa#höchstfeuerbeständig
:höchstfeuerbeständig rdf:type owl:NamedIndividual ,
                               :FireResistance ;
                      :isMoreFireResistantThan :hochfeuerbeständig ;
                      rdfs:label "höchstfeuerbeständig"@de ,
                                 "mosthighly-fire-resistant"@en .


###  https://purl.org/fisa#leichtentflammbar
:leichtentflammbar rdf:type owl:NamedIndividual ,
                            :FireBehaviour ;
                   :isMoreFlammableThan :normalentflammbar ;
                   rdfs:label "highly-flammable"@en ,
                              "leichtentflammbar"@de .


###  https://purl.org/fisa#nichtbrennbar
:nichtbrennbar rdf:type owl:NamedIndividual ,
                        :FireBehaviour ;
               rdfs:label "nichtbrennbar"@de ,
                          "non-flammable"@en .


###  https://purl.org/fisa#normalentflammbar
:normalentflammbar rdf:type owl:NamedIndividual ,
                            :FireBehaviour ;
                   :isMoreFlammableThan :schwerentflammbar ;
                   rdfs:label "normal-flammable"@en ,
                              "normalentflammbar"@de .


###  https://purl.org/fisa#ohneAnforderung
:ohneAnforderung rdf:type owl:NamedIndividual ,
                          :SpaceClosure ;
                 rdfs:label "WithoutRequirement"@en ,
                            "ohneAnforderung"@de .


###  https://purl.org/fisa#schwerentflammbar
:schwerentflammbar rdf:type owl:NamedIndividual ,
                            :FireBehaviour ;
                   :isMoreFlammableThan :nichtbrennbar ;
                   rdfs:label "retardent-flammable"@en ,
                              "schwerentflammbar"@de .


###  https://purl.org/fisa#10_EG
<https://purl.org/fisa#10_EG> rdf:type owl:NamedIndividual ,
                                       :GroundStorey ;
                              <https://w3id.org/bot#hasSpace> <https://purl.org/fisa#10_Raum01> ,
                                                              <https://purl.org/fisa#10_Raum02> ,
                                                              <https://purl.org/fisa#10_Raum03> ;
                              rdfs:label "B07_GroundStorey"@en ,
                                         "Geb07_Erdgeschoss"@de .


###  https://purl.org/fisa#10_Raum01
<https://purl.org/fisa#10_Raum01> rdf:type owl:NamedIndividual ,
                                           <https://w3id.org/bot#Space> ;
                                  :hasUsage :SalesRoom ;
                                  :usesGrossFloorArea "1900.0"^^xsd:double ;
                                  rdfs:label "B07_Space01"@en ,
                                             "Geb07_Raum01"@de .


###  https://purl.org/fisa#10_Raum02
<https://purl.org/fisa#10_Raum02> rdf:type owl:NamedIndividual ,
                                           <https://w3id.org/bot#Space> ;
                                  :hasUsage :StoreStreet ;
                                  :usesGrossFloorArea "300.0"^^xsd:double ;
                                  rdfs:label "B07_Space02"@en ,
                                             "Geb07_Raum02"@de .


###  https://purl.org/fisa#10_Raum03
<https://purl.org/fisa#10_Raum03> rdf:type owl:NamedIndividual ,
                                           <https://w3id.org/bot#Space> ;
                                  :hasUsage :OfficeRoom ;
                                  :usesGrossFloorArea "150.0"^^xsd:double ;
                                  rdfs:label "B07_Space03"@en ,
                                             "Geb07_Raum03"@de .


###  https://purl.org/fisa#11_Außenwand01
<https://purl.org/fisa#11_Außenwand01> rdf:type owl:NamedIndividual ,
                                                :ExternalWall ;
                                       :hasFireResistance :feuerhemmend ;
                                       <https://w3id.org/bot#hasSubElement> <https://purl.org/fisa#11_Befestigung> ,
                                                                            <https://purl.org/fisa#11_Dämmstoff> ,
                                                                            <https://purl.org/fisa#11_Dämmstoff02> ,
                                                                            <https://purl.org/fisa#11_GProfil> ;
                                       :isLoadBearing "false"^^xsd:boolean ;
                                       :isSpaceEnclosing "true"^^xsd:boolean ;
                                       rdfs:label "B08_ExternalWall01"@en ,
                                                  "Geb08_Außenwand01"@de .


###  https://purl.org/fisa#11_Befestigung
<https://purl.org/fisa#11_Befestigung> rdf:type owl:NamedIndividual ,
                                                :Fastening ;
                                       :hasFireResistance :feuerhemmend ;
                                       :isLoadBearing "false"^^xsd:boolean ;
                                       rdfs:label "B08_Fastening"@en ,
                                                  "Geb08_Befestigung"@de .


###  https://purl.org/fisa#11_Dämmstoff
<https://purl.org/fisa#11_Dämmstoff> rdf:type owl:NamedIndividual ,
                                              :Insulation ;
                                     :hasFireBehaviour :brennbar ;
                                     rdfs:label "B08_Insulation01"@en ,
                                                "Geb08_Dämmstoff01"@de .


###  https://purl.org/fisa#11_Dämmstoff02
<https://purl.org/fisa#11_Dämmstoff02> rdf:type owl:NamedIndividual ,
                                                :Insulation ;
                                       :hasFireBehaviour :normalentflammbar ;
                                       rdfs:label "B08_Insulation02"@en ,
                                                  "Geb08_Dämmstoff02"@de .


###  https://purl.org/fisa#11_GProfil
<https://purl.org/fisa#11_GProfil> rdf:type owl:NamedIndividual ,
                                            :ClosedProfile ;
                                   :hasFireBehaviour :nichtbrennbar ;
                                   :hasFireResistance :feuerhemmend ;
                                   <https://w3id.org/bot#containsElement> <https://purl.org/fisa#11_Dämmstoff> ,
                                                                          <https://purl.org/fisa#11_Dämmstoff02> ;
                                   rdfs:label "B08_ClosedProfile01"@en ,
                                              "Geb08_GeschlossenesProfil01"@de .


###  https://purl.org/fisa#11_OG
<https://purl.org/fisa#11_OG> rdf:type owl:NamedIndividual ,
                                       :UpperStorey ;
                              <https://w3id.org/bot#hasSpace> <https://purl.org/fisa#11_Raum> ;
                              rdfs:label "B08_UpperStorey"@en ,
                                         "Geb08_Obergeschoss"@de .


###  https://purl.org/fisa#11_Raum
<https://purl.org/fisa#11_Raum> rdf:type owl:NamedIndividual ,
                                         <https://w3id.org/bot#Space> ;
                                <https://w3id.org/bot#hasElement> <https://purl.org/fisa#11_Außenwand01> ;
                                rdfs:label "B08_Space"@en ,
                                           "Geb08_Raum"@de .


[ rdfs:comment "Bauteil (Bauwesen)"
] .

#################################################################
#    Annotations
#################################################################

:Administrative rdfs:comment "Beschreibt einen Raum der Verwaltung bzw. einen für Verwaltungsaufgaben ausgelegten Raum."@de ,
                              "Describes a space of administration or a space used for administrative tasks."@en ;
                 rdfs:label "Administrative"@en ,
                            "Verwaltung"@de .


:Agriculture rdfs:comment "Die Aktivitäten, Strukturen und Einrichtungen, die mit der Produktion von landwirtschaftlichen Erzeugnissen verbunden sind."@de ,
                          "The activities, structures and facilities associated with the production of agricultural products."@en ;
             rdfs:label "Agriculture"@en ,
                        "Landwirtschaft"@de .


:AnimalHusbandry rdfs:comment "Die Aktivität des Haltens und Pflegens von Tieren in baulichen Anlagen oder Einrichtungen."@de ,
                              "The activity of keeping and caring for animals in structures or facilities."@en ;
                 rdfs:label "AnimalHusbandry"@en ,
                            "Tierhaltung"@de .


:Bathroom rdfs:comment "Beschreibt einen Raum, der als Bad genutzt wird bzw. mit Sanitäranlagen ausgestattet ist."@de ,
                       "Describes a space used as a bathroom or equipped with sanitary facilities."@en ;
          rdfs:label "Bad"@de ,
                     "Bathroom"@en .


:BuildingClass1a <http://purl.org/dc/terms/description> """Gebäude werden in folgende Gebäudeklassen eingeteilt:
1. Gebäudeklasse 1:
a) freistehende Gebäude mit einer Höhe bis zu 7 m und nicht mehr als zwei Nutzungseinheiten von insgesamt nicht mehr als 400 m2 und
[...]"""@de ;
                 rdfs:comment """Buildings are divided into the following building classes:
1. building class 1:
(a) freestanding/detached buildings with a height of up to 7 m and not more than two units of use totaling not more than 400 m2 and
[...]"""@en ;
                 rdfs:isDefinedBy :MBO ;
                 rdfs:label "BuildingClass1a"@en ,
                            "Gebäudeklasse1a"@de ;
                 :gemäß "§2 (3) 1. a) MBO"@de .


:BuildingClass1b <http://purl.org/dc/terms/description> """Gebäude werden in folgende Gebäudeklassen eingeteilt:
1. Gebäudeklasse 1:
[...]
b) freistehende land- oder forstwirtschaftlich genutzte Gebäude,
[...]"""@de ;
                 rdfs:comment """Buildings are divided into the following building classes:
1. building class 1:
[...]
(b) freestanding/detached agricultural or forestry buildings,
[...]"""@en ;
                 rdfs:isDefinedBy :MBO ;
                 rdfs:label "BuildingClass1b"@en ,
                            "Gebäudeklasse1b"@de ;
                 :gemäß "§2 (3) 1. b) MBO"@de .


:BuildingClass2 <http://purl.org/dc/terms/description> """Gebäude werden in folgende Gebäudeklassen eingeteilt:
[...]
2. Gebäudeklasse 2:
Gebäude mit einer Höhe bis zu 7 m und nicht mehr als zwei Nutzungseinheiten von insgesamt nicht mehr als 400 m2,
[...]"""@de ;
                rdfs:comment """Buildings are divided into the following building classes:
[...]
Building class 2:
Buildings with a height of up to 7 m and no more than two units of a combined gross floor area of no more than 400 m2,
[...]"""@en ;
                rdfs:isDefinedBy :MBO ;
                rdfs:label "BuildingClass2"@en ,
                           "Gebäudeklasse2"@de ;
                :gemäß "§2 (3) 2. MBO"@de .


:BuildingClass3 <http://purl.org/dc/terms/description> """Gebäude werden in folgende Gebäudeklassen eingeteilt:
[...]
3. Gebäudeklasse 3:
sonstige Gebäude mit einer Höhe bis zu 7 m,
[...]"""@de ;
                rdfs:comment """Buildings are divided into the following building classes:
[...]
3. building class 3:
Other buildings with a height of up to 7 m,
[...]"""@en ;
                rdfs:isDefinedBy :MBO ;
                rdfs:label "BuildingClass3"@en ,
                           "Gebäudeklasse3"@de ;
                :gemäß "§2 (3) 3. MBO"@de .


:BuildingClass4 <http://purl.org/dc/terms/description> """Gebäude werden in folgende Gebäudeklassen eingeteilt:
[...]
4. Gebäudeklasse 4:
Gebäude mit einer Höhe bis zu 13 m und Nutzungseinheiten mit jeweils nicht mehr als 400 m2,
[...]"""@de ;
                rdfs:comment """Buildings are divided into the following building classes:
[...]
Building class 4:
Buildings with a height of up to 13m and utilization units not exceeding 400 m2 each,
[...]"""@en ;
                rdfs:isDefinedBy :MBO ;
                rdfs:label "BuildingClass4"@en ,
                           "Gebäudeklasse4"@de ;
                :gemäß "§2 (3) 4. MBO"@de .


:BuildingClass5 <http://purl.org/dc/terms/description> """Gebäude werden in folgende Gebäudeklassen eingeteilt:
[...]
5. Gebäudeklasse 5:
sonstige Gebäude einschließlich unterirdischer Gebäude.
[...]"""@de ;
                rdfs:comment """Buildings are divided into the following building classes:
[...]
5. building class 5:
Other buildings including underground buildings.
[...]"""@en ;
                rdfs:isDefinedBy :MBO ;
                rdfs:label "BuildingClass5"@en ,
                           "Gebäudeklasse5"@de ;
                :gemäß "§2 (3) 5. MBO"@de .


:Canteen rdfs:comment "Beschreibt eine Kantine oder Mensa, welche Gastbewirtschaftung und Kochen vereinen kann."@de ,
                      "Describes a canteen or cafeteria, which can combine catering and cooking."@en ;
         rdfs:label "Canteen"@en ,
                    "Kantine"@de .


:Care rdfs:comment "Die Aktivitäten und Einrichtungen, die der Betreuung, Unterbringung und Versorgung von Personen mit Pflegebedürftigkeit oder eingeschränkter Selbstrettungsfähigkeit dienen."@de ,
                   "The activities and facilities used to provide care, housing, and services to persons in need of care or with limited self-rescue capabilities."@en ;
      rdfs:label "Care"@en ,
                 "Pflege"@de .


:CareForPeople rdfs:comment "Die Aktivitäten und Einrichtungen, die der Unterstützung, Beaufsichtigung und Versorgung von Menschen mit unterschiedlichen Bedürfnissen und Anforderungen dienen."@de ,
                            "The activities and facilities designed to support, supervise, and care for people with diverse needs and requirements."@en ;
               rdfs:label "BetreuungVonPersonen"@de ,
                          "CareForPeople"@en .


:ChildCare rdfs:comment "Die Aktivitäten und Einrichtungen, die der Unterstützung, Beaufsichtigung und Versorgung von Menschen mit unterschiedlichen Bedürfnissen und Anforderungen dienen."@de ,
                        "The activities and facilities designed to support, supervise, and care for people with diverse needs and requirements."@en ;
           rdfs:label "BetreuungVonKindern"@de ,
                      "ChildCare"@en .


:Corridor rdfs:comment "A horizontal space or corridar or passageway within a building that serves as a connection between different spaces, or areas."@en ,
                       "Ein horizontaler Raum oder Durchgang innerhalb eines Gebäudes, der als Verbindung zwischen verschiedenen Räumen, Zimmern oder Bereichen dient."@de ;
          rdfs:label "Corridor"@en ,
                     "Flur"@de .


:Education rdfs:comment "Nutzungszwecke der Bildung, Schulung und Ausbildung von Menschen."@de ,
                        "Utilization purposes of education, training and education of people."@en ;
           rdfs:label "Bildung"@de ,
                      "Education"@en .


:EmergencyMedicalService rdfs:comment "Dient dem Nutzungszweck der medizinischen Notfallversorgung, wie z.B. in einem Krankenhaus."@de ,
                                      "Serves the purpose of use for emergency medical care, such as in a hospital."@en ;
                         rdfs:label "EmergencyMedicalService"@en ,
                                    "MedizinischeNotversorgung"@de .


:ExternalDevelopment rdfs:comment "Die äußere Erschließung umfasst die Flächen und Wege, die vom öffentlichen Verkehrsraum zu einer baulichen Anlage führen."@de ,
                                  "Dient dem Nutzungszweck der Erschließung von Grundstücken."@de ,
                                  "Serves the intended use of external site development."@en ,
                                  "The external development includes the areas and paths that lead from the public traffic area to a structural facility."@en ;
                     rdfs:label "Erschließung"@de ,
                                "ExternalDevelopment"@en ,
                                "ÄußereErschließung"@de .


:Foyer rdfs:comment "An (often) open entrance or reception area in a building used to welcome, direct, and orient visitors."@en ,
                    "Einen (oft) offenen Eingangsbereich oder Empfangsbereich in einem Gebäude, der dazu dient, Besucher zu empfangen, zu leiten und zu orientieren."@de ;
       rdfs:label "Foyer"@de ,
                  "Foyer"@en .


:Gym rdfs:comment "A space or facility within a building used for physical activities, sports, and fitness."@en ,
                  "Ein Raum oder eine Einrichtung innerhalb eines Gebäudes, die für körperliche Aktivitäten, Sport und Fitness genutzt wird."@de ;
     rdfs:label "Fitnessraum"@de ,
                "Gym"@en ;
     <http://www.w3.org/2004/02/skos/core#altLabel> "FitnessSpace"@en .


:HazardousEnvironment rdfs:comment "Dient dem Nutzungszweck der Definition von Gefahrensumgebungen."@de ,
                                   "Serves the utilization purpose of defining hazardous environments."@en ;
                      rdfs:label "Gefahrensumgebung"@de ,
                                 "HazardousEnvironment"@en .


:Hospitality rdfs:comment "Dient dem Nutzungszweck der Definition der Gastwirtschaft."@de ,
                          "Serves the utilization purpose of defining hospitality."@en ;
             rdfs:label "Gastwirtschaft"@de ,
                        "Hospitality"@en .


:Institution rdfs:comment "Dient dem Nutzungszweck der Definition von Einrichtungen."@de ,
                          "Serves the utilization purpose of defining Institutions."@en ;
             rdfs:label "Einrichtung"@de ,
                        "Institution"@en .


:Kindergarden rdfs:comment "Dient dem Nutzungszweck von Kindergärten."@de ,
                           "Serves the utilization purpose of defining kindergardens."@en ;
              rdfs:label "Kindergarden"@en ,
                         "Kindergarten"@de .


:Kitchen rdfs:comment "A space where food and drinks are stored and prepared."@en ,
                      "Ein Raum, in dem Speisen und Getränke gelagert und zubereitet werden."@de ;
         rdfs:label "Kitchen"@en ,
                    "Küche"@de .


:Lab rdfs:comment "Dient dem Nutzungszweck von Laboren."@de ,
                  "Serves the utilization purpose of defining labs."@en ;
     rdfs:label "Lab"@en ,
                "Labor"@de .


:LawEnforcement rdfs:comment "Dient dem Nutzungszweck der Definition vom Justizvollzug."@de ,
                             "Serves the utilization purpose of defining law enforcement."@en ;
                rdfs:label "Justizvollzug"@de ,
                           "LawEnforcement"@en .


:Leisure rdfs:comment "Dient dem Nutzungszweck von Freizeit."@de ,
                      "Serves the utilization purpose of leisure."@en ;
         rdfs:label "Freizeit"@de ,
                    "Leisure"@en .


:LivingRoom rdfs:comment "An area within a building that is intended to be occupied by people."@en ,
                         "Einen Bereich innerhalb eines Gebäudes, der dazu bestimmt ist, von Menschen bewohnt zu werden."@de ;
            rdfs:label "LivingRoom"@en ,
                       "Wohnraum"@de .


:MeetingRoom rdfs:comment "A space within a building used to gather people for various purposes."@en ,
                          "Ein Raum innerhalb eines Gebäudes, der dazu dient, Menschen für verschiedene Zwecke zu versammeln."@de ;
             rdfs:label "MeetingRoom"@en ,
                        "Versammlungsraum"@de .


:OfficeRoom rdfs:comment "A space within a building designed to be used as a workstation for office activities."@en ,
                         "Ein Raum innerhalb eines Gebäudes, der dazu dient, als Arbeitsplatz für Bürotätigkeiten genutzt zu werden."@de ;
            rdfs:label "Büroraum"@de ,
                       "OfficeRoom"@en .


:OtherRoomUsage rdfs:comment "A space within a building designed to be used as with any other purpose."@en ,
                             "Ein Raum innerhalb eines Gebäudes, der zu irgendeinem anderen Zweck genutzt werden kann/soll."@de ;
                rdfs:label "AndereRaumNutzung"@de ,
                           "OtherRoomUsage"@en .


:OvernightAccommodation rdfs:comment "Dient dem Nutzungszweck der Definition von Übernachtungsmöglichkeiten."@de ,
                                     "Serves the utilization purpose of defining overnight accommodations."@en ;
                        rdfs:label "OvernightAccommodation"@en ,
                                   "Unterbringung"@de ,
                                   "Übernachtung"@de .


:Parking rdfs:comment """Dient dem Nutzungszweck vom Parken.

_
Hierunter fallen auch die Stellplätze für Fahrräder im Innenbereich."""@de ,
                      """Serves the utilization purpose of defining parking.

_
This includes indoor bicycle parking."""@en ;
         rdfs:label "Parken"@de ,
                    "Parking"@en .


:Residential rdfs:comment "Dient dem Nutzungszweck vom Wohnen."@de ,
                          "Serves the utilization purpose of defining living spaces."@en ;
             rdfs:label "Residential"@en ,
                        "Wohnen"@de ;
             <http://www.w3.org/2004/02/skos/core#altLabel> "Living"@en .


:Sales rdfs:comment "Dient dem Nutzungszweck von Verkaufsräumen etc."@de ,
                    "Serves the utilization purpose of defining sales premises."@en ;
       rdfs:label "Sales"@en ,
                  "Verkauf"@de .


:SalesRoom rdfs:comment "A space within a building used to sell goods or services to customers."@en ,
                        "Ein Raum innerhalb eines Gebäudes, der dazu dient, Waren oder Dienstleistungen an Kunden zu verkaufen."@de ;
           rdfs:label "SalesRoom"@en ,
                      "VerkaufsRaum"@de .


:SceneArea rdfs:comment "Dient dem Nutzungszweck zur Definition von Szenenflächen."@de ,
                        "Serves the utilization purpose of defining scene areas."@en ;
           rdfs:label "SceneArea"@en ,
                      "Szenenflächen"@de .


:SpectatorFacility rdfs:comment "Dient dem Nutzungszweck zur Definition von Zuschaueranlagen, wie z.B. Tribünen."@de ,
                                "Serves the utilization purpose of defining spectator facilities, such as/including tribunes."@en ;
                   rdfs:label "SpectatorFacility"@en ,
                              "Zuschaueranlage"@de ;
                   <http://www.w3.org/2004/02/skos/core#altLabel> "Tribune"@en ,
                                                                  "Tribüne"@de .


:Sport rdfs:comment "Dient dem Nutzungszweck vom Typ Sport."@de ,
                    "Serves the utilization purpose of defining sport spaces/areas."@en ;
       rdfs:label "Sport"@de ,
                  "Sport"@en ;
       <http://www.w3.org/2004/02/skos/core#altLabel> "Fitness"@de ,
                                                      "Fitness"@en .


:StairSpace rdfs:comment "A vertical space within a building used to provide stairs."@en ,
                         "Ein vertikaler Raum innerhalb eines Gebäudes, der dazu dient, Treppen bereitzustellen."@de ;
            rdfs:label "StairSpace"@en ,
                       "Treppenraum"@de .


:Storage rdfs:comment "Dient dem Nutzungszweck der Lagerung."@de ,
                      "Serves the utilization purpose of defining storage areas."@en ;
         rdfs:label "Lagerung"@de ,
                    "Storage"@en .


:StoreStreet rdfs:comment "An aisle or passageway located within a building and lined with stores, stores, or retail establishments."@en ,
                          "Einen innerhalb eines Gebäudes befindlichen Gang oder eine Passage, der von Geschäften, Läden oder Verkaufseinrichtungen gesäumt ist."@de ;
             rdfs:label "Ladenstraße"@de ,
                        "StoreStreet"@en .


:Technology rdfs:comment "Dient dem Nutzungszweck zur Definition von Technikräumen."@de ,
                         "Serves the utilization purpose of defining spaces with/for technical equipment."@en ;
            rdfs:label "Technik"@de ,
                       "Technology"@en ;
            <http://www.w3.org/2004/02/skos/core#altLabel> "Utility"@en .


:Work rdfs:comment "Dient dem Nutzungszweck von Arbeitsplätzen."@de ,
                   "Serves the utilization purpose of defining places of work."@en ;
      rdfs:label "Arbeit"@de ,
                 "Work"@en .


#################################################################
#    General axioms
#################################################################

[ rdf:type owl:AllDisjointClasses ;
  owl:members ( :AccessibilityOfFireFighters
                :AreaForFireFighters
                :ConstructionalMovingArea
                :ExtinguishingWaterAccess
                :FireFighterAccessEntrance
                :FireFighterAccessPoint
                :InstallationArea
              )
] .


[ rdf:type owl:AllDisjointClasses ;
  owl:members ( :Anteroom
                :Elevator
                :FireFighterLift
                :NecessaryCorridor
                :NecessaryStairSpace
                :ResidenceSpace
                :SafetyStairSpace
                :SecurityGate
                :SpaceOfIncreasedFireRisk
                :StairSpaceExtension
              )
] .


[ rdf:type owl:AllDisjointClasses ;
  owl:members ( :Apron
                :Parapet
                :Profile
              )
] .


[ rdf:type owl:AllDisjointClasses ;
  owl:members ( :AssemblyProduct
                :Cladding
                :Closing
                :Installation
                :Insulation
                :Roof
                :Roofing
                :Slab
                :Stairs
                :StairsParts
                :SystemFlooring
                :Wall
                :WallParts
              )
] .


[ rdf:type owl:AllDisjointClasses ;
  owl:members ( :AtticSpace
                :CavitySpace
                :FireCompartment
                :SmokeCompartment
                :StructuralFacility
                :Surrounding
                :UtilizationUnit
                <https://w3id.org/bot#Site>
                <https://w3id.org/bot#Space>
                <https://w3id.org/bot#Storey>
              )
] .


[ rdf:type owl:AllDisjointClasses ;
  owl:members ( :BuildingClass1
                :BuildingClass2
                :BuildingClass3
                :BuildingClass4
                :BuildingClass5
              )
] .


[ rdf:type owl:AllDisjointClasses ;
  owl:members ( :ClientSpecification
                :GeneralInformation
                :PlanningDocument
                :RuleOfApplication
              )
] .


[ rdf:type owl:AllDisjointClasses ;
  owl:members ( :CombustionAppliance
                :Opening
                :Structure
                :SurfaceType
                :TechnicalComponent
                <https://w3id.org/bot#Element>
              )
] .


[ rdf:type owl:AllDisjointClasses ;
  owl:members ( :CompartmentWall
                :DriveShaftWall
                :ExternalWall
                :FireWall
                :WallOfANecessaryCorridor
                :WallOfANecessaryStaircase
              )
] .


[ rdf:type owl:AllDisjointClasses ;
  owl:members ( :DefensiveFireSafety
                :OrganizationalFireSafety
                :StructuralFireSafety
                :TechnicalFireSafety
              )
] .


[ rdf:type owl:AllDisjointClasses ;
  owl:members ( :Door
                :FireDamper
                :Gate
                :Glazing
                :Window
              )
] .


[ rdf:type owl:AllDisjointClasses ;
  owl:members ( :Eurocode
                :Mustervorschrift
                :Norm
              )
] .


[ rdf:type owl:AllDisjointClasses ;
  owl:members ( :Fastening
                :JointSealing
                :Posts
                :Transom
              )
] .


[ rdf:type owl:AllDisjointClasses ;
  owl:members ( :FireBrigadeLifts
                :FireControlOfLifts
                :HeatExtractionDevice
                :LightningSafetySystem
                :ObjectRadioSystemForFireBrigade
              )
] .


[ rdf:type owl:AllDisjointClasses ;
  owl:members ( :FireResistantEnclosure
                :LoadbearingEnclosingComponent
                :LoadbearingNonEnclosingComponent
                :NonLoadbearingEnclosingComponent
                :NonLoadbearingNonEnclosingComponent
                :PositionAccessibleForFireService
              )
] .


[ rdf:type owl:AllDisjointClasses ;
  owl:members ( :FireWallAsExternalWall
                :InternalFireWall
                :WallinsteadOfFireWall
              )
] .


[ rdf:type owl:AllDisjointClasses ;
  owl:members ( :MBeVO
                :MEltBauVO
                :MVKVO
                :MVStättVO
              )
] .


[ rdf:type owl:AllDisjointClasses ;
  owl:members ( :MHHR
                :MSchulbauR
                :MWR
                :M_FIBauR
              )
] .


[ rdf:type owl:AllDisjointClasses ;
  owl:members ( :SpaceUsage
                :SpecialPurposeCondition
                :StandardConstructionType
                :UtilizationPurpose
              )
] .


[ rdf:type owl:AllDisjointClasses ;
  owl:members ( <https://purl.org/fisa#DIN4102-12:1998-11>
                <https://purl.org/fisa#DIN4102-15:1990-05>
                <https://purl.org/fisa#DIN4102-17:2017-12>
                <https://purl.org/fisa#DIN4102-1:1998-05>
              )
] .


[ rdf:type owl:AllDifferent ;
  owl:distinctMembers ( :BuildingClass1a
                        :BuildingClass1b
                        :BuildingClass2
                        :BuildingClass3
                        :BuildingClass4
                        :BuildingClass5
                      )
] .


[ rdf:type owl:AllDifferent ;
  owl:distinctMembers ( :Geb01_NE01
                        :Geb02_NE01
                        :Geb02_NE02
                        :Geb03_NE01
                        :Geb03_NE02
                        :Geb03_NE03
                        :Geb04_NE01
                        :Geb04_NE02
                        :Geb05_NE01
                      )
] .


[ rdf:type owl:AllDifferent ;
  owl:distinctMembers ( :Gebäude02
                        :Gebäude03
                        :Gebäude04
                        :Gebäude05
                        :Gebäude1a
                        :Gebäude1b
                      )
] .


[ rdf:type owl:AllDifferent ;
  owl:distinctMembers ( :brennbar
                        :leichtentflammbar
                        :nichtbrennbar
                        :normalentflammbar
                        :schwerentflammbar
                      )
] .


[ rdf:type owl:AllDifferent ;
  owl:distinctMembers ( :feuerbeständig
                        :feuerhemmend
                        :hochfeuerbeständig
                        :hochfeuerhemmend
                        :höchstfeuerbeständig
                      )
] .


#################################################################
#    Rules
#################################################################

owl:b rdf:type <http://www.w3.org/2003/11/swrl#Variable> .

owl:sf rdf:type <http://www.w3.org/2003/11/swrl#Variable> .

owl:spr rdf:type <http://www.w3.org/2003/11/swrl#Variable> .

owl:gfa rdf:type <http://www.w3.org/2003/11/swrl#Variable> .

<urn:swrl:var#b> rdf:type <http://www.w3.org/2003/11/swrl#Variable> .

<urn:swrl:var#ew> rdf:type <http://www.w3.org/2003/11/swrl#Variable> .

<urn:swrl:var#st> rdf:type <http://www.w3.org/2003/11/swrl#Variable> .

<urn:swrl:var#sp> rdf:type <http://www.w3.org/2003/11/swrl#Variable> .

<urn:swrl:var#se> rdf:type <http://www.w3.org/2003/11/swrl#Variable> .

<urn:swrl:var#bc> rdf:type <http://www.w3.org/2003/11/swrl#Variable> .

<urn:swrl:var#fr> rdf:type <http://www.w3.org/2003/11/swrl#Variable> .

owl:be rdf:type <http://www.w3.org/2003/11/swrl#Variable> .

owl:se rdf:type <http://www.w3.org/2003/11/swrl#Variable> .

owl:c rdf:type <http://www.w3.org/2003/11/swrl#Variable> .

<urn:swrl:var#cp> rdf:type <http://www.w3.org/2003/11/swrl#Variable> .

<urn:swrl:var#i> rdf:type <http://www.w3.org/2003/11/swrl#Variable> .

<urn:swrl:var#fb> rdf:type <http://www.w3.org/2003/11/swrl#Variable> .

owl:h rdf:type <http://www.w3.org/2003/11/swrl#Variable> .

owl:nuu rdf:type <http://www.w3.org/2003/11/swrl#Variable> .

owl:cgfa rdf:type <http://www.w3.org/2003/11/swrl#Variable> .

owl:luu rdf:type <http://www.w3.org/2003/11/swrl#Variable> .

owl:sp rdf:type <http://www.w3.org/2003/11/swrl#Variable> .

owl:ugfa rdf:type <http://www.w3.org/2003/11/swrl#Variable> .

owl:spu rdf:type <http://www.w3.org/2003/11/swrl#Variable> .

owl:nop rdf:type <http://www.w3.org/2003/11/swrl#Variable> .

[ <http://swrl.stanford.edu/ontologies/3.3/swrla.owl#isRuleEnabled> "true"^^xsd:boolean ;
   rdfs:comment "" ;
   rdfs:label "§2 (3) 5. - Teil 3" ;
   rdf:type <http://www.w3.org/2003/11/swrl#Imp> ;
   <http://www.w3.org/2003/11/swrl#body> [ rdf:type <http://www.w3.org/2003/11/swrl#AtomList> ;
                                           rdf:first [ rdf:type <http://www.w3.org/2003/11/swrl#ClassAtom> ;
                                                       <http://www.w3.org/2003/11/swrl#classPredicate> <https://w3id.org/bot#Building> ;
                                                       <http://www.w3.org/2003/11/swrl#argument1> owl:b
                                                     ] ;
                                           rdf:rest [ rdf:type <http://www.w3.org/2003/11/swrl#AtomList> ;
                                                      rdf:first [ rdf:type <http://www.w3.org/2003/11/swrl#DatavaluedPropertyAtom> ;
                                                                  <http://www.w3.org/2003/11/swrl#propertyPredicate> :isUndergroundBuilding ;
                                                                  <http://www.w3.org/2003/11/swrl#argument1> owl:b ;
                                                                  <http://www.w3.org/2003/11/swrl#argument2> "true"^^xsd:boolean
                                                                ] ;
                                                      rdf:rest rdf:nil
                                                    ]
                                         ] ;
   <http://www.w3.org/2003/11/swrl#head> [ rdf:type <http://www.w3.org/2003/11/swrl#AtomList> ;
                                           rdf:first [ rdf:type <http://www.w3.org/2003/11/swrl#IndividualPropertyAtom> ;
                                                       <http://www.w3.org/2003/11/swrl#propertyPredicate> :hasBuildingClass ;
                                                       <http://www.w3.org/2003/11/swrl#argument1> owl:b ;
                                                       <http://www.w3.org/2003/11/swrl#argument2> :BuildingClass5
                                                     ] ;
                                           rdf:rest rdf:nil
                                         ]
 ] .

[ <http://swrl.stanford.edu/ontologies/3.3/swrla.owl#isRuleEnabled> "true"^^xsd:boolean ;
   rdfs:comment "lead to the type of Special Purpose Construction" ;
   rdfs:label "Fulfilled Special Purpose Conditions" ;
   rdf:type <http://www.w3.org/2003/11/swrl#Imp> ;
   <http://www.w3.org/2003/11/swrl#body> [ rdf:type <http://www.w3.org/2003/11/swrl#AtomList> ;
                                           rdf:first [ rdf:type <http://www.w3.org/2003/11/swrl#ClassAtom> ;
                                                       <http://www.w3.org/2003/11/swrl#classPredicate> :SpecialPurposeCondition ;
                                                       <http://www.w3.org/2003/11/swrl#argument1> owl:sf
                                                     ] ;
                                           rdf:rest [ rdf:type <http://www.w3.org/2003/11/swrl#AtomList> ;
                                                      rdf:first [ rdf:type <http://www.w3.org/2003/11/swrl#ClassAtom> ;
                                                                  <http://www.w3.org/2003/11/swrl#classPredicate> :StructuralFacility ;
                                                                  <http://www.w3.org/2003/11/swrl#argument1> owl:sf
                                                                ] ;
                                                      rdf:rest rdf:nil
                                                    ]
                                         ] ;
   <http://www.w3.org/2003/11/swrl#head> [ rdf:type <http://www.w3.org/2003/11/swrl#AtomList> ;
                                           rdf:first [ rdf:type <http://www.w3.org/2003/11/swrl#ClassAtom> ;
                                                       <http://www.w3.org/2003/11/swrl#classPredicate> :SpecialPurposeConstruction ;
                                                       <http://www.w3.org/2003/11/swrl#argument1> owl:sf
                                                     ] ;
                                           rdf:rest rdf:nil
                                         ]
 ] .

[ <http://swrl.stanford.edu/ontologies/3.3/swrla.owl#isRuleEnabled> "true"^^xsd:boolean ;
   rdfs:comment "Fassung 1995, zuletzt geändert 02/2014 - by example: when is a Sales Premises unregulated and regulated according to Special Purpose Prescriptive MVKVO" ;
   rdfs:label "§1 MVKVO #regulated" ;
   rdf:type <http://www.w3.org/2003/11/swrl#Imp> ;
   <http://www.w3.org/2003/11/swrl#body> [ rdf:type <http://www.w3.org/2003/11/swrl#AtomList> ;
                                           rdf:first [ rdf:type <http://www.w3.org/2003/11/swrl#ClassAtom> ;
                                                       <http://www.w3.org/2003/11/swrl#classPredicate> :SalesPremises ;
                                                       <http://www.w3.org/2003/11/swrl#argument1> owl:spr
                                                     ] ;
                                           rdf:rest [ rdf:type <http://www.w3.org/2003/11/swrl#AtomList> ;
                                                      rdf:first [ rdf:type <http://www.w3.org/2003/11/swrl#DatavaluedPropertyAtom> ;
                                                                  <http://www.w3.org/2003/11/swrl#propertyPredicate> :hasGFASalesSpaces ;
                                                                  <http://www.w3.org/2003/11/swrl#argument1> owl:spr ;
                                                                  <http://www.w3.org/2003/11/swrl#argument2> owl:gfa
                                                                ] ;
                                                      rdf:rest [ rdf:type <http://www.w3.org/2003/11/swrl#AtomList> ;
                                                                 rdf:first [ rdf:type <http://www.w3.org/2003/11/swrl#BuiltinAtom> ;
                                                                             <http://www.w3.org/2003/11/swrl#builtin> <http://www.w3.org/2003/11/swrlb#greaterThan> ;
                                                                             <http://www.w3.org/2003/11/swrl#arguments> [ rdf:type rdf:List ;
                                                                                                                          rdf:first owl:gfa ;
                                                                                                                          rdf:rest [ rdf:type rdf:List ;
                                                                                                                                     rdf:first 2000.0 ;
                                                                                                                                     rdf:rest rdf:nil
                                                                                                                                   ]
                                                                                                                        ]
                                                                           ] ;
                                                                 rdf:rest rdf:nil
                                                               ]
                                                    ]
                                         ] ;
   <http://www.w3.org/2003/11/swrl#head> [ rdf:type <http://www.w3.org/2003/11/swrl#AtomList> ;
                                           rdf:first [ rdf:type <http://www.w3.org/2003/11/swrl#ClassAtom> ;
                                                       <http://www.w3.org/2003/11/swrl#classPredicate> :RegulatedSpecialPurposeConstruction ;
                                                       <http://www.w3.org/2003/11/swrl#argument1> owl:spr
                                                     ] ;
                                           rdf:rest rdf:nil
                                         ]
 ] .

[ rdfs:comment "all other sub-Components of non-load-bearing external walls"@en ,
                "§28 (2) Sentence 2 - 3. - Part 3"@en ;
   rdf:type <http://www.w3.org/2003/11/swrl#Imp> ;
   <http://www.w3.org/2003/11/swrl#body> [ rdf:type <http://www.w3.org/2003/11/swrl#AtomList> ;
                                           rdf:first [ rdf:type <http://www.w3.org/2003/11/swrl#ClassAtom> ;
                                                       <http://www.w3.org/2003/11/swrl#classPredicate> <https://w3id.org/bot#Building> ;
                                                       <http://www.w3.org/2003/11/swrl#argument1> <urn:swrl:var#b>
                                                     ] ;
                                           rdf:rest [ rdf:type <http://www.w3.org/2003/11/swrl#AtomList> ;
                                                      rdf:first [ rdf:type <http://www.w3.org/2003/11/swrl#DatavaluedPropertyAtom> ;
                                                                  <http://www.w3.org/2003/11/swrl#propertyPredicate> :isSpaceEnclosing ;
                                                                  <http://www.w3.org/2003/11/swrl#argument1> <urn:swrl:var#ew> ;
                                                                  <http://www.w3.org/2003/11/swrl#argument2> "true"^^xsd:boolean
                                                                ] ;
                                                      rdf:rest [ rdf:type <http://www.w3.org/2003/11/swrl#AtomList> ;
                                                                 rdf:first [ rdf:type <http://www.w3.org/2003/11/swrl#IndividualPropertyAtom> ;
                                                                             <http://www.w3.org/2003/11/swrl#propertyPredicate> :hasFireResistance ;
                                                                             <http://www.w3.org/2003/11/swrl#argument1> <urn:swrl:var#ew> ;
                                                                             <http://www.w3.org/2003/11/swrl#argument2> :feuerhemmend
                                                                           ] ;
                                                                 rdf:rest [ rdf:type <http://www.w3.org/2003/11/swrl#AtomList> ;
                                                                            rdf:first [ rdf:type <http://www.w3.org/2003/11/swrl#IndividualPropertyAtom> ;
                                                                                        <http://www.w3.org/2003/11/swrl#propertyPredicate> <https://w3id.org/bot#hasSpace> ;
                                                                                        <http://www.w3.org/2003/11/swrl#argument1> <urn:swrl:var#st> ;
                                                                                        <http://www.w3.org/2003/11/swrl#argument2> <urn:swrl:var#sp>
                                                                                      ] ;
                                                                            rdf:rest [ rdf:type <http://www.w3.org/2003/11/swrl#AtomList> ;
                                                                                       rdf:first [ rdf:type <http://www.w3.org/2003/11/swrl#ClassAtom> ;
                                                                                                   <http://www.w3.org/2003/11/swrl#classPredicate> [ rdf:type owl:Class ;
                                                                                                                                                     owl:complementOf :Door
                                                                                                                                                   ] ;
                                                                                                   <http://www.w3.org/2003/11/swrl#argument1> <urn:swrl:var#se>
                                                                                                 ] ;
                                                                                       rdf:rest [ rdf:type <http://www.w3.org/2003/11/swrl#AtomList> ;
                                                                                                  rdf:first [ rdf:type <http://www.w3.org/2003/11/swrl#DatavaluedPropertyAtom> ;
                                                                                                              <http://www.w3.org/2003/11/swrl#propertyPredicate> :isLoadBearing ;
                                                                                                              <http://www.w3.org/2003/11/swrl#argument1> <urn:swrl:var#ew> ;
                                                                                                              <http://www.w3.org/2003/11/swrl#argument2> "false"^^xsd:boolean
                                                                                                            ] ;
                                                                                                  rdf:rest [ rdf:type <http://www.w3.org/2003/11/swrl#AtomList> ;
                                                                                                             rdf:first [ rdf:type <http://www.w3.org/2003/11/swrl#ClassAtom> ;
                                                                                                                         <http://www.w3.org/2003/11/swrl#classPredicate> :ExternalWall ;
                                                                                                                         <http://www.w3.org/2003/11/swrl#argument1> <urn:swrl:var#ew>
                                                                                                                       ] ;
                                                                                                             rdf:rest [ rdf:type <http://www.w3.org/2003/11/swrl#AtomList> ;
                                                                                                                        rdf:first [ rdf:type <http://www.w3.org/2003/11/swrl#ClassAtom> ;
                                                                                                                                    <http://www.w3.org/2003/11/swrl#classPredicate> <https://w3id.org/bot#Element> ;
                                                                                                                                    <http://www.w3.org/2003/11/swrl#argument1> <urn:swrl:var#se>
                                                                                                                                  ] ;
                                                                                                                        rdf:rest [ rdf:type <http://www.w3.org/2003/11/swrl#AtomList> ;
                                                                                                                                   rdf:first [ rdf:type <http://www.w3.org/2003/11/swrl#IndividualPropertyAtom> ;
                                                                                                                                               <http://www.w3.org/2003/11/swrl#propertyPredicate> <https://w3id.org/bot#hasElement> ;
                                                                                                                                               <http://www.w3.org/2003/11/swrl#argument1> <urn:swrl:var#sp> ;
                                                                                                                                               <http://www.w3.org/2003/11/swrl#argument2> <urn:swrl:var#ew>
                                                                                                                                             ] ;
                                                                                                                                   rdf:rest [ rdf:type <http://www.w3.org/2003/11/swrl#AtomList> ;
                                                                                                                                              rdf:first [ rdf:type <http://www.w3.org/2003/11/swrl#IndividualPropertyAtom> ;
                                                                                                                                                          <http://www.w3.org/2003/11/swrl#propertyPredicate> :hasBuildingClass ;
                                                                                                                                                          <http://www.w3.org/2003/11/swrl#argument1> <urn:swrl:var#b> ;
                                                                                                                                                          <http://www.w3.org/2003/11/swrl#argument2> <urn:swrl:var#bc>
                                                                                                                                                        ] ;
                                                                                                                                              rdf:rest [ rdf:type <http://www.w3.org/2003/11/swrl#AtomList> ;
                                                                                                                                                         rdf:first [ rdf:type <http://www.w3.org/2003/11/swrl#ClassAtom> ;
                                                                                                                                                                     <http://www.w3.org/2003/11/swrl#classPredicate> [ rdf:type owl:Class ;
                                                                                                                                                                                                                       owl:complementOf :JointSealing
                                                                                                                                                                                                                     ] ;
                                                                                                                                                                     <http://www.w3.org/2003/11/swrl#argument1> <urn:swrl:var#se>
                                                                                                                                                                   ] ;
                                                                                                                                                         rdf:rest [ rdf:type <http://www.w3.org/2003/11/swrl#AtomList> ;
                                                                                                                                                                    rdf:first [ rdf:type <http://www.w3.org/2003/11/swrl#IndividualPropertyAtom> ;
                                                                                                                                                                                <http://www.w3.org/2003/11/swrl#propertyPredicate> <https://w3id.org/bot#hasStorey> ;
                                                                                                                                                                                <http://www.w3.org/2003/11/swrl#argument1> <urn:swrl:var#b> ;
                                                                                                                                                                                <http://www.w3.org/2003/11/swrl#argument2> <urn:swrl:var#st>
                                                                                                                                                                              ] ;
                                                                                                                                                                    rdf:rest [ rdf:type <http://www.w3.org/2003/11/swrl#AtomList> ;
                                                                                                                                                                               rdf:first [ rdf:type <http://www.w3.org/2003/11/swrl#ClassAtom> ;
                                                                                                                                                                                           <http://www.w3.org/2003/11/swrl#classPredicate> [ rdf:type owl:Class ;
                                                                                                                                                                                                                                             owl:complementOf :BuildingClass1
                                                                                                                                                                                                                                           ] ;
                                                                                                                                                                                           <http://www.w3.org/2003/11/swrl#argument1> <urn:swrl:var#bc>
                                                                                                                                                                                         ] ;
                                                                                                                                                                               rdf:rest [ rdf:type <http://www.w3.org/2003/11/swrl#AtomList> ;
                                                                                                                                                                                          rdf:first [ rdf:type <http://www.w3.org/2003/11/swrl#ClassAtom> ;
                                                                                                                                                                                                      <http://www.w3.org/2003/11/swrl#classPredicate> [ rdf:type owl:Class ;
                                                                                                                                                                                                                                                        owl:complementOf :BuildingClass2
                                                                                                                                                                                                                                                      ] ;
                                                                                                                                                                                                      <http://www.w3.org/2003/11/swrl#argument1> <urn:swrl:var#bc>
                                                                                                                                                                                                    ] ;
                                                                                                                                                                                          rdf:rest [ rdf:type <http://www.w3.org/2003/11/swrl#AtomList> ;
                                                                                                                                                                                                     rdf:first [ rdf:type <http://www.w3.org/2003/11/swrl#ClassAtom> ;
                                                                                                                                                                                                                 <http://www.w3.org/2003/11/swrl#classPredicate> [ rdf:type owl:Class ;
                                                                                                                                                                                                                                                                   owl:complementOf :Window
                                                                                                                                                                                                                                                                 ] ;
                                                                                                                                                                                                                 <http://www.w3.org/2003/11/swrl#argument1> <urn:swrl:var#se>
                                                                                                                                                                                                               ] ;
                                                                                                                                                                                                     rdf:rest [ rdf:type <http://www.w3.org/2003/11/swrl#AtomList> ;
                                                                                                                                                                                                                rdf:first [ rdf:type <http://www.w3.org/2003/11/swrl#ClassAtom> ;
                                                                                                                                                                                                                            <http://www.w3.org/2003/11/swrl#classPredicate> [ rdf:type owl:Class ;
                                                                                                                                                                                                                                                                              owl:complementOf :BuildingClass3
                                                                                                                                                                                                                                                                            ] ;
                                                                                                                                                                                                                            <http://www.w3.org/2003/11/swrl#argument1> <urn:swrl:var#bc>
                                                                                                                                                                                                                          ] ;
                                                                                                                                                                                                                rdf:rest [ rdf:type <http://www.w3.org/2003/11/swrl#AtomList> ;
                                                                                                                                                                                                                           rdf:first [ rdf:type <http://www.w3.org/2003/11/swrl#ClassAtom> ;
                                                                                                                                                                                                                                       <http://www.w3.org/2003/11/swrl#classPredicate> [ rdf:type owl:Class ;
                                                                                                                                                                                                                                                                                         owl:complementOf :Insulation
                                                                                                                                                                                                                                                                                       ] ;
                                                                                                                                                                                                                                       <http://www.w3.org/2003/11/swrl#argument1> <urn:swrl:var#se>
                                                                                                                                                                                                                                     ] ;
                                                                                                                                                                                                                           rdf:rest [ rdf:type <http://www.w3.org/2003/11/swrl#AtomList> ;
                                                                                                                                                                                                                                      rdf:first [ rdf:type <http://www.w3.org/2003/11/swrl#IndividualPropertyAtom> ;
                                                                                                                                                                                                                                                  <http://www.w3.org/2003/11/swrl#propertyPredicate> <https://w3id.org/bot#hasSubElement> ;
                                                                                                                                                                                                                                                  <http://www.w3.org/2003/11/swrl#argument1> <urn:swrl:var#ew> ;
                                                                                                                                                                                                                                                  <http://www.w3.org/2003/11/swrl#argument2> <urn:swrl:var#se>
                                                                                                                                                                                                                                                ] ;
                                                                                                                                                                                                                                      rdf:rest rdf:nil
                                                                                                                                                                                                                                    ]
                                                                                                                                                                                                                         ]
                                                                                                                                                                                                              ]
                                                                                                                                                                                                   ]
                                                                                                                                                                                        ]
                                                                                                                                                                             ]
                                                                                                                                                                  ]
                                                                                                                                                       ]
                                                                                                                                            ]
                                                                                                                                 ]
                                                                                                                      ]
                                                                                                           ]
                                                                                                ]
                                                                                     ]
                                                                          ]
                                                               ]
                                                    ]
                                         ] ;
   <http://www.w3.org/2003/11/swrl#head> [ rdf:type <http://www.w3.org/2003/11/swrl#AtomList> ;
                                           rdf:first [ rdf:type <http://www.w3.org/2003/11/swrl#IndividualPropertyAtom> ;
                                                       <http://www.w3.org/2003/11/swrl#propertyPredicate> :isPermittedWithFireBehaviour ;
                                                       <http://www.w3.org/2003/11/swrl#argument1> <urn:swrl:var#se> ;
                                                       <http://www.w3.org/2003/11/swrl#argument2> :brennbar
                                                     ] ;
                                           rdf:rest rdf:nil
                                         ]
 ] .

[ rdfs:comment "§28 (2) Sentence 1 - Part 1.2"@en ;
   rdf:type <http://www.w3.org/2003/11/swrl#Imp> ;
   <http://www.w3.org/2003/11/swrl#body> [ rdf:type <http://www.w3.org/2003/11/swrl#AtomList> ;
                                           rdf:first [ rdf:type <http://www.w3.org/2003/11/swrl#ClassAtom> ;
                                                       <http://www.w3.org/2003/11/swrl#classPredicate> <https://w3id.org/bot#Building> ;
                                                       <http://www.w3.org/2003/11/swrl#argument1> <urn:swrl:var#b>
                                                     ] ;
                                           rdf:rest [ rdf:type <http://www.w3.org/2003/11/swrl#AtomList> ;
                                                      rdf:first [ rdf:type <http://www.w3.org/2003/11/swrl#DatavaluedPropertyAtom> ;
                                                                  <http://www.w3.org/2003/11/swrl#propertyPredicate> :isSpaceEnclosing ;
                                                                  <http://www.w3.org/2003/11/swrl#argument1> <urn:swrl:var#ew> ;
                                                                  <http://www.w3.org/2003/11/swrl#argument2> "true"^^xsd:boolean
                                                                ] ;
                                                      rdf:rest [ rdf:type <http://www.w3.org/2003/11/swrl#AtomList> ;
                                                                 rdf:first [ rdf:type <http://www.w3.org/2003/11/swrl#IndividualPropertyAtom> ;
                                                                             <http://www.w3.org/2003/11/swrl#propertyPredicate> <https://w3id.org/bot#hasSpace> ;
                                                                             <http://www.w3.org/2003/11/swrl#argument1> <urn:swrl:var#st> ;
                                                                             <http://www.w3.org/2003/11/swrl#argument2> <urn:swrl:var#sp>
                                                                           ] ;
                                                                 rdf:rest [ rdf:type <http://www.w3.org/2003/11/swrl#AtomList> ;
                                                                            rdf:first [ rdf:type <http://www.w3.org/2003/11/swrl#IndividualPropertyAtom> ;
                                                                                        <http://www.w3.org/2003/11/swrl#propertyPredicate> :isMoreFireResistantThan ;
                                                                                        <http://www.w3.org/2003/11/swrl#argument1> <urn:swrl:var#fr> ;
                                                                                        <http://www.w3.org/2003/11/swrl#argument2> :feuerhemmend
                                                                                      ] ;
                                                                            rdf:rest [ rdf:type <http://www.w3.org/2003/11/swrl#AtomList> ;
                                                                                       rdf:first [ rdf:type <http://www.w3.org/2003/11/swrl#DatavaluedPropertyAtom> ;
                                                                                                   <http://www.w3.org/2003/11/swrl#propertyPredicate> :isLoadBearing ;
                                                                                                   <http://www.w3.org/2003/11/swrl#argument1> <urn:swrl:var#ew> ;
                                                                                                   <http://www.w3.org/2003/11/swrl#argument2> "false"^^xsd:boolean
                                                                                                 ] ;
                                                                                       rdf:rest [ rdf:type <http://www.w3.org/2003/11/swrl#AtomList> ;
                                                                                                  rdf:first [ rdf:type <http://www.w3.org/2003/11/swrl#ClassAtom> ;
                                                                                                              <http://www.w3.org/2003/11/swrl#classPredicate> :ExternalWall ;
                                                                                                              <http://www.w3.org/2003/11/swrl#argument1> <urn:swrl:var#ew>
                                                                                                            ] ;
                                                                                                  rdf:rest [ rdf:type <http://www.w3.org/2003/11/swrl#AtomList> ;
                                                                                                             rdf:first [ rdf:type <http://www.w3.org/2003/11/swrl#IndividualPropertyAtom> ;
                                                                                                                         <http://www.w3.org/2003/11/swrl#propertyPredicate> <https://w3id.org/bot#hasElement> ;
                                                                                                                         <http://www.w3.org/2003/11/swrl#argument1> <urn:swrl:var#sp> ;
                                                                                                                         <http://www.w3.org/2003/11/swrl#argument2> <urn:swrl:var#ew>
                                                                                                                       ] ;
                                                                                                             rdf:rest [ rdf:type <http://www.w3.org/2003/11/swrl#AtomList> ;
                                                                                                                        rdf:first [ rdf:type <http://www.w3.org/2003/11/swrl#IndividualPropertyAtom> ;
                                                                                                                                    <http://www.w3.org/2003/11/swrl#propertyPredicate> :hasBuildingClass ;
                                                                                                                                    <http://www.w3.org/2003/11/swrl#argument1> <urn:swrl:var#b> ;
                                                                                                                                    <http://www.w3.org/2003/11/swrl#argument2> <urn:swrl:var#bc>
                                                                                                                                  ] ;
                                                                                                                        rdf:rest [ rdf:type <http://www.w3.org/2003/11/swrl#AtomList> ;
                                                                                                                                   rdf:first [ rdf:type <http://www.w3.org/2003/11/swrl#IndividualPropertyAtom> ;
                                                                                                                                               <http://www.w3.org/2003/11/swrl#propertyPredicate> <https://w3id.org/bot#hasStorey> ;
                                                                                                                                               <http://www.w3.org/2003/11/swrl#argument1> <urn:swrl:var#b> ;
                                                                                                                                               <http://www.w3.org/2003/11/swrl#argument2> <urn:swrl:var#st>
                                                                                                                                             ] ;
                                                                                                                                   rdf:rest [ rdf:type <http://www.w3.org/2003/11/swrl#AtomList> ;
                                                                                                                                              rdf:first [ rdf:type <http://www.w3.org/2003/11/swrl#ClassAtom> ;
                                                                                                                                                          <http://www.w3.org/2003/11/swrl#classPredicate> [ rdf:type owl:Class ;
                                                                                                                                                                                                            owl:complementOf :BuildingClass1
                                                                                                                                                                                                          ] ;
                                                                                                                                                          <http://www.w3.org/2003/11/swrl#argument1> <urn:swrl:var#bc>
                                                                                                                                                        ] ;
                                                                                                                                              rdf:rest [ rdf:type <http://www.w3.org/2003/11/swrl#AtomList> ;
                                                                                                                                                         rdf:first [ rdf:type <http://www.w3.org/2003/11/swrl#ClassAtom> ;
                                                                                                                                                                     <http://www.w3.org/2003/11/swrl#classPredicate> [ rdf:type owl:Class ;
                                                                                                                                                                                                                       owl:complementOf :BuildingClass2
                                                                                                                                                                                                                     ] ;
                                                                                                                                                                     <http://www.w3.org/2003/11/swrl#argument1> <urn:swrl:var#bc>
                                                                                                                                                                   ] ;
                                                                                                                                                         rdf:rest [ rdf:type <http://www.w3.org/2003/11/swrl#AtomList> ;
                                                                                                                                                                    rdf:first [ rdf:type <http://www.w3.org/2003/11/swrl#ClassAtom> ;
                                                                                                                                                                                <http://www.w3.org/2003/11/swrl#classPredicate> [ rdf:type owl:Class ;
                                                                                                                                                                                                                                  owl:complementOf :BuildingClass3
                                                                                                                                                                                                                                ] ;
                                                                                                                                                                                <http://www.w3.org/2003/11/swrl#argument1> <urn:swrl:var#bc>
                                                                                                                                                                              ] ;
                                                                                                                                                                    rdf:rest [ rdf:type <http://www.w3.org/2003/11/swrl#AtomList> ;
                                                                                                                                                                               rdf:first [ rdf:type <http://www.w3.org/2003/11/swrl#IndividualPropertyAtom> ;
                                                                                                                                                                                           <http://www.w3.org/2003/11/swrl#propertyPredicate> :hasFireResistance ;
                                                                                                                                                                                           <http://www.w3.org/2003/11/swrl#argument1> <urn:swrl:var#ew> ;
                                                                                                                                                                                           <http://www.w3.org/2003/11/swrl#argument2> <urn:swrl:var#fr>
                                                                                                                                                                                         ] ;
                                                                                                                                                                               rdf:rest rdf:nil
                                                                                                                                                                             ]
                                                                                                                                                                  ]
                                                                                                                                                       ]
                                                                                                                                            ]
                                                                                                                                 ]
                                                                                                                      ]
                                                                                                           ]
                                                                                                ]
                                                                                     ]
                                                                          ]
                                                               ]
                                                    ]
                                         ] ;
   <http://www.w3.org/2003/11/swrl#head> [ rdf:type <http://www.w3.org/2003/11/swrl#AtomList> ;
                                           rdf:first [ rdf:type <http://www.w3.org/2003/11/swrl#IndividualPropertyAtom> ;
                                                       <http://www.w3.org/2003/11/swrl#propertyPredicate> :isPermittedWithFireBehaviour ;
                                                       <http://www.w3.org/2003/11/swrl#argument1> <urn:swrl:var#ew> ;
                                                       <http://www.w3.org/2003/11/swrl#argument2> :brennbar
                                                     ] ;
                                           rdf:rest rdf:nil
                                         ]
 ] .

[ <http://swrl.stanford.edu/ontologies/3.3/swrla.owl#isRuleEnabled> "true"^^xsd:boolean ;
   rdfs:comment "" ;
   rdfs:label "§2 (3) 1b" ;
   rdf:type <http://www.w3.org/2003/11/swrl#Imp> ;
   <http://www.w3.org/2003/11/swrl#body> [ rdf:type <http://www.w3.org/2003/11/swrl#AtomList> ;
                                           rdf:first [ rdf:type <http://www.w3.org/2003/11/swrl#IndividualPropertyAtom> ;
                                                       <http://www.w3.org/2003/11/swrl#propertyPredicate> :hasUsage ;
                                                       <http://www.w3.org/2003/11/swrl#argument1> owl:b ;
                                                       <http://www.w3.org/2003/11/swrl#argument2> :Agriculture
                                                     ] ;
                                           rdf:rest [ rdf:type <http://www.w3.org/2003/11/swrl#AtomList> ;
                                                      rdf:first [ rdf:type <http://www.w3.org/2003/11/swrl#DatavaluedPropertyAtom> ;
                                                                  <http://www.w3.org/2003/11/swrl#propertyPredicate> :isFreestanding ;
                                                                  <http://www.w3.org/2003/11/swrl#argument1> owl:b ;
                                                                  <http://www.w3.org/2003/11/swrl#argument2> "true"^^xsd:boolean
                                                                ] ;
                                                      rdf:rest [ rdf:type <http://www.w3.org/2003/11/swrl#AtomList> ;
                                                                 rdf:first [ rdf:type <http://www.w3.org/2003/11/swrl#ClassAtom> ;
                                                                             <http://www.w3.org/2003/11/swrl#classPredicate> <https://w3id.org/bot#Building> ;
                                                                             <http://www.w3.org/2003/11/swrl#argument1> owl:b
                                                                           ] ;
                                                                 rdf:rest rdf:nil
                                                               ]
                                                    ]
                                         ] ;
   <http://www.w3.org/2003/11/swrl#head> [ rdf:type <http://www.w3.org/2003/11/swrl#AtomList> ;
                                           rdf:first [ rdf:type <http://www.w3.org/2003/11/swrl#IndividualPropertyAtom> ;
                                                       <http://www.w3.org/2003/11/swrl#propertyPredicate> :hasBuildingClass ;
                                                       <http://www.w3.org/2003/11/swrl#argument1> owl:b ;
                                                       <http://www.w3.org/2003/11/swrl#argument2> :BuildingClass1b
                                                     ] ;
                                           rdf:rest rdf:nil
                                         ]
 ] .

[ <http://swrl.stanford.edu/ontologies/3.3/swrla.owl#isRuleEnabled> "true"^^xsd:boolean ;
   rdfs:comment "" ;
   rdfs:label "(Un)fulfilled Load-Bearing" ;
   rdf:type <http://www.w3.org/2003/11/swrl#Imp> ;
   <http://www.w3.org/2003/11/swrl#body> [ rdf:type <http://www.w3.org/2003/11/swrl#AtomList> ;
                                           rdf:first [ rdf:type <http://www.w3.org/2003/11/swrl#IndividualPropertyAtom> ;
                                                       <http://www.w3.org/2003/11/swrl#propertyPredicate> <https://w3id.org/bot#hasSubElement> ;
                                                       <http://www.w3.org/2003/11/swrl#argument1> owl:be ;
                                                       <http://www.w3.org/2003/11/swrl#argument2> owl:se
                                                     ] ;
                                           rdf:rest [ rdf:type <http://www.w3.org/2003/11/swrl#AtomList> ;
                                                      rdf:first [ rdf:type <http://www.w3.org/2003/11/swrl#ClassAtom> ;
                                                                  <http://www.w3.org/2003/11/swrl#classPredicate> <https://w3id.org/bot#Element> ;
                                                                  <http://www.w3.org/2003/11/swrl#argument1> owl:be
                                                                ] ;
                                                      rdf:rest [ rdf:type <http://www.w3.org/2003/11/swrl#AtomList> ;
                                                                 rdf:first [ rdf:type <http://www.w3.org/2003/11/swrl#DatavaluedPropertyAtom> ;
                                                                             <http://www.w3.org/2003/11/swrl#propertyPredicate> :isLoadBearing ;
                                                                             <http://www.w3.org/2003/11/swrl#argument1> owl:be ;
                                                                             <http://www.w3.org/2003/11/swrl#argument2> "false"^^xsd:boolean
                                                                           ] ;
                                                                 rdf:rest rdf:nil
                                                               ]
                                                    ]
                                         ] ;
   <http://www.w3.org/2003/11/swrl#head> [ rdf:type <http://www.w3.org/2003/11/swrl#AtomList> ;
                                           rdf:first [ rdf:type <http://www.w3.org/2003/11/swrl#DatavaluedPropertyAtom> ;
                                                       <http://www.w3.org/2003/11/swrl#propertyPredicate> :isLoadBearing ;
                                                       <http://www.w3.org/2003/11/swrl#argument1> owl:se ;
                                                       <http://www.w3.org/2003/11/swrl#argument2> "false"^^xsd:boolean
                                                     ] ;
                                           rdf:rest rdf:nil
                                         ]
 ] .

[ <http://swrl.stanford.edu/ontologies/3.3/swrla.owl#isRuleEnabled> "true"^^xsd:boolean ;
   rdfs:comment "" ;
   rdfs:label "Fulfilled Space Closure" ;
   rdf:type <http://www.w3.org/2003/11/swrl#Imp> ;
   <http://www.w3.org/2003/11/swrl#body> [ rdf:type <http://www.w3.org/2003/11/swrl#AtomList> ;
                                           rdf:first [ rdf:type <http://www.w3.org/2003/11/swrl#IndividualPropertyAtom> ;
                                                       <http://www.w3.org/2003/11/swrl#propertyPredicate> <https://w3id.org/bot#hasSubElement> ;
                                                       <http://www.w3.org/2003/11/swrl#argument1> owl:c ;
                                                       <http://www.w3.org/2003/11/swrl#argument2> owl:se
                                                     ] ;
                                           rdf:rest [ rdf:type <http://www.w3.org/2003/11/swrl#AtomList> ;
                                                      rdf:first [ rdf:type <http://www.w3.org/2003/11/swrl#ClassAtom> ;
                                                                  <http://www.w3.org/2003/11/swrl#classPredicate> :Component ;
                                                                  <http://www.w3.org/2003/11/swrl#argument1> owl:c
                                                                ] ;
                                                      rdf:rest [ rdf:type <http://www.w3.org/2003/11/swrl#AtomList> ;
                                                                 rdf:first [ rdf:type <http://www.w3.org/2003/11/swrl#DatavaluedPropertyAtom> ;
                                                                             <http://www.w3.org/2003/11/swrl#propertyPredicate> :isSpaceEnclosing ;
                                                                             <http://www.w3.org/2003/11/swrl#argument1> owl:c ;
                                                                             <http://www.w3.org/2003/11/swrl#argument2> "true"^^xsd:boolean
                                                                           ] ;
                                                                 rdf:rest rdf:nil
                                                               ]
                                                    ]
                                         ] ;
   <http://www.w3.org/2003/11/swrl#head> [ rdf:type <http://www.w3.org/2003/11/swrl#AtomList> ;
                                           rdf:first [ rdf:type <http://www.w3.org/2003/11/swrl#DatavaluedPropertyAtom> ;
                                                       <http://www.w3.org/2003/11/swrl#propertyPredicate> :isSpaceEnclosing ;
                                                       <http://www.w3.org/2003/11/swrl#argument1> owl:se ;
                                                       <http://www.w3.org/2003/11/swrl#argument2> "true"^^xsd:boolean
                                                     ] ;
                                           rdf:rest rdf:nil
                                         ]
 ] .

[ rdfs:comment "all Insulations with flammable materials in closed profiles"@en ,
                "§28 (2) Sentence 2 - 3. - Part 1"@en ;
   rdf:type <http://www.w3.org/2003/11/swrl#Imp> ;
   <http://www.w3.org/2003/11/swrl#body> [ rdf:type <http://www.w3.org/2003/11/swrl#AtomList> ;
                                           rdf:first [ rdf:type <http://www.w3.org/2003/11/swrl#IndividualPropertyAtom> ;
                                                       <http://www.w3.org/2003/11/swrl#propertyPredicate> :hasFireBehaviour ;
                                                       <http://www.w3.org/2003/11/swrl#argument1> <urn:swrl:var#cp> ;
                                                       <http://www.w3.org/2003/11/swrl#argument2> :nichtbrennbar
                                                     ] ;
                                           rdf:rest [ rdf:type <http://www.w3.org/2003/11/swrl#AtomList> ;
                                                      rdf:first [ rdf:type <http://www.w3.org/2003/11/swrl#ClassAtom> ;
                                                                  <http://www.w3.org/2003/11/swrl#classPredicate> <https://w3id.org/bot#Building> ;
                                                                  <http://www.w3.org/2003/11/swrl#argument1> <urn:swrl:var#b>
                                                                ] ;
                                                      rdf:rest [ rdf:type <http://www.w3.org/2003/11/swrl#AtomList> ;
                                                                 rdf:first [ rdf:type <http://www.w3.org/2003/11/swrl#DatavaluedPropertyAtom> ;
                                                                             <http://www.w3.org/2003/11/swrl#propertyPredicate> :isSpaceEnclosing ;
                                                                             <http://www.w3.org/2003/11/swrl#argument1> <urn:swrl:var#ew> ;
                                                                             <http://www.w3.org/2003/11/swrl#argument2> "true"^^xsd:boolean
                                                                           ] ;
                                                                 rdf:rest [ rdf:type <http://www.w3.org/2003/11/swrl#AtomList> ;
                                                                            rdf:first [ rdf:type <http://www.w3.org/2003/11/swrl#IndividualPropertyAtom> ;
                                                                                        <http://www.w3.org/2003/11/swrl#propertyPredicate> :hasFireResistance ;
                                                                                        <http://www.w3.org/2003/11/swrl#argument1> <urn:swrl:var#ew> ;
                                                                                        <http://www.w3.org/2003/11/swrl#argument2> :feuerhemmend
                                                                                      ] ;
                                                                            rdf:rest [ rdf:type <http://www.w3.org/2003/11/swrl#AtomList> ;
                                                                                       rdf:first [ rdf:type <http://www.w3.org/2003/11/swrl#IndividualPropertyAtom> ;
                                                                                                   <http://www.w3.org/2003/11/swrl#propertyPredicate> <https://w3id.org/bot#hasSpace> ;
                                                                                                   <http://www.w3.org/2003/11/swrl#argument1> <urn:swrl:var#st> ;
                                                                                                   <http://www.w3.org/2003/11/swrl#argument2> <urn:swrl:var#sp>
                                                                                                 ] ;
                                                                                       rdf:rest [ rdf:type <http://www.w3.org/2003/11/swrl#AtomList> ;
                                                                                                  rdf:first [ rdf:type <http://www.w3.org/2003/11/swrl#DatavaluedPropertyAtom> ;
                                                                                                              <http://www.w3.org/2003/11/swrl#propertyPredicate> :isLoadBearing ;
                                                                                                              <http://www.w3.org/2003/11/swrl#argument1> <urn:swrl:var#ew> ;
                                                                                                              <http://www.w3.org/2003/11/swrl#argument2> "false"^^xsd:boolean
                                                                                                            ] ;
                                                                                                  rdf:rest [ rdf:type <http://www.w3.org/2003/11/swrl#AtomList> ;
                                                                                                             rdf:first [ rdf:type <http://www.w3.org/2003/11/swrl#ClassAtom> ;
                                                                                                                         <http://www.w3.org/2003/11/swrl#classPredicate> :ExternalWall ;
                                                                                                                         <http://www.w3.org/2003/11/swrl#argument1> <urn:swrl:var#ew>
                                                                                                                       ] ;
                                                                                                             rdf:rest [ rdf:type <http://www.w3.org/2003/11/swrl#AtomList> ;
                                                                                                                        rdf:first [ rdf:type <http://www.w3.org/2003/11/swrl#IndividualPropertyAtom> ;
                                                                                                                                    <http://www.w3.org/2003/11/swrl#propertyPredicate> :hasFireBehaviour ;
                                                                                                                                    <http://www.w3.org/2003/11/swrl#argument1> <urn:swrl:var#i> ;
                                                                                                                                    <http://www.w3.org/2003/11/swrl#argument2> :brennbar
                                                                                                                                  ] ;
                                                                                                                        rdf:rest [ rdf:type <http://www.w3.org/2003/11/swrl#AtomList> ;
                                                                                                                                   rdf:first [ rdf:type <http://www.w3.org/2003/11/swrl#IndividualPropertyAtom> ;
                                                                                                                                               <http://www.w3.org/2003/11/swrl#propertyPredicate> :isSubElementOf ;
                                                                                                                                               <http://www.w3.org/2003/11/swrl#argument1> <urn:swrl:var#cp> ;
                                                                                                                                               <http://www.w3.org/2003/11/swrl#argument2> <urn:swrl:var#ew>
                                                                                                                                             ] ;
                                                                                                                                   rdf:rest [ rdf:type <http://www.w3.org/2003/11/swrl#AtomList> ;
                                                                                                                                              rdf:first [ rdf:type <http://www.w3.org/2003/11/swrl#IndividualPropertyAtom> ;
                                                                                                                                                          <http://www.w3.org/2003/11/swrl#propertyPredicate> <https://w3id.org/bot#hasElement> ;
                                                                                                                                                          <http://www.w3.org/2003/11/swrl#argument1> <urn:swrl:var#sp> ;
                                                                                                                                                          <http://www.w3.org/2003/11/swrl#argument2> <urn:swrl:var#ew>
                                                                                                                                                        ] ;
                                                                                                                                              rdf:rest [ rdf:type <http://www.w3.org/2003/11/swrl#AtomList> ;
                                                                                                                                                         rdf:first [ rdf:type <http://www.w3.org/2003/11/swrl#ClassAtom> ;
                                                                                                                                                                     <http://www.w3.org/2003/11/swrl#classPredicate> :Insulation ;
                                                                                                                                                                     <http://www.w3.org/2003/11/swrl#argument1> <urn:swrl:var#i>
                                                                                                                                                                   ] ;
                                                                                                                                                         rdf:rest [ rdf:type <http://www.w3.org/2003/11/swrl#AtomList> ;
                                                                                                                                                                    rdf:first [ rdf:type <http://www.w3.org/2003/11/swrl#IndividualPropertyAtom> ;
                                                                                                                                                                                <http://www.w3.org/2003/11/swrl#propertyPredicate> :hasBuildingClass ;
                                                                                                                                                                                <http://www.w3.org/2003/11/swrl#argument1> <urn:swrl:var#b> ;
                                                                                                                                                                                <http://www.w3.org/2003/11/swrl#argument2> <urn:swrl:var#bc>
                                                                                                                                                                              ] ;
                                                                                                                                                                    rdf:rest [ rdf:type <http://www.w3.org/2003/11/swrl#AtomList> ;
                                                                                                                                                                               rdf:first [ rdf:type <http://www.w3.org/2003/11/swrl#IndividualPropertyAtom> ;
                                                                                                                                                                                           <http://www.w3.org/2003/11/swrl#propertyPredicate> <https://w3id.org/bot#hasStorey> ;
                                                                                                                                                                                           <http://www.w3.org/2003/11/swrl#argument1> <urn:swrl:var#b> ;
                                                                                                                                                                                           <http://www.w3.org/2003/11/swrl#argument2> <urn:swrl:var#st>
                                                                                                                                                                                         ] ;
                                                                                                                                                                               rdf:rest [ rdf:type <http://www.w3.org/2003/11/swrl#AtomList> ;
                                                                                                                                                                                          rdf:first [ rdf:type <http://www.w3.org/2003/11/swrl#ClassAtom> ;
                                                                                                                                                                                                      <http://www.w3.org/2003/11/swrl#classPredicate> [ rdf:type owl:Class ;
                                                                                                                                                                                                                                                        owl:complementOf :BuildingClass1
                                                                                                                                                                                                                                                      ] ;
                                                                                                                                                                                                      <http://www.w3.org/2003/11/swrl#argument1> <urn:swrl:var#bc>
                                                                                                                                                                                                    ] ;
                                                                                                                                                                                          rdf:rest [ rdf:type <http://www.w3.org/2003/11/swrl#AtomList> ;
                                                                                                                                                                                                     rdf:first [ rdf:type <http://www.w3.org/2003/11/swrl#ClassAtom> ;
                                                                                                                                                                                                                 <http://www.w3.org/2003/11/swrl#classPredicate> [ rdf:type owl:Class ;
                                                                                                                                                                                                                                                                   owl:complementOf :BuildingClass2
                                                                                                                                                                                                                                                                 ] ;
                                                                                                                                                                                                                 <http://www.w3.org/2003/11/swrl#argument1> <urn:swrl:var#bc>
                                                                                                                                                                                                               ] ;
                                                                                                                                                                                                     rdf:rest [ rdf:type <http://www.w3.org/2003/11/swrl#AtomList> ;
                                                                                                                                                                                                                rdf:first [ rdf:type <http://www.w3.org/2003/11/swrl#ClassAtom> ;
                                                                                                                                                                                                                            <http://www.w3.org/2003/11/swrl#classPredicate> [ rdf:type owl:Class ;
                                                                                                                                                                                                                                                                              owl:complementOf :BuildingClass3
                                                                                                                                                                                                                                                                            ] ;
                                                                                                                                                                                                                            <http://www.w3.org/2003/11/swrl#argument1> <urn:swrl:var#bc>
                                                                                                                                                                                                                          ] ;
                                                                                                                                                                                                                rdf:rest [ rdf:type <http://www.w3.org/2003/11/swrl#AtomList> ;
                                                                                                                                                                                                                           rdf:first [ rdf:type <http://www.w3.org/2003/11/swrl#ClassAtom> ;
                                                                                                                                                                                                                                       <http://www.w3.org/2003/11/swrl#classPredicate> :ClosedProfile ;
                                                                                                                                                                                                                                       <http://www.w3.org/2003/11/swrl#argument1> <urn:swrl:var#cp>
                                                                                                                                                                                                                                     ] ;
                                                                                                                                                                                                                           rdf:rest [ rdf:type <http://www.w3.org/2003/11/swrl#AtomList> ;
                                                                                                                                                                                                                                      rdf:first [ rdf:type <http://www.w3.org/2003/11/swrl#IndividualPropertyAtom> ;
                                                                                                                                                                                                                                                  <http://www.w3.org/2003/11/swrl#propertyPredicate> <https://w3id.org/bot#hasSubElement> ;
                                                                                                                                                                                                                                                  <http://www.w3.org/2003/11/swrl#argument1> <urn:swrl:var#ew> ;
                                                                                                                                                                                                                                                  <http://www.w3.org/2003/11/swrl#argument2> <urn:swrl:var#se>
                                                                                                                                                                                                                                                ] ;
                                                                                                                                                                                                                                      rdf:rest [ rdf:type <http://www.w3.org/2003/11/swrl#AtomList> ;
                                                                                                                                                                                                                                                 rdf:first [ rdf:type <http://www.w3.org/2003/11/swrl#IndividualPropertyAtom> ;
                                                                                                                                                                                                                                                             <http://www.w3.org/2003/11/swrl#propertyPredicate> <https://w3id.org/bot#containsElement> ;
                                                                                                                                                                                                                                                             <http://www.w3.org/2003/11/swrl#argument1> <urn:swrl:var#cp> ;
                                                                                                                                                                                                                                                             <http://www.w3.org/2003/11/swrl#argument2> <urn:swrl:var#i>
                                                                                                                                                                                                                                                           ] ;
                                                                                                                                                                                                                                                 rdf:rest rdf:nil
                                                                                                                                                                                                                                               ]
                                                                                                                                                                                                                                    ]
                                                                                                                                                                                                                         ]
                                                                                                                                                                                                              ]
                                                                                                                                                                                                   ]
                                                                                                                                                                                        ]
                                                                                                                                                                             ]
                                                                                                                                                                  ]
                                                                                                                                                       ]
                                                                                                                                            ]
                                                                                                                                 ]
                                                                                                                      ]
                                                                                                           ]
                                                                                                ]
                                                                                     ]
                                                                          ]
                                                               ]
                                                    ]
                                         ] ;
   <http://www.w3.org/2003/11/swrl#head> [ rdf:type <http://www.w3.org/2003/11/swrl#AtomList> ;
                                           rdf:first [ rdf:type <http://www.w3.org/2003/11/swrl#DatavaluedPropertyAtom> ;
                                                       <http://www.w3.org/2003/11/swrl#propertyPredicate> :hasDescription ;
                                                       <http://www.w3.org/2003/11/swrl#argument1> <urn:swrl:var#i> ;
                                                       <http://www.w3.org/2003/11/swrl#argument2> "§28 (2) won't apply here."
                                                     ] ;
                                           rdf:rest rdf:nil
                                         ]
 ] .

[ rdfs:comment "all Insulations with other than flammable materials in closed profiles"@en ,
                "§28 (2) Sentence 2 - 3. - Part 2"@en ;
   rdf:type <http://www.w3.org/2003/11/swrl#Imp> ;
   <http://www.w3.org/2003/11/swrl#body> [ rdf:type <http://www.w3.org/2003/11/swrl#AtomList> ;
                                           rdf:first [ rdf:type <http://www.w3.org/2003/11/swrl#IndividualPropertyAtom> ;
                                                       <http://www.w3.org/2003/11/swrl#propertyPredicate> :hasFireBehaviour ;
                                                       <http://www.w3.org/2003/11/swrl#argument1> <urn:swrl:var#cp> ;
                                                       <http://www.w3.org/2003/11/swrl#argument2> :nichtbrennbar
                                                     ] ;
                                           rdf:rest [ rdf:type <http://www.w3.org/2003/11/swrl#AtomList> ;
                                                      rdf:first [ rdf:type <http://www.w3.org/2003/11/swrl#ClassAtom> ;
                                                                  <http://www.w3.org/2003/11/swrl#classPredicate> <https://w3id.org/bot#Building> ;
                                                                  <http://www.w3.org/2003/11/swrl#argument1> <urn:swrl:var#b>
                                                                ] ;
                                                      rdf:rest [ rdf:type <http://www.w3.org/2003/11/swrl#AtomList> ;
                                                                 rdf:first [ rdf:type <http://www.w3.org/2003/11/swrl#DatavaluedPropertyAtom> ;
                                                                             <http://www.w3.org/2003/11/swrl#propertyPredicate> :isSpaceEnclosing ;
                                                                             <http://www.w3.org/2003/11/swrl#argument1> <urn:swrl:var#ew> ;
                                                                             <http://www.w3.org/2003/11/swrl#argument2> "true"^^xsd:boolean
                                                                           ] ;
                                                                 rdf:rest [ rdf:type <http://www.w3.org/2003/11/swrl#AtomList> ;
                                                                            rdf:first [ rdf:type <http://www.w3.org/2003/11/swrl#DifferentIndividualsAtom> ;
                                                                                        <http://www.w3.org/2003/11/swrl#argument1> <urn:swrl:var#fb> ;
                                                                                        <http://www.w3.org/2003/11/swrl#argument2> :brennbar
                                                                                      ] ;
                                                                            rdf:rest [ rdf:type <http://www.w3.org/2003/11/swrl#AtomList> ;
                                                                                       rdf:first [ rdf:type <http://www.w3.org/2003/11/swrl#IndividualPropertyAtom> ;
                                                                                                   <http://www.w3.org/2003/11/swrl#propertyPredicate> :hasFireResistance ;
                                                                                                   <http://www.w3.org/2003/11/swrl#argument1> <urn:swrl:var#ew> ;
                                                                                                   <http://www.w3.org/2003/11/swrl#argument2> :feuerhemmend
                                                                                                 ] ;
                                                                                       rdf:rest [ rdf:type <http://www.w3.org/2003/11/swrl#AtomList> ;
                                                                                                  rdf:first [ rdf:type <http://www.w3.org/2003/11/swrl#IndividualPropertyAtom> ;
                                                                                                              <http://www.w3.org/2003/11/swrl#propertyPredicate> <https://w3id.org/bot#hasSpace> ;
                                                                                                              <http://www.w3.org/2003/11/swrl#argument1> <urn:swrl:var#st> ;
                                                                                                              <http://www.w3.org/2003/11/swrl#argument2> <urn:swrl:var#sp>
                                                                                                            ] ;
                                                                                                  rdf:rest [ rdf:type <http://www.w3.org/2003/11/swrl#AtomList> ;
                                                                                                             rdf:first [ rdf:type <http://www.w3.org/2003/11/swrl#DatavaluedPropertyAtom> ;
                                                                                                                         <http://www.w3.org/2003/11/swrl#propertyPredicate> :isLoadBearing ;
                                                                                                                         <http://www.w3.org/2003/11/swrl#argument1> <urn:swrl:var#ew> ;
                                                                                                                         <http://www.w3.org/2003/11/swrl#argument2> "false"^^xsd:boolean
                                                                                                                       ] ;
                                                                                                             rdf:rest [ rdf:type <http://www.w3.org/2003/11/swrl#AtomList> ;
                                                                                                                        rdf:first [ rdf:type <http://www.w3.org/2003/11/swrl#IndividualPropertyAtom> ;
                                                                                                                                    <http://www.w3.org/2003/11/swrl#propertyPredicate> :hasFireBehaviour ;
                                                                                                                                    <http://www.w3.org/2003/11/swrl#argument1> <urn:swrl:var#i> ;
                                                                                                                                    <http://www.w3.org/2003/11/swrl#argument2> <urn:swrl:var#fb>
                                                                                                                                  ] ;
                                                                                                                        rdf:rest [ rdf:type <http://www.w3.org/2003/11/swrl#AtomList> ;
                                                                                                                                   rdf:first [ rdf:type <http://www.w3.org/2003/11/swrl#ClassAtom> ;
                                                                                                                                               <http://www.w3.org/2003/11/swrl#classPredicate> :ExternalWall ;
                                                                                                                                               <http://www.w3.org/2003/11/swrl#argument1> <urn:swrl:var#ew>
                                                                                                                                             ] ;
                                                                                                                                   rdf:rest [ rdf:type <http://www.w3.org/2003/11/swrl#AtomList> ;
                                                                                                                                              rdf:first [ rdf:type <http://www.w3.org/2003/11/swrl#IndividualPropertyAtom> ;
                                                                                                                                                          <http://www.w3.org/2003/11/swrl#propertyPredicate> :isSubElementOf ;
                                                                                                                                                          <http://www.w3.org/2003/11/swrl#argument1> <urn:swrl:var#cp> ;
                                                                                                                                                          <http://www.w3.org/2003/11/swrl#argument2> <urn:swrl:var#ew>
                                                                                                                                                        ] ;
                                                                                                                                              rdf:rest [ rdf:type <http://www.w3.org/2003/11/swrl#AtomList> ;
                                                                                                                                                         rdf:first [ rdf:type <http://www.w3.org/2003/11/swrl#IndividualPropertyAtom> ;
                                                                                                                                                                     <http://www.w3.org/2003/11/swrl#propertyPredicate> <https://w3id.org/bot#hasElement> ;
                                                                                                                                                                     <http://www.w3.org/2003/11/swrl#argument1> <urn:swrl:var#sp> ;
                                                                                                                                                                     <http://www.w3.org/2003/11/swrl#argument2> <urn:swrl:var#ew>
                                                                                                                                                                   ] ;
                                                                                                                                                         rdf:rest [ rdf:type <http://www.w3.org/2003/11/swrl#AtomList> ;
                                                                                                                                                                    rdf:first [ rdf:type <http://www.w3.org/2003/11/swrl#ClassAtom> ;
                                                                                                                                                                                <http://www.w3.org/2003/11/swrl#classPredicate> :Insulation ;
                                                                                                                                                                                <http://www.w3.org/2003/11/swrl#argument1> <urn:swrl:var#i>
                                                                                                                                                                              ] ;
                                                                                                                                                                    rdf:rest [ rdf:type <http://www.w3.org/2003/11/swrl#AtomList> ;
                                                                                                                                                                               rdf:first [ rdf:type <http://www.w3.org/2003/11/swrl#IndividualPropertyAtom> ;
                                                                                                                                                                                           <http://www.w3.org/2003/11/swrl#propertyPredicate> :hasBuildingClass ;
                                                                                                                                                                                           <http://www.w3.org/2003/11/swrl#argument1> <urn:swrl:var#b> ;
                                                                                                                                                                                           <http://www.w3.org/2003/11/swrl#argument2> <urn:swrl:var#bc>
                                                                                                                                                                                         ] ;
                                                                                                                                                                               rdf:rest [ rdf:type <http://www.w3.org/2003/11/swrl#AtomList> ;
                                                                                                                                                                                          rdf:first [ rdf:type <http://www.w3.org/2003/11/swrl#IndividualPropertyAtom> ;
                                                                                                                                                                                                      <http://www.w3.org/2003/11/swrl#propertyPredicate> <https://w3id.org/bot#hasStorey> ;
                                                                                                                                                                                                      <http://www.w3.org/2003/11/swrl#argument1> <urn:swrl:var#b> ;
                                                                                                                                                                                                      <http://www.w3.org/2003/11/swrl#argument2> <urn:swrl:var#st>
                                                                                                                                                                                                    ] ;
                                                                                                                                                                                          rdf:rest [ rdf:type <http://www.w3.org/2003/11/swrl#AtomList> ;
                                                                                                                                                                                                     rdf:first [ rdf:type <http://www.w3.org/2003/11/swrl#ClassAtom> ;
                                                                                                                                                                                                                 <http://www.w3.org/2003/11/swrl#classPredicate> [ rdf:type owl:Class ;
                                                                                                                                                                                                                                                                   owl:complementOf :BuildingClass1
                                                                                                                                                                                                                                                                 ] ;
                                                                                                                                                                                                                 <http://www.w3.org/2003/11/swrl#argument1> <urn:swrl:var#bc>
                                                                                                                                                                                                               ] ;
                                                                                                                                                                                                     rdf:rest [ rdf:type <http://www.w3.org/2003/11/swrl#AtomList> ;
                                                                                                                                                                                                                rdf:first [ rdf:type <http://www.w3.org/2003/11/swrl#ClassAtom> ;
                                                                                                                                                                                                                            <http://www.w3.org/2003/11/swrl#classPredicate> [ rdf:type owl:Class ;
                                                                                                                                                                                                                                                                              owl:complementOf :BuildingClass2
                                                                                                                                                                                                                                                                            ] ;
                                                                                                                                                                                                                            <http://www.w3.org/2003/11/swrl#argument1> <urn:swrl:var#bc>
                                                                                                                                                                                                                          ] ;
                                                                                                                                                                                                                rdf:rest [ rdf:type <http://www.w3.org/2003/11/swrl#AtomList> ;
                                                                                                                                                                                                                           rdf:first [ rdf:type <http://www.w3.org/2003/11/swrl#ClassAtom> ;
                                                                                                                                                                                                                                       <http://www.w3.org/2003/11/swrl#classPredicate> [ rdf:type owl:Class ;
                                                                                                                                                                                                                                                                                         owl:complementOf :BuildingClass3
                                                                                                                                                                                                                                                                                       ] ;
                                                                                                                                                                                                                                       <http://www.w3.org/2003/11/swrl#argument1> <urn:swrl:var#bc>
                                                                                                                                                                                                                                     ] ;
                                                                                                                                                                                                                           rdf:rest [ rdf:type <http://www.w3.org/2003/11/swrl#AtomList> ;
                                                                                                                                                                                                                                      rdf:first [ rdf:type <http://www.w3.org/2003/11/swrl#ClassAtom> ;
                                                                                                                                                                                                                                                  <http://www.w3.org/2003/11/swrl#classPredicate> :ClosedProfile ;
                                                                                                                                                                                                                                                  <http://www.w3.org/2003/11/swrl#argument1> <urn:swrl:var#cp>
                                                                                                                                                                                                                                                ] ;
                                                                                                                                                                                                                                      rdf:rest [ rdf:type <http://www.w3.org/2003/11/swrl#AtomList> ;
                                                                                                                                                                                                                                                 rdf:first [ rdf:type <http://www.w3.org/2003/11/swrl#IndividualPropertyAtom> ;
                                                                                                                                                                                                                                                             <http://www.w3.org/2003/11/swrl#propertyPredicate> <https://w3id.org/bot#hasSubElement> ;
                                                                                                                                                                                                                                                             <http://www.w3.org/2003/11/swrl#argument1> <urn:swrl:var#ew> ;
                                                                                                                                                                                                                                                             <http://www.w3.org/2003/11/swrl#argument2> <urn:swrl:var#se>
                                                                                                                                                                                                                                                           ] ;
                                                                                                                                                                                                                                                 rdf:rest [ rdf:type <http://www.w3.org/2003/11/swrl#AtomList> ;
                                                                                                                                                                                                                                                            rdf:first [ rdf:type <http://www.w3.org/2003/11/swrl#IndividualPropertyAtom> ;
                                                                                                                                                                                                                                                                        <http://www.w3.org/2003/11/swrl#propertyPredicate> <https://w3id.org/bot#containsElement> ;
                                                                                                                                                                                                                                                                        <http://www.w3.org/2003/11/swrl#argument1> <urn:swrl:var#cp> ;
                                                                                                                                                                                                                                                                        <http://www.w3.org/2003/11/swrl#argument2> <urn:swrl:var#i>
                                                                                                                                                                                                                                                                      ] ;
                                                                                                                                                                                                                                                            rdf:rest rdf:nil
                                                                                                                                                                                                                                                          ]
                                                                                                                                                                                                                                               ]
                                                                                                                                                                                                                                    ]
                                                                                                                                                                                                                         ]
                                                                                                                                                                                                              ]
                                                                                                                                                                                                   ]
                                                                                                                                                                                        ]
                                                                                                                                                                             ]
                                                                                                                                                                  ]
                                                                                                                                                       ]
                                                                                                                                            ]
                                                                                                                                 ]
                                                                                                                      ]
                                                                                                           ]
                                                                                                ]
                                                                                     ]
                                                                          ]
                                                               ]
                                                    ]
                                         ] ;
   <http://www.w3.org/2003/11/swrl#head> [ rdf:type <http://www.w3.org/2003/11/swrl#AtomList> ;
                                           rdf:first [ rdf:type <http://www.w3.org/2003/11/swrl#DatavaluedPropertyAtom> ;
                                                       <http://www.w3.org/2003/11/swrl#propertyPredicate> :hasDescription ;
                                                       <http://www.w3.org/2003/11/swrl#argument1> <urn:swrl:var#i> ;
                                                       <http://www.w3.org/2003/11/swrl#argument2> "§28 (2) applies here."
                                                     ] ;
                                           rdf:rest [ rdf:type <http://www.w3.org/2003/11/swrl#AtomList> ;
                                                      rdf:first [ rdf:type <http://www.w3.org/2003/11/swrl#IndividualPropertyAtom> ;
                                                                  <http://www.w3.org/2003/11/swrl#propertyPredicate> :isPermittedWithFireBehaviour ;
                                                                  <http://www.w3.org/2003/11/swrl#argument1> <urn:swrl:var#i> ;
                                                                  <http://www.w3.org/2003/11/swrl#argument2> :brennbar
                                                                ] ;
                                                      rdf:rest rdf:nil
                                                    ]
                                         ]
 ] .

[ <http://swrl.stanford.edu/ontologies/3.3/swrla.owl#isRuleEnabled> "true"^^xsd:boolean ;
   rdfs:comment "" ;
   rdfs:label "§2 (3) 5. - Teil 1" ;
   rdf:type <http://www.w3.org/2003/11/swrl#Imp> ;
   <http://www.w3.org/2003/11/swrl#body> [ rdf:type <http://www.w3.org/2003/11/swrl#AtomList> ;
                                           rdf:first [ rdf:type <http://www.w3.org/2003/11/swrl#DatavaluedPropertyAtom> ;
                                                       <http://www.w3.org/2003/11/swrl#propertyPredicate> :hasAverageHeight ;
                                                       <http://www.w3.org/2003/11/swrl#argument1> owl:b ;
                                                       <http://www.w3.org/2003/11/swrl#argument2> owl:h
                                                     ] ;
                                           rdf:rest [ rdf:type <http://www.w3.org/2003/11/swrl#AtomList> ;
                                                      rdf:first [ rdf:type <http://www.w3.org/2003/11/swrl#ClassAtom> ;
                                                                  <http://www.w3.org/2003/11/swrl#classPredicate> <https://w3id.org/bot#Building> ;
                                                                  <http://www.w3.org/2003/11/swrl#argument1> owl:b
                                                                ] ;
                                                      rdf:rest [ rdf:type <http://www.w3.org/2003/11/swrl#AtomList> ;
                                                                 rdf:first [ rdf:type <http://www.w3.org/2003/11/swrl#DatavaluedPropertyAtom> ;
                                                                             <http://www.w3.org/2003/11/swrl#propertyPredicate> :under400_meta ;
                                                                             <http://www.w3.org/2003/11/swrl#argument1> owl:b ;
                                                                             <http://www.w3.org/2003/11/swrl#argument2> "false"^^xsd:boolean
                                                                           ] ;
                                                                 rdf:rest [ rdf:type <http://www.w3.org/2003/11/swrl#AtomList> ;
                                                                            rdf:first [ rdf:type <http://www.w3.org/2003/11/swrl#BuiltinAtom> ;
                                                                                        <http://www.w3.org/2003/11/swrl#builtin> <http://www.w3.org/2003/11/swrlb#greaterThan> ;
                                                                                        <http://www.w3.org/2003/11/swrl#arguments> [ rdf:type rdf:List ;
                                                                                                                                     rdf:first owl:h ;
                                                                                                                                     rdf:rest [ rdf:type rdf:List ;
                                                                                                                                                rdf:first 7 ;
                                                                                                                                                rdf:rest rdf:nil
                                                                                                                                              ]
                                                                                                                                   ]
                                                                                      ] ;
                                                                            rdf:rest rdf:nil
                                                                          ]
                                                               ]
                                                    ]
                                         ] ;
   <http://www.w3.org/2003/11/swrl#head> [ rdf:type <http://www.w3.org/2003/11/swrl#AtomList> ;
                                           rdf:first [ rdf:type <http://www.w3.org/2003/11/swrl#IndividualPropertyAtom> ;
                                                       <http://www.w3.org/2003/11/swrl#propertyPredicate> :hasBuildingClass ;
                                                       <http://www.w3.org/2003/11/swrl#argument1> owl:b ;
                                                       <http://www.w3.org/2003/11/swrl#argument2> :BuildingClass5
                                                     ] ;
                                           rdf:rest rdf:nil
                                         ]
 ] .

[ <http://swrl.stanford.edu/ontologies/3.3/swrla.owl#isRuleEnabled> "true"^^xsd:boolean ;
   rdfs:comment "" ;
   rdfs:label "§2 (3) 4 - Part 1" ;
   rdf:type <http://www.w3.org/2003/11/swrl#Imp> ;
   <http://www.w3.org/2003/11/swrl#body> [ rdf:type <http://www.w3.org/2003/11/swrl#AtomList> ;
                                           rdf:first [ rdf:type <http://www.w3.org/2003/11/swrl#DatavaluedPropertyAtom> ;
                                                       <http://www.w3.org/2003/11/swrl#propertyPredicate> :hasAverageHeight ;
                                                       <http://www.w3.org/2003/11/swrl#argument1> owl:b ;
                                                       <http://www.w3.org/2003/11/swrl#argument2> owl:h
                                                     ] ;
                                           rdf:rest [ rdf:type <http://www.w3.org/2003/11/swrl#AtomList> ;
                                                      rdf:first [ rdf:type <http://www.w3.org/2003/11/swrl#ClassAtom> ;
                                                                  <http://www.w3.org/2003/11/swrl#classPredicate> <https://w3id.org/bot#Building> ;
                                                                  <http://www.w3.org/2003/11/swrl#argument1> owl:b
                                                                ] ;
                                                      rdf:rest [ rdf:type <http://www.w3.org/2003/11/swrl#AtomList> ;
                                                                 rdf:first [ rdf:type <http://www.w3.org/2003/11/swrl#BuiltinAtom> ;
                                                                             <http://www.w3.org/2003/11/swrl#builtin> <http://www.w3.org/2003/11/swrlb#lessThanOrEqual> ;
                                                                             <http://www.w3.org/2003/11/swrl#arguments> [ rdf:type rdf:List ;
                                                                                                                          rdf:first owl:h ;
                                                                                                                          rdf:rest [ rdf:type rdf:List ;
                                                                                                                                     rdf:first 13.0 ;
                                                                                                                                     rdf:rest rdf:nil
                                                                                                                                   ]
                                                                                                                        ]
                                                                           ] ;
                                                                 rdf:rest [ rdf:type <http://www.w3.org/2003/11/swrl#AtomList> ;
                                                                            rdf:first [ rdf:type <http://www.w3.org/2003/11/swrl#DatavaluedPropertyAtom> ;
                                                                                        <http://www.w3.org/2003/11/swrl#propertyPredicate> :under400_meta ;
                                                                                        <http://www.w3.org/2003/11/swrl#argument1> owl:b ;
                                                                                        <http://www.w3.org/2003/11/swrl#argument2> "true"^^xsd:boolean
                                                                                      ] ;
                                                                            rdf:rest [ rdf:type <http://www.w3.org/2003/11/swrl#AtomList> ;
                                                                                       rdf:first [ rdf:type <http://www.w3.org/2003/11/swrl#BuiltinAtom> ;
                                                                                                   <http://www.w3.org/2003/11/swrl#builtin> <http://www.w3.org/2003/11/swrlb#greaterThan> ;
                                                                                                   <http://www.w3.org/2003/11/swrl#arguments> [ rdf:type rdf:List ;
                                                                                                                                                rdf:first owl:h ;
                                                                                                                                                rdf:rest [ rdf:type rdf:List ;
                                                                                                                                                           rdf:first 7.0 ;
                                                                                                                                                           rdf:rest rdf:nil
                                                                                                                                                         ]
                                                                                                                                              ]
                                                                                                 ] ;
                                                                                       rdf:rest rdf:nil
                                                                                     ]
                                                                          ]
                                                               ]
                                                    ]
                                         ] ;
   <http://www.w3.org/2003/11/swrl#head> [ rdf:type <http://www.w3.org/2003/11/swrl#AtomList> ;
                                           rdf:first [ rdf:type <http://www.w3.org/2003/11/swrl#IndividualPropertyAtom> ;
                                                       <http://www.w3.org/2003/11/swrl#propertyPredicate> :hasBuildingClass ;
                                                       <http://www.w3.org/2003/11/swrl#argument1> owl:b ;
                                                       <http://www.w3.org/2003/11/swrl#argument2> :BuildingClass4
                                                     ] ;
                                           rdf:rest rdf:nil
                                         ]
 ] .

[ <http://swrl.stanford.edu/ontologies/3.3/swrla.owl#isRuleEnabled> "true"^^xsd:boolean ;
   rdfs:comment "" ;
   rdfs:label "§2 (3) 3. - Teil 2" ;
   rdf:type <http://www.w3.org/2003/11/swrl#Imp> ;
   <http://www.w3.org/2003/11/swrl#body> [ rdf:type <http://www.w3.org/2003/11/swrl#AtomList> ;
                                           rdf:first [ rdf:type <http://www.w3.org/2003/11/swrl#DatavaluedPropertyAtom> ;
                                                       <http://www.w3.org/2003/11/swrl#propertyPredicate> :hasAverageHeight ;
                                                       <http://www.w3.org/2003/11/swrl#argument1> owl:b ;
                                                       <http://www.w3.org/2003/11/swrl#argument2> owl:h
                                                     ] ;
                                           rdf:rest [ rdf:type <http://www.w3.org/2003/11/swrl#AtomList> ;
                                                      rdf:first [ rdf:type <http://www.w3.org/2003/11/swrl#ClassAtom> ;
                                                                  <http://www.w3.org/2003/11/swrl#classPredicate> <https://w3id.org/bot#Building> ;
                                                                  <http://www.w3.org/2003/11/swrl#argument1> owl:b
                                                                ] ;
                                                      rdf:rest [ rdf:type <http://www.w3.org/2003/11/swrl#AtomList> ;
                                                                 rdf:first [ rdf:type <http://www.w3.org/2003/11/swrl#BuiltinAtom> ;
                                                                             <http://www.w3.org/2003/11/swrl#builtin> <http://www.w3.org/2003/11/swrlb#lessThanOrEqual> ;
                                                                             <http://www.w3.org/2003/11/swrl#arguments> [ rdf:type rdf:List ;
                                                                                                                          rdf:first owl:h ;
                                                                                                                          rdf:rest [ rdf:type rdf:List ;
                                                                                                                                     rdf:first 7.0 ;
                                                                                                                                     rdf:rest rdf:nil
                                                                                                                                   ]
                                                                                                                        ]
                                                                           ] ;
                                                                 rdf:rest [ rdf:type <http://www.w3.org/2003/11/swrl#AtomList> ;
                                                                            rdf:first [ rdf:type <http://www.w3.org/2003/11/swrl#BuiltinAtom> ;
                                                                                        <http://www.w3.org/2003/11/swrl#builtin> <http://www.w3.org/2003/11/swrlb#greaterThan> ;
                                                                                        <http://www.w3.org/2003/11/swrl#arguments> [ rdf:type rdf:List ;
                                                                                                                                     rdf:first owl:nuu ;
                                                                                                                                     rdf:rest [ rdf:type rdf:List ;
                                                                                                                                                rdf:first 2 ;
                                                                                                                                                rdf:rest rdf:nil
                                                                                                                                              ]
                                                                                                                                   ]
                                                                                      ] ;
                                                                            rdf:rest [ rdf:type <http://www.w3.org/2003/11/swrl#AtomList> ;
                                                                                       rdf:first [ rdf:type <http://www.w3.org/2003/11/swrl#DatavaluedPropertyAtom> ;
                                                                                                   <http://www.w3.org/2003/11/swrl#propertyPredicate> :hasTotalAmountOfUtilizationUnits ;
                                                                                                   <http://www.w3.org/2003/11/swrl#argument1> owl:b ;
                                                                                                   <http://www.w3.org/2003/11/swrl#argument2> owl:nuu
                                                                                                 ] ;
                                                                                       rdf:rest rdf:nil
                                                                                     ]
                                                                          ]
                                                               ]
                                                    ]
                                         ] ;
   <http://www.w3.org/2003/11/swrl#head> [ rdf:type <http://www.w3.org/2003/11/swrl#AtomList> ;
                                           rdf:first [ rdf:type <http://www.w3.org/2003/11/swrl#IndividualPropertyAtom> ;
                                                       <http://www.w3.org/2003/11/swrl#propertyPredicate> :hasBuildingClass ;
                                                       <http://www.w3.org/2003/11/swrl#argument1> owl:b ;
                                                       <http://www.w3.org/2003/11/swrl#argument2> :BuildingClass3
                                                     ] ;
                                           rdf:rest rdf:nil
                                         ]
 ] .

[ <http://swrl.stanford.edu/ontologies/3.3/swrla.owl#isRuleEnabled> "true"^^xsd:boolean ;
   rdfs:comment "" ;
   rdfs:label "§2 (3) 3. - Teil 1" ;
   rdf:type <http://www.w3.org/2003/11/swrl#Imp> ;
   <http://www.w3.org/2003/11/swrl#body> [ rdf:type <http://www.w3.org/2003/11/swrl#AtomList> ;
                                           rdf:first [ rdf:type <http://www.w3.org/2003/11/swrl#DatavaluedPropertyAtom> ;
                                                       <http://www.w3.org/2003/11/swrl#propertyPredicate> :hasAverageHeight ;
                                                       <http://www.w3.org/2003/11/swrl#argument1> owl:b ;
                                                       <http://www.w3.org/2003/11/swrl#argument2> owl:h
                                                     ] ;
                                           rdf:rest [ rdf:type <http://www.w3.org/2003/11/swrl#AtomList> ;
                                                      rdf:first [ rdf:type <http://www.w3.org/2003/11/swrl#BuiltinAtom> ;
                                                                  <http://www.w3.org/2003/11/swrl#builtin> <http://www.w3.org/2003/11/swrlb#greaterThan> ;
                                                                  <http://www.w3.org/2003/11/swrl#arguments> [ rdf:type rdf:List ;
                                                                                                               rdf:first owl:cgfa ;
                                                                                                               rdf:rest [ rdf:type rdf:List ;
                                                                                                                          rdf:first 400 ;
                                                                                                                          rdf:rest rdf:nil
                                                                                                                        ]
                                                                                                             ]
                                                                ] ;
                                                      rdf:rest [ rdf:type <http://www.w3.org/2003/11/swrl#AtomList> ;
                                                                 rdf:first [ rdf:type <http://www.w3.org/2003/11/swrl#ClassAtom> ;
                                                                             <http://www.w3.org/2003/11/swrl#classPredicate> <https://w3id.org/bot#Building> ;
                                                                             <http://www.w3.org/2003/11/swrl#argument1> owl:b
                                                                           ] ;
                                                                 rdf:rest [ rdf:type <http://www.w3.org/2003/11/swrl#AtomList> ;
                                                                            rdf:first [ rdf:type <http://www.w3.org/2003/11/swrl#BuiltinAtom> ;
                                                                                        <http://www.w3.org/2003/11/swrl#builtin> <http://www.w3.org/2003/11/swrlb#lessThanOrEqual> ;
                                                                                        <http://www.w3.org/2003/11/swrl#arguments> [ rdf:type rdf:List ;
                                                                                                                                     rdf:first owl:h ;
                                                                                                                                     rdf:rest [ rdf:type rdf:List ;
                                                                                                                                                rdf:first 7.0 ;
                                                                                                                                                rdf:rest rdf:nil
                                                                                                                                              ]
                                                                                                                                   ]
                                                                                      ] ;
                                                                            rdf:rest [ rdf:type <http://www.w3.org/2003/11/swrl#AtomList> ;
                                                                                       rdf:first [ rdf:type <http://www.w3.org/2003/11/swrl#DatavaluedPropertyAtom> ;
                                                                                                   <http://www.w3.org/2003/11/swrl#propertyPredicate> :hasCombinedGrossFloorArea ;
                                                                                                   <http://www.w3.org/2003/11/swrl#argument1> owl:b ;
                                                                                                   <http://www.w3.org/2003/11/swrl#argument2> owl:cgfa
                                                                                                 ] ;
                                                                                       rdf:rest [ rdf:type <http://www.w3.org/2003/11/swrl#AtomList> ;
                                                                                                  rdf:first [ rdf:type <http://www.w3.org/2003/11/swrl#BuiltinAtom> ;
                                                                                                              <http://www.w3.org/2003/11/swrl#builtin> <http://www.w3.org/2003/11/swrlb#lessThanOrEqual> ;
                                                                                                              <http://www.w3.org/2003/11/swrl#arguments> [ rdf:type rdf:List ;
                                                                                                                                                           rdf:first owl:nuu ;
                                                                                                                                                           rdf:rest [ rdf:type rdf:List ;
                                                                                                                                                                      rdf:first 2 ;
                                                                                                                                                                      rdf:rest rdf:nil
                                                                                                                                                                    ]
                                                                                                                                                         ]
                                                                                                            ] ;
                                                                                                  rdf:rest [ rdf:type <http://www.w3.org/2003/11/swrl#AtomList> ;
                                                                                                             rdf:first [ rdf:type <http://www.w3.org/2003/11/swrl#DatavaluedPropertyAtom> ;
                                                                                                                         <http://www.w3.org/2003/11/swrl#propertyPredicate> :hasTotalAmountOfUtilizationUnits ;
                                                                                                                         <http://www.w3.org/2003/11/swrl#argument1> owl:b ;
                                                                                                                         <http://www.w3.org/2003/11/swrl#argument2> owl:nuu
                                                                                                                       ] ;
                                                                                                             rdf:rest rdf:nil
                                                                                                           ]
                                                                                                ]
                                                                                     ]
                                                                          ]
                                                               ]
                                                    ]
                                         ] ;
   <http://www.w3.org/2003/11/swrl#head> [ rdf:type <http://www.w3.org/2003/11/swrl#AtomList> ;
                                           rdf:first [ rdf:type <http://www.w3.org/2003/11/swrl#IndividualPropertyAtom> ;
                                                       <http://www.w3.org/2003/11/swrl#propertyPredicate> :hasBuildingClass ;
                                                       <http://www.w3.org/2003/11/swrl#argument1> owl:b ;
                                                       <http://www.w3.org/2003/11/swrl#argument2> :BuildingClass3
                                                     ] ;
                                           rdf:rest rdf:nil
                                         ]
 ] .

[ <http://swrl.stanford.edu/ontologies/3.3/swrla.owl#isRuleEnabled> "true"^^xsd:boolean ;
   rdfs:comment "" ;
   rdfs:label "§2 (3) 2." ;
   rdf:type <http://www.w3.org/2003/11/swrl#Imp> ;
   <http://www.w3.org/2003/11/swrl#body> [ rdf:type <http://www.w3.org/2003/11/swrl#AtomList> ;
                                           rdf:first [ rdf:type <http://www.w3.org/2003/11/swrl#DatavaluedPropertyAtom> ;
                                                       <http://www.w3.org/2003/11/swrl#propertyPredicate> :hasAverageHeight ;
                                                       <http://www.w3.org/2003/11/swrl#argument1> owl:b ;
                                                       <http://www.w3.org/2003/11/swrl#argument2> owl:h
                                                     ] ;
                                           rdf:rest [ rdf:type <http://www.w3.org/2003/11/swrl#AtomList> ;
                                                      rdf:first [ rdf:type <http://www.w3.org/2003/11/swrl#BuiltinAtom> ;
                                                                  <http://www.w3.org/2003/11/swrl#builtin> <http://www.w3.org/2003/11/swrlb#lessThanOrEqual> ;
                                                                  <http://www.w3.org/2003/11/swrl#arguments> [ rdf:type rdf:List ;
                                                                                                               rdf:first owl:cgfa ;
                                                                                                               rdf:rest [ rdf:type rdf:List ;
                                                                                                                          rdf:first 400 ;
                                                                                                                          rdf:rest rdf:nil
                                                                                                                        ]
                                                                                                             ]
                                                                ] ;
                                                      rdf:rest [ rdf:type <http://www.w3.org/2003/11/swrl#AtomList> ;
                                                                 rdf:first [ rdf:type <http://www.w3.org/2003/11/swrl#ClassAtom> ;
                                                                             <http://www.w3.org/2003/11/swrl#classPredicate> <https://w3id.org/bot#Building> ;
                                                                             <http://www.w3.org/2003/11/swrl#argument1> owl:b
                                                                           ] ;
                                                                 rdf:rest [ rdf:type <http://www.w3.org/2003/11/swrl#AtomList> ;
                                                                            rdf:first [ rdf:type <http://www.w3.org/2003/11/swrl#DatavaluedPropertyAtom> ;
                                                                                        <http://www.w3.org/2003/11/swrl#propertyPredicate> :isFreestanding ;
                                                                                        <http://www.w3.org/2003/11/swrl#argument1> owl:b ;
                                                                                        <http://www.w3.org/2003/11/swrl#argument2> "false"^^xsd:boolean
                                                                                      ] ;
                                                                            rdf:rest [ rdf:type <http://www.w3.org/2003/11/swrl#AtomList> ;
                                                                                       rdf:first [ rdf:type <http://www.w3.org/2003/11/swrl#BuiltinAtom> ;
                                                                                                   <http://www.w3.org/2003/11/swrl#builtin> <http://www.w3.org/2003/11/swrlb#lessThanOrEqual> ;
                                                                                                   <http://www.w3.org/2003/11/swrl#arguments> [ rdf:type rdf:List ;
                                                                                                                                                rdf:first owl:h ;
                                                                                                                                                rdf:rest [ rdf:type rdf:List ;
                                                                                                                                                           rdf:first 7.0 ;
                                                                                                                                                           rdf:rest rdf:nil
                                                                                                                                                         ]
                                                                                                                                              ]
                                                                                                 ] ;
                                                                                       rdf:rest [ rdf:type <http://www.w3.org/2003/11/swrl#AtomList> ;
                                                                                                  rdf:first [ rdf:type <http://www.w3.org/2003/11/swrl#DatavaluedPropertyAtom> ;
                                                                                                              <http://www.w3.org/2003/11/swrl#propertyPredicate> :hasCombinedGrossFloorArea ;
                                                                                                              <http://www.w3.org/2003/11/swrl#argument1> owl:b ;
                                                                                                              <http://www.w3.org/2003/11/swrl#argument2> owl:cgfa
                                                                                                            ] ;
                                                                                                  rdf:rest [ rdf:type <http://www.w3.org/2003/11/swrl#AtomList> ;
                                                                                                             rdf:first [ rdf:type <http://www.w3.org/2003/11/swrl#BuiltinAtom> ;
                                                                                                                         <http://www.w3.org/2003/11/swrl#builtin> <http://www.w3.org/2003/11/swrlb#lessThanOrEqual> ;
                                                                                                                         <http://www.w3.org/2003/11/swrl#arguments> [ rdf:type rdf:List ;
                                                                                                                                                                      rdf:first owl:nuu ;
                                                                                                                                                                      rdf:rest [ rdf:type rdf:List ;
                                                                                                                                                                                 rdf:first 2 ;
                                                                                                                                                                                 rdf:rest rdf:nil
                                                                                                                                                                               ]
                                                                                                                                                                    ]
                                                                                                                       ] ;
                                                                                                             rdf:rest [ rdf:type <http://www.w3.org/2003/11/swrl#AtomList> ;
                                                                                                                        rdf:first [ rdf:type <http://www.w3.org/2003/11/swrl#DatavaluedPropertyAtom> ;
                                                                                                                                    <http://www.w3.org/2003/11/swrl#propertyPredicate> :hasTotalAmountOfUtilizationUnits ;
                                                                                                                                    <http://www.w3.org/2003/11/swrl#argument1> owl:b ;
                                                                                                                                    <http://www.w3.org/2003/11/swrl#argument2> owl:nuu
                                                                                                                                  ] ;
                                                                                                                        rdf:rest rdf:nil
                                                                                                                      ]
                                                                                                           ]
                                                                                                ]
                                                                                     ]
                                                                          ]
                                                               ]
                                                    ]
                                         ] ;
   <http://www.w3.org/2003/11/swrl#head> [ rdf:type <http://www.w3.org/2003/11/swrl#AtomList> ;
                                           rdf:first [ rdf:type <http://www.w3.org/2003/11/swrl#IndividualPropertyAtom> ;
                                                       <http://www.w3.org/2003/11/swrl#propertyPredicate> :hasBuildingClass ;
                                                       <http://www.w3.org/2003/11/swrl#argument1> owl:b ;
                                                       <http://www.w3.org/2003/11/swrl#argument2> :BuildingClass2
                                                     ] ;
                                           rdf:rest rdf:nil
                                         ]
 ] .

[ <http://swrl.stanford.edu/ontologies/3.3/swrla.owl#isRuleEnabled> "true"^^xsd:boolean ;
   rdfs:comment "" ;
   rdfs:label "§2 (3) 1a" ;
   rdf:type <http://www.w3.org/2003/11/swrl#Imp> ;
   <http://www.w3.org/2003/11/swrl#body> [ rdf:type <http://www.w3.org/2003/11/swrl#AtomList> ;
                                           rdf:first [ rdf:type <http://www.w3.org/2003/11/swrl#DatavaluedPropertyAtom> ;
                                                       <http://www.w3.org/2003/11/swrl#propertyPredicate> :hasAverageHeight ;
                                                       <http://www.w3.org/2003/11/swrl#argument1> owl:b ;
                                                       <http://www.w3.org/2003/11/swrl#argument2> owl:h
                                                     ] ;
                                           rdf:rest [ rdf:type <http://www.w3.org/2003/11/swrl#AtomList> ;
                                                      rdf:first [ rdf:type <http://www.w3.org/2003/11/swrl#BuiltinAtom> ;
                                                                  <http://www.w3.org/2003/11/swrl#builtin> <http://www.w3.org/2003/11/swrlb#lessThanOrEqual> ;
                                                                  <http://www.w3.org/2003/11/swrl#arguments> [ rdf:type rdf:List ;
                                                                                                               rdf:first owl:cgfa ;
                                                                                                               rdf:rest [ rdf:type rdf:List ;
                                                                                                                          rdf:first 400 ;
                                                                                                                          rdf:rest rdf:nil
                                                                                                                        ]
                                                                                                             ]
                                                                ] ;
                                                      rdf:rest [ rdf:type <http://www.w3.org/2003/11/swrl#AtomList> ;
                                                                 rdf:first [ rdf:type <http://www.w3.org/2003/11/swrl#DatavaluedPropertyAtom> ;
                                                                             <http://www.w3.org/2003/11/swrl#propertyPredicate> :isFreestanding ;
                                                                             <http://www.w3.org/2003/11/swrl#argument1> owl:b ;
                                                                             <http://www.w3.org/2003/11/swrl#argument2> "true"^^xsd:boolean
                                                                           ] ;
                                                                 rdf:rest [ rdf:type <http://www.w3.org/2003/11/swrl#AtomList> ;
                                                                            rdf:first [ rdf:type <http://www.w3.org/2003/11/swrl#ClassAtom> ;
                                                                                        <http://www.w3.org/2003/11/swrl#classPredicate> <https://w3id.org/bot#Building> ;
                                                                                        <http://www.w3.org/2003/11/swrl#argument1> owl:b
                                                                                      ] ;
                                                                            rdf:rest [ rdf:type <http://www.w3.org/2003/11/swrl#AtomList> ;
                                                                                       rdf:first [ rdf:type <http://www.w3.org/2003/11/swrl#BuiltinAtom> ;
                                                                                                   <http://www.w3.org/2003/11/swrl#builtin> <http://www.w3.org/2003/11/swrlb#lessThanOrEqual> ;
                                                                                                   <http://www.w3.org/2003/11/swrl#arguments> [ rdf:type rdf:List ;
                                                                                                                                                rdf:first owl:h ;
                                                                                                                                                rdf:rest [ rdf:type rdf:List ;
                                                                                                                                                           rdf:first 7.0 ;
                                                                                                                                                           rdf:rest rdf:nil
                                                                                                                                                         ]
                                                                                                                                              ]
                                                                                                 ] ;
                                                                                       rdf:rest [ rdf:type <http://www.w3.org/2003/11/swrl#AtomList> ;
                                                                                                  rdf:first [ rdf:type <http://www.w3.org/2003/11/swrl#DatavaluedPropertyAtom> ;
                                                                                                              <http://www.w3.org/2003/11/swrl#propertyPredicate> :hasCombinedGrossFloorArea ;
                                                                                                              <http://www.w3.org/2003/11/swrl#argument1> owl:b ;
                                                                                                              <http://www.w3.org/2003/11/swrl#argument2> owl:cgfa
                                                                                                            ] ;
                                                                                                  rdf:rest [ rdf:type <http://www.w3.org/2003/11/swrl#AtomList> ;
                                                                                                             rdf:first [ rdf:type <http://www.w3.org/2003/11/swrl#BuiltinAtom> ;
                                                                                                                         <http://www.w3.org/2003/11/swrl#builtin> <http://www.w3.org/2003/11/swrlb#lessThanOrEqual> ;
                                                                                                                         <http://www.w3.org/2003/11/swrl#arguments> [ rdf:type rdf:List ;
                                                                                                                                                                      rdf:first owl:nuu ;
                                                                                                                                                                      rdf:rest [ rdf:type rdf:List ;
                                                                                                                                                                                 rdf:first 2 ;
                                                                                                                                                                                 rdf:rest rdf:nil
                                                                                                                                                                               ]
                                                                                                                                                                    ]
                                                                                                                       ] ;
                                                                                                             rdf:rest [ rdf:type <http://www.w3.org/2003/11/swrl#AtomList> ;
                                                                                                                        rdf:first [ rdf:type <http://www.w3.org/2003/11/swrl#DatavaluedPropertyAtom> ;
                                                                                                                                    <http://www.w3.org/2003/11/swrl#propertyPredicate> :hasTotalAmountOfUtilizationUnits ;
                                                                                                                                    <http://www.w3.org/2003/11/swrl#argument1> owl:b ;
                                                                                                                                    <http://www.w3.org/2003/11/swrl#argument2> owl:nuu
                                                                                                                                  ] ;
                                                                                                                        rdf:rest rdf:nil
                                                                                                                      ]
                                                                                                           ]
                                                                                                ]
                                                                                     ]
                                                                          ]
                                                               ]
                                                    ]
                                         ] ;
   <http://www.w3.org/2003/11/swrl#head> [ rdf:type <http://www.w3.org/2003/11/swrl#AtomList> ;
                                           rdf:first [ rdf:type <http://www.w3.org/2003/11/swrl#IndividualPropertyAtom> ;
                                                       <http://www.w3.org/2003/11/swrl#propertyPredicate> :hasBuildingClass ;
                                                       <http://www.w3.org/2003/11/swrl#argument1> owl:b ;
                                                       <http://www.w3.org/2003/11/swrl#argument2> :BuildingClass1a
                                                     ] ;
                                           rdf:rest rdf:nil
                                         ]
 ] .

[ <http://swrl.stanford.edu/ontologies/3.3/swrla.owl#isRuleEnabled> "true"^^xsd:boolean ;
   rdfs:comment "" ;
   rdfs:label "§2 (3) 5. - Teil 2" ;
   rdf:type <http://www.w3.org/2003/11/swrl#Imp> ;
   <http://www.w3.org/2003/11/swrl#body> [ rdf:type <http://www.w3.org/2003/11/swrl#AtomList> ;
                                           rdf:first [ rdf:type <http://www.w3.org/2003/11/swrl#DatavaluedPropertyAtom> ;
                                                       <http://www.w3.org/2003/11/swrl#propertyPredicate> :hasAverageHeight ;
                                                       <http://www.w3.org/2003/11/swrl#argument1> owl:b ;
                                                       <http://www.w3.org/2003/11/swrl#argument2> owl:h
                                                     ] ;
                                           rdf:rest [ rdf:type <http://www.w3.org/2003/11/swrl#AtomList> ;
                                                      rdf:first [ rdf:type <http://www.w3.org/2003/11/swrl#BuiltinAtom> ;
                                                                  <http://www.w3.org/2003/11/swrl#builtin> <http://www.w3.org/2003/11/swrlb#greaterThanOrEqual> ;
                                                                  <http://www.w3.org/2003/11/swrl#arguments> [ rdf:type rdf:List ;
                                                                                                               rdf:first owl:luu ;
                                                                                                               rdf:rest [ rdf:type rdf:List ;
                                                                                                                          rdf:first 400.0 ;
                                                                                                                          rdf:rest rdf:nil
                                                                                                                        ]
                                                                                                             ]
                                                                ] ;
                                                      rdf:rest [ rdf:type <http://www.w3.org/2003/11/swrl#AtomList> ;
                                                                 rdf:first [ rdf:type <http://www.w3.org/2003/11/swrl#ClassAtom> ;
                                                                             <http://www.w3.org/2003/11/swrl#classPredicate> <https://w3id.org/bot#Building> ;
                                                                             <http://www.w3.org/2003/11/swrl#argument1> owl:b
                                                                           ] ;
                                                                 rdf:rest [ rdf:type <http://www.w3.org/2003/11/swrl#AtomList> ;
                                                                            rdf:first [ rdf:type <http://www.w3.org/2003/11/swrl#DatavaluedPropertyAtom> ;
                                                                                        <http://www.w3.org/2003/11/swrl#propertyPredicate> :largestUtilizationSpace ;
                                                                                        <http://www.w3.org/2003/11/swrl#argument1> owl:b ;
                                                                                        <http://www.w3.org/2003/11/swrl#argument2> owl:luu
                                                                                      ] ;
                                                                            rdf:rest [ rdf:type <http://www.w3.org/2003/11/swrl#AtomList> ;
                                                                                       rdf:first [ rdf:type <http://www.w3.org/2003/11/swrl#BuiltinAtom> ;
                                                                                                   <http://www.w3.org/2003/11/swrl#builtin> <http://www.w3.org/2003/11/swrlb#greaterThan> ;
                                                                                                   <http://www.w3.org/2003/11/swrl#arguments> [ rdf:type rdf:List ;
                                                                                                                                                rdf:first owl:h ;
                                                                                                                                                rdf:rest [ rdf:type rdf:List ;
                                                                                                                                                           rdf:first 7 ;
                                                                                                                                                           rdf:rest rdf:nil
                                                                                                                                                         ]
                                                                                                                                              ]
                                                                                                 ] ;
                                                                                       rdf:rest rdf:nil
                                                                                     ]
                                                                          ]
                                                               ]
                                                    ]
                                         ] ;
   <http://www.w3.org/2003/11/swrl#head> [ rdf:type <http://www.w3.org/2003/11/swrl#AtomList> ;
                                           rdf:first [ rdf:type <http://www.w3.org/2003/11/swrl#IndividualPropertyAtom> ;
                                                       <http://www.w3.org/2003/11/swrl#propertyPredicate> :hasBuildingClass ;
                                                       <http://www.w3.org/2003/11/swrl#argument1> owl:b ;
                                                       <http://www.w3.org/2003/11/swrl#argument2> :BuildingClass5
                                                     ] ;
                                           rdf:rest rdf:nil
                                         ]
 ] .

[ <http://swrl.stanford.edu/ontologies/3.3/swrla.owl#isRuleEnabled> "true"^^xsd:boolean ;
   rdfs:comment "" ;
   rdfs:label "§2 (3) 4. - Part 2" ;
   rdf:type <http://www.w3.org/2003/11/swrl#Imp> ;
   <http://www.w3.org/2003/11/swrl#body> [ rdf:type <http://www.w3.org/2003/11/swrl#AtomList> ;
                                           rdf:first [ rdf:type <http://www.w3.org/2003/11/swrl#DatavaluedPropertyAtom> ;
                                                       <http://www.w3.org/2003/11/swrl#propertyPredicate> :hasAverageHeight ;
                                                       <http://www.w3.org/2003/11/swrl#argument1> owl:b ;
                                                       <http://www.w3.org/2003/11/swrl#argument2> owl:h
                                                     ] ;
                                           rdf:rest [ rdf:type <http://www.w3.org/2003/11/swrl#AtomList> ;
                                                      rdf:first [ rdf:type <http://www.w3.org/2003/11/swrl#BuiltinAtom> ;
                                                                  <http://www.w3.org/2003/11/swrl#builtin> <http://www.w3.org/2003/11/swrlb#lessThan> ;
                                                                  <http://www.w3.org/2003/11/swrl#arguments> [ rdf:type rdf:List ;
                                                                                                               rdf:first owl:luu ;
                                                                                                               rdf:rest [ rdf:type rdf:List ;
                                                                                                                          rdf:first 400.0 ;
                                                                                                                          rdf:rest rdf:nil
                                                                                                                        ]
                                                                                                             ]
                                                                ] ;
                                                      rdf:rest [ rdf:type <http://www.w3.org/2003/11/swrl#AtomList> ;
                                                                 rdf:first [ rdf:type <http://www.w3.org/2003/11/swrl#ClassAtom> ;
                                                                             <http://www.w3.org/2003/11/swrl#classPredicate> <https://w3id.org/bot#Building> ;
                                                                             <http://www.w3.org/2003/11/swrl#argument1> owl:b
                                                                           ] ;
                                                                 rdf:rest [ rdf:type <http://www.w3.org/2003/11/swrl#AtomList> ;
                                                                            rdf:first [ rdf:type <http://www.w3.org/2003/11/swrl#DatavaluedPropertyAtom> ;
                                                                                        <http://www.w3.org/2003/11/swrl#propertyPredicate> :largestUtilizationSpace ;
                                                                                        <http://www.w3.org/2003/11/swrl#argument1> owl:b ;
                                                                                        <http://www.w3.org/2003/11/swrl#argument2> owl:luu
                                                                                      ] ;
                                                                            rdf:rest [ rdf:type <http://www.w3.org/2003/11/swrl#AtomList> ;
                                                                                       rdf:first [ rdf:type <http://www.w3.org/2003/11/swrl#BuiltinAtom> ;
                                                                                                   <http://www.w3.org/2003/11/swrl#builtin> <http://www.w3.org/2003/11/swrlb#lessThanOrEqual> ;
                                                                                                   <http://www.w3.org/2003/11/swrl#arguments> [ rdf:type rdf:List ;
                                                                                                                                                rdf:first owl:h ;
                                                                                                                                                rdf:rest [ rdf:type rdf:List ;
                                                                                                                                                           rdf:first 13.0 ;
                                                                                                                                                           rdf:rest rdf:nil
                                                                                                                                                         ]
                                                                                                                                              ]
                                                                                                 ] ;
                                                                                       rdf:rest [ rdf:type <http://www.w3.org/2003/11/swrl#AtomList> ;
                                                                                                  rdf:first [ rdf:type <http://www.w3.org/2003/11/swrl#BuiltinAtom> ;
                                                                                                              <http://www.w3.org/2003/11/swrl#builtin> <http://www.w3.org/2003/11/swrlb#greaterThan> ;
                                                                                                              <http://www.w3.org/2003/11/swrl#arguments> [ rdf:type rdf:List ;
                                                                                                                                                           rdf:first owl:h ;
                                                                                                                                                           rdf:rest [ rdf:type rdf:List ;
                                                                                                                                                                      rdf:first 7.0 ;
                                                                                                                                                                      rdf:rest rdf:nil
                                                                                                                                                                    ]
                                                                                                                                                         ]
                                                                                                            ] ;
                                                                                                  rdf:rest rdf:nil
                                                                                                ]
                                                                                     ]
                                                                          ]
                                                               ]
                                                    ]
                                         ] ;
   <http://www.w3.org/2003/11/swrl#head> [ rdf:type <http://www.w3.org/2003/11/swrl#AtomList> ;
                                           rdf:first [ rdf:type <http://www.w3.org/2003/11/swrl#IndividualPropertyAtom> ;
                                                       <http://www.w3.org/2003/11/swrl#propertyPredicate> :hasBuildingClass ;
                                                       <http://www.w3.org/2003/11/swrl#argument1> owl:b ;
                                                       <http://www.w3.org/2003/11/swrl#argument2> :BuildingClass4
                                                     ] ;
                                           rdf:rest rdf:nil
                                         ]
 ] .

[ <http://swrl.stanford.edu/ontologies/3.3/swrla.owl#isRuleEnabled> "true"^^xsd:boolean ;
   rdfs:comment "Special Purpose Condition" ;
   rdfs:label "§2 (4) 5. MBO" ;
   rdf:type <http://www.w3.org/2003/11/swrl#Imp> ;
   <http://www.w3.org/2003/11/swrl#body> [ rdf:type <http://www.w3.org/2003/11/swrl#AtomList> ;
                                           rdf:first [ rdf:type <http://www.w3.org/2003/11/swrl#DatavaluedPropertyAtom> ;
                                                       <http://www.w3.org/2003/11/swrl#propertyPredicate> :usesGrossFloorArea ;
                                                       <http://www.w3.org/2003/11/swrl#argument1> owl:sp ;
                                                       <http://www.w3.org/2003/11/swrl#argument2> owl:ugfa
                                                     ] ;
                                           rdf:rest [ rdf:type <http://www.w3.org/2003/11/swrl#AtomList> ;
                                                      rdf:first [ rdf:type <http://www.w3.org/2003/11/swrl#ClassAtom> ;
                                                                  <http://www.w3.org/2003/11/swrl#classPredicate> <https://w3id.org/bot#Building> ;
                                                                  <http://www.w3.org/2003/11/swrl#argument1> owl:b
                                                                ] ;
                                                      rdf:rest [ rdf:type <http://www.w3.org/2003/11/swrl#AtomList> ;
                                                                 rdf:first [ rdf:type <http://www.w3.org/2003/11/swrl#BuiltinAtom> ;
                                                                             <http://www.w3.org/2003/11/swrl#builtin> <http://www.w3.org/2003/11/swrlb#greaterThan> ;
                                                                             <http://www.w3.org/2003/11/swrl#arguments> [ rdf:type rdf:List ;
                                                                                                                          rdf:first owl:ugfa ;
                                                                                                                          rdf:rest [ rdf:type rdf:List ;
                                                                                                                                     rdf:first 400.0 ;
                                                                                                                                     rdf:rest rdf:nil
                                                                                                                                   ]
                                                                                                                        ]
                                                                           ] ;
                                                                 rdf:rest [ rdf:type <http://www.w3.org/2003/11/swrl#AtomList> ;
                                                                            rdf:first [ rdf:type <http://www.w3.org/2003/11/swrl#IndividualPropertyAtom> ;
                                                                                        <http://www.w3.org/2003/11/swrl#propertyPredicate> <https://w3id.org/bot#hasSpace> ;
                                                                                        <http://www.w3.org/2003/11/swrl#argument1> owl:b ;
                                                                                        <http://www.w3.org/2003/11/swrl#argument2> owl:sp
                                                                                      ] ;
                                                                            rdf:rest [ rdf:type <http://www.w3.org/2003/11/swrl#AtomList> ;
                                                                                       rdf:first [ rdf:type <http://www.w3.org/2003/11/swrl#IndividualPropertyAtom> ;
                                                                                                   <http://www.w3.org/2003/11/swrl#propertyPredicate> :hasSpaceUsage ;
                                                                                                   <http://www.w3.org/2003/11/swrl#argument1> owl:sp ;
                                                                                                   <http://www.w3.org/2003/11/swrl#argument2> owl:spu
                                                                                                 ] ;
                                                                                       rdf:rest [ rdf:type <http://www.w3.org/2003/11/swrl#AtomList> ;
                                                                                                  rdf:first [ rdf:type <http://www.w3.org/2003/11/swrl#SameIndividualAtom> ;
                                                                                                              <http://www.w3.org/2003/11/swrl#argument1> owl:spu ;
                                                                                                              <http://www.w3.org/2003/11/swrl#argument2> :OfficeRoom
                                                                                                            ] ;
                                                                                                  rdf:rest rdf:nil
                                                                                                ]
                                                                                     ]
                                                                          ]
                                                               ]
                                                    ]
                                         ] ;
   <http://www.w3.org/2003/11/swrl#head> [ rdf:type <http://www.w3.org/2003/11/swrl#AtomList> ;
                                           rdf:first [ rdf:type <http://www.w3.org/2003/11/swrl#ClassAtom> ;
                                                       <http://www.w3.org/2003/11/swrl#classPredicate> <https://purl.org/fisa#SpecialPurposeConditionAcc§2_S4_P5> ;
                                                       <http://www.w3.org/2003/11/swrl#argument1> owl:b
                                                     ] ;
                                           rdf:rest rdf:nil
                                         ]
 ] .

[ rdfs:comment "§28 (2) Sentence 1 - Part 1"@en ;
   rdf:type <http://www.w3.org/2003/11/swrl#Imp> ;
   <http://www.w3.org/2003/11/swrl#body> [ rdf:type <http://www.w3.org/2003/11/swrl#AtomList> ;
                                           rdf:first [ rdf:type <http://www.w3.org/2003/11/swrl#DatavaluedPropertyAtom> ;
                                                       <http://www.w3.org/2003/11/swrl#propertyPredicate> :isLoadBearing ;
                                                       <http://www.w3.org/2003/11/swrl#argument1> <urn:swrl:var#ew> ;
                                                       <http://www.w3.org/2003/11/swrl#argument2> "false"^^xsd:boolean
                                                     ] ;
                                           rdf:rest [ rdf:type <http://www.w3.org/2003/11/swrl#AtomList> ;
                                                      rdf:first [ rdf:type <http://www.w3.org/2003/11/swrl#ClassAtom> ;
                                                                  <http://www.w3.org/2003/11/swrl#classPredicate> :ExternalWall ;
                                                                  <http://www.w3.org/2003/11/swrl#argument1> <urn:swrl:var#ew>
                                                                ] ;
                                                      rdf:rest [ rdf:type <http://www.w3.org/2003/11/swrl#AtomList> ;
                                                                 rdf:first [ rdf:type <http://www.w3.org/2003/11/swrl#ClassAtom> ;
                                                                             <http://www.w3.org/2003/11/swrl#classPredicate> <https://w3id.org/bot#Building> ;
                                                                             <http://www.w3.org/2003/11/swrl#argument1> <urn:swrl:var#b>
                                                                           ] ;
                                                                 rdf:rest [ rdf:type <http://www.w3.org/2003/11/swrl#AtomList> ;
                                                                            rdf:first [ rdf:type <http://www.w3.org/2003/11/swrl#IndividualPropertyAtom> ;
                                                                                        <http://www.w3.org/2003/11/swrl#propertyPredicate> <https://w3id.org/bot#hasElement> ;
                                                                                        <http://www.w3.org/2003/11/swrl#argument1> <urn:swrl:var#sp> ;
                                                                                        <http://www.w3.org/2003/11/swrl#argument2> <urn:swrl:var#ew>
                                                                                      ] ;
                                                                            rdf:rest [ rdf:type <http://www.w3.org/2003/11/swrl#AtomList> ;
                                                                                       rdf:first [ rdf:type <http://www.w3.org/2003/11/swrl#IndividualPropertyAtom> ;
                                                                                                   <http://www.w3.org/2003/11/swrl#propertyPredicate> :hasBuildingClass ;
                                                                                                   <http://www.w3.org/2003/11/swrl#argument1> <urn:swrl:var#b> ;
                                                                                                   <http://www.w3.org/2003/11/swrl#argument2> <urn:swrl:var#bc>
                                                                                                 ] ;
                                                                                       rdf:rest [ rdf:type <http://www.w3.org/2003/11/swrl#AtomList> ;
                                                                                                  rdf:first [ rdf:type <http://www.w3.org/2003/11/swrl#IndividualPropertyAtom> ;
                                                                                                              <http://www.w3.org/2003/11/swrl#propertyPredicate> <https://w3id.org/bot#hasStorey> ;
                                                                                                              <http://www.w3.org/2003/11/swrl#argument1> <urn:swrl:var#b> ;
                                                                                                              <http://www.w3.org/2003/11/swrl#argument2> <urn:swrl:var#st>
                                                                                                            ] ;
                                                                                                  rdf:rest [ rdf:type <http://www.w3.org/2003/11/swrl#AtomList> ;
                                                                                                             rdf:first [ rdf:type <http://www.w3.org/2003/11/swrl#ClassAtom> ;
                                                                                                                         <http://www.w3.org/2003/11/swrl#classPredicate> [ rdf:type owl:Class ;
                                                                                                                                                                           owl:complementOf :BuildingClass1
                                                                                                                                                                         ] ;
                                                                                                                         <http://www.w3.org/2003/11/swrl#argument1> <urn:swrl:var#bc>
                                                                                                                       ] ;
                                                                                                             rdf:rest [ rdf:type <http://www.w3.org/2003/11/swrl#AtomList> ;
                                                                                                                        rdf:first [ rdf:type <http://www.w3.org/2003/11/swrl#ClassAtom> ;
                                                                                                                                    <http://www.w3.org/2003/11/swrl#classPredicate> [ rdf:type owl:Class ;
                                                                                                                                                                                      owl:complementOf :BuildingClass2
                                                                                                                                                                                    ] ;
                                                                                                                                    <http://www.w3.org/2003/11/swrl#argument1> <urn:swrl:var#bc>
                                                                                                                                  ] ;
                                                                                                                        rdf:rest [ rdf:type <http://www.w3.org/2003/11/swrl#AtomList> ;
                                                                                                                                   rdf:first [ rdf:type <http://www.w3.org/2003/11/swrl#ClassAtom> ;
                                                                                                                                               <http://www.w3.org/2003/11/swrl#classPredicate> [ rdf:type owl:Class ;
                                                                                                                                                                                                 owl:complementOf :BuildingClass3
                                                                                                                                                                                               ] ;
                                                                                                                                               <http://www.w3.org/2003/11/swrl#argument1> <urn:swrl:var#bc>
                                                                                                                                             ] ;
                                                                                                                                   rdf:rest [ rdf:type <http://www.w3.org/2003/11/swrl#AtomList> ;
                                                                                                                                              rdf:first [ rdf:type <http://www.w3.org/2003/11/swrl#IndividualPropertyAtom> ;
                                                                                                                                                          <http://www.w3.org/2003/11/swrl#propertyPredicate> <https://w3id.org/bot#hasSpace> ;
                                                                                                                                                          <http://www.w3.org/2003/11/swrl#argument1> <urn:swrl:var#st> ;
                                                                                                                                                          <http://www.w3.org/2003/11/swrl#argument2> <urn:swrl:var#sp>
                                                                                                                                                        ] ;
                                                                                                                                              rdf:rest rdf:nil
                                                                                                                                            ]
                                                                                                                                 ]
                                                                                                                      ]
                                                                                                           ]
                                                                                                ]
                                                                                     ]
                                                                          ]
                                                               ]
                                                    ]
                                         ] ;
   <http://www.w3.org/2003/11/swrl#head> [ rdf:type <http://www.w3.org/2003/11/swrl#AtomList> ;
                                           rdf:first [ rdf:type <http://www.w3.org/2003/11/swrl#IndividualPropertyAtom> ;
                                                       <http://www.w3.org/2003/11/swrl#propertyPredicate> :hasRequirementOfFireBehaviour ;
                                                       <http://www.w3.org/2003/11/swrl#argument1> <urn:swrl:var#ew> ;
                                                       <http://www.w3.org/2003/11/swrl#argument2> :nichtbrennbar
                                                     ] ;
                                           rdf:rest rdf:nil
                                         ]
 ] .

[ rdfs:comment "§28 (2) Sentence 1 - Part 1.1"@en ;
   rdf:type <http://www.w3.org/2003/11/swrl#Imp> ;
   <http://www.w3.org/2003/11/swrl#body> [ rdf:type <http://www.w3.org/2003/11/swrl#AtomList> ;
                                           rdf:first [ rdf:type <http://www.w3.org/2003/11/swrl#DatavaluedPropertyAtom> ;
                                                       <http://www.w3.org/2003/11/swrl#propertyPredicate> :isLoadBearing ;
                                                       <http://www.w3.org/2003/11/swrl#argument1> <urn:swrl:var#ew> ;
                                                       <http://www.w3.org/2003/11/swrl#argument2> "false"^^xsd:boolean
                                                     ] ;
                                           rdf:rest [ rdf:type <http://www.w3.org/2003/11/swrl#AtomList> ;
                                                      rdf:first [ rdf:type <http://www.w3.org/2003/11/swrl#ClassAtom> ;
                                                                  <http://www.w3.org/2003/11/swrl#classPredicate> :ExternalWall ;
                                                                  <http://www.w3.org/2003/11/swrl#argument1> <urn:swrl:var#ew>
                                                                ] ;
                                                      rdf:rest [ rdf:type <http://www.w3.org/2003/11/swrl#AtomList> ;
                                                                 rdf:first [ rdf:type <http://www.w3.org/2003/11/swrl#ClassAtom> ;
                                                                             <http://www.w3.org/2003/11/swrl#classPredicate> <https://w3id.org/bot#Building> ;
                                                                             <http://www.w3.org/2003/11/swrl#argument1> <urn:swrl:var#b>
                                                                           ] ;
                                                                 rdf:rest [ rdf:type <http://www.w3.org/2003/11/swrl#AtomList> ;
                                                                            rdf:first [ rdf:type <http://www.w3.org/2003/11/swrl#IndividualPropertyAtom> ;
                                                                                        <http://www.w3.org/2003/11/swrl#propertyPredicate> <https://w3id.org/bot#hasElement> ;
                                                                                        <http://www.w3.org/2003/11/swrl#argument1> <urn:swrl:var#sp> ;
                                                                                        <http://www.w3.org/2003/11/swrl#argument2> <urn:swrl:var#ew>
                                                                                      ] ;
                                                                            rdf:rest [ rdf:type <http://www.w3.org/2003/11/swrl#AtomList> ;
                                                                                       rdf:first [ rdf:type <http://www.w3.org/2003/11/swrl#DatavaluedPropertyAtom> ;
                                                                                                   <http://www.w3.org/2003/11/swrl#propertyPredicate> :isSpaceEnclosing ;
                                                                                                   <http://www.w3.org/2003/11/swrl#argument1> <urn:swrl:var#ew> ;
                                                                                                   <http://www.w3.org/2003/11/swrl#argument2> "true"^^xsd:boolean
                                                                                                 ] ;
                                                                                       rdf:rest [ rdf:type <http://www.w3.org/2003/11/swrl#AtomList> ;
                                                                                                  rdf:first [ rdf:type <http://www.w3.org/2003/11/swrl#IndividualPropertyAtom> ;
                                                                                                              <http://www.w3.org/2003/11/swrl#propertyPredicate> :hasBuildingClass ;
                                                                                                              <http://www.w3.org/2003/11/swrl#argument1> <urn:swrl:var#b> ;
                                                                                                              <http://www.w3.org/2003/11/swrl#argument2> <urn:swrl:var#bc>
                                                                                                            ] ;
                                                                                                  rdf:rest [ rdf:type <http://www.w3.org/2003/11/swrl#AtomList> ;
                                                                                                             rdf:first [ rdf:type <http://www.w3.org/2003/11/swrl#IndividualPropertyAtom> ;
                                                                                                                         <http://www.w3.org/2003/11/swrl#propertyPredicate> <https://w3id.org/bot#hasStorey> ;
                                                                                                                         <http://www.w3.org/2003/11/swrl#argument1> <urn:swrl:var#b> ;
                                                                                                                         <http://www.w3.org/2003/11/swrl#argument2> <urn:swrl:var#st>
                                                                                                                       ] ;
                                                                                                             rdf:rest [ rdf:type <http://www.w3.org/2003/11/swrl#AtomList> ;
                                                                                                                        rdf:first [ rdf:type <http://www.w3.org/2003/11/swrl#ClassAtom> ;
                                                                                                                                    <http://www.w3.org/2003/11/swrl#classPredicate> [ rdf:type owl:Class ;
                                                                                                                                                                                      owl:complementOf :BuildingClass1
                                                                                                                                                                                    ] ;
                                                                                                                                    <http://www.w3.org/2003/11/swrl#argument1> <urn:swrl:var#bc>
                                                                                                                                  ] ;
                                                                                                                        rdf:rest [ rdf:type <http://www.w3.org/2003/11/swrl#AtomList> ;
                                                                                                                                   rdf:first [ rdf:type <http://www.w3.org/2003/11/swrl#ClassAtom> ;
                                                                                                                                               <http://www.w3.org/2003/11/swrl#classPredicate> [ rdf:type owl:Class ;
                                                                                                                                                                                                 owl:complementOf :BuildingClass2
                                                                                                                                                                                               ] ;
                                                                                                                                               <http://www.w3.org/2003/11/swrl#argument1> <urn:swrl:var#bc>
                                                                                                                                             ] ;
                                                                                                                                   rdf:rest [ rdf:type <http://www.w3.org/2003/11/swrl#AtomList> ;
                                                                                                                                              rdf:first [ rdf:type <http://www.w3.org/2003/11/swrl#ClassAtom> ;
                                                                                                                                                          <http://www.w3.org/2003/11/swrl#classPredicate> [ rdf:type owl:Class ;
                                                                                                                                                                                                            owl:complementOf :BuildingClass3
                                                                                                                                                                                                          ] ;
                                                                                                                                                          <http://www.w3.org/2003/11/swrl#argument1> <urn:swrl:var#bc>
                                                                                                                                                        ] ;
                                                                                                                                              rdf:rest [ rdf:type <http://www.w3.org/2003/11/swrl#AtomList> ;
                                                                                                                                                         rdf:first [ rdf:type <http://www.w3.org/2003/11/swrl#IndividualPropertyAtom> ;
                                                                                                                                                                     <http://www.w3.org/2003/11/swrl#propertyPredicate> :hasFireResistance ;
                                                                                                                                                                     <http://www.w3.org/2003/11/swrl#argument1> <urn:swrl:var#ew> ;
                                                                                                                                                                     <http://www.w3.org/2003/11/swrl#argument2> :feuerhemmend
                                                                                                                                                                   ] ;
                                                                                                                                                         rdf:rest [ rdf:type <http://www.w3.org/2003/11/swrl#AtomList> ;
                                                                                                                                                                    rdf:first [ rdf:type <http://www.w3.org/2003/11/swrl#IndividualPropertyAtom> ;
                                                                                                                                                                                <http://www.w3.org/2003/11/swrl#propertyPredicate> <https://w3id.org/bot#hasSpace> ;
                                                                                                                                                                                <http://www.w3.org/2003/11/swrl#argument1> <urn:swrl:var#st> ;
                                                                                                                                                                                <http://www.w3.org/2003/11/swrl#argument2> <urn:swrl:var#sp>
                                                                                                                                                                              ] ;
                                                                                                                                                                    rdf:rest rdf:nil
                                                                                                                                                                  ]
                                                                                                                                                       ]
                                                                                                                                            ]
                                                                                                                                 ]
                                                                                                                      ]
                                                                                                           ]
                                                                                                ]
                                                                                     ]
                                                                          ]
                                                               ]
                                                    ]
                                         ] ;
   <http://www.w3.org/2003/11/swrl#head> [ rdf:type <http://www.w3.org/2003/11/swrl#AtomList> ;
                                           rdf:first [ rdf:type <http://www.w3.org/2003/11/swrl#IndividualPropertyAtom> ;
                                                       <http://www.w3.org/2003/11/swrl#propertyPredicate> :isPermittedWithFireBehaviour ;
                                                       <http://www.w3.org/2003/11/swrl#argument1> <urn:swrl:var#ew> ;
                                                       <http://www.w3.org/2003/11/swrl#argument2> :brennbar
                                                     ] ;
                                           rdf:rest rdf:nil
                                         ]
 ] .

[ <http://swrl.stanford.edu/ontologies/3.3/swrla.owl#isRuleEnabled> "true"^^xsd:boolean ;
   rdfs:comment "Fassung 1995, zuletzt geändert 02/2014 & MVKVO - by example: when is a Sales Premises unregulated and regulated according to Special Purpose Prescriptive MVKVO" ;
   rdfs:label "§1 MVKVO #unregulated" ;
   rdf:type <http://www.w3.org/2003/11/swrl#Imp> ;
   <http://www.w3.org/2003/11/swrl#body> [ rdf:type <http://www.w3.org/2003/11/swrl#AtomList> ;
                                           rdf:first [ rdf:type <http://www.w3.org/2003/11/swrl#BuiltinAtom> ;
                                                       <http://www.w3.org/2003/11/swrl#builtin> <http://www.w3.org/2003/11/swrlb#greaterThan> ;
                                                       <http://www.w3.org/2003/11/swrl#arguments> [ rdf:type rdf:List ;
                                                                                                    rdf:first owl:gfa ;
                                                                                                    rdf:rest [ rdf:type rdf:List ;
                                                                                                               rdf:first 800.0 ;
                                                                                                               rdf:rest rdf:nil
                                                                                                             ]
                                                                                                  ]
                                                     ] ;
                                           rdf:rest [ rdf:type <http://www.w3.org/2003/11/swrl#AtomList> ;
                                                      rdf:first [ rdf:type <http://www.w3.org/2003/11/swrl#ClassAtom> ;
                                                                  <http://www.w3.org/2003/11/swrl#classPredicate> :SalesPremises ;
                                                                  <http://www.w3.org/2003/11/swrl#argument1> owl:spr
                                                                ] ;
                                                      rdf:rest [ rdf:type <http://www.w3.org/2003/11/swrl#AtomList> ;
                                                                 rdf:first [ rdf:type <http://www.w3.org/2003/11/swrl#DatavaluedPropertyAtom> ;
                                                                             <http://www.w3.org/2003/11/swrl#propertyPredicate> :hasGFASalesSpaces ;
                                                                             <http://www.w3.org/2003/11/swrl#argument1> owl:spr ;
                                                                             <http://www.w3.org/2003/11/swrl#argument2> owl:gfa
                                                                           ] ;
                                                                 rdf:rest [ rdf:type <http://www.w3.org/2003/11/swrl#AtomList> ;
                                                                            rdf:first [ rdf:type <http://www.w3.org/2003/11/swrl#BuiltinAtom> ;
                                                                                        <http://www.w3.org/2003/11/swrl#builtin> <http://www.w3.org/2003/11/swrlb#lessThanOrEqual> ;
                                                                                        <http://www.w3.org/2003/11/swrl#arguments> [ rdf:type rdf:List ;
                                                                                                                                     rdf:first owl:gfa ;
                                                                                                                                     rdf:rest [ rdf:type rdf:List ;
                                                                                                                                                rdf:first 2000.0 ;
                                                                                                                                                rdf:rest rdf:nil
                                                                                                                                              ]
                                                                                                                                   ]
                                                                                      ] ;
                                                                            rdf:rest rdf:nil
                                                                          ]
                                                               ]
                                                    ]
                                         ] ;
   <http://www.w3.org/2003/11/swrl#head> [ rdf:type <http://www.w3.org/2003/11/swrl#AtomList> ;
                                           rdf:first [ rdf:type <http://www.w3.org/2003/11/swrl#ClassAtom> ;
                                                       <http://www.w3.org/2003/11/swrl#classPredicate> :UnregulatedSpecialPurposeConstruction ;
                                                       <http://www.w3.org/2003/11/swrl#argument1> owl:spr
                                                     ] ;
                                           rdf:rest rdf:nil
                                         ]
 ] .

[ <http://swrl.stanford.edu/ontologies/3.3/swrla.owl#isRuleEnabled> "true"^^xsd:boolean ;
   rdfs:comment "Special Purpose Condition" ;
   rdfs:label "§2 (4) 6. MBO" ;
   rdf:type <http://www.w3.org/2003/11/swrl#Imp> ;
   <http://www.w3.org/2003/11/swrl#body> [ rdf:type <http://www.w3.org/2003/11/swrl#AtomList> ;
                                           rdf:first [ rdf:type <http://www.w3.org/2003/11/swrl#BuiltinAtom> ;
                                                       <http://www.w3.org/2003/11/swrl#builtin> <http://www.w3.org/2003/11/swrlb#greaterThan> ;
                                                       <http://www.w3.org/2003/11/swrl#arguments> [ rdf:type rdf:List ;
                                                                                                    rdf:first owl:nop ;
                                                                                                    rdf:rest [ rdf:type rdf:List ;
                                                                                                               rdf:first 100.0 ;
                                                                                                               rdf:rest rdf:nil
                                                                                                             ]
                                                                                                  ]
                                                     ] ;
                                           rdf:rest [ rdf:type <http://www.w3.org/2003/11/swrl#AtomList> ;
                                                      rdf:first [ rdf:type <http://www.w3.org/2003/11/swrl#ClassAtom> ;
                                                                  <http://www.w3.org/2003/11/swrl#classPredicate> <https://w3id.org/bot#Building> ;
                                                                  <http://www.w3.org/2003/11/swrl#argument1> owl:b
                                                                ] ;
                                                      rdf:rest [ rdf:type <http://www.w3.org/2003/11/swrl#AtomList> ;
                                                                 rdf:first [ rdf:type <http://www.w3.org/2003/11/swrl#DatavaluedPropertyAtom> ;
                                                                             <http://www.w3.org/2003/11/swrl#propertyPredicate> :hasNumberOfPeople ;
                                                                             <http://www.w3.org/2003/11/swrl#argument1> owl:sp ;
                                                                             <http://www.w3.org/2003/11/swrl#argument2> owl:nop
                                                                           ] ;
                                                                 rdf:rest [ rdf:type <http://www.w3.org/2003/11/swrl#AtomList> ;
                                                                            rdf:first [ rdf:type <http://www.w3.org/2003/11/swrl#IndividualPropertyAtom> ;
                                                                                        <http://www.w3.org/2003/11/swrl#propertyPredicate> <https://w3id.org/bot#hasSpace> ;
                                                                                        <http://www.w3.org/2003/11/swrl#argument1> owl:b ;
                                                                                        <http://www.w3.org/2003/11/swrl#argument2> owl:sp
                                                                                      ] ;
                                                                            rdf:rest rdf:nil
                                                                          ]
                                                               ]
                                                    ]
                                         ] ;
   <http://www.w3.org/2003/11/swrl#head> [ rdf:type <http://www.w3.org/2003/11/swrl#AtomList> ;
                                           rdf:first [ rdf:type <http://www.w3.org/2003/11/swrl#ClassAtom> ;
                                                       <http://www.w3.org/2003/11/swrl#classPredicate> <https://purl.org/fisa#SpecialPurposeConditionAcc§2_S4_P6> ;
                                                       <http://www.w3.org/2003/11/swrl#argument1> owl:b
                                                     ] ;
                                           rdf:rest rdf:nil
                                         ]
 ] .

###  Generated by the OWL API (version 5.1.18) https://github.com/owlcs/owlapi/
